@prefix : <https://w3id.org/i40/sto#> .
@prefix cc: <http://creativecommons.org/ns#> .
@prefix dbo: <http://dbpedia.org/ontology#> .
@prefix dbont: <http://dbpedia.org/ontology/> .
@prefix dbpcy: <http://dbpedia.org/class/yago/> .
@prefix dbprop: <http://dbpedia.org/property/> .
@prefix dbr: <http://dbpedia.org/resource#> .
@prefix dbrc: <http://dbpedia.org/resource/Category:> .
@prefix dbres: <http://dbpedia.org/resource/> .
@prefix dc11: <http://purl.org/dc/elements/1.1/> .
@prefix dcterms: <http://purl.org/dc/terms/> .
@prefix deo: <http://purl.org/spar/deo/> .
@prefix doap: <http://usefulinc.com/ns/doap#> .
@prefix dul: <http://www.ontologydesignpatterns.org/ont/dul/DUL.owl#> .
@prefix foaf: <http://xmlns.com/foaf/0.1/> .
@prefix geo: <http://www.geonames.org/ontology#> .
@prefix ids: <https://w3id.org/ids/core/> .
@prefix idsram: <https://w3id.org/ids/ram/> .
@prefix iira: <http://example.org/iira#> .
@prefix lang: <http://lexvo.org/id/iso639-3/> .
@prefix lingg: <http://purl.org/linguistics/gold/> .
@prefix muto: <http://purl.org/muto/core#> .
@prefix obda: <https://w3id.org/obda/vocabulary#> .
@prefix om2: <http://www.ontology-of-units-of-measure.org/resource/om-2/> .
@prefix owl: <http://www.w3.org/2002/07/owl#> .
@prefix prov: <http://www.w3.org/ns/prov#> .
@prefix rami: <https://w3id.org/i40/rami#> .
@prefix rdf: <http://www.w3.org/1999/02/22-rdf-syntax-ns#> .
@prefix rdfs: <http://www.w3.org/2000/01/rdf-schema#> .
@prefix schema: <http://schema.org/> .
@prefix skos: <http://www.w3.org/2004/02/skos/core#> .
@prefix sto: <https://w3id.org/i40/sto#> .
@prefix vann: <http://purl.org/vocab/vann/> .
@prefix voaf: <http://purl.org/vocommons/voaf#> .
@prefix vocvr: <http://purl.org/voc/vrank#> .
@prefix wike: <http://www.wikidata.org/entity/> .
@prefix xml: <http://www.w3.org/XML/1998/namespace> .
@prefix xsd: <http://www.w3.org/2001/XMLSchema#> .

cc:attributionName a owl:AnnotationProperty .

cc:attributionURL a owl:AnnotationProperty .

dbr:HoehenkirchenSiegertsbrunn a owl:NamedIndividual .

iira:BusinessViewpoint a iira:Viewpoint,
        owl:NamedIndividual ;
    rdfs:label "IIRA Business Viewpoint"@en ;
    sto:isDescribedin iira:IIRA .

iira:DistributedDataManagement a iira:CrosscuttingFunction,
        owl:NamedIndividual .

iira:ImplementationViewpoint a iira:Viewpoint,
        owl:NamedIndividual ;
    rdfs:label "IIRA Implementation Viewpoint"@en ;
    sto:isDescribedin iira:IIRA .

iira:IndustrialAnalytics a iira:CrosscuttingFunction,
        owl:NamedIndividual .

iira:IntelligentAndResilientControl a iira:CrosscuttingFunction,
        owl:NamedIndividual .

iira:PhysicalSystems a owl:NamedIndividual,
        sto:StandardClassification ;
    rdfs:label "IIRA Physical Systems"@en ;
    dul:isPartOf iira:FunctionalViewpoint ;
    sto:alignesWith rami:Asset ;
    sto:isDescribedin iira:IIRA .

iira:Reliability a iira:SystemCharacteristics,
        owl:NamedIndividual ;
    rdfs:label "IIRA Reliability"@en .

iira:Resilience a iira:SystemCharacteristics,
        owl:NamedIndividual ;
    rdfs:label "IIRA Resilience"@en .

iira:Scalability a iira:SystemCharacteristics,
        owl:NamedIndividual ;
    rdfs:label "IIRA Scalability"@en .

iira:UsageViewpoint a iira:Viewpoint,
        owl:NamedIndividual ;
    rdfs:label "IIRA Usage Viewpoint"@en ;
    sto:isDescribedin iira:IIRA .

dc11:description a owl:AnnotationProperty .

dc11:title a owl:AnnotationProperty .

dcterms:creator a owl:AnnotationProperty .

dcterms:description a owl:AnnotationProperty .

dcterms:hasLicense a owl:ObjectProperty ;
    rdfs:label "has License"@en ;
    dcterms:hasVersion <http://dublincore.org/usage/terms/history/#license-002> ;
    dcterms:issued "2004-06-14"^^xsd:date ;
    dcterms:modified "2017-12-19"^^xsd:date ;
    rdfs:comment "A legal document giving official permission to do something with the resource."@en,
        "A legal document giving official permission to do something with the resource. In this ontology denotes the license of a Standard."@en,
        "Represent the license document for a given Standard"@en ;
    rdfs:domain sto:Standard ;
    rdfs:isDefinedBy dcterms: ;
    rdfs:range dcterms:LicenseDocument .

dcterms:hasVersion a owl:AnnotationProperty .

dcterms:issued a owl:AnnotationProperty .

dcterms:modified a owl:AnnotationProperty .

dcterms:title a owl:AnnotationProperty .

<http://wikipedia.org/wiki/IEEE_Smart_Grid> a owl:NamedIndividual .

om2:hasNumericalValue a owl:AnnotationProperty .

om2:hasUnit a owl:AnnotationProperty .

dul:isComponentOf a owl:ObjectProperty ;
    rdfs:label "is Component Of"@en ;
    rdfs:comment "Represents Standards that are component of other Standards. This relation is not transitive"@en ;
    rdfs:domain sto:Standard ;
    rdfs:isDefinedBy <http://www.ontologydesignpatterns.org/ont/dul/DUL.owl> ;
    rdfs:range sto:Standard ;
    rdfs:subPropertyOf sto:relatedTo .

dul:isMemberOf a owl:AnnotationProperty .

skos:altLabel a owl:AnnotationProperty .

skos:definition a owl:AnnotationProperty .

skos:note a owl:AnnotationProperty .

skos:prefLabel a owl:AnnotationProperty .

prov:wasGeneratedBy a owl:ObjectProperty ;
    rdfs:label "was Generated By"@en ;
    rdfs:comment "Standard A has influences in Standard B. For example, IEC_61499 hasInfluenceIn IEC_61804-2(EDDL)"@en ;
    rdfs:isDefinedBy "https://www.w3.org/TR/prov-o/#wasGeneratedBy"@en ;
    rdfs:subPropertyOf sto:relatedTo .

foaf:familyName a owl:AnnotationProperty .

foaf:mbox a owl:AnnotationProperty .

foaf:name a owl:AnnotationProperty .

rami:Body a owl:NamedIndividual,
        sto:StandardizationFramework ;
    rdfs:label "Administration Shell Body"@en ;
    dul:isPartOf sto:AdministrationShell ;
    rdfs:comment "TODO: Find better class assignement"@en .

rami:Header a owl:NamedIndividual,
        sto:StandardizationFramework ;
    rdfs:label "Administration Shell Header"@en ;
    dul:isPartOf sto:AdministrationShell ;
    rdfs:comment "TODO: find better class assignment"@en .

rami:InstanceMaintenance a owl:NamedIndividual,
        rami:RAMILifeCycleLayer ;
    rdfs:label "Instance Maintenance"@en .

rami:InstanceProduction a owl:NamedIndividual,
        rami:RAMILifeCycleLayer ;
    rdfs:label "Instance Production"@en .

rami:TypeDevelopment a owl:NamedIndividual,
        rami:RAMILifeCycleLayer ;
    rdfs:label "Type Development"@en .

rami:TypeMaintenance a owl:NamedIndividual,
        rami:RAMILifeCycleLayer ;
    rdfs:label "Type Maintenance"@en .

rami:safety a owl:NamedIndividual .

sto:ASAM_ODS a owl:NamedIndividual,
        sto:Standard ;
    rdfs:label "ASAM ODS"@en ;
    rdfs:comment "Set up a test data management system on top of test systems that produce measured or calculated data from testing activities"@en ;
    sto:hasOfficialResource <https://wiki.asam.net/display/STANDARDS/ASAM+ODS> ;
    sto:hasPublisher sto:ASAM .

sto:ASME_Y1441 a owl:NamedIndividual,
        sto:Standard ;
    rdfs:label "ASME Y14.41"@en ;
    dcterms:subject dbrc:American_Society_of_Mechanical_Engineers ;
    rdfs:comment "ASME Y14.41 establishs requirements for model-based definition upon CAD software and those who use CAD software to create product definition within the 3D model."@en ;
    sto:hasClassification sto:ModelingPractice ;
    sto:hasDBpediaResource dbres:ASME_Y14.41 ;
    sto:hasOfficialResource <https://www.asme.org/products/codes-standards/y1441-2012-digital-product-definition-data> ;
    sto:hasPublisher sto:ASME ;
    sto:hasWikipediaArticle <https://en.wikipedia.org/wiki/ASME_Y14.41> .

sto:ArchitectureDescription a owl:Class ;
    rdfs:label "Architecture Description" ;
    rdfs:comment "ISO 42010 definition of an Architecture Description"@en ;
    rdfs:seeAlso "https://www.iso.org/standard/50508.html" ;
    owl:equivalentClass sto:StandardizationFramework .

sto:B2MML a dbpcy:WikicatANSIStandards,
        dbpcy:WikicatStandards,
        dbpcy:WikicatXML-basedStandards,
        dbont:Language,
        dbont:ProgrammingLanguage,
        dbont:Software,
        schema:Language,
        owl:NamedIndividual,
        owl:Thing,
        wike:Q315,
        wike:Q34770,
        wike:Q9143,
        sto:Standard ;
    rdfs:label "Business To Manufacturing Markup Language" ;
    dcterms:subject dbrc:ANSI_standards,
        dbrc:Manufacturing,
        dbrc:Supply_chain_management ;
    lingg:hypernym dbres:Implementation ;
    rdfs:comment "B2MML or Business To Manufacturing Markup Language is an XML implementation of the ANSI/ISA-95 family of standards (ISA-95)"@en ;
    skos:altLabel "IEC 62264"@en ;
    sto:hasClassification sto:BusinessProcessExecution,
        sto:EnterpriseLevel ;
    sto:hasDBpediaResource dbres:B2MML ;
    sto:hasDeveloper sto:MESA ;
    sto:hasOfficialResource <https://services.mesa.org/ResourceLibrary/ShowResource/0f47758b-60f0-40c6-a71b-fa7b2363fb3a> ;
    sto:hasPublisher sto:MESA ;
    sto:hasTag "B2MML"@en ;
    sto:hasWikipediaArticle <https://en.wikipedia.org/wiki/B2MML> ;
    sto:isImplementationOf sto:ISA-95 .

sto:BBF_TR-069 a dbpcy:WikicatApplicationLayerProtocols,
        dbpcy:WikicatComputerSecurityExploits,
        dbpcy:WikicatInternetStandards,
        dbpcy:WikicatStandards,
        dbont:Software,
        owl:NamedIndividual,
        sto:Standard ;
    rdfs:label "BBF TR-069"@en ;
    dcterms:subject dbrc:Digital_subscriber_line,
        dbrc:Internet_Standards ;
    lingg:hypernym dbres:Specification ;
    rdfs:comment "Digital Enhanced Cordless Telecommunications (DECT) is the ETSI standard for short-range cordless communications, which can be adapted for many applications and can be used over unlicensed frequency allocations world-wide."@en ;
    sto:hasDBpediaResource dbres:TR-069 ;
    sto:hasDeveloper sto:BBF ;
    sto:hasOfficialResource <https://www.broadband-forum.org/standards-and-software/technical-specifications/tr-069-files-tools> ;
    sto:hasPublisher sto:BBF ;
    sto:hasTag "CPE WAN Management Protocol"@en ;
    sto:hasWikipediaArticle <https://en.wikipedia.org/wiki/TR-069> .

sto:BPEL a dbpcy:WikicatMarkupLanguages,
        dbpcy:WikicatProgrammingLanguages,
        dbpcy:WikicatSpecificationLanguages,
        dbpcy:WikicatWebServiceSpecifications,
        dbpcy:WikicatWebServices,
        dbpcy:WikicatXML-basedStandards,
        dbont:Language,
        owl:NamedIndividual,
        sto:Standard ;
    rdfs:label "Business Process Execution Language"@en ;
    dcterms:subject dbrc:Process_management,
        dbrc:Specification_languages,
        dbrc:Web_service_specifications,
        dbrc:Workflow_technology,
        dbrc:XML-based_standards ;
    lingg:hypernym dbres:Language ;
    rdfs:comment "The Web Services Business Process Execution Language (WS-BPEL), commonly known as BPEL Business Process Execution Language, is a standard executable language for specifying actions within business processes with web services."@en ;
    sto:hasClassification sto:BusinessProcessExecution ;
    sto:hasDBpediaResource dbres:Business_Process_Execution_Language ;
    sto:hasOfficialResource <https://www.oasis-open.org/committees/tc_home.php?wg_abbrev=wsbpel> ;
    sto:hasPublisher sto:OASIS ;
    sto:hasTag "BPEL"@en ;
    sto:hasWikipediaArticle <https://en.wikipedia.org/wiki/Business_Process_Execution_Language> .

sto:ConditionMonitoring a owl:NamedIndividual,
        rami:AdminShellSubmodel ;
    sto:isDescribedin sto:AdministrationShell .

sto:Configuration a owl:NamedIndividual,
        rami:AdminShellSubmodel ;
    sto:isDescribedin sto:AdministrationShell .

sto:DIN_EN_50128 a owl:NamedIndividual,
        sto:Standard ;
    rdfs:label "DIN EN 50128"@en ;
    rdfs:comment "Die EN 50128 ist eine Europäische Norm für sicherheitsrelevante Software der Eisenbahn, sowohl strecken- als auch zugseitig. Zusammen mit der EN 50129 für die Hardware und den Zulassungsprozessen ist die EN 50128 eine Spezialisierung der EN 61508. Die EN 50128 ist eine Prozessnorm. Sie stellt dar, welche Verfahren, Prinzipien und Maßnahmen anzuwenden sind, damit die Software als sicher gilt."@de ;
    sto:hasClassification idsram:Certification,
        idsram:Safety ;
    sto:hasOfficialResource <https://www.beuth.de/de/norm/din-en-50128/148018416> ;
    sto:hasPublicationDate "2012-03-01"^^xsd:date ;
    sto:hasPublisher sto:DIN .

sto:DIN_EN_50129 a owl:NamedIndividual,
        sto:Standard ;
    rdfs:label "DIN EN 50129"@en ;
    dcterms:title "Railway applications - Communications, signalling and processing systems - Safety related electronic systems for signalling"@en ;
    rdfs:comment "Für alle Eisenbahnsignalsysteme, -Teilsysteme und -Einrichtungen sind jedoch Gefährdungsanalyse und Risikobewertungsprozesse, wie in DIN EN 50126 und in dieser Norm definiert, notwendig, um die Sicherheitsanforderungen zu identifizieren."@de,
        "Specifies risk analysis for railway systems"@en ;
    sto:hasClassification idsram:Certification,
        idsram:Safety ;
    sto:hasOfficialResource <https://www.beuth.de/de/norm/din-en-50129/67478433> ;
    sto:hasPublisher sto:DIN .

sto:DIN_EN_50155 a dbont:Company,
        owl:NamedIndividual,
        sto:Standard ;
    rdfs:label "DIN EN 50155"@en ;
    dcterms:subject dbrc:EN_standards ;
    dcterms:title "Railway applications - Rolling stock - Electronic equipment"@en ;
    lingg:hypernym dbres:Equipment ;
    rdfs:comment "Diese Norm wird bei der Konstruktion, Fertigung und Prüfung von auf Schienenfahrzeugen eingebauten elektronischen Betriebsmitteln verwendet. Sie beschreibt außerdem die elektrischen sowie die Umweltbedingungen für den Betrieb. Die Norm gilt für alle elektronischen Betriebsmittel für die Steuerung, die Regelung, den Schutz, die Diagnose, die Versorgung und so weiter, die auf Schienenfahrzeugen installiert sind. Als ein elektronisches Betriebsmittel gilt dabei ein Betriebsmittel, das hauptsächlich aus Halbleiterbauelementen und üblicherweise zugehörigen Bauelementen aufgebaut ist. Auch Sensoren (Strom, Spannung, Geschwindigkeit und so weiter) und bestückte Leiterplatten von Zündeinheiten für leistungselektronische Geräte sind von dieser Norm umfasst. Vollständige Zündeinheiten und leistungselektronische Schaltkreise sind in EN 61287-1 enthalten. Die Norm umfasst die Betriebsbedingungen, die Konstruktionsanforderungen, die Dokumentation und die Prüfung der elektronischen Betriebsmittel sowie die grundlegenden Hardware- und Softwareanforderungen, die für ein leistungsfähiges, zuverlässiges Betriebsmittel als erforderlich erachtet werden. Zuständig ist das DKE/UK 351.1 \"Fahrzeuge\" der DKE Deutsche Kommission Elektrotechnik Elektronik Informationstechnik in DIN und VDE."@de,
        "EN 50155:2017 is an international standard covering electronic equipment used on rolling stock for railway applications. The standard covers aspects of this electronic equipment, including temperature, humidity, shock, vibration, and other parameters. A copy of the standard may be purchased from authorised standards agencies, e.g. BSI in the UK."@en ;
    sto:hasClassification idsram:Certification,
        idsram:Safety ;
    sto:hasDBpediaResource dbres:EN_50155 ;
    sto:hasOfficialResource <https://www.beuth.de/de/norm/din-en-50155/275256249> ;
    sto:hasWikipediaArticle <https://en.wikipedia.org/wiki/EN_50155> .

sto:DIN_EN_50159 a owl:NamedIndividual,
        sto:Standard ;
    rdfs:label "DIN EN 50159"@en ;
    dcterms:title "Railway applications - Communication, signalling and processing systems - Safety-related communication in transmission systems"@en ;
    rdfs:comment "This European Standard is applicable for safety-relevant electronic systems which use a transmission system for digital communication purposes which has not been necessarily designed for safety-relevant applications and which - remains under the control of the designer and does not change during the life cycle, or - which is partly unknown and also does not remain constant, for which unauthorized access can be excluded, however, or - which is not under control of the designer and where unauthorized access shall also be considered. The responsible Committee is Subcommittee UK 351.3 \"Bahn-Signalanlagen\" (\"Signalling systems for railways\") of the DKE (German Commission for Electrical, Electronic and Information Technologies) at DIN and VDE."@en ;
    sto:hasClassification idsram:Certification,
        idsram:Safety ;
    sto:hasOfficialResource <https://www.beuth.de/de/norm/din-en-50159/137853742> .

sto:DIN_EN_61511 a owl:NamedIndividual,
        sto:Standard ;
    rdfs:label "DIN EN 61511"@en ;
    dcterms:title "Functional safety - Safety instrumented systems for the process industry sector - Part 1: Framework, definitions, system, hardware and software requirements"@en ;
    rdfs:comment "This standard gives requirements for the specification, design, installation, operation and maintenance of a safety instrumented system (SIS), so that it can be confidently entrusted to achieve or maintain a safe state of the process. This standard has been developed as a process sector implementation of IEC 61508."@en ;
    sto:hasClassification idsram:Certification,
        idsram:Safety ;
    sto:hasPublisher sto:DIN .

sto:DIN_EN_ISO_13849 a dbpcy:WikicatISOStandards,
        dbpcy:WikicatSafetyCodes,
        owl:NamedIndividual,
        sto:Standard ;
    rdfs:label "DIN EN ISO 13849"@en ;
    dcterms:subject dbrc:ISO_standards,
        dbrc:Safety_codes ;
    rdfs:comment """ISO 13849 is a safety standard which deals with safety-related design principles of employed control systems to establish different safety Performance Levels (PL). It replaced EN 954-1 in December 2011.\r
    Part 1 defines the general principles for design.\r
    Part 2 describes the validation."""@en ;
    sto:hasClassification idsram:Certification,
        idsram:Safety ;
    sto:hasDBpediaResource dbres:ISO_13849 ;
    sto:hasPublisher sto:DIN,
        sto:ISO ;
    sto:hasWikipediaArticle <https://en.wikipedia.org/wiki/ISO_13849> .

sto:DIN_EN_ISO_IEC_17025 a owl:NamedIndividual,
        sto:Standard ;
    rdfs:label "DIN EN ISO/IEC 17025"@en ;
    dcterms:title "General requirements for the competence of testing and calibration laboratories"@en ;
    rdfs:comment "DIN EN ISO/IEC 17025 legt allgemeine Anforderungen an die Kompetenz, an die Unparteilichkeit und für die einheitliche Arbeitsweise von Laboratorien fest. Die Norm ist auf alle Organisationen anwendbar, die Labortätigkeiten durchführen, unabhängig von der Anzahl der Mitarbeiter. Sie reiht sich in die Normenreihe DIN EN ISO/IEC 17000 ein. Kunden von Laboratorien, Behörden, Organisationen und Programme, die eine Begutachtung unter Gleichrangigen anwenden, Akkreditierungsstellen und andere können diese Norm zur Bestätigung oder Anerkennung der Kompetenz von Laboratorien nutzen."@de,
        "ISO 17025 specifies general requirements for laboratories."@en ;
    sto:hasClassification idsram:Certification ;
    sto:hasOfficialResource <https://www.beuth.de/de/norm/din-en-iso-iec-17025/278030106> ;
    sto:hasPublisher sto:DIN,
        sto:IEC,
        sto:ISO .

sto:DIN_SPEC_16592 a owl:NamedIndividual,
        sto:Standard ;
    rdfs:label "DIN SPEC 16592"@en ;
    rdfs:comment "Combining OPC Unified Architecture and Automation Markup Language."@en ;
    prov:wasGeneratedBy sto:IEC_62541,
        sto:IEC_62714 ;
    sto:hasDeveloper sto:DIN ;
    sto:hasOfficialResource <https://www.beuth.de/de/technische-regel/din-spec-16592/265597431> ;
    sto:hasPublisher sto:DIN .

sto:DIN_SPEC_27070 a owl:NamedIndividual,
        sto:Standard ;
    rdfs:label "DIN SPEC 27070"@en ;
    dcterms:title "Reference architecture of a security gateway for the exchange of industry data and services"@en ;
    rdfs:comment "security gateway for data protection of personal data"@en ;
    sto:alignesWith <ids:TrustedConnector> ;
    sto:hasClassification idsram:Security ;
    sto:hasPublisher sto:DIN .

sto:DIN_SPEC_92222 a owl:NamedIndividual,
        sto:Standard ;
    rdfs:label "DIN SPEC 92222"@en ;
    dcterms:title "Reference Model for Industrial Cloud Federation"@en ;
    rdfs:comment "ensuring interoperability and communication of IT systems in cloud scenarios"@en ;
    sto:hasClassification idsram:Security ;
    sto:hasDeveloper sto:DIN .

sto:ENISA_CloudComputing a owl:NamedIndividual,
        sto:Standard ;
    rdfs:label "ENISA Cloud Computing"@en ;
    dcterms:title "Cloud Computing - Benefits, risks and recommendations for information security"@en ;
    rdfs:comment "ENISA, supported by a group of subject matter expert comprising representatives from Industries, Academia and Governmental Organizations, has conducted, in the context of the Emerging and Future Risk Framework project, an risks assessment on cloud computing business model and technologies. The result is an in-depth and independent analysis that outlines some of the information security benefits and key security risks of cloud computing. The report provide also a set of practical recommendations.Produced by ENISA with contributions from a group of subject matter expert comprising representatives from Industry, Academia and Governmental Organizations, a risk assessment of cloud computing business model and technologies. This is an in-depth and independent analysis that outlines some of the information security benefits and key security risks of cloud computing. The report provide also a set of practical recommendations. It is produced in the context of the Emerging and Future Risk Framework project."@en ;
    sto:domainName "Cloud Computing"@en ;
    sto:hasClassification iira:Security ;
    sto:hasOfficialResource <https://resilience.enisa.europa.eu/cloud-security-and-resilience/publications/cloud-computing-benefits-risks-and-recommendations-for-information-security> ;
    sto:hasPublicationDate "2012-12-01"^^xsd:date ;
    sto:hasPublisher sto:ENISA .

sto:ETSI_LTN a owl:NamedIndividual,
        sto:Standard ;
    rdfs:label "ETSI LTN"@en ;
    rdfs:comment "Machine-to-Machine communications and the Internet of Things (IoT) involve the connection of potentially billions of connected objects which need only low throughput connectivity. The anticipated benefits of creating new dedicated IoT Low Throughput Networks (LTN) include lower costs, the creation of new applications, a reduction in electromagnetic radiation by improving data transmission efficiency LTN are expected to be crucial to the success of IoT standardization and implementation, and to provide the basis for many new and innovative applications. "@en ;
    sto:hasDeveloper sto:ETSI ;
    sto:hasDomain sto:M2M ;
    sto:hasOfficialResource <http://www.etsi.org/technologies-clusters/technologies/low-throughput-networks> ;
    sto:hasPublisher sto:ETSI ;
    sto:hasTag "Low Throughput Networks"@en ;
    sto:relatedTo sto:ETSI_DECT .

sto:ETSI_ULE a dbpcy:WikicatMobileTelecommunicationsStandards,
        dbont:Work,
        owl:NamedIndividual,
        sto:Standard ;
    rdfs:label "Ultra Low Energy"@en ;
    dcterms:subject dbrc:Mobile_telecommunications_standards ;
    lingg:hypernym dbres:Standard ;
    rdfs:comment "DECT Ultra Low Energy (DECT ULE) is a technology based on DECT, and intended for Machine-to-Machine communications such as Home and Industrial automation. The main characteristics of the technology are ultra-low power consumption (much lower than IEEE 802.11) and wider coverage (much wider than IEEE 802.15 and Bluetooth Low Energy)."@en ;
    sto:hasDBpediaResource dbres:ULE_-_Ultra_Low_Energy ;
    sto:hasDeveloper sto:ETSI ;
    sto:hasOfficialResource <http://www.etsi.org/technologies-clusters/technologies/dect/dect-ule> ;
    sto:hasPublisher sto:ETSI ;
    sto:hasTag "ETSI ULE"@en ;
    sto:hasWikipediaArticle <https://en.wikipedia.org/wiki/DECT_Ultra_Low_Energy>,
        "http://en.wikipedia.org/wiki/ULE_-_Ultra_Low_Energy" ;
    sto:relatedTo sto:ETSI_DECT .

sto:EndOfLifeReclying a owl:NamedIndividual .

sto:FileSizeIEC_61334_1996_P3_S21 a om2:Measure,
        owl:NamedIndividual ;
    rdfs:label "FileSize IEC 61334-3-21:1996 "@en ;
    om2:hasNumericalValue "1112.0"^^xsd:float ;
    om2:hasUnit om2:kilobyte ;
    rdfs:comment "Specifies the file size of the document for standard IEC 61334-3-21:1996 "@en .

sto:IEC_11404 a owl:NamedIndividual ;
    owl:sameAs sto:ISO_11404 .

sto:IEC_14443 a dbpcy:PositiveIdentification106885389,
        dbpcy:WikicatContactlessSmartCards,
        dbpcy:WikicatIECStandards,
        <http://dbpedia.org/class/yago/WikicatISO/IECStandards>,
        dbpcy:WikicatISOStandards,
        dbpcy:WikicatSmartCards,
        dbont:Work,
        owl:NamedIndividual,
        sto:Standard ;
    rdfs:label "ISO/IEC 14443"@en ;
    dcterms:subject dbrc:Contactless_smart_cards,
        <http://dbpedia.org/resource/Category:ISO/IEC_standards> ;
    lingg:hypernym dbres:Standard ;
    rdfs:comment "The ISO/IEC 14443 standard is a four-part international standard for contact-less smart cards operating at 13.56 MHz in close proximity (~10cm) with a reader antenna. This ISO standard describes the modulation and transmission protocols between card and reader to create interoperability for contact-less smart card products. There are two main communication protocols supported by the ISO/IEC 14443 standard, they are addressed as Type A and Type B. Most High Frequency (13.56 MHz) proximity tags are using these guidelines for their communication."@en ;
    owl:sameAs sto:ISO_14443 ;
    sto:hasDBpediaResource <http://dbpedia.org/resource/ISO/IEC_14443> ;
    sto:hasOfficialResource <https://www.iso.org/standard/70170.html> ;
    sto:hasPublisher sto:IEC,
        sto:ISO ;
    sto:hasTag "IEC 14443"@en ;
    sto:hasWikipediaArticle <https://en.wikipedia.org/wiki/ISO/IEC_14443> .

sto:IEC_15408 a owl:NamedIndividual ;
    owl:sameAs sto:ISO_15408 .

sto:IEC_15459 a owl:NamedIndividual,
        sto:Standard ;
    rdfs:label "IEC 15459"@en ;
    rdfs:comment "ISO/IEC 15459-1:2014 specifies a unique string of characters for the identification of individual transport units. The character string is intended to be represented in a bar code label or other AIDC media attached to the entity to meet management needs. To address management needs, different types of entities are recognized in the various parts of ISO/IEC 15459, which allows different requirements to be met by the identities associated with each type. The rules for the unique identification for individual transport units, to identify physical logistical transfers, with the identity relevant for the duration of one or more items in the load being held or transported as part of that load, are defined and supported by example."@en ;
    owl:sameAs sto:ISO_15459 ;
    sto:hasOfficialResource <https://www.iso.org/standard/54779.html> ;
    sto:hasPublisher sto:IEC,
        sto:ISO ;
    sto:hasTag "Information technology -- Automatic identification and data capture techniques -- Unique identification"@en .

sto:IEC_24760 a owl:NamedIndividual,
        sto:Standard ;
    rdfs:label "IEC 24760"@en ;
    rdfs:comment "ISO/IEC 24760: it defines terms for identity management, and also specifies core concepts of identity and identity management and their relationships. It is applicable to any information system that processes identity information. A bibliography of documents describing various aspects of identity information management is provided."@en ;
    owl:sameAs sto:ISO_24760 ;
    sto:alignesWith sto:Identification ;
    sto:hasClassification iira:Security,
        rami:ControlDevice,
        rami:FieldDevice,
        rami:Information,
        rami:Product,
        rami:Safety,
        rami:Security,
        rami:Station,
        sto:ProductModelDataExchange ;
    sto:hasDomain sto:ITSecurity ;
    sto:hasOfficialResource <https://www.iso.org/standard/57914.html> ;
    sto:hasPublicationDate "2011-01-12"^^xsd:date ;
    sto:hasPublisher sto:IEC ;
    sto:relatedTo sto:IEC_62443 .

sto:IEC_27018 a owl:NamedIndividual ;
    owl:sameAs sto:ISO_27018 .

sto:IEC_27031 a owl:NamedIndividual ;
    owl:sameAs sto:ISO_27031 .

sto:IEC_27036 a owl:NamedIndividual ;
    owl:sameAs sto:ISO_27036 .

sto:IEC_29100 a owl:NamedIndividual ;
    owl:sameAs sto:ISO_29100 .

sto:IEC_29115 a owl:NamedIndividual,
        sto:Standard ;
    rdfs:label "IEC 29115"@en ;
    dcterms:title "Information technology -- Security techniques -- Entity authentication assurance framework"@en ;
    rdfs:comment """ISO/IEC 29115:2013 provides a framework for managing entity authentication assurance in a given context. In particular, it:\r
\r
- specifies four levels of entity authentication assurance;\r
\r
- specifies criteria and guidelines for achieving each of the four levels of entity authentication assurance;\r
\r
- provides guidance for mapping other authentication assurance schemes to the four LoAs;\r
\r
- provides guidance for exchanging the results of authentication that are based on the four LoAs; and\r
\r
- provides guidance concerning controls that should be used to mitigate authentication threats."""@en ;
    owl:sameAs sto:ISO_29115 ;
    sto:hasClassification iira:Security ;
    sto:hasOfficialResource <https://www.iso.org/standard/45138.html> ;
    sto:hasPublisher sto:IEC,
        sto:ISO .

sto:IEC_29161 a owl:NamedIndividual,
        sto:Standard ;
    rdfs:label "IEC 29161"@en ;
    rdfs:comment "ISO/IEC 29161:2016 establishes a unique identification scheme for the Internet of Things (IoT), based on existing and evolving data structures. This International Standard specifies the common rules applicable for unique identification that are required to ensure full compatibility across different identities. The unique identification is a universal construct for any physical object, virtual object, or person. It is used in IoT information systems that need to track or otherwise refer to entities. It is intended for use with any IoT media."@en ;
    owl:sameAs sto:ISO_29161 ;
    sto:hasDomain "Automatic identification and data capture techniques"@en ;
    sto:hasOfficialResource <https://www.iso.org/standard/45240.html> ;
    sto:hasPublicationDate "2016-08-01"^^xsd:date ;
    sto:hasPublisher sto:IEC,
        sto:ISO ;
    sto:hasTag "Information technology -- Data structure -- Unique identification for the Internet of Things"@en .

sto:IEC_29182-1 a owl:NamedIndividual,
        sto:Standard ;
    rdfs:label "IEC 29182-1"@en ;
    rdfs:comment "ISO/IEC 29182-1: provides a general overview of the characteristics of a sensor network and the organization of the entities that comprise such a network. It also describes the general requirements that are identified for sensor networks."@en ;
    sto:hasClassification rami:Communications,
        rami:ControlDevice,
        rami:FieldDevice,
        sto:ProductionSystemModelData ;
    sto:hasDomain sto:M2M ;
    sto:hasOfficialResource <https://www.iso.org/standard/45261.html> ;
    sto:hasPublicationDate "2013-06-01"^^xsd:date ;
    sto:hasPublisher sto:IEC,
        sto:ISO ;
    sto:relatedTo sto:IEC_61158 .

sto:IEC_29190 a owl:NamedIndividual ;
    owl:sameAs sto:ISO_29190 .

sto:IEC_42010 a <http://dbpedia.org/class/yago/WikicatISO/IECStandards>,
        dbont:Work,
        owl:NamedIndividual,
        sto:Standard ;
    rdfs:label "IEC 42010"@en ;
    dcterms:subject dbrc:IEEE_standards,
        <http://dbpedia.org/resource/Category:ISO/IEC_standards>,
        dbrc:Software_architecture ;
    lingg:hypernym dbres:Standard ;
    rdfs:comment "ISO/IEC/IEEE 42010:2011 defines requirements on the description of system, software and enterprise architectures. It aims to standardise the practice of architecture description by defining standard terms, presenting a conceptual foundation for expressing, communicating and reviewing architectures and specifying requirements that apply to architecture descriptions, architecture frameworks and architecture description languages."@en ;
    skos:note "The IIRA is based on this standards" ;
    sto:hasDBpediaResource <http://dbpedia.org/page/ISO/IEC_42010> ;
    sto:hasOfficialResource <http://www.iso-architecture.org/ieee-1471/> ;
    sto:hasPublisher sto:IEC,
        sto:ISO ;
    sto:hasTag "ISO/IEC/IEEE 42010"@en ;
    sto:hasWikipediaArticle <https://en.wikipedia.org/wiki/ISO/IEC_42010> .

sto:IEC_60027_2006 a dbpcy:WikicatIECStandards,
        dbpcy:WikicatStandards,
        dbont:Organisation,
        owl:NamedIndividual,
        sto:Standard ;
    rdfs:label "IEC 60027-6:2006"@en ;
    dcterms:subject dbrc:IEC_standards ;
    dcterms:title "Letter symbols to be used in electrical technology - Part 6: Control technology"@en ;
    lingg:hypernym dbres:Commission ;
    rdfs:comment "This part of IEC 60027 is applicable to control technology. It gives names and symbols for quantities, signals and functions, and their units."@en ;
    sto:hasAvailableLanguage lang:eng,
        lang:fra,
        lang:spa ;
    sto:hasDBpediaResource <http://dbpedia.org/page/IEC_60027> ;
    sto:hasEdition "1.0"^^xsd:float ;
    sto:hasFileSize sto:FileSizeIEC_60027_2006 ;
    sto:hasICS sto:ICS_01_060 ;
    sto:hasImplementationFormat "Document"@en ;
    sto:hasOfficialResource <https://webstore.iec.ch/publication/96> ;
    sto:hasPages "29"^^xsd:int ;
    sto:hasPublicationDate "2006-12-14"^^xsd:date ;
    sto:hasPublisher sto:IEC ;
    sto:hasStabilityDate "2019-01-01"^^xsd:gYear ;
    sto:hasStatus "Valid"@en ;
    sto:hasTag "IEC 60027:2006"@en ;
    sto:hasTechnicalCommittee sto:TC_25 ;
    sto:hasWikipediaArticle <https://en.wikipedia.org/wiki/IEC_60027> .

sto:IEC_60038_2009 a dbpcy:WikicatIECStandards,
        owl:NamedIndividual,
        sto:Standard ;
    rdfs:label "IEC 60038:2009"@en ;
    dcterms:subject dbrc:Electric_power_distribution,
        dbrc:Electrical_wiring,
        dbrc:IEC_standards ;
    dcterms:title "IEC standard voltages"@en ;
    rdfs:comment "IEC 60038:2009 specifies standard voltage values which are intended to serve as preferential values for the nominal voltage of electrical supply systems, and as reference values for equipment and system design. This seventh edition supersedes the sixth edition (1993), its Amendment 1 (1994) and its Amendment 2 (1997). It constitutes a technical revision. The significant technical changes are: -the addition of the values of 230 V (50 Hz) and 230/400 V (60 Hz) to Table 1;-the replacement of the utilization voltage range at LV by a reference to the relevant standard and an informative annex;- the addition of the value of 30 kV to Table 3;- the replacement of the value of 1 050 kV by 1 100 kV in Table 5. It has the status of a horizontal standard in accordance with IEC Guide 108."@en ;
    sto:hasAvailableLanguage lang:eng,
        lang:fra,
        lang:spa ;
    sto:hasDBpediaResource <http://dbpedia.org/page/IEC_60038> ;
    sto:hasEdition "7.0"^^xsd:float ;
    sto:hasFileSize sto:FileSizeIEC_60038_2009 ;
    sto:hasICS sto:ICS_29_020 ;
    sto:hasImplementationFormat "Document"@en ;
    sto:hasOfficialResource <https://webstore.iec.ch/publication/153> ;
    sto:hasPages "26"^^xsd:int ;
    sto:hasPublicationDate "2009-06-17"^^xsd:date ;
    sto:hasPublisher sto:IEC ;
    sto:hasStabilityDate "2020-01-01"^^xsd:gYear ;
    sto:hasStatus "Valid"@en ;
    sto:hasTag "IEC 60038:2009"@en ;
    sto:hasTechnicalCommittee sto:TC_8 ;
    sto:hasWikipediaArticle <https://en.wikipedia.org/wiki/IEC_60038> .

sto:IEC_60050_1984 a owl:NamedIndividual,
        sto:Standard ;
    rdfs:label "IEC 60050-371:1984"@en ;
    dcterms:title "International Electrotechnical Vocabulary. Chapter 371: Telecontrol"@en ;
    rdfs:comment "Terms on telecontrol, teleprotection and associated telecommunications for electric power systems. It has the status of a horizontal standard in accordance with IEC Guide 108."@en ;
    sto:hasAvailableLanguage lang:en,
        lang:fra,
        lang:rus ;
    sto:hasEdition "1.0"^^xsd:float ;
    sto:hasFileSize sto:FileSizeIEC_60050_1984 ;
    sto:hasICS sto:ICS_01_040_35,
        sto:ICS_35_240_50 ;
    sto:hasImplementationFormat "Document"@en ;
    sto:hasOfficialResource <https://webstore.iec.ch/publication/196> ;
    sto:hasPages "44"^^xsd:int ;
    sto:hasPublicationDate "1984-11-30"^^xsd:date ;
    sto:hasPublisher sto:IEC ;
    sto:hasStatus "Valid"@en ;
    sto:hasTag "IEC 60050-371:1984"@en ;
    sto:hasTechnicalCommittee sto:TC_1 .

sto:IEC_60050_1998 a dbont:Agent,
        dbont:Organisation,
        schema:Organization,
        dul:Agent,
        dul:SocialPerson,
        owl:NamedIndividual,
        owl:Thing,
        wike:Q24229398,
        wike:Q43229,
        sto:Standard ;
    rdfs:label "IEC 60050-101:1998"@en ;
    dcterms:subject dbrc:International_Electrotechnical_Commission,
        dbrc:Standards_organizations ;
    dcterms:title "International Electrotechnical Vocabulary - Part 101: Mathematics"@en ;
    rdfs:comment "It has the status of a horizontal standard in accordance with IEC Guide 108."@en ;
    sto:hasAvailableLanguage lang:eng,
        lang:fra,
        lang:spa ;
    sto:hasDBpediaResource <http://dbpedia.org/page/International_Electrotechnical_Vocabulary> ;
    sto:hasEdition "2.0"^^xsd:float ;
    sto:hasFileSize sto:FileSizeIEC_60050_1998 ;
    sto:hasICS sto:ICS_01_040_07 ;
    sto:hasImplementationFormat "Document"@en ;
    sto:hasOfficialResource <https://webstore.iec.ch/publication/159> ;
    sto:hasPages 129,
        "129"^^xsd:int ;
    sto:hasPublicationDate "1998-04-30"^^xsd:date ;
    sto:hasPublisher sto:IEC ;
    sto:hasStatus "Replaced"@en ;
    sto:hasTag "IEC 60050-101:1998"@en ;
    sto:hasTechnicalCommittee sto:TC_1 ;
    sto:hasWikipediaArticle <https://en.wikipedia.org/wiki/International_Electrotechnical_Vocabulary> .

sto:IEC_60050_2013 a owl:NamedIndividual,
        sto:Standard ;
    rdfs:label "IEC 60050-351:2013"@en ;
    dcterms:title "International Electrotechnical Vocabulary - Part 351: Control technology"@en ;
    rdfs:comment "IEC 60050-351:2013 gives the general terminology used in control technology, as well as general terms pertaining to specific applications and associated technologies. This new edition reviews and complements the previous one. It has the status of a horizontal standard in accordance with IEC Guide 108."@en ;
    sto:hasAvailableLanguage lang:eng,
        lang:fra ;
    sto:hasEdition "4.0"^^xsd:float ;
    sto:hasFileSize sto:FileSizeIEC_60050_2013 ;
    sto:hasICS sto:ICS_01_040_07,
        sto:ICS_25_040_40 ;
    sto:hasImplementationFormat "Document"@en ;
    sto:hasOfficialResource <https://webstore.iec.ch/publication/194> ;
    sto:hasPages "457"^^xsd:int ;
    sto:hasPublicationDate "2013-11-25"^^xsd:date ;
    sto:hasPublisher sto:IEC ;
    sto:hasStatus "Valid"@en ;
    sto:hasTag "IEC 60050-351:2013"@en ;
    sto:hasTechnicalCommittee sto:TC_1 .

sto:IEC_60073_2002 a owl:NamedIndividual,
        sto:Standard ;
    rdfs:label "IEC 60073:2002 "@en ;
    dcterms:title "Basic and safety principles for man-machine interface, marking and identification - Coding principles for indicators and actuators"@en ;
    rdfs:comment "Establishes general rules for assigning particular meanings to certain visual, acoustsic and tactile indications. It has the status of a Basic Safety Publication in accordance with IEC Guide 104."@en ;
    sto:hasAvailableLanguage lang:eng,
        lang:fra,
        lang:spa ;
    sto:hasEdition "6.0"^^xsd:float ;
    sto:hasFileSize sto:FileSizeIEC_60073_2002 ;
    sto:hasICS sto:ICS_01_070,
        sto:ICS_29_020 ;
    sto:hasImplementationFormat "Document"@en ;
    sto:hasOfficialResource <https://webstore.iec.ch/publication/587> ;
    sto:hasPages "61"^^xsd:int ;
    sto:hasPublicationDate "2002-05-22"^^xsd:date ;
    sto:hasPublisher sto:IEC ;
    sto:hasStabilityDate "2025-01-01"^^xsd:gYear ;
    sto:hasStatus "Valid"@en ;
    sto:hasTag "IEC_60073:2002"@en ;
    sto:hasTechnicalCommittee sto:TC_3 .

sto:IEC_60086 a owl:NamedIndividual,
        sto:Standard ;
    rdfs:label "IEC 60086"@en ;
    rdfs:comment "Standard battery nomenclature describes portable dry cell batteries that have physical dimensions and electrical characteristics interchangeable between manufacturers."@en ;
    sto:hasDBpediaResource <http://dbpedia.org/page/Battery_nomenclature#IEC_60086> ;
    sto:hasOfficialResource <https://webstore.iec.ch/publication/22991> ;
    sto:hasPublisher sto:IEC ;
    sto:hasWikipediaArticle <https://en.wikipedia.org/wiki/Battery_nomenclature#IEC_60086> .

sto:IEC_60204_2000 a owl:NamedIndividual,
        sto:Standard ;
    rdfs:label "IEC 60204-11:2000"@en ;
    dcterms:title "Safety of machinery - Electrical equipment of machines - Part 11: Requirements for HV equipment for voltages above 1 000 V a.c. or 1 500 V d.c. and not exceeding 36 kV"@en ;
    rdfs:comment "Applies to the electrical and electronic equipment and systems of machines, including a group of machines working together in a coordinated manner, but excluding higher level system aspects (i.e. communications between systems)."@en ;
    sto:hasAvailableLanguage lang:eng,
        lang:fra,
        lang:spa ;
    sto:hasEdition "1.0"^^xsd:float ;
    sto:hasFileSize sto:FileSizeIEC_60204_2000 ;
    sto:hasICS sto:ICS_13_110,
        sto:ICS_29_020 ;
    sto:hasImplementationFormat "Document"@en ;
    sto:hasOfficialResource <https://webstore.iec.ch/publication/1022> ;
    sto:hasPages "111"^^xsd:int ;
    sto:hasPublicationDate "2000-07-31"^^xsd:date ;
    sto:hasPublisher sto:IEC ;
    sto:hasStabilityDate "2018-01-01"^^xsd:gYear ;
    sto:hasStatus "Valid"@en ;
    sto:hasTag "IEC 60204:2000"@en ;
    sto:hasTechnicalCommittee sto:TC_44 .

sto:IEC_60255_149_2013 a owl:NamedIndividual,
        sto:Standard ;
    rdfs:label "IEC 60255-149:2013 "@en ;
    dcterms:title "Measuring relays and protection equipment - Part 149: Functional requirements for thermal electrical relays"@en ;
    rdfs:comment "IEC 60255-149:2013 specifies minimum requirements for thermal protection relays. This standard includes specification of the protection function, measurement characteristics and test methodologies. The object is to establish a common and reproducible reference for evaluating dependent time relays which protect equipment from thermal damage by measuring a.c. current flowing through the equipment. Complementary input energizing quantities such as ambient, coolant, top oil and winding temperature may be applicable for the thermal protection specification set forth in this standard. This standard covers protection relays based on a thermal model with memory function."@en ;
    sto:hasAvailableLanguage lang:eng,
        lang:fra ;
    sto:hasEdition "1.0"^^xsd:float ;
    sto:hasFileSize sto:FileSizeIEC_60255_149_2013 ;
    sto:hasICS sto:ICS_29_120_70 ;
    sto:hasImplementationFormat "Document"@en ;
    sto:hasOfficialResource <https://webstore.iec.ch/publication/1165> ;
    sto:hasPages "93"^^xsd:int ;
    sto:hasPublicationDate "2013-07-30"^^xsd:date ;
    sto:hasPublisher sto:IEC ;
    sto:hasStatus "Valid"@en ;
    sto:hasTag "IEC 60255-149:2013 "@en ;
    sto:hasTechnicalCommittee sto:TC_95 .

sto:IEC_60255_151_2009 a owl:NamedIndividual,
        sto:Standard ;
    rdfs:label "IEC 60255-151:2009 "@en ;
    dcterms:title "Measuring relays and protection equipment - Part 151: Functional requirements for over/under current protection"@en ;
    rdfs:comment "IEC 60255-151:2009 specifies minimum requirements for over/under current relays. It includes a specification of the protection function, measurement characteristics and time delay characteristics. Defines the influencing factors that affect the accuracy under steady state conditions and performance characteristics during dynamic conditions."@en ;
    sto:hasAvailableLanguage lang:eng,
        lang:fra ;
    sto:hasEdition "1.0"^^xsd:float ;
    sto:hasFileSize sto:FileSizeIEC_60255_151_2009 ;
    sto:hasICS sto:ICS_29_120_70 ;
    sto:hasImplementationFormat "Document"@en ;
    sto:hasOfficialResource <https://webstore.iec.ch/publication/1166> ;
    sto:hasPages "63"^^xsd:int ;
    sto:hasPublicationDate "2009-08-28"^^xsd:date ;
    sto:hasPublisher sto:IEC ;
    sto:hasStatus "Valid"@en ;
    sto:hasTag "IEC 60255-151:2009 "@en ;
    sto:hasTechnicalCommittee sto:TC_95 .

sto:IEC_60255_2009 a owl:NamedIndividual,
        sto:Standard ;
    rdfs:label "IEC 60255-1:2009 "@en ;
    dcterms:title "Measuring relays and protection equipment - Part 1: Common requirements"@en ;
    rdfs:comment "IEC 60255-1:2009 specifies common rules and requirements applicable to measuring relays and protection equipment including any combination of devices to form schemes for power system protection such as control, monitoring and process interface equipment in order to obtain uniformity of requirements and tests. Covers all measuring relays and protection equipment used for protection within the power system environment."@en ;
    sto:hasAvailableLanguage lang:eng,
        lang:fra,
        lang:spa ;
    sto:hasEdition "1.0"^^xsd:float ;
    sto:hasFileSize sto:FileSizeIEC_60255_2009 ;
    sto:hasICS sto:ICS_29_120_70 ;
    sto:hasImplementationFormat "Document"@en ;
    sto:hasOfficialResource <https://webstore.iec.ch/publication/1160> ;
    sto:hasPages "89"^^xsd:int ;
    sto:hasPublicationDate "2009-08-18"^^xsd:date ;
    sto:hasPublisher sto:IEC ;
    sto:hasStabilityDate "2018-01-01"^^xsd:gYear ;
    sto:hasStatus "Valid"@en ;
    sto:hasTag "IEC 60255-1:2009 "@en ;
    sto:hasTechnicalCommittee sto:TC_95 .

sto:IEC_60255_2010 a owl:NamedIndividual,
        sto:Standard ;
    rdfs:label "IEC 60255-127:2010"@en,
        "IEC 60255-149:2013 "@en ;
    dcterms:title "Measuring relays and protection equipment - Part 127: Functional requirements for over/under voltage protection"@en ;
    rdfs:comment "IEC 60255-127:2010 specifies minimum requirements for over/under voltage relays. The standard includes specification of the protection function, measurement characteristics and time delay characteristics."@en ;
    sto:hasAvailableLanguage lang:eng,
        lang:fra ;
    sto:hasEdition "1.0"^^xsd:float ;
    sto:hasFileSize sto:FileSizeIEC_60255_2010 ;
    sto:hasICS sto:ICS_29_120_70 ;
    sto:hasImplementationFormat "Document"@en ;
    sto:hasOfficialResource <https://webstore.iec.ch/publication/1165> ;
    sto:hasPages "93"^^xsd:int ;
    sto:hasPublicationDate "2010-04-27"^^xsd:date ;
    sto:hasPublisher sto:IEC ;
    sto:hasStatus "Valid"@en ;
    sto:hasTag "IEC 60255-127:2010"@en,
        "IEC 60255-149:2013 "@en ;
    sto:hasTechnicalCommittee sto:TC_95 .

sto:IEC_60255_2013 a owl:NamedIndividual,
        sto:Standard ;
    rdfs:label "IEC 60255-27:2013 "@en ;
    dcterms:title "Measuring relays and protection equipment - Part 27: Product safety requirements"@en ;
    rdfs:comment "IEC 60255-27:2013 describes the product safety requirements for measuring relays and protection equipment having a rated a.c. voltage up to 1 000 V with a rated frequency up to 65 Hz, or a rated d.c. voltage up to 1 500 V. Above these limits, IEC 60664-1 is applicable for the determination of clearance, creepage distance and withstand test voltage. This standard details essential safety requirements to minimize the risk of fire and hazards caused by electric shock or injury to the user. This new edition includes the following significant technical changes with respect to the previous edition:- the removal of tables and diagrams which are from other standards and referring instead directly to the source standard;- all aspects of IEC 60255-5 have been covered and this standard will be withdrawn."@en ;
    sto:hasAvailableLanguage lang:eng,
        lang:fra ;
    sto:hasEdition "2.0"^^xsd:float ;
    sto:hasFileSize sto:FileSizeIEC_60255_2013 ;
    sto:hasICS sto:ICS_29_120_70 ;
    sto:hasImplementationFormat "Document"@en ;
    sto:hasOfficialResource <https://webstore.iec.ch/publication/1172> ;
    sto:hasPages "197"^^xsd:int ;
    sto:hasPublicationDate "2013-10-15"^^xsd:date ;
    sto:hasPublisher sto:IEC ;
    sto:hasStabilityDate "2018-01-01"^^xsd:gYear ;
    sto:hasStatus "Valid"@en ;
    sto:hasTag "IEC 60255-27:2013 "@en ;
    sto:hasTechnicalCommittee sto:TC_95 .

sto:IEC_60286_3_2013 a owl:NamedIndividual,
        sto:Standard ;
    rdfs:label "IEC 60286-3:2013"@en ;
    dcterms:title "Packaging of components for automatic handling - Part 3: Packaging of surface mount components on continuous tapes"@en ;
    rdfs:comment "IEC 60286-3:2013 is applicable to the tape packaging of electronic components without leads or with lead stumps, intended to be connected to electronic circuits. It includes only those dimensions that are essential for the taping of components intended for the above-mentioned purposes. This standard also includes requirements related to the packaging of singulated die products including bare die and bumped die (flip chips). This fifth edition cancels and replaces the fourth edition, published in 2007, as well as IEC 60286-3-1, published in 2009 and IEC 60286-3-2, published in 2009. It constitutes a full layout revision. In addition, this edition includes the following significant technical changes with respect to the previous edition:a) IEC 60286-3:2013 is applicable to the tape packaging of electronic components without leads or with lead stumps, intended to be connected to electronic circuits. It includes only those dimensions that are essential for the taping of components intended for the above-mentioned purposes. This standard also includes requirements related to the packaging of singulated die products including bare die and bumped die (flip chips). This fifth edition cancels and replaces the fourth edition, published in 2007, as well as IEC 60286-3-1, published in 2009 and IEC 60286-3-2, published in 2009.It constitutes a full layout revision. In addition, this edition includes the following significant technical changes with respect to the previous edition:a) integration of IEC 60286-3-1:2009 as type 1b (Packaging of surface mount components on continuous pressed carrier tapes);b) integration of IEC 60286-3-2:2009 as type 2b (Packaging of surface mount components on blister carrier tapes 4 mm in width).ntegration of IEC 60286-3-1:2009 as type 1b (Packaging of surface mount components on continuous pressed carrier tapes);b) integration of IEC 60286-3-2:2009 as type 2b (Packaging of surface mount components on blister carrier tapes 4 mm in width)."@en ;
    sto:hasAvailableLanguage lang:eng,
        lang:fra ;
    sto:hasEdition "5.0"^^xsd:float ;
    sto:hasFileSize sto:FileSizeIEC_60286_3_2013 ;
    sto:hasICS sto:ICS_31_020,
        sto:ICS_31_240 ;
    sto:hasImplementationFormat "Document"@en ;
    sto:hasOfficialResource <https://webstore.iec.ch/publication/1258> ;
    sto:hasPages "77"^^xsd:int ;
    sto:hasPublicationDate "2013-05-17"^^xsd:date ;
    sto:hasPublisher sto:IEC ;
    sto:hasStabilityDate "2024-01-01"^^xsd:gYear ;
    sto:hasStatus "Valid"@en ;
    sto:hasTag "IEC 60286-3:2013"@en ;
    sto:hasTechnicalCommittee sto:TC_40 .

sto:IEC_60286_4_2013 a owl:NamedIndividual,
        sto:Standard ;
    rdfs:label "IEC 60286-3:2013"@en ;
    dcterms:title "Packaging of components for automatic handling - Part 4: Stick magazines for electronic components encapsulated in packages of different forms"@en ;
    rdfs:comment "IEC 60286-4:2013 is applicable to stick magazines (including end stoppers) intended to be used for storage of electronic components, for transport from the manufacturer to the customer and for in-house use in the manufacturing plant. They are also used to feed automatic placement machines for surface mounting as well as for through-hole mounting of electronic components. This edition includes the following significant technical changes with respect to the previous edition: Clause 4 describes the guidelines for customer specific stick magazine design. It replaces the magazine design rules for IEC outlined components and rules for orientation of components in stick magazines which have been moved to Annexes A to D."@en ;
    sto:hasAvailableLanguage lang:eng,
        lang:fra ;
    sto:hasEdition "3.0"^^xsd:float ;
    sto:hasFileSize sto:FileSizeIEC_60286_4_2013 ;
    sto:hasICS sto:ICS_31_020,
        sto:ICS_31_240 ;
    sto:hasImplementationFormat "Document"@en ;
    sto:hasOfficialResource <https://webstore.iec.ch/publication/1259> ;
    sto:hasPages "32"^^xsd:int ;
    sto:hasPublicationDate "2013-07-26"^^xsd:date ;
    sto:hasPublisher sto:IEC ;
    sto:hasStabilityDate "2022-01-01"^^xsd:gYear ;
    sto:hasStatus "Valid"@en ;
    sto:hasTag "IEC 60286-3:2013"@en ;
    sto:hasTechnicalCommittee sto:TC_40 .

sto:IEC_60286_5_2018 a owl:NamedIndividual,
        sto:Standard ;
    rdfs:label "IEC 60286-5:2018"@en ;
    dcterms:title "Packaging of components for automatic handling - Part 5: Matrix trays"@en ;
    rdfs:comment "IEC 60286-5:2018 RLV contains the International Standard and its Redline version. The Redline version is available in English only. The Redline version provides you with a quick and easy way to compare all the changes between this standard and its previous edition. The Redline version is not an official IEC Standard, only the current version of the standard is to be considered the official document.IEC 60286-5:2018 describes the common dimensions, tolerances and characteristics of the tray. It includes only those dimensions that are essential for the handling of the trays for the stated purpose and for placing or removing components from the trays. This edition includes the following significant technical changes with respect to the previous edition: - The generic rules for the design of matrix trays are given in this document. Newly developed trays which follow these rules will not be listed individually. Only those trays which conform to the design rules set forth herein are classified as 'standard trays' and are thus preferred for use.- An update of the matrix trays, which do not conform to the design rules set forth herein, are considered as 'non-standard trays' and are not preferred for use, is listed in Annex A."@en ;
    sto:hasAvailableLanguage lang:eng ;
    sto:hasEdition "3.0"^^xsd:float ;
    sto:hasFileSize sto:FileSizeIEC_60286_5_2018 ;
    sto:hasICS sto:ICS_31_020 ;
    sto:hasImplementationFormat "Document"@en ;
    sto:hasOfficialResource <https://webstore.iec.ch/publication/63037> ;
    sto:hasPages "71"^^xsd:int ;
    sto:hasPublicationDate "2018-04-25"^^xsd:date ;
    sto:hasPublisher sto:IEC ;
    sto:hasStabilityDate "2024-01-01"^^xsd:gYear ;
    sto:hasStatus "RLV-Redline version"@en ;
    sto:hasTag "IEC 60286-5:2018"@en ;
    sto:hasTechnicalCommittee sto:TC_40 .

sto:IEC_60364 a dbpcy:WikicatIECStandards,
        dbont:Organisation,
        owl:NamedIndividual,
        sto:Standard ;
    rdfs:label "IEC 60364"@en ;
    dcterms:subject dbrc:Electric_power_distribution,
        dbrc:IEC_standards ;
    lingg:hypernym dbres:Commission ;
    rdfs:comment "Electrical Installations for Buildings is the International Electrotechnical Commission's international standard on electrical installations of buildings"@en ;
    sto:hasDBpediaResource <http://dbpedia.org/page/IEC_60364> ;
    sto:hasPublisher sto:IEC ;
    sto:hasWikipediaArticle <https://en.wikipedia.org/wiki/IEC_60364> .

sto:IEC_60381_1978 a owl:NamedIndividual,
        sto:Standard ;
    rdfs:label "IEC 60381-2:1978"@en ;
    dcterms:title "Analogue signals for process control systems. Part 2: Direct voltage signals"@en ;
    rdfs:comment "Applicable to analogue direct voltage signals used in industrial process measurement and control systems. lt specifies ranges of analogue direct voltage signals and the signal common; it also deals with ripple content. The analogue direct voltage signal, unlike the analogue direct current signal specified in IEC 60381-1, is not intended for transmission over long distances. This standard does not apply to signals used entirely within an element."@en ;
    sto:hasAvailableLanguage lang:en,
        lang:fra,
        lang:rus ;
    sto:hasEdition "1.0"^^xsd:float ;
    sto:hasFileSize sto:FileSizeIEC_60381_1978 ;
    sto:hasICS sto:ICS_33_200,
        sto:ICS_35_240_50 ;
    sto:hasImplementationFormat "Document"@en ;
    sto:hasOfficialResource <https://webstore.iec.ch/publication/1949> ;
    sto:hasPages "9"^^xsd:int ;
    sto:hasPublicationDate "1978-01-01"^^xsd:date ;
    sto:hasPublisher sto:IEC ;
    sto:hasStabilityDate "2018-01-01"^^xsd:gYear ;
    sto:hasStatus "Valid"@en ;
    sto:hasTag "IEC 60381-2:1978"@en ;
    sto:hasTechnicalCommittee sto:TC_65 .

sto:IEC_60381_1982 a owl:NamedIndividual,
        sto:Standard ;
    rdfs:label "IEC 60381-1:1982"@en ;
    dcterms:title "Analogue signals for process control systems. Part 1: Direct current signals"@en ;
    rdfs:comment "Applicable to analogue direct current signals used in industrial-process measurement and control systems to transmit information between elements of systems. Does not apply to signals used entirely within an element."@en ;
    sto:hasAvailableLanguage lang:eng,
        lang:fra ;
    sto:hasEdition "2.0"^^xsd:float ;
    sto:hasFileSize sto:FileSizeIEC_60381_1982 ;
    sto:hasICS sto:ICS_33_200 ;
    sto:hasImplementationFormat "Document"@en ;
    sto:hasOfficialResource <https://webstore.iec.ch/publication/1948> ;
    sto:hasPages "9"^^xsd:int ;
    sto:hasPublicationDate "1982-01-01"^^xsd:date ;
    sto:hasPublisher sto:IEC ;
    sto:hasStabilityDate "2018-01-01"^^xsd:gYear ;
    sto:hasStatus "Valid"@en ;
    sto:hasTag "IEC 60381-1:1982"@en ;
    sto:hasTechnicalCommittee sto:TC_40 .

sto:IEC_60382 a owl:NamedIndividual,
        sto:Standard ;
    rdfs:label "IEC 60382:1991"@en ;
    dcterms:title "Analogue pneumatic signal for process control systems"@en ;
    rdfs:comment "Applies to analogue pneumatic signals used in process control systems to transmit information between the elements of systems and gives definitions, units and the recommended value of the range of the analogue pneumatic signal."@en ;
    sto:hasAvailableLanguage lang:eng,
        lang:fra ;
    sto:hasEdition "2.0"^^xsd:float ;
    sto:hasFileSize sto:FileSizeIEC_60382 ;
    sto:hasICS sto:ICS_25_040_40 ;
    sto:hasOfficialResource <https://webstore.iec.ch/publication/1950> ;
    sto:hasPages "9"^^xsd:int ;
    sto:hasPublicationDate "1991-11-01"^^xsd:date ;
    sto:hasPublisher sto:IEC ;
    sto:hasStabilityDate "2018-01-01"^^xsd:gYear ;
    sto:hasTag "IEC 60382:1991"@en ;
    sto:hasTechnicalCommittee sto:TC_65 .

sto:IEC_60382_1991 a owl:NamedIndividual,
        sto:Standard ;
    rdfs:label "IEC 60382:1991"@en ;
    dcterms:title "Analogue pneumatic signal for process control systems"@en ;
    rdfs:comment "Applies to analogue pneumatic signals used in process control systems to transmit information between the elements of systems and gives definitions, units and the recommended value of the range of the analogue pneumatic signal."@en ;
    sto:hasAvailableLanguage lang:eng,
        lang:fra ;
    sto:hasEdition "2.0"^^xsd:float ;
    sto:hasFileSize sto:FileSizeIEC_60382_1991 ;
    sto:hasICS sto:ICS_25_040_40 ;
    sto:hasImplementationFormat "Document"@en ;
    sto:hasOfficialResource <https://webstore.iec.ch/publication/1950> ;
    sto:hasPages "9"^^xsd:int ;
    sto:hasPublicationDate "1991-11-01"^^xsd:date ;
    sto:hasPublisher sto:IEC ;
    sto:hasStabilityDate "2018-01-01"^^xsd:gYear ;
    sto:hasStatus "Valid"@en ;
    sto:hasTag "IEC 60382:1991"@en ;
    sto:hasTechnicalCommittee sto:TC_65 .

sto:IEC_60839-5-2 a owl:NamedIndividual,
        sto:Standard ;
    rdfs:label "IEC 60839-5-2"@en ;
    rdfs:comment "IEC 60839-5-2:2016 specifies the general equipment requirements for the performance, reliability, resilience, security and safety characteristics of supervised premises transceiver (SPT) installed in supervised premises and used in alarm transmission systems (ATS). A supervised premises transceiver can be a stand-alone device or an integrated part of an alarm system. These requirements also apply to the SPT sharing means of interconnection, control, communication and power supplies with other applications. The alarm transmission system requirements and classifications are defined within IEC 60839-5-1. This new edition includes the following significant technical changes with respect to the previous edition: reflects the current technological state of art (IP networks) ,harmonizes with the ATS categories introduced in IEC 60839-5-1:2014; introduces test requirements."@en ;
    sto:hasClassification rami:Communication,
        rami:ControlDevice,
        rami:FieldDevice,
        rami:Security ;
    sto:hasOfficialResource <https://webstore.iec.ch/publication/24120> ;
    sto:hasPublicationDate "2016-02-03"^^xsd:date ;
    sto:hasPublisher sto:IEC .

sto:IEC_60839_P7_1 a owl:NamedIndividual,
        sto:Standard ;
    rdfs:label "IEC 60839-7-1:2001"@en ;
    dcterms:title "Alarm systems - Part 7-1: Message formats and protocols for serial data interfaces in alarm transmission systems – General"@en ;
    rdfs:comment "Describes the requirements for standard serial data interfaces in alarm transmission systems. Gives an outline of how alarm transmission systems are connected and the various types of serial data interfaces that might be employed."@en ;
    sto:hasAvailableLanguage lang:eng,
        lang:fra ;
    sto:hasEdition "1.0"^^xsd:float ;
    sto:hasFileSize sto:FileSizeIEC_60839_P7_1 ;
    sto:hasICS sto:ICS_13_320 ;
    sto:hasOfficialResource <https://webstore.iec.ch/publication/3666> ;
    sto:hasPages "39"^^xsd:int ;
    sto:hasPublicationDate "1968-03-01"^^xsd:date,
        "2001-03-09"^^xsd:date ;
    sto:hasPublisher sto:IEC ;
    sto:hasStabilityDate "2018-01-01"^^xsd:gYear ;
    sto:hasTag "IEC 60839-7-1:2001"@en ;
    sto:hasTechnicalCommittee sto:TC_79 .

sto:IEC_60839_P7_2 a owl:NamedIndividual,
        sto:Standard ;
    rdfs:label "IEC 60839-7-2:2001"@en ;
    dcterms:title "Alarm systems - Part 7-2: Message formats and protocols for serial data interfaces in alarm transmission systems - Common application layer protocol"@en ;
    rdfs:comment "Specifies a common application layer protocol (message structure, formats and transmission procedures) to be used at standard interfaces in alarm transmission systems. Should be used at all such interfaces where equipment from one supplier is intended to inter-work with equipment from other suppliers."@en ;
    sto:hasAvailableLanguage lang:eng,
        lang:fra ;
    sto:hasEdition "1.0"^^xsd:float ;
    sto:hasFileSize sto:FileSizeIEC_60839_P7_2 ;
    sto:hasICS sto:ICS_13_320 ;
    sto:hasOfficialResource <https://webstore.iec.ch/publication/3669> ;
    sto:hasPages "53"^^xsd:int ;
    sto:hasPublicationDate "1968-03-01"^^xsd:date,
        "2001-03-09"^^xsd:date ;
    sto:hasPublisher sto:IEC ;
    sto:hasStabilityDate "2018-01-01"^^xsd:gYear ;
    sto:hasTag "IEC 60839-7-2:2001"@en ;
    sto:hasTechnicalCommittee sto:TC_79 .

sto:IEC_60839_P7_3 a owl:NamedIndividual,
        sto:Standard ;
    rdfs:label "IEC 60839-7-3:2001"@en ;
    dcterms:title "Alarm systems - Part 7-3: Message formats and protocols for serial data interfaces in alarm transmission systems - Common data link layer protocol"@en ;
    rdfs:comment "Specifies the data link layer message structure, formats and transmission procedures which should be used at standard serial data interfaces in alarm transmission systems where the transmission network employed does not offer a standard protocol. Is necessary in order to ensure compatibility of equipment from different suppliers."@en ;
    sto:hasAvailableLanguage lang:eng,
        lang:fra ;
    sto:hasEdition "1.0"^^xsd:float ;
    sto:hasFileSize sto:FileSizeIEC_60839_P7_3 ;
    sto:hasICS sto:ICS_13_320 ;
    sto:hasOfficialResource <https://webstore.iec.ch/publication/3671> ;
    sto:hasPages "29"^^xsd:int ;
    sto:hasPublicationDate "1968-03-01"^^xsd:date,
        "2001-03-09"^^xsd:date ;
    sto:hasPublisher sto:IEC ;
    sto:hasStabilityDate "2018-01-01"^^xsd:gYear ;
    sto:hasTag "IEC 60839-7-3:2001"@en ;
    sto:hasTechnicalCommittee sto:TC_79 .

sto:IEC_60839_P7_4 a owl:NamedIndividual,
        sto:Standard ;
    rdfs:label "IEC 60839-7-4:2001"@en ;
    dcterms:title "Alarm systems - Part 7-4: Message formats and protocols for serial data interfaces in alarm transmission systems - Common transport layer protocol"@en ;
    rdfs:comment "Specifies the transport layer message structure, formats and transmission procedures to be used at standard interfaces in alarm transmission systems. Should be used at all such interfaces where equipment from one supplier is intended to inter-work with equipment from other suppliers, and where the underlying system architecture does not provide the necessary facilities to support the common application layer."@en ;
    sto:hasAvailableLanguage lang:eng,
        lang:fra ;
    sto:hasEdition "1.0"^^xsd:float ;
    sto:hasFileSize sto:FileSizeIEC_60839_P7_4 ;
    sto:hasICS sto:ICS_13_320 ;
    sto:hasOfficialResource <https://webstore.iec.ch/publication/3672> ;
    sto:hasPages "23"^^xsd:int ;
    sto:hasPublicationDate "1968-03-01"^^xsd:date,
        "2001-03-09"^^xsd:date ;
    sto:hasPublisher sto:IEC ;
    sto:hasStabilityDate "2018-01-01"^^xsd:gYear ;
    sto:hasTag "IEC 60839-7-4:2001"@en ;
    sto:hasTechnicalCommittee sto:TC_79 .

sto:IEC_60839_P7_5 a owl:NamedIndividual,
        sto:Standard ;
    rdfs:label "IEC 60839-7-5:2001"@en ;
    dcterms:title "Alarm systems - Part 7-5: Message formats and protocols for serial data interfaces in alarm transmission systems - Alarm system interfaces employing a two-wire configuration in accordance with ISO/IEC 8482"@en ;
    rdfs:comment "Specifies the requirements for standard interfaces using a two-wire connection employing ISO/IEC 8482 signalling for use between the control and indicating equipment of an alarm system and one or more alarm system transceivers connected to alarm transmission systems."@en ;
    sto:hasAvailableLanguage lang:eng,
        lang:fra ;
    sto:hasEdition "1.0"^^xsd:float ;
    sto:hasFileSize sto:FileSizeIEC_60839_P7_5 ;
    sto:hasICS sto:ICS_13_320 ;
    sto:hasOfficialResource <https://webstore.iec.ch/publication/3673> ;
    sto:hasPages "13"^^xsd:int ;
    sto:hasPublicationDate "1968-03-01"^^xsd:date,
        "2001-03-09"^^xsd:date ;
    sto:hasPublisher sto:IEC ;
    sto:hasStabilityDate "2018-01-01"^^xsd:gYear ;
    sto:hasTag "IEC 60839-7-5:2001"@en ;
    sto:hasTechnicalCommittee sto:TC_79 .

sto:IEC_60839_P7_6 a owl:NamedIndividual,
        sto:Standard ;
    rdfs:label "IEC 60839-7-6:2001"@en ;
    dcterms:title "Alarm systems - Part 7-6: Message formats and protocols for serial data interfaces in alarm transmission systems - Alarm system interfaces employing ITU-T Recommendation V.24/V.28 signalling"@en ;
    rdfs:comment "Specifies the requirements for standard interfaces employing ITU-T V.24/V.28 signalling for communications between the control and indicating equipment of an alarm system and transmission equipment used for remote communications, where the transmission equipment is general purpose equipment. Is intended to be used as interfacing to standard modems, packet switching networks, X.25 PADs, etc."@en ;
    sto:hasAvailableLanguage lang:eng,
        lang:fra ;
    sto:hasEdition "1.0"^^xsd:float ;
    sto:hasFileSize sto:FileSizeIEC_60839_P7_6 ;
    sto:hasICS sto:ICS_13_320 ;
    sto:hasOfficialResource <https://webstore.iec.ch/publication/3674> ;
    sto:hasPages "9"^^xsd:int ;
    sto:hasPublicationDate "1968-03-01"^^xsd:date,
        "2001-03-09"^^xsd:date ;
    sto:hasPublisher sto:IEC ;
    sto:hasStabilityDate "2018-01-01"^^xsd:gYear ;
    sto:hasTag "IEC 60839-7-6:2001"@en ;
    sto:hasTechnicalCommittee sto:TC_79 .

sto:IEC_60839_P7_7 a owl:NamedIndividual,
        sto:Standard ;
    rdfs:label "IEC 60839-7-7:2001"@en ;
    dcterms:title "Alarm systems - Part 7-7: Message formats and protocols for serial data interfaces in alarm transmission systems - Alarm system interfaces for plug-in alarm system transceivers"@en ;
    rdfs:comment "Specifies the requirements for standard interfaces between the control and indicating equipment (CIE) of an alarm system and an alarm system transceiver where the alarm system transceiver is intended to plug into a standard space inside the CIE of the alarm system."@en ;
    sto:hasAvailableLanguage lang:eng,
        lang:fra ;
    sto:hasEdition "1.0"^^xsd:float ;
    sto:hasFileSize sto:FileSizeIEC_60839_P7_7 ;
    sto:hasICS sto:ICS_13_320 ;
    sto:hasOfficialResource <https://webstore.iec.ch/publication/3675> ;
    sto:hasPages "21"^^xsd:int ;
    sto:hasPublicationDate "1968-03-01"^^xsd:date,
        "2001-03-09"^^xsd:date ;
    sto:hasPublisher sto:IEC ;
    sto:hasStabilityDate "2018-01-01"^^xsd:gYear ;
    sto:hasTag "IEC 60839-7-7:2001"@en ;
    sto:hasTechnicalCommittee sto:TC_79 .

sto:IEC_60848 a owl:NamedIndividual,
        sto:Standard ;
    rdfs:label "IEC 60848:2013"@en ;
    dcterms:title "GRAFCET specification language for sequential function charts"@en ;
    rdfs:comment "IEC 60848:2013 defines the GRAFCET specification language for the functional description of the behaviour of the sequential part of a control system. It specifies the symbols and rules for the graphical representation of this language, as well as for its interpretation and has been prepared for automated production systems of industrial applications. This third edition cancels and replaces the second edition published in 2002 and constitutes a global technical revision with the extended definition of the concept of variables introducing: internal variable, input variable and output variable."@en ;
    sto:hasAvailableLanguage lang:eng,
        lang:fra ;
    sto:hasEdition "3.0"^^xsd:float ;
    sto:hasFileSize sto:FileSizeIEC_60848 ;
    sto:hasICS sto:ICS_29_020 ;
    sto:hasOfficialResource <https://webstore.iec.ch/publication/3684> ;
    sto:hasPages "109"^^xsd:int ;
    sto:hasPublicationDate "1958-02-13"^^xsd:date,
        "2013-02-27"^^xsd:date ;
    sto:hasPublisher sto:IEC ;
    sto:hasStabilityDate "2020-01-01"^^xsd:gYear ;
    sto:hasTag "IEC 60848:2013"@en ;
    sto:hasTechnicalCommittee sto:TC_3 .

sto:IEC_60864_P1 a owl:NamedIndividual,
        sto:Standard ;
    rdfs:label "IEC 60864-1:1986 "@en ;
    dcterms:title "Standardization of interconnections between broadcasting transmitters or transmitter systems and supervisory equipment. Part 1: Interface standards for systems using dedicated interconnections"@en ;
    rdfs:comment "Applies to all classes of transmitters for sound and television broadcasting. Deals with the interface between a transmitter (or system of transmitters) and the supervisory equipment which is intended to remotely monitor and/or control the transmitter(s). Details the interconnections and facilities to be provided with a view to achieving compatibility between different types and makes of transmitters and supervisory equipment."@en ;
    sto:hasAvailableLanguage lang:eng,
        lang:fra ;
    sto:hasEdition "1.0"^^xsd:float ;
    sto:hasFileSize sto:FileSizeIEC_60864_P1 ;
    sto:hasICS sto:ICS_33_060_20,
        sto:ICS_33_200 ;
    sto:hasOfficialResource <https://webstore.iec.ch/publication/3727> ;
    sto:hasPages "43"^^xsd:int ;
    sto:hasPublicationDate "1986-01-01"^^xsd:date ;
    sto:hasPublisher sto:IEC ;
    sto:hasStabilityDate "2020-01-01"^^xsd:gYear ;
    sto:hasTag "IEC 60864-1:1986 "@en ;
    sto:hasTechnicalCommittee sto:TC_103 .

sto:IEC_60864_P2 a owl:NamedIndividual,
        sto:Standard ;
    rdfs:label "IEC 60864-2:1997"@en ;
    dcterms:title "Standardization of interconnections between broadcasting transmitters or transmitter systems and supervisory equipment - Part 2: Interface standards for systems using data bus type interconnections"@en ;
    rdfs:comment "Deals with the interface between a transmitter (or system of transmitters) and the supervisory equipment which is entended to remotely monitor and/or control the transmitter(s). It details the interconnections and facilities to be provided with a view to achieving compatibility between different types and makes of transmitters and supervisory equipement."@en,
        "Deals with the itnerface between a transmitter (or system of transmitters) and the supervisory equipment which is entended to remotely monitor and/or control the transmitter(s). It details the interconnections and facilities to be provided with a view to achieving compatibility between different types and makes of transmitters and supervisory equipement."@en ;
    sto:hasAvailableLanguage lang:eng,
        lang:fra ;
    sto:hasEdition "1.0"^^xsd:float ;
    sto:hasFileSize sto:FileSizeIEC_60864_P2 ;
    sto:hasICS sto:ICS_33_060_20,
        sto:ICS_33_200 ;
    sto:hasOfficialResource <https://webstore.iec.ch/publication/3728> ;
    sto:hasPages "79"^^xsd:int ;
    sto:hasPublicationDate "1997-06-17"^^xsd:date ;
    sto:hasPublisher sto:IEC ;
    sto:hasStabilityDate "2020-01-01"^^xsd:gYear ;
    sto:hasTag "IEC 60864-2:1997"@en ;
    sto:hasTechnicalCommittee sto:TC_103 .

sto:IEC_60870 a dbpcy:WikicatIECStandards,
        dbpcy:WikicatNetworkProtocols,
        owl:NamedIndividual,
        sto:Standard ;
    rdfs:label "IEC 60870"@en ;
    dcterms:subject dbrc:Electric_power,
        dbrc:IEC_standards ;
    rdfs:comment "In electrical engineering and power system automation, the IEC 60870 series define systems used for telecontrol (supervisory control and data acquisition)"@en ;
    sto:hasDBpediaResource <http://dbpedia.org/page/IEC_60870> ;
    sto:hasPublisher sto:IEC ;
    sto:hasWikipediaArticle <https://en.wikipedia.org/wiki/IEC_60870> .

sto:IEC_60870_P2_S1_1995 a dbpcy:WikicatIECStandards,
        dbpcy:WikicatNetworkProtocols,
        owl:NamedIndividual,
        sto:Standard ;
    rdfs:label "IEC 60870-2-1:1995"@en ;
    dcterms:subject dbrc:Electric_power,
        dbrc:IEC_standards ;
    dcterms:title "Telecontrol equipment and systems - Part 2: Operating conditions - Section 1: Power supply and electromagnetic compatibility"@en ;
    rdfs:comment "Specifies classes for environmental conditions under which telecontrol equipment has to operate."@en ;
    sto:hasAvailableLanguage lang:eng,
        lang:fra,
        lang:spa ;
    sto:hasDBpediaResource <https://dbpedia.org/resource/IEC_60870> ;
    sto:hasEdition "2.0"^^xsd:float ;
    sto:hasFileSize sto:FileSizeIEC_60870_1995_P2_S1 ;
    sto:hasICS sto:ICS_29_020,
        sto:ICS_33_100_10,
        sto:ICS_33_200 ;
    sto:hasOfficialResource <https://webstore.iec.ch/publication/3738> ;
    sto:hasPages "43"^^xsd:int ;
    sto:hasPublicationDate "1995-12-08"^^xsd:date ;
    sto:hasPublisher sto:IEC ;
    sto:hasStabilityDate "2018-01-01"^^xsd:gYear ;
    sto:hasTag "IEC 60870-2-1:1995"@en ;
    sto:hasTechnicalCommittee sto:TC_57 ;
    sto:hasWikipediaArticle <https://en.wikipedia.org/wiki/IEC_60870> .

sto:IEC_60870_P2_S2_1996 a dbpcy:WikicatIECStandards,
        dbpcy:WikicatNetworkProtocols,
        owl:NamedIndividual,
        sto:Standard ;
    rdfs:label "IEC 60870-2-2:1996"@en ;
    dcterms:subject dbrc:Electric_power,
        dbrc:IEC_standards ;
    dcterms:title "Telecontrol equipment and systems - Part 2: Operating conditions -Section 2: Environmental conditions (climatic, mechanical and othernon electrical influences)"@en ;
    rdfs:comment "Applies to telecontrol equipment and systems with coded bit serial data transmission for monitoring and control of geographically wides pread processes. Specifies classes for environmental conditions under which the various components of the systems have to operate."@en ;
    sto:hasAvailableLanguage lang:eng,
        lang:fra,
        lang:spa ;
    sto:hasDBpediaResource <https://dbpedia.org/resource/IEC_60870> ;
    sto:hasEdition "1.0"^^xsd:float ;
    sto:hasFileSize sto:FileSizeIEC_60870_1996_P2_S2 ;
    sto:hasICS sto:ICS_29_020,
        sto:ICS_33_200 ;
    sto:hasOfficialResource <https://webstore.iec.ch/publication/3739> ;
    sto:hasPages "33"^^xsd:int ;
    sto:hasPublicationDate "1996-08-19"^^xsd:date ;
    sto:hasPublisher sto:IEC ;
    sto:hasStabilityDate "2018-01-01"^^xsd:gYear ;
    sto:hasTag "IEC 60870-2-2:1996"@en ;
    sto:hasTechnicalCommittee sto:TC_57 ;
    sto:hasWikipediaArticle <https://en.wikipedia.org/wiki/IEC_60870> .

sto:IEC_60870_P5_S101_2003 a dbpcy:WikicatIECStandards,
        dbpcy:WikicatNetworkProtocols,
        owl:NamedIndividual,
        sto:Standard ;
    rdfs:label "IEC 60870-5-101:2003"@en ;
    dcterms:subject dbrc:Electric_power,
        dbrc:IEC_standards ;
    dcterms:title "Telecontrol equipment and systems - Part 5-101: Transmissionprotocols - Companion standard for basic telecontrol tasks"@en ;
    rdfs:comment """IEC 60870-5-101:2003+A1:2015 Applies to telecontrol equipment and systems with coded bit serial data transmission for monitoring and controlling geographically widespread processes. Defines a telecontrol companion standard that enables interoperability among compatible telecontrol equipment. The defined telecontrol companion standard utilizes standards of the IEC 60870-5 series of documents. \r
This publication is of high relevance for Smart Grid. This consolidated version consists of the second edition (2003) and its amendment 1 (2015). Therefore, no need to order amendment in addition to this publication."""@en,
        "IEC 60870-5-101:2003+A1:2015 Applies to telecontrol equipment and systems with coded bit serial data transmission for monitoring and controlling geographically widespread processes. Defines a telecontrol companion standard that enables interoperability among compatible telecontrol equipment. The defined telecontrol companion standard utilizes standards of the IEC 60870-5 series of documents. This publication is of high relevance for Smart Grid. This consolidated version consists of the second edition (2003) and its amendment 1 (2015). Therefore, no need to order amendment in addition to this publication."@en,
        "IEC 60870-5-101:2003+A1:2015 Applies to telecontrol equipment and systems with coded bit serial data transmission for monitoring and controlling geographically widespread processes. Defines a telecontrol companion standard that enables interoperability among compatible telecontrol equipment. The defined telecontrol companion standard utilizes standards of the IEC 60870-5 series of documents. nThis publication is of high relevance for Smart Grid. This consolidated version consists of the second edition (2003) and its amendment 1 (2015). Therefore, no need to order amendment in addition to this publication."@en ;
    sto:hasAvailableLanguage lang:eng ;
    sto:hasDBpediaResource <https://dbpedia.org/resource/IEC_60870> ;
    sto:hasEdition "2.1"^^xsd:float ;
    sto:hasFileSize sto:FileSizeIEC_60870_P5_S101_2003 ;
    sto:hasICS sto:ICS_33_200 ;
    sto:hasOfficialResource <https://webstore.iec.ch/publication/23822> ;
    sto:hasPages "360"^^xsd:int ;
    sto:hasPublicationDate "2015-11-26"^^xsd:date,
        "2015-11-30"^^xsd:date ;
    sto:hasPublisher sto:IEC ;
    sto:hasStabilityDate "2018-01-01"^^xsd:gYear ;
    sto:hasTag "IEC 60870-5-101:2003"@en ;
    sto:hasTechnicalCommittee sto:TC_57 ;
    sto:hasWikipediaArticle <https://en.wikipedia.org/wiki/IEC_60870> .

sto:IEC_60870_P5_S102_1996 a dbpcy:WikicatIECStandards,
        dbpcy:WikicatNetworkProtocols,
        owl:NamedIndividual,
        sto:Standard ;
    rdfs:label "IEC 60870-5-102:1996"@en ;
    dcterms:subject dbrc:Electric_power,
        dbrc:IEC_standards ;
    dcterms:title "Telecontrol equipment and systems - Part 5: Transmission protocols - Section 102: Companion standard for the transmission of integrated totals in electric power systems"@en ;
    rdfs:comment """Standardizes the transmission of integrated totals representing the amount of electrical energy transferred between power utilities, or between a power utility and independent producers on a high voltage or medium voltage network.\r
This publication is of high relevance for Smart Grid."""@en,
        "Standardizes the transmission of integrated totals representing the amount of electrical energy transferred between power utilities, or between a power utility and independent producers on a high voltage or medium voltage network.nThis publication is of high relevance for Smart Grid."@en ;
    sto:hasAvailableLanguage lang:eng,
        lang:fra ;
    sto:hasDBpediaResource <https://dbpedia.org/resource/IEC_60870> ;
    sto:hasEdition "1.0"^^xsd:float ;
    sto:hasFileSize sto:FileSizeIEC_60870_P5_S102_1996 ;
    sto:hasICS sto:ICS_33_200 ;
    sto:hasOfficialResource <https://webstore.iec.ch/publication/3744> ;
    sto:hasPages "99"^^xsd:int ;
    sto:hasPublicationDate "1996-06-18"^^xsd:date ;
    sto:hasPublisher sto:IEC ;
    sto:hasStabilityDate "2018-01-01"^^xsd:gYear ;
    sto:hasTag "IEC 60870-5-102:1996"@en ;
    sto:hasTechnicalCommittee sto:TC_57 ;
    sto:hasWikipediaArticle <https://en.wikipedia.org/wiki/IEC_60870> .

sto:IEC_60870_P5_S103_1997 a dbpcy:WikicatIECStandards,
        dbpcy:WikicatNetworkProtocols,
        owl:NamedIndividual,
        sto:Standard ;
    rdfs:label "IEC 60870-5-103:1997"@en ;
    dcterms:subject dbrc:Electric_power,
        dbrc:IEC_standards ;
    dcterms:title "Telecontrol equipment and systems - Part 5-103: Transmission protocols - Companion standard for the informative interface of protection equipment"@en ;
    rdfs:comment """Applies to protection equipment with coded bit serial data transmission for exchanging information with control systems. Defines a companion standard that enables interoperability between protection equipment and devices of a control system in a substation.\r
This publication is of high relevance for Smart Grid."""@en,
        "Applies to protection equipment with coded bit serial data transmission for exchanging information with control systems. Defines a companion standard that enables interoperability between protection equipment and devices of a control system in a substation.nThis publication is of high relevance for Smart Grid."@en ;
    sto:hasAvailableLanguage lang:eng,
        lang:fra ;
    sto:hasDBpediaResource <https://dbpedia.org/resource/IEC_60870> ;
    sto:hasEdition "1.0"^^xsd:float ;
    sto:hasFileSize sto:FileSizeIEC_60870_P5_S103_1997 ;
    sto:hasICS sto:ICS_33_200 ;
    sto:hasOfficialResource <https://webstore.iec.ch/publication/3745> ;
    sto:hasPages "203"^^xsd:int ;
    sto:hasPublicationDate "1997-12-11"^^xsd:date ;
    sto:hasPublisher sto:IEC ;
    sto:hasStabilityDate "2018-01-01"^^xsd:gYear ;
    sto:hasTag "IEC 60870-5-103:1997"@en ;
    sto:hasTechnicalCommittee sto:TC_57 ;
    sto:hasWikipediaArticle <https://en.wikipedia.org/wiki/IEC_60870> .

sto:IEC_60870_P5_S104_2016 a dbpcy:WikicatIECStandards,
        dbpcy:WikicatNetworkProtocols,
        owl:NamedIndividual,
        sto:Standard ;
    rdfs:label "IEC 60870-5-104:2006"@en ;
    dcterms:subject dbrc:Electric_power,
        dbrc:IEC_standards ;
    dcterms:title "Telecontrol equipment and systems - Part 5-104: Transmission protocols - Network access for IEC 60870-5-101 using standardtransport profiles"@en ;
    rdfs:comment """IEC 60870-5-104:2006+A1:2016 Defines a telecontrol companion standard that enables interoperability among compatible telecontrol equipment. Applies to telecontrol equipment and systems with coded bit serial data transmission for monitoring and controlling geographically widespread processes. \r
This publication is of high relevance for Smart Grid. This consolidated version consists of the second edition (2006) and its amendment 1 (2012). Therefore, no need to order amendment in addition to this publication."""@en,
        "IEC 60870-5-104:2006+A1:2016 Defines a telecontrol companion standard that enables interoperability among compatible telecontrol equipment. Applies to telecontrol equipment and systems with coded bit serial data transmission for monitoring and controlling geographically widespread processes. nThis publication is of high relevance for Smart Grid. This consolidated version consists of the second edition (2006) and its amendment 1 (2012). Therefore, no need to order amendment in addition to this publication."@en ;
    sto:hasAvailableLanguage lang:eng,
        lang:fra ;
    sto:hasDBpediaResource <https://dbpedia.org/resource/IEC_60870> ;
    sto:hasEdition "2.1"^^xsd:float ;
    sto:hasFileSize sto:FileSizeIEC_60870_P5_S104_2016 ;
    sto:hasICS sto:ICS_33_200 ;
    sto:hasOfficialResource <https://webstore.iec.ch/publication/25035> ;
    sto:hasPages "281"^^xsd:int ;
    sto:hasPublicationDate "2016-06-07"^^xsd:date ;
    sto:hasPublisher sto:IEC ;
    sto:hasStabilityDate "2018-01-01"^^xsd:gYear ;
    sto:hasTag "IEC 60870-5-104:2006"@en ;
    sto:hasTechnicalCommittee sto:TC_57 ;
    sto:hasWikipediaArticle <https://en.wikipedia.org/wiki/IEC_60870> .

sto:IEC_60870_P5_S1_1990 a dbpcy:WikicatIECStandards,
        dbpcy:WikicatNetworkProtocols,
        owl:NamedIndividual,
        sto:Standard ;
    rdfs:label "IEC 60870-5-1:1990"@en ;
    dcterms:subject dbrc:Electric_power,
        dbrc:IEC_standards ;
    dcterms:title "Telecontrol equipment and systems. Part 5: Transmission protocols - Section One: Transmission frame formats"@en ;
    rdfs:comment "Covers asynchronous data transmission with half duplex and duplex link protocols operating with window size one for message transfers. Specifies the basic requirements for services to be provided by the link plus physical layers, for telecontrol applications. In particular it specifies standards on coding, formatting and synchronizing data frames of variable and filed lengths which meet specified data integrity requirements."@en ;
    sto:hasAvailableLanguage lang:eng,
        lang:fra ;
    sto:hasDBpediaResource <https://dbpedia.org/resource/IEC_60870> ;
    sto:hasEdition "1.0"^^xsd:float ;
    sto:hasFileSize sto:FileSizeIEC_60870_1990_P5_S1 ;
    sto:hasICS sto:ICS_33_200 ;
    sto:hasOfficialResource <https://webstore.iec.ch/publication/3742> ;
    sto:hasPages "79"^^xsd:int ;
    sto:hasPublicationDate "1990-02-01"^^xsd:date ;
    sto:hasPublisher sto:IEC ;
    sto:hasStabilityDate "2018-01-01"^^xsd:gYear ;
    sto:hasTag "IEC 60870-5-1:1990"@en ;
    sto:hasTechnicalCommittee sto:TC_57 ;
    sto:hasWikipediaArticle <https://en.wikipedia.org/wiki/IEC_60870> .

sto:IEC_60870_P5_S2_1992 a dbpcy:WikicatIECStandards,
        dbpcy:WikicatNetworkProtocols,
        owl:NamedIndividual,
        sto:Standard ;
    rdfs:label "IEC 60870-5-2:1992"@en ;
    dcterms:subject dbrc:Electric_power,
        dbrc:IEC_standards ;
    dcterms:title "Telecontrol equipment and systems - Part 5: Transmission protocols - Section 2: Link transmission procedures"@en ;
    rdfs:comment """Applies to telecontrol equipment and systems with coded bit serial data transmission for monitoring and controlling geographically widespread processes. \r
This publication is of high relevance for Smart Grid."""@en,
        "Applies to telecontrol equipment and systems with coded bit serial data transmission for monitoring and controlling geographically widespread processes. nThis publication is of high relevance for Smart Grid."@en ;
    sto:hasAvailableLanguage lang:eng,
        lang:fra ;
    sto:hasDBpediaResource <https://dbpedia.org/resource/IEC_60870> ;
    sto:hasEdition "1.0"^^xsd:float ;
    sto:hasFileSize sto:FileSizeIEC_60870_1992_P5_S2 ;
    sto:hasICS sto:ICS_33_200 ;
    sto:hasOfficialResource <https://webstore.iec.ch/publication/3747> ;
    sto:hasPages "99"^^xsd:int ;
    sto:hasPublicationDate "1992-04-30"^^xsd:date ;
    sto:hasPublisher sto:IEC ;
    sto:hasStabilityDate "2018-01-01"^^xsd:gYear ;
    sto:hasTag "IEC 60870-5-2:1992"@en ;
    sto:hasTechnicalCommittee sto:TC_57 ;
    sto:hasWikipediaArticle <https://en.wikipedia.org/wiki/IEC_60870> .

sto:IEC_60870_P5_S3_1992 a dbpcy:WikicatIECStandards,
        dbpcy:WikicatNetworkProtocols,
        owl:NamedIndividual,
        sto:Standard ;
    rdfs:label "IEC 60870-5-3:1992"@en ;
    dcterms:subject dbrc:Electric_power,
        dbrc:IEC_standards ;
    dcterms:title "Telecontrol equipment and systems - Part 5: Transmission protocols - Section 3: General structure of application data"@en ;
    rdfs:comment """Applies to telecontrol equipment and systems with coded bit serial data transmission for monitoring and controlling geographically widespread processes; specifies rules for structuring application data units in transmission frames of telecontrol systems.\r
This publication is of high relevance for Smart Grid."""@en,
        "Applies to telecontrol equipment and systems with coded bit serial data transmission for monitoring and controlling geographically widespread processes; specifies rules for structuring application data units in transmission frames of telecontrol systems.nThis publication is of high relevance for Smart Grid."@en ;
    sto:hasAvailableLanguage lang:eng,
        lang:fra ;
    sto:hasDBpediaResource <https://dbpedia.org/resource/IEC_60870> ;
    sto:hasEdition "1.0"^^xsd:float ;
    sto:hasFileSize sto:FileSizeIEC_60870_1992_P5_S3 ;
    sto:hasICS sto:ICS_33_200 ;
    sto:hasOfficialResource <https://webstore.iec.ch/publication/3748> ;
    sto:hasPages "43"^^xsd:int ;
    sto:hasPublicationDate "1992-09-29"^^xsd:date ;
    sto:hasPublisher sto:IEC ;
    sto:hasStabilityDate "2018-01-01"^^xsd:gYear ;
    sto:hasTag "IEC 60870-5-3:1992"@en ;
    sto:hasTechnicalCommittee sto:TC_57 ;
    sto:hasWikipediaArticle <https://en.wikipedia.org/wiki/IEC_60870> .

sto:IEC_60870_P5_S4_1993 a dbpcy:WikicatIECStandards,
        dbpcy:WikicatNetworkProtocols,
        owl:NamedIndividual,
        sto:Standard ;
    rdfs:label "IEC 60870-5-4:1993"@en ;
    dcterms:subject dbrc:Electric_power,
        dbrc:IEC_standards ;
    dcterms:title "Telecontrol equipment and systems - Part 5: Transmission protocols - Section 4: Definition and coding of application information elements"@en ;
    rdfs:comment """Gives rules for defining information elements and presents a set of information elements, in particular of digital and analog process variables frequently used in telecontrol applications. \r
This publication is of high relevance for Smart Grid."""@en,
        "Gives rules for defining information elements and presents a set of information elements, in particular of digital and analog process variables frequently used in telecontrol applications. nThis publication is of high relevance for Smart Grid."@en ;
    sto:hasAvailableLanguage lang:eng,
        lang:fra ;
    sto:hasDBpediaResource <https://dbpedia.org/resource/IEC_60870> ;
    sto:hasEdition "1.0"^^xsd:float ;
    sto:hasFileSize sto:FileSizeIEC_60870_P5_S4_1993 ;
    sto:hasICS sto:ICS_33_200 ;
    sto:hasOfficialResource <https://webstore.iec.ch/publication/3749> ;
    sto:hasPages "45"^^xsd:int ;
    sto:hasPublicationDate "1993-08-06"^^xsd:date ;
    sto:hasPublisher sto:IEC ;
    sto:hasStabilityDate "2018-01-01"^^xsd:gYear ;
    sto:hasTag "IEC 60870-5-4:1993"@en ;
    sto:hasTechnicalCommittee sto:TC_57 ;
    sto:hasWikipediaArticle <https://en.wikipedia.org/wiki/IEC_60870> .

sto:IEC_60870_P5_S5_1995 a dbpcy:WikicatIECStandards,
        dbpcy:WikicatNetworkProtocols,
        owl:NamedIndividual,
        sto:Standard ;
    rdfs:label "IEC 60870-5-5:1995"@en ;
    dcterms:subject dbrc:Electric_power,
        dbrc:IEC_standards ;
    dcterms:title "Telecontrol equipment and systems - Part 5: Transmission protocols - Section 5: Basic application functions"@en ;
    rdfs:comment """Applies to telecontrol equipment and systems with coded bit serial data transmission for monitoring and controlling geographically widespread processes. It defines a telecontrol companion standard that enables interoperability among compatible telecontrol equipment. \r
This publication is of high relevance for Smart Grid."""@en,
        "Applies to telecontrol equipment and systems with coded bit serial data transmission for monitoring and controlling geographically widespread processes. It defines a telecontrol companion standard that enables interoperability among compatible telecontrol equipment. nThis publication is of high relevance for Smart Grid."@en ;
    sto:hasAvailableLanguage lang:eng,
        lang:fra ;
    sto:hasDBpediaResource <https://dbpedia.org/resource/IEC_60870> ;
    sto:hasEdition "1.0"^^xsd:float ;
    sto:hasFileSize sto:FileSizeIEC_60870_P5_S5_1995 ;
    sto:hasICS sto:ICS_33_200 ;
    sto:hasOfficialResource <https://webstore.iec.ch/publication/3750> ;
    sto:hasPages "101"^^xsd:int ;
    sto:hasPublicationDate "1995-06-04"^^xsd:date ;
    sto:hasPublisher sto:IEC ;
    sto:hasStabilityDate "2018-01-01"^^xsd:gYear ;
    sto:hasTag "IEC 60870-5-5:1995"@en ;
    sto:hasTechnicalCommittee sto:TC_57 ;
    sto:hasWikipediaArticle <https://en.wikipedia.org/wiki/IEC_60870> .

sto:IEC_60870_P5_S6_2006 a dbpcy:WikicatIECStandards,
        dbpcy:WikicatNetworkProtocols,
        owl:NamedIndividual,
        sto:Standard ;
    rdfs:label "IEC 60870-5-6:2006"@en ;
    dcterms:subject dbrc:Electric_power,
        dbrc:IEC_standards ;
    dcterms:title "Telecontrol equipment and systems - Part 5-6: Guidelines for conformance testing for the IEC 60870-5 companion standards"@en ;
    rdfs:comment "IEC 60870-5-6:2006 Specifies methods for conformance testing of telecontrol equipment, amongst substation automation systems and telecontrol systems, including front-end functions of SCADA. Facilitates interoperability by providing a standard method of testing protocol implementations. Is expected to minimize the risk of non-interoperability."@en ;
    sto:hasAvailableLanguage lang:eng,
        lang:fra ;
    sto:hasDBpediaResource <https://dbpedia.org/resource/IEC_60870> ;
    sto:hasEdition "1.0"^^xsd:float ;
    sto:hasFileSize sto:FileSizeIEC_60870_P5_S6_2006 ;
    sto:hasICS sto:ICS_33_200 ;
    sto:hasOfficialResource <https://webstore.iec.ch/publication/3751> ;
    sto:hasPages "46"^^xsd:int ;
    sto:hasPublicationDate "2006-03-08"^^xsd:date ;
    sto:hasPublisher sto:IEC ;
    sto:hasStabilityDate "2018-01-01"^^xsd:gYear ;
    sto:hasTag "IEC 60870-5-6:2006"@en ;
    sto:hasTechnicalCommittee sto:TC_57 ;
    sto:hasWikipediaArticle <https://en.wikipedia.org/wiki/IEC_60870> .

sto:IEC_60870_P6_S2_1995 a dbpcy:WikicatIECStandards,
        dbpcy:WikicatNetworkProtocols,
        owl:NamedIndividual,
        sto:Standard ;
    rdfs:label "IEC 60870-6-2:1995"@en ;
    dcterms:subject dbrc:Electric_power,
        dbrc:IEC_standards ;
    dcterms:title "Telecontrol equipment and systems - Part 6: Telecontrol protocols compatible with ISO standards and ITU-T recommendations - Section 2: Use of basic standards (OSI layers 1-4)"@en ;
    rdfs:comment """Considers the standards related to layers 1-4 of the OSI reference model and describes the role and the functions carried out by each layer.\r
This publication is of high relevance for Smart Grid."""@en,
        "Considers the standards related to layers 1-4 of the OSI reference model and describes the role and the functions carried out by each layer.nThis publication is of high relevance for Smart Grid."@en ;
    sto:hasAvailableLanguage lang:eng,
        lang:fra ;
    sto:hasDBpediaResource <https://dbpedia.org/resource/IEC_60870> ;
    sto:hasEdition "1.0"^^xsd:float ;
    sto:hasFileSize sto:FileSizeIEC_60870_P6_S2_1995 ;
    sto:hasICS sto:ICS_33_200 ;
    sto:hasOfficialResource <https://webstore.iec.ch/publication/3757> ;
    sto:hasPages "83"^^xsd:int ;
    sto:hasPublicationDate "1995-10-31"^^xsd:date ;
    sto:hasPublisher sto:IEC ;
    sto:hasStabilityDate "2018-01-01"^^xsd:gYear ;
    sto:hasTag "IEC 60870-6-2:1995"@en ;
    sto:hasTechnicalCommittee sto:TC_57 ;
    sto:hasWikipediaArticle <https://en.wikipedia.org/wiki/IEC_60870> .

sto:IEC_60870_P6_S501_1995 a dbpcy:WikicatIECStandards,
        dbpcy:WikicatNetworkProtocols,
        owl:NamedIndividual,
        sto:Standard ;
    rdfs:label "IEC 60870-6-501:1995"@en ;
    dcterms:subject dbrc:Electric_power,
        dbrc:IEC_standards ;
    dcterms:title "Telecontrol equipment and systems - Part 6: Telecontrol protocols compatible with ISO standards and ITU-T recommendations - Section 501: TASE.1 Service definitions"@en ;
    rdfs:comment """Defines the services provided by a telecontrol specific application-service-element - the Telecontrol Application Service Element No. 1 (TASE.1) - for the exchange of process data in telecontrol systems.\r
This publication is of high relevance for Smart Grid."""@en,
        "Defines the services provided by a telecontrol specific application-service-element - the Telecontrol Application Service Element No. 1 (TASE.1) - for the exchange of process data in telecontrol systems.nThis publication is of high relevance for Smart Grid."@en ;
    sto:hasAvailableLanguage lang:eng,
        lang:fra ;
    sto:hasDBpediaResource <https://dbpedia.org/resource/IEC_60870> ;
    sto:hasEdition "1.0"^^xsd:float ;
    sto:hasFileSize sto:FileSizeIEC_60870_P6_S501_1995 ;
    sto:hasICS sto:ICS_33_200 ;
    sto:hasOfficialResource <https://webstore.iec.ch/publication/3758> ;
    sto:hasPages "170"^^xsd:int ;
    sto:hasPublicationDate "1995-12-18"^^xsd:date ;
    sto:hasPublisher sto:IEC ;
    sto:hasStabilityDate "2018-01-01"^^xsd:gYear ;
    sto:hasTag "IEC 60870-6-501:1995"@en ;
    sto:hasTechnicalCommittee sto:TC_57 ;
    sto:hasWikipediaArticle <https://en.wikipedia.org/wiki/IEC_60870> .

sto:IEC_60870_P6_S502_1995 a dbpcy:WikicatIECStandards,
        dbpcy:WikicatNetworkProtocols,
        owl:NamedIndividual,
        sto:Standard ;
    rdfs:label "IEC 60870-6-502:1995"@en ;
    dcterms:subject dbrc:Electric_power,
        dbrc:IEC_standards ;
    dcterms:title "Telecontrol equipment and systems - Part 6: Telecontrol protocols compatible with ISO standards and ITU-T recommendations - Section 502: TASE.1 Protocol definitions"@en ;
    rdfs:comment """Specifies the protocol for the services provided by an application-service-element - the Telecontrol Application Service Element No. 1 (TASE.1) - to support the exchange of process data between telecontrol systems.\r
This publication is of high relevance for Smart Grid."""@en,
        "Specifies the protocol for the services provided by an application-service-element - the Telecontrol Application Service Element No. 1 (TASE.1) - to support the exchange of process data between telecontrol systems.nThis publication is of high relevance for Smart Grid."@en ;
    sto:hasAvailableLanguage lang:eng,
        lang:fra ;
    sto:hasDBpediaResource <https://dbpedia.org/resource/IEC_60870> ;
    sto:hasEdition "1.0"^^xsd:float ;
    sto:hasFileSize sto:FileSizeIEC_60870_P6_S502_1995 ;
    sto:hasICS sto:ICS_33_200 ;
    sto:hasOfficialResource <https://webstore.iec.ch/publication/3759> ;
    sto:hasPages "57"^^xsd:int ;
    sto:hasPublicationDate "1995-12-05"^^xsd:date ;
    sto:hasPublisher sto:IEC ;
    sto:hasStabilityDate "2018-01-01"^^xsd:gYear ;
    sto:hasTag "IEC 60870-6-502:1995"@en ;
    sto:hasTechnicalCommittee sto:TC_57 ;
    sto:hasWikipediaArticle <https://en.wikipedia.org/wiki/IEC_60870> .

sto:IEC_60870_P6_S503_2014 a dbpcy:WikicatIECStandards,
        dbpcy:WikicatNetworkProtocols,
        owl:NamedIndividual,
        sto:Standard ;
    rdfs:label "IEC 60870-6-503:2014"@en ;
    dcterms:subject dbrc:Electric_power,
        dbrc:IEC_standards ;
    dcterms:title "Telecontrol equipment and systems - Part 6-503: Telecontrol protocols compatible with ISO standards and ITU-T recommendations - TASE.2 Services and protocol"@en ;
    rdfs:comment "IEC 60870-6-503:2014 specifies a method of exchanging time-critical control centre data through wide-area and local-area networks using a full ISO compliant protocol stack. It contains provisions for supporting both centralized and distributed architectures. This standard includes the exchange of real-time data indications, control operations, time-series data, scheduling and accounting information, remote program control and event notification. This new edition includes the following significant technical changes with respect to the previous edition: - certain objects were made informative; - services associated with the informative objects were made informative; - certain TASE.2 conformance blocks were made out-of-scope."@en,
        "IEC 60870-6-503:2014 specifies a method of exchanging time-critical control centre data through wide-area and local-area networks using a full ISO compliant protocol stack. It contains provisions for supporting both centralized and distributed architectures. This standard includes the exchange of real-time data indications, control operations, time-series data, scheduling and accounting information, remote program control and event notification. This new edition includes the following significant technical changes with respect to the previous edition:n- certain objects were made informative;n- services associated with the informative objects were made informative;n- certain TASE.2 conformance blocks were made out-of-scope."@en ;
    sto:hasAvailableLanguage lang:eng,
        lang:fra ;
    sto:hasDBpediaResource <https://dbpedia.org/resource/IEC_60870> ;
    sto:hasEdition "3.0"^^xsd:float ;
    sto:hasFileSize sto:FileSizeIEC_60870_P6_S503_2014 ;
    sto:hasICS sto:ICS_33_200 ;
    sto:hasOfficialResource <https://webstore.iec.ch/publication/3760> ;
    sto:hasPages "310"^^xsd:int ;
    sto:hasPublicationDate "2014-07-15"^^xsd:date ;
    sto:hasPublisher sto:IEC ;
    sto:hasStabilityDate "2018-01-01"^^xsd:gYear ;
    sto:hasTag "IEC 60870-6-503:2014"@en ;
    sto:hasTechnicalCommittee sto:TC_57 ;
    sto:hasWikipediaArticle <https://en.wikipedia.org/wiki/IEC_60870> .

sto:IEC_60870_P6_S601_1994 a dbpcy:WikicatIECStandards,
        dbpcy:WikicatNetworkProtocols,
        owl:NamedIndividual,
        sto:Standard ;
    rdfs:label "IEC 60870-6-601:1994"@en ;
    dcterms:subject dbrc:Electric_power,
        dbrc:IEC_standards ;
    dcterms:title "Telecontrol equipment and systems - Part 6: Telecontrol protocol s compatible with ISO standards and ITU-T recommendations - Sect ion 601: Functional profile for providing the connection-oriente d transport service in an end system connected via permanent acc ess to a packet switched data network"@en ;
    rdfs:comment """Defines the functional profile which provides the connection-oriented transport service in an end system connected via permanent access to a packet switched data network.\r
This publication is of high relevance for Smart Grid."""@en,
        "Defines the functional profile which provides the connection-oriented transport service in an end system connected via permanent access to a packet switched data network.nThis publication is of high relevance for Smart Grid."@en ;
    sto:hasAvailableLanguage lang:eng,
        lang:fra ;
    sto:hasDBpediaResource <https://dbpedia.org/resource/IEC_60870> ;
    sto:hasEdition "1.0"^^xsd:float ;
    sto:hasFileSize sto:FileSizeIEC_60870_P6_S601_1994 ;
    sto:hasICS sto:ICS_33_200 ;
    sto:hasOfficialResource <https://webstore.iec.ch/publication/3765> ;
    sto:hasPages "25"^^xsd:int ;
    sto:hasPublicationDate "1994-12-21"^^xsd:date ;
    sto:hasPublisher sto:IEC ;
    sto:hasStabilityDate "2018-01-01"^^xsd:gYear ;
    sto:hasTag "IEC 60870-6-601:1994"@en ;
    sto:hasTechnicalCommittee sto:TC_57 ;
    sto:hasWikipediaArticle <https://en.wikipedia.org/wiki/IEC_60870> .

sto:IEC_60870_P6_S701_1998 a dbpcy:WikicatIECStandards,
        dbpcy:WikicatNetworkProtocols,
        owl:NamedIndividual,
        sto:Standard ;
    rdfs:label "IEC 60870-6-701:1998"@en ;
    dcterms:subject dbrc:Electric_power,
        dbrc:IEC_standards ;
    dcterms:title "Telecontrol equipment and systems - Part 6-701: Telecontrol protocols compatible with ISO standards and ITU-T recommendations - Functional profile for providing the TASE.1 application service in end systems"@en ;
    rdfs:comment """Describes the functional profile which defines the provision of the TASE.1 communication services between two control centre end systems.\r
This publication is of high relevance for Smart Grid"""@en,
        "Describes the functional profile which defines the provision of the TASE.1 communication services between two control centre end systems.nThis publication is of high relevance for Smart Grid"@en ;
    sto:hasAvailableLanguage lang:eng,
        lang:fra ;
    sto:hasDBpediaResource <https://dbpedia.org/resource/IEC_60870> ;
    sto:hasEdition "1.0"^^xsd:float ;
    sto:hasFileSize sto:FileSizeIEC_60870_P6_S701_1998 ;
    sto:hasICS sto:ICS_33_200 ;
    sto:hasOfficialResource <https://webstore.iec.ch/publication/3767> ;
    sto:hasPages "37"^^xsd:int ;
    sto:hasPublicationDate "1998-08-07"^^xsd:date ;
    sto:hasPublisher sto:IEC ;
    sto:hasStabilityDate "2018-01-01"^^xsd:gYear ;
    sto:hasTag "IEC 60870-6-701:1998"@en ;
    sto:hasTechnicalCommittee sto:TC_57 ;
    sto:hasWikipediaArticle <https://en.wikipedia.org/wiki/IEC_60870> .

sto:IEC_60870_P6_S702_2014 a dbpcy:WikicatIECStandards,
        dbpcy:WikicatNetworkProtocols,
        owl:NamedIndividual,
        sto:Standard ;
    rdfs:label "IEC 60870-6-702:2014"@en ;
    dcterms:subject dbrc:Electric_power,
        dbrc:IEC_standards ;
    dcterms:title "Telecontrol equipment and systems - Part 6-702: Telecontrol protocols compatible with ISO standards and ITU-T recommendations - Functional profile for providing the TASE.2 application service in end systems"@en ;
    rdfs:comment """IEC 60870-6-702:2014 is a functional profile (FP) and defines the provision of the TASE.2 communications services between two control centre end systems. It is supported by the transport services implemented in accordance with transport-profiles defined for the type of network that interconnects the control centre end systems. The main changes with respect to the previous edition are listed below:\r
- certain objects were moved from being normative to informative\r
- certain TASE.2 conformance blocks have been made out-of-scope. These changes were made in order to remove TASE.2 blocks that were seldom used and whose capabilities are typically implemented by some other means besides TASE.2. This was done to promote interoperability of implementations from an application perspective."""@en,
        "IEC 60870-6-702:2014 is a functional profile (FP) and defines the provision of the TASE.2 communications services between two control centre end systems. It is supported by the transport services implemented in accordance with transport-profiles defined for the type of network that interconnects the control centre end systems. The main changes with respect to the previous edition are listed below:n- certain objects were moved from being normative to informative;n- certain TASE.2 conformance blocks have been made out-of-scope. These changes were made in order to remove TASE.2 blocks that were seldom used and whose capabilities are typically implemented by some other means besides TASE.2. This was done to promote interoperability of implementations from an application perspective."@en ;
    sto:hasAvailableLanguage lang:eng,
        lang:fra ;
    sto:hasDBpediaResource <https://dbpedia.org/resource/IEC_60870> ;
    sto:hasEdition "2.0"^^xsd:float ;
    sto:hasFileSize sto:FileSizeIEC_60870_P6_S702_2014 ;
    sto:hasICS sto:ICS_33_200 ;
    sto:hasOfficialResource <https://webstore.iec.ch/publication/3768> ;
    sto:hasPages "71"^^xsd:int ;
    sto:hasPublicationDate "2014-07-15"^^xsd:date ;
    sto:hasPublisher sto:IEC ;
    sto:hasStabilityDate "2018-01-01"^^xsd:gYear ;
    sto:hasTag "IEC 60870-6-702:2014"@en ;
    sto:hasTechnicalCommittee sto:TC_57 ;
    sto:hasWikipediaArticle <https://en.wikipedia.org/wiki/IEC_60870> .

sto:IEC_60870_P6_S802_2014 a dbpcy:WikicatIECStandards,
        dbpcy:WikicatNetworkProtocols,
        owl:NamedIndividual,
        sto:Standard ;
    rdfs:label "IEC 60870-6-802:2014"@en ;
    dcterms:subject dbrc:Electric_power,
        dbrc:IEC_standards ;
    dcterms:title "Telecontrol equipment and systems - Part 6-802: Telecontrol protocols compatible with ISO standards and ITU-T recommendations - TASE.2 Object models"@en ;
    rdfs:comment "IEC 60870-6-802:2014 specifies a method of exchanging time-critical control centre data through wide-area and local-area networks using a full ISO compliant protocol stack. It contains provisions for supporting both centralized and distributed architectures. The standard includes the exchange of real-time data indications, control operations, time series data, scheduling and accounting information, remote program control and event notification. This new edition includes the following significant technical changes with respect to the previous edition: -certain objects have been changed from informative to normative; - certain TASE.2 conformance blocks have been made out of scope."@en,
        "IEC 60870-6-802:2014 specifies a method of exchanging time-critical control centre data through wide-area and local-area networks using a full ISO compliant protocol stack. It contains provisions for supporting both centralized and distributed architectures. The standard includes the exchange of real-time data indications, control operations, time series data, scheduling and accounting information, remote program control and event notification. This new edition includes the following significant technical changes with respect to the previous edition:n- certain objects have been changed from informative to normative;n- certain TASE.2 conformance blocks have been made out of scope."@en ;
    sto:hasAvailableLanguage lang:eng,
        lang:fra ;
    sto:hasDBpediaResource <https://dbpedia.org/resource/IEC_60870> ;
    sto:hasEdition "3.0"^^xsd:float ;
    sto:hasFileSize sto:FileSizeIEC_60870_P6_S802_2014 ;
    sto:hasICS sto:ICS_33_200 ;
    sto:hasOfficialResource <https://webstore.iec.ch/publication/3769> ;
    sto:hasPages "188"^^xsd:int ;
    sto:hasPublicationDate "2014-07-15"^^xsd:date ;
    sto:hasPublisher sto:IEC ;
    sto:hasStabilityDate "2019-01-01"^^xsd:gYear ;
    sto:hasTag "IEC 60870-6-802:2014"@en ;
    sto:hasTechnicalCommittee sto:TC_57 ;
    sto:hasWikipediaArticle <https://en.wikipedia.org/wiki/IEC_60870> .

sto:IEC_60904 a owl:NamedIndividual,
        sto:Standard ;
    rdfs:label "IEC 60904"@en ;
    rdfs:comment "Photovoltaic devices"@en ;
    sto:hasOfficialResource <https://webstore.iec.ch/publication/3881> ;
    sto:hasPublicationDate "2017-05-18"^^xsd:date ;
    sto:hasPublisher sto:IEC .

sto:IEC_60946 a owl:NamedIndividual,
        sto:Standard ;
    rdfs:label "IEC 60946:1988"@en ;
    dcterms:title "Binary direct voltage signals for process measurement and control systems"@en ;
    rdfs:comment "Applies to non-multiplexed two wire binary direct voltage signals of nominal 24 V level that are used in industrial-process measurement and control systems to transmit information between elements of systems."@en ;
    sto:hasAvailableLanguage lang:eng,
        lang:fra ;
    sto:hasEdition "1.0"^^xsd:float ;
    sto:hasFileSize sto:FileSizeIEC_60946 ;
    sto:hasICS sto:ICS_25_040_40 ;
    sto:hasOfficialResource <https://webstore.iec.ch/publication/3961> ;
    sto:hasPages "13"^^xsd:int ;
    sto:hasPublicationDate "1988-09-29"^^xsd:date ;
    sto:hasPublisher sto:IEC ;
    sto:hasStabilityDate "2018-01-01"^^xsd:gYear ;
    sto:hasTag "IEC 60946:1988"@en ;
    sto:hasTechnicalCommittee sto:TC_65 .

sto:IEC_61000_P6_S2_2016 a owl:NamedIndividual,
        sto:Standard ;
    rdfs:label "IEC 61000-6-2:2016"@en ;
    dcterms:title "Electromagnetic compatibility (EMC) - Part 6-2: Generic standards - Immunity standard for industrial environments"@en ;
    rdfs:comment """IEC 61000-6-2:2016 RLV contains the International Standard and its Redline version. The Redline version is available in English only. The Redline version provides you with a quick and easy way to compare all the changes between this standard and its previous edition. The Redline version is not an official IEC Standard, only the current version of the standard is to be considered the official document.\r
IEC 61000-6-2:2016 for EMC immunity requirements applies to electrical and electronic equipment intended for use in industrial locations, as described below. Immunity requirements in the frequency range 0 Hz to 400 GHz are covered. No tests need to be performed at frequencies where no requirements are specified. This generic EMC immunity standard is applicable if no relevant dedicated product or product-family EMC immunity standard exists. This third edition cancels and replaces the second edition published in 2005. This edition constitutes a technical revision."""@en,
        "IEC 61000-6-2:2016 RLV contains the International Standard and its Redline version. The Redline version is available in English only. The Redline version provides you with a quick and easy way to compare all the changes between this standard and its previous edition. The Redline version is not an official IEC Standard, only the current version of the standard is to be considered the official document. IEC 61000-6-2:2016 for EMC immunity requirements applies to electrical and electronic equipment intended for use in industrial locations, as described below. Immunity requirements in the frequency range 0 Hz to 400 GHz are covered. No tests need to be performed at frequencies where no requirements are specified. This generic EMC immunity standard is applicable if no relevant dedicated product or product-family EMC immunity standard exists. This third edition cancels and replaces the second edition published in 2005. This edition constitutes a technical revision."@en,
        "IEC 61000-6-2:2016 RLV contains the International Standard and its Redline version. The Redline version is available in English only. The Redline version provides you with a quick and easy way to compare all the changes between this standard and its previous edition. The Redline version is not an official IEC Standard, only the current version of the standard is to be considered the official document.nIEC 61000-6-2:2016 for EMC immunity requirements applies to electrical and electronic equipment intended for use in industrial locations, as described below. Immunity requirements in the frequency range 0 Hz to 400 GHz are covered. No tests need to be performed at frequencies where no requirements are specified. This generic EMC immunity standard is applicable if no relevant dedicated product or product-family EMC immunity standard exists. This third edition cancels and replaces the second edition published in 2005. This edition constitutes a technical revision."@en ;
    sto:hasAvailableLanguage lang:eng ;
    sto:hasEdition "3.0"^^xsd:float ;
    sto:hasFileSize sto:FileSizeIEC_61000_P6_S2_2016 ;
    sto:hasICS sto:ICS_33_100_20 ;
    sto:hasOfficialResource <https://webstore.iec.ch/publication/25629> ;
    sto:hasPages "57"^^xsd:int ;
    sto:hasPublicationDate "2016-08-10"^^xsd:date ;
    sto:hasPublisher sto:IEC ;
    sto:hasStabilityDate "2020-01-01"^^xsd:gYear ;
    sto:hasTag "IEC 61000-6-2:2016"@en ;
    sto:hasTechnicalCommittee sto:TC_77 .

sto:IEC_61010_P2_S012_2016 a owl:NamedIndividual,
        sto:Standard ;
    rdfs:label "IEC 61010-2-012:2016"@en ;
    dcterms:title "Safety requirements for electrical equipment for measurement, control, and laboratory use - Part 2-012: Particular requirements for climatic and environmental testing and other temperature conditioning equipment"@en ;
    rdfs:comment """IEC 61010-2-012:2016 specifies safety requirements for electrical equipment and their accessories within the categories a) through c), wherever they are intended to be used, whenever that equipment incorporates one or more of the following characteristics:\r
- A REFRIGERATING SYSTEM that is acted on or impacted by an integral heating function such that the combined heating and cooling system generates additional and/or more severe HAZARDS than those for the two systems if treated separately.\r
- The materials being treated in the intended application introduce significant heat into the REFRIGERATING SYSTEM that the cooling system in the application yield additional and/or more severe HAZARDS than those for the cooling system if operated at the maximum RATED ambient alone.\r
- An irradiation function for the materials being treated presenting additional HAZARDS.\r
- A function to expose the materials being treated to excessive humidity, carbon dioxide, salt mist, or other substances which may result in additional HAZARDS.\r
- A function of MECHANICAL MOVEMENT presenting additional HAZARDS.\r
- Provision for an OPERATOR to walk-in to the operating area to load or unload the materials being treated.\r
It has the status of a group safety publication in accordance with IEC Guide 104.\r
This publication is to be read in conjunction with IEC 61010-1:2010."""@en,
        "IEC 61010-2-012:2016 specifies safety requirements for electrical equipment and their accessories within the categories a) through c), wherever they are intended to be used, whenever that equipment incorporates one or more of the following characteristics:- A REFRIGERATING SYSTEM that is acted on or impacted by an integral heating function such that the combined heating and cooling system generates additional and/or more severe HAZARDS than those for the two systems if treated separately.- The materials being treated in the intended application introduce significant heat into the REFRIGERATING SYSTEM that the cooling system in the application yield additional and/or more severe HAZARDS than those for the cooling system if operated at the maximum RATED ambient alone.- An irradiation function for the materials being treated presenting additional HAZARDS.- A function to expose the materials being treated to excessive humidity, carbon dioxide, salt mist, or other substances which may result in additional HAZARDS.- A function of MECHANICAL MOVEMENT presenting additional HAZARDS.- Provision for an OPERATOR to walk-in to the operating area to load or unload the materials being treated.It has the status of a group safety publication in accordance with IEC Guide 104. This publication is to be read in conjunction with IEC 61010-1:2010."@en,
        "IEC 61010-2-012:2016 specifies safety requirements for electrical equipment and their accessories within the categories a) through c), wherever they are intended to be used, whenever that equipment incorporates one or more of the following characteristics:n- A REFRIGERATING SYSTEM that is acted on or impacted by an integral heating function such that the combined heating and cooling system generates additional and/or more severe HAZARDS than those for the two systems if treated separately.n- The materials being treated in the intended application introduce significant heat into the REFRIGERATING SYSTEM that the cooling system in the application yield additional and/or more severe HAZARDS than those for the cooling system if operated at the maximum RATED ambient alone.n- An irradiation function for the materials being treated presenting additional HAZARDS.n- A function to expose the materials being treated to excessive humidity, carbon dioxide, salt mist, or other substances which may result in additional HAZARDS.n- A function of MECHANICAL MOVEMENT presenting additional HAZARDS.n- Provision for an OPERATOR to walk-in to the operating area to load or unload the materials being treated.nIt has the status of a group safety publication in accordance with IEC Guide 104.nThis publication is to be read in conjunction with IEC 61010-1:2010."@en ;
    sto:hasAvailableLanguage lang:eng,
        lang:fra ;
    sto:hasEdition "1.0"^^xsd:float ;
    sto:hasFileSize sto:FileSizeIEC_61010_P2_S012_2016 ;
    sto:hasICS sto:ICS_19_08 ;
    sto:hasOfficialResource <https://webstore.iec.ch/publication/25400> ;
    sto:hasPages "174"^^xsd:int ;
    sto:hasPublicationDate "2016-07-12"^^xsd:date ;
    sto:hasPublisher sto:IEC ;
    sto:hasStabilityDate "2020-01-01"^^xsd:gYear ;
    sto:hasTag "IEC 61010-2-012:2016"@en ;
    sto:hasTechnicalCommittee sto:TC_66 .

sto:IEC_61010_P2_S201_2017 a owl:NamedIndividual,
        sto:Standard ;
    rdfs:label "IEC 61010-2-201:2017"@en ;
    dcterms:title "Safety requirements for electrical equipment for measurement, control, and laboratory use - Part 2-201: Particular requirements for control equipment"@en ;
    rdfs:comment "IEC 61010-2-201:2017 RLV contains the International Standard and its Redline version. The Redline version is available in English only. The Redline version provides you with a quick and easy way to compare all the changes between this standard and its previous edition. The Redline version is not an official IEC Standard, only the current version of the standard is to be considered the official document.IEC 61010-2-201:2017 specifies safety requirements and related verification tests for any product performing the function of control equipment and/or their associated peripherals. In addition, these products have as their intended use the command and control of machines, automated manufacturing and industrial processes, e.g. discrete and continuous control.This second edition cancels and replaces the first edition published in 2013. This edition constitutes a technical revision. This second edition includes the following significant technical changes with respect to the previous edition;a) clarify, change, delete definitions which were causing confusion,b) change and clarify the temperature testing methodology,c) change documentation methodologies allowed,d) change some terminal markings,e) add clarity to some of the informative annexes,f) add Annex E with changes,g) add Annexes AA – FF."@en,
        "nIEC 61010-2-201:2017 RLV contains the International Standard and its Redline version. The Redline version is available in English only. The Redline version provides you with a quick and easy way to compare all the changes between this standard and its previous edition. The Redline version is not an official IEC Standard, only the current version of the standard is to be considered the official document.nnIEC 61010-2-201:2017 specifies safety requirements and related verification tests for any product performing the function of control equipment and/or their associated peripherals. In addition, these products have as their intended use the command and control of machines, automated manufacturing and industrial processes, e.g. discrete and continuous control.nThis second edition cancels and replaces the first edition published in 2013. This edition constitutes a technical revision. This second edition includes the following significant technical changes with respect to the previous edition;na) clarify, change, delete definitions which were causing confusion,nb) change and clarify the temperature testing methodology,nc) change documentation methodologies allowed,nd) change some terminal markings,ne) add clarity to some of the informative annexes,nf) add Annex E with changes,ng) add Annexes AA – FF."@en ;
    sto:hasAvailableLanguage lang:eng ;
    sto:hasEdition "2.0"^^xsd:float ;
    sto:hasFileSize sto:FileSizeIEC_61010_P2_S201_2017 ;
    sto:hasICS sto:ICS_17_020,
        sto:ICS_19_020,
        sto:ICS_25_040_40,
        sto:_020 ;
    sto:hasOfficialResource <https://webstore.iec.ch/publication/60204> ;
    sto:hasPages "235"^^xsd:int ;
    sto:hasPublicationDate "2017-03-24"^^xsd:date ;
    sto:hasPublisher sto:IEC ;
    sto:hasStabilityDate "2020-01-01"^^xsd:gYear ;
    sto:hasTag "IEC 61010-2-201:2017"@en ;
    sto:hasTechnicalCommittee sto:TC_65 .

sto:IEC_61010_P2_S202_2016 a owl:NamedIndividual,
        sto:Standard ;
    rdfs:label "IEC 61010-2-202:2016"@en ;
    dcterms:title "Safety requirements for electrical equipment for measurement, control and laboratory use - Part 2-202: Particular requirements for electrically operated valve actuators"@en ;
    rdfs:comment """IEC 61010-2-202:2016 specifies the safety requirements for electric ACTUATORs and SOLENOIDs, as applied to valves, intended to be installed in an industrial process or discrete control environment. \r
\r
This publication is to be read in conjunction with IEC 61010-1:2010."""@en,
        "IEC 61010-2-202:2016 specifies the safety requirements for electric ACTUATORs and SOLENOIDs, as applied to valves, intended to be installed in an industrial process or discrete control environment. nnThis publication is to be read in conjunction with IEC 61010-1:2010."@en ;
    sto:hasAvailableLanguage lang:eng,
        lang:fra ;
    sto:hasEdition "1.0"^^xsd:float ;
    sto:hasFileSize sto:FileSizeIEC_61010_P2_S202_2016 ;
    sto:hasICS sto:ICS_13_110,
        sto:ICS_17_020,
        sto:ICS_19_020,
        sto:_020 ;
    sto:hasOfficialResource <https://webstore.iec.ch/publication/25399> ;
    sto:hasPages "25"^^xsd:int ;
    sto:hasPublicationDate "2016-07-12"^^xsd:date ;
    sto:hasPublisher sto:IEC ;
    sto:hasStabilityDate "2019-01-01"^^xsd:gYear ;
    sto:hasTag "IEC 61010-2-202:2016"@en ;
    sto:hasTechnicalCommittee sto:TC_65 .

sto:IEC_61160 a owl:NamedIndividual,
        sto:Standard ;
    rdfs:label "IEC 61160:2005"@en ;
    dcterms:title "Design review"@en ;
    rdfs:comment "This International Standard makes recommendations for the implementation of design review as a means of verifying that the design input requirements have been met and stimulating the improvement of the product's design. The intention is for it to be applied during the design and development phase of a product's life cycle."@en ;
    sto:hasAvailableLanguage lang:eng,
        lang:fra,
        lang:spa ;
    sto:hasEdition "2.0"^^xsd:float ;
    sto:hasFileSize sto:FileSizeIEC_61160 ;
    sto:hasICS sto:ICS_03_100_40,
        sto:ICS_03_120_01 ;
    sto:hasOfficialResource <https://webstore.iec.ch/publication/4707> ;
    sto:hasPages "69"^^xsd:int ;
    sto:hasPublicationDate "2005-09-27"^^xsd:date ;
    sto:hasPublisher sto:IEC ;
    sto:hasStabilityDate "2020-01-01"^^xsd:gYear ;
    sto:hasTag "IEC 61160:2005"@en ;
    sto:hasTechnicalCommittee sto:TC_56 .

sto:IEC_61310_P1 a owl:NamedIndividual,
        sto:Standard ;
    rdfs:label "IEC 61310-1:2007"@en ;
    dcterms:title "Safety of machinery - Indication, marking and actuation - Part 1: Requirements for visual, acoustic and tactile signals"@en ;
    rdfs:comment "Specifies requirements for visual, acoustic and tactile methods of indicating safety-related information, at the human-machine interface and to exposed persons. It specifies a system of colours, safety signs, markings and other warnings, intended for use in the indication of hazardous situations and health hazards and for meeting certain emergencies. It also specifies ways of coding visual, acoustic and tactile signals for indicators and actuators to facilitate the safe use and monitoring of the machinery. It includes the following significant technical changes with respect to the previous edition: Adapted to the basic standards IEC 60073, IEC 60417, ISO 3864-1, ISO 7000 and ISO 7010"@en ;
    sto:hasAvailableLanguage lang:eng,
        lang:fra,
        lang:spa ;
    sto:hasEdition "2.0"^^xsd:float ;
    sto:hasFileSize sto:FileSizeIEC_61310_P1 ;
    sto:hasICS sto:ICS_13_110 ;
    sto:hasOfficialResource <https://webstore.iec.ch/publication/5263> ;
    sto:hasPages "43"^^xsd:int ;
    sto:hasPublicationDate "2007-02-16"^^xsd:date ;
    sto:hasPublisher sto:IEC ;
    sto:hasStabilityDate "2021-01-01"^^xsd:gYear ;
    sto:hasTag "IEC 61310-1:2007"@en ;
    sto:hasTechnicalCommittee sto:TC_44 .

sto:IEC_61310_P2 a owl:NamedIndividual,
        sto:Standard ;
    rdfs:label "IEC 61310-2:2007"@en ;
    dcterms:title "Safety of machinery - Indication, marking and actuation - Part 2: Requirements for marking"@en ;
    rdfs:comment "It gives general rules on marking for identification of machinery, for safe use related to mechanical and electrical hazards, and for the avoidance of hazards arising from incorrect connections. Includes the following significant technical changes with respect to the previous edition: Annex A: additional safety signs included and updated."@en ;
    sto:hasAvailableLanguage lang:eng,
        lang:fra,
        lang:spa ;
    sto:hasEdition "2.0"^^xsd:float ;
    sto:hasFileSize sto:FileSizeIEC_61310_P2 ;
    sto:hasICS sto:ICS_13_110 ;
    sto:hasOfficialResource <https://webstore.iec.ch/publication/5264> ;
    sto:hasPages "25"^^xsd:int ;
    sto:hasPublicationDate "2007-02-16"^^xsd:date ;
    sto:hasPublisher sto:IEC ;
    sto:hasStabilityDate "2021-01-01"^^xsd:gYear ;
    sto:hasTag "IEC 61310-2:2007"@en ;
    sto:hasTechnicalCommittee sto:TC_44 .

sto:IEC_61310_P3 a owl:NamedIndividual,
        sto:Standard ;
    rdfs:label "IEC 61310-3:2007"@en ;
    dcterms:title "Safety of machinery - Indication, marking and actuation - Part 3: Requirements for the location and operation of actuators"@en ;
    rdfs:comment "Specifies safety-related requirements for actuators, operated by the hand or by other parts of the human body, at the human-machine interface. It gives general requirements for the standard direction of movement for actuators; the arrangement of an actuator in relation to other actuators; the correlation between an action and its final effects. It includes the following significant technical changes with respect to the previous edition: Table 1, Table 2 and Table A.1 have been revised editorially."@en ;
    sto:hasAvailableLanguage lang:eng,
        lang:fra,
        lang:spa ;
    sto:hasEdition "2.0"^^xsd:float ;
    sto:hasFileSize sto:FileSizeIEC_61310_P3 ;
    sto:hasICS sto:ICS_13_110 ;
    sto:hasOfficialResource <https://webstore.iec.ch/publication/5265> ;
    sto:hasPages "25"^^xsd:int ;
    sto:hasPublicationDate "2007-02-16"^^xsd:date ;
    sto:hasPublisher sto:IEC ;
    sto:hasStabilityDate "2021-01-01"^^xsd:gYear ;
    sto:hasTag "IEC 61310-3:2007"@en ;
    sto:hasTechnicalCommittee sto:TC_44 .

sto:IEC_61334 a dbont:Work,
        owl:NamedIndividual,
        sto:Standard ;
    rdfs:label "IEC 61334"@en ;
    dcterms:subject dbrc:Networking_standards,
        dbrc:Wide_area_networks ;
    lingg:hypernym dbres:Standard ;
    rdfs:comment "IEC 61334 , known as Distribution automation using distribution line carrier systems, is a standard for low-speed reliable power line communications by electricity meters, water meters and SCADA."@en ;
    sto:hasDBpediaResource <http://dbpedia.org/page/IEC_61334> ;
    sto:hasOfficialResource <https://webstore.iec.ch/publication/5308> ;
    sto:hasPublisher sto:IEC ;
    sto:hasWikipediaArticle "http://en.wikipedia.org/wiki/IEC_61334" .

sto:IEC_61334_P3_S1_1998 a dbont:Work,
        owl:NamedIndividual,
        sto:Standard ;
    rdfs:label "IEC 61334-3-1:1998 "@en ;
    dcterms:subject dbrc:Networking_standards,
        dbrc:Wide_area_networks ;
    dcterms:title "Distribution automation using distribution line carrier systems - Part 3-1: Mains signalling requirements - Frequency bands and output levels"@en ;
    lingg:hypernym dbres:Standard ;
    rdfs:comment """Applies to electrical equipment used in distribution line carrier systems on both medium-voltage and low-voltage distribution networks. Specifies requirements such as frequency bands, output levels, spurious emissions, etc.\r
This publication is of high relevance for Smart Grid."""@en,
        "Applies to electrical equipment used in distribution line carrier systems on both medium-voltage and low-voltage distribution networks. Specifies requirements such as frequency bands, output levels, spurious emissions, etc.nThis publication is of high relevance for Smart Grid."@en ;
    sto:hasAvailableLanguage lang:eng,
        lang:fra ;
    sto:hasDBpediaResource <https://dbpedia.org/resource/IEC_61334> ;
    sto:hasEdition "1.0"^^xsd:float ;
    sto:hasFileSize sto:FileSizeIEC_61334_1998_P3_S1 ;
    sto:hasICS sto:ICS_29_240_20,
        sto:ICS_33_200 ;
    sto:hasOfficialResource <https://webstore.iec.ch/publication/5297> ;
    sto:hasPages "27"^^xsd:int ;
    sto:hasPublicationDate "1998-11-24"^^xsd:date ;
    sto:hasPublisher sto:IEC ;
    sto:hasStabilityDate "2018-01-01"^^xsd:gYear ;
    sto:hasTag "IEC 61334-3-1:1998 "@en ;
    sto:hasTechnicalCommittee sto:TC_57 ;
    sto:hasWikipediaArticle <https://en.wikipedia.org/wiki/IEC_61334> .

sto:IEC_61334_P3_S21_1996 a dbont:Work,
        owl:NamedIndividual,
        sto:Standard ;
    rdfs:label "IEC 61334-3-21:1996 "@en ;
    dcterms:subject dbrc:Networking_standards,
        dbrc:Wide_area_networks ;
    dcterms:title "Distribution automation using distribution line carrier systems - Part 3: Mains signalling requirements - Section 21: MV phase-to-phase isolated capacitive coupling device"@en ;
    lingg:hypernym dbres:Standard ;
    rdfs:comment """Establishes definitions, requirements, methods of testing and rated values for phase-to-phase isolated capacitive coupling devices to be used in medium-voltage (MV) distribution line carrier systems.\r
This publication is of high relevance for Smart Grid."""@en,
        "Establishes definitions, requirements, methods of testing and rated values for phase-to-phase isolated capacitive coupling devices to be used in medium-voltage (MV) distribution line carrier systems.nThis publication is of high relevance for Smart Grid."@en ;
    sto:hasAvailableLanguage lang:eng,
        lang:fra ;
    sto:hasDBpediaResource <https://dbpedia.org/resource/IEC_61334> ;
    sto:hasEdition "1.0"^^xsd:float ;
    sto:hasFileSize sto:FileSizeIEC_61334_1996_P3_S1 ;
    sto:hasICS sto:ICS_29_240_20,
        sto:ICS_33_200 ;
    sto:hasOfficialResource <https://webstore.iec.ch/publication/5298> ;
    sto:hasPages "33"^^xsd:int ;
    sto:hasPublicationDate "1996-03-27"^^xsd:date ;
    sto:hasPublisher sto:IEC ;
    sto:hasStabilityDate "2018-01-01"^^xsd:gYear ;
    sto:hasTag "IEC 61334-3-21:1996 "@en ;
    sto:hasTechnicalCommittee sto:TC_57 ;
    sto:hasWikipediaArticle <https://en.wikipedia.org/wiki/IEC_61334> .

sto:IEC_61334_P3_S22_2001 a dbont:Work,
        owl:NamedIndividual,
        sto:Standard ;
    rdfs:label "IEC 61334-3-22:2001"@en,
        "IEC 61334-3-22:2001�"@en ;
    dcterms:subject dbrc:Networking_standards,
        dbrc:Wide_area_networks ;
    dcterms:title "Distribution automation using distribution line carrier systems - Part 3-22: Mains signalling requirements - MV phase-to-earth and screen-to-earth intrusive coupling devices"@en ;
    lingg:hypernym dbres:Standard ;
    rdfs:comment """Establishes definitions, requirements, methods of testing and rated values for phase-to-earth capacitive and screen-to-earth intrusive inductive coupling devices to be used in medium voltage DLC systems.\r
This publication is of high relevance for Smart Grid."""@en,
        "Establishes definitions, requirements, methods of testing and rated values for phase-to-earth capacitive and screen-to-earth intrusive inductive coupling devices to be used in medium voltage DLC systems.nThis publication is of high relevance for Smart Grid."@en ;
    sto:hasAvailableLanguage lang:eng,
        lang:fra ;
    sto:hasDBpediaResource <https://dbpedia.org/resource/IEC_61334> ;
    sto:hasEdition "1.0"^^xsd:float ;
    sto:hasFileSize sto:FileSizeIEC_61334_1996_P3_S22 ;
    sto:hasICS sto:ICS_29_240_20,
        sto:ICS_33_200 ;
    sto:hasOfficialResource <https://webstore.iec.ch/publication/5299> ;
    sto:hasPages "35"^^xsd:int ;
    sto:hasPublicationDate "2001-01-12"^^xsd:date ;
    sto:hasPublisher sto:IEC ;
    sto:hasStabilityDate "2018-01-01"^^xsd:gYear ;
    sto:hasTag "IEC 61334-3-22:2001 "@en ;
    sto:hasTechnicalCommittee sto:TC_57 ;
    sto:hasWikipediaArticle <https://en.wikipedia.org/wiki/IEC_61334> .

sto:IEC_61334_P4_S1_1996 a dbont:Work,
        owl:NamedIndividual,
        sto:Standard ;
    rdfs:label "IEC 61334-4-1:1996 "@en ;
    dcterms:subject dbrc:Networking_standards,
        dbrc:Wide_area_networks ;
    dcterms:title "Distribution automation using distribution line carrier systems - Part 4: Data communication protocols - Section 1: Reference model of the communication system"@en ;
    lingg:hypernym dbres:Standard ;
    rdfs:comment """Provides a basic description of the communication system based on a three layer model. Application examples are control and monitoring of the distribution network, order broadcast, control of user interfaces, public lighting, automatic meter reading, etc.\r
This publication is of high relevance for Smart Grid."""@en,
        "Provides a basic description of the communication system based on a three layer model. Application examples are control and monitoring of the distribution network, order broadcast, control of user interfaces, public lighting, automatic meter reading, etc.nThis publication is of high relevance for Smart Grid."@en ;
    sto:hasAvailableLanguage lang:eng,
        lang:fra ;
    sto:hasDBpediaResource <https://dbpedia.org/resource/IEC_61334> ;
    sto:hasEdition "1.0"^^xsd:float ;
    sto:hasFileSize sto:FileSizeIEC_61334_1996_P4_S1 ;
    sto:hasICS sto:ICS_29_240_20,
        sto:ICS_33_200 ;
    sto:hasOfficialResource <https://webstore.iec.ch/publication/5300> ;
    sto:hasPages "43"^^xsd:int ;
    sto:hasPublicationDate "1996-07-31"^^xsd:date ;
    sto:hasPublisher sto:IEC ;
    sto:hasStabilityDate "2018-01-01"^^xsd:gYear ;
    sto:hasTag "IEC 61334-4-1:1996 "@en ;
    sto:hasTechnicalCommittee sto:TC_57 ;
    sto:hasWikipediaArticle <https://en.wikipedia.org/wiki/IEC_61334> .

sto:IEC_61334_P4_S32_1996 a dbont:Work,
        owl:NamedIndividual,
        sto:Standard ;
    rdfs:label "IEC 61334-4-32:1996 "@en ;
    dcterms:subject dbrc:Networking_standards,
        dbrc:Wide_area_networks ;
    dcterms:title "Distribution automation using distribution line carrier systems - Part 4: Data communication protocols - Section 32: Data link layer - Logical link control (LLC)"@en ;
    lingg:hypernym dbres:Standard ;
    rdfs:comment """Covers the services required of, or by, the DCP Logical Link Control (LLC) sublayer entity at the logical interfaces with the application layer and the MAC sublayer.\r
This publication is of high relevance for Smart Grid."""@en,
        "Covers the services required of, or by, the DCP Logical Link Control (LLC) sublayer entity at the logical interfaces with the application layer and the MAC sublayer.nThis publication is of high relevance for Smart Grid."@en ;
    sto:hasAvailableLanguage lang:eng,
        lang:fra ;
    sto:hasDBpediaResource <https://dbpedia.org/resource/IEC_61334> ;
    sto:hasEdition "1.0"^^xsd:float ;
    sto:hasFileSize sto:FileSizeIEC_61334_1996_P4_S32 ;
    sto:hasICS sto:ICS_29_240_20,
        sto:ICS_33_200 ;
    sto:hasOfficialResource <https://webstore.iec.ch/publication/5301> ;
    sto:hasPages "69"^^xsd:int ;
    sto:hasPublicationDate "1996-09-26"^^xsd:date ;
    sto:hasPublisher sto:IEC ;
    sto:hasStabilityDate "2018-01-01"^^xsd:gYear ;
    sto:hasTag "IEC 61334-4-32:1996 "@en ;
    sto:hasTechnicalCommittee sto:TC_57 ;
    sto:hasWikipediaArticle <https://en.wikipedia.org/wiki/IEC_61334> .

sto:IEC_61334_P4_S33_1998 a dbont:Work,
        owl:NamedIndividual,
        sto:Standard ;
    rdfs:label "IEC 61334-4-33:1998 "@en ;
    dcterms:subject dbrc:Networking_standards,
        dbrc:Wide_area_networks ;
    dcterms:title "Distribution automation using distribution line carrier systems - Part 4-33: Data communication protocols - Data link layer - Connection oriented protocol"@en ;
    lingg:hypernym dbres:Standard ;
    rdfs:comment "Covers the services required by the data communication protocol (DCP) logical link control (LLC) sublayer entity at the logical interfaces with the LLC -user layer and the MAC sublayer, using the connection-oriented LLC procedures.This publication is of high relevance for Smart Grid."@en,
        "Covers the services required by the data communication protocol (DCP) logical link control (LLC) sublayer entity at the logical interfaces with the LLC -user layer and the MAC sublayer, using the connection-oriented LLC procedures.nThis publication is of high relevance for Smart Grid."@en ;
    sto:hasAvailableLanguage lang:eng,
        lang:fra ;
    sto:hasDBpediaResource <https://dbpedia.org/resource/IEC_61334> ;
    sto:hasEdition "1.0"^^xsd:float ;
    sto:hasFileSize sto:FileSizeIEC_61334_1998_P4_S3 ;
    sto:hasICS sto:ICS_29_240_20,
        sto:ICS_33_200 ;
    sto:hasOfficialResource <https://webstore.iec.ch/publication/5302> ;
    sto:hasPages "51"^^xsd:int ;
    sto:hasPublicationDate "1998-07-10"^^xsd:date ;
    sto:hasPublisher sto:IEC ;
    sto:hasStabilityDate "2018-01-01"^^xsd:gYear ;
    sto:hasTag "IEC 61334-4-33:1998 "@en ;
    sto:hasTechnicalCommittee sto:TC_57 ;
    sto:hasWikipediaArticle <https://en.wikipedia.org/wiki/IEC_61334> .

sto:IEC_61334_P4_S41_1996 a dbont:Work,
        owl:NamedIndividual,
        sto:Standard ;
    rdfs:label "IEC 61334-4-41:1996"@en,
        "IEC 61334-4-41:1996�"@en ;
    dcterms:subject dbrc:Networking_standards,
        dbrc:Wide_area_networks ;
    dcterms:title "Distribution automation using distribution line carrier systems - Part 4: Data communication protocols - Section 41: Application protocol - Distribution line message specification"@en ;
    lingg:hypernym dbres:Standard ;
    rdfs:comment """Defines the distribution line message specification (DLMS) within the OSI application layer.\r
This publication is of high relevance for Smart Grid."""@en,
        "Defines the distribution line message specification (DLMS) within the OSI application layer.nThis publication is of high relevance for Smart Grid."@en ;
    sto:hasAvailableLanguage lang:eng,
        lang:fra ;
    sto:hasDBpediaResource <https://dbpedia.org/resource/IEC_61334> ;
    sto:hasEdition "1.0"^^xsd:float ;
    sto:hasFileSize sto:FileSizeIEC_61334_1996_P4_S41 ;
    sto:hasICS sto:ICS_29_240_20,
        sto:ICS_33_200 ;
    sto:hasOfficialResource <https://webstore.iec.ch/publication/5303> ;
    sto:hasPages "247"^^xsd:int ;
    sto:hasPublicationDate "1996-08-13"^^xsd:date ;
    sto:hasPublisher sto:IEC ;
    sto:hasStabilityDate "2018-01-01"^^xsd:gYear ;
    sto:hasTag "IEC 61334-4-41:1996"@en ;
    sto:hasTechnicalCommittee sto:TC_57 ;
    sto:hasWikipediaArticle <https://en.wikipedia.org/wiki/IEC_61334> .

sto:IEC_61334_P4_S42_1996 a dbont:Work,
        owl:NamedIndividual,
        sto:Standard ;
    rdfs:label "IEC 61334-4-42:1996"@en ;
    dcterms:subject dbrc:Networking_standards,
        dbrc:Wide_area_networks ;
    dcterms:title "Distribution automation using distribution line carrier systems -Part 4: Data communication protocols - Section 42: Applicationprotocols - Application laye"@en ;
    lingg:hypernym dbres:Standard ;
    rdfs:comment """Describes the rules used to design an application service element, the ISO connectionless ACSE (Application Control Service Element), and the DLMS Application Service Element.\r
This publication is of high relevance for Smart Grid."""@en,
        "Describes the rules used to design an application service element, the ISO connectionless ACSE (Application Control Service Element), and the DLMS Application Service Element.nThis publication is of high relevance for Smart Grid."@en ;
    sto:hasAvailableLanguage lang:eng,
        lang:fra ;
    sto:hasDBpediaResource <https://dbpedia.org/resource/IEC_61334> ;
    sto:hasEdition "1.0"^^xsd:float ;
    sto:hasFileSize sto:FileSizeIEC_61334_1996_P4_S42 ;
    sto:hasICS sto:ICS_29_240_20,
        sto:ICS_33_200 ;
    sto:hasOfficialResource <https://webstore.iec.ch/publication/5304> ;
    sto:hasPages "89"^^xsd:int ;
    sto:hasPublicationDate "1996-10-09"^^xsd:date ;
    sto:hasPublisher sto:IEC ;
    sto:hasStabilityDate "2018-01-01"^^xsd:gYear ;
    sto:hasTag "IEC 61334-4-42:1996"@en ;
    sto:hasTechnicalCommittee sto:TC_57 ;
    sto:hasWikipediaArticle <https://en.wikipedia.org/wiki/IEC_61334> .

sto:IEC_61334_P4_S511_2000 a dbont:Work,
        owl:NamedIndividual,
        sto:Standard ;
    rdfs:label "IEC 61334-4-511:2000"@en ;
    dcterms:subject dbrc:Networking_standards,
        dbrc:Wide_area_networks ;
    dcterms:title "Distribution automation using distribution line carrier systems - Part 4-511: Data communication protocols - Systems management - CIASE protocol"@en ;
    lingg:hypernym dbres:Standard ;
    rdfs:comment """Specifies the data communication protocol (DCP) management requirements. Describes the management services in an abstract way as well as the underlying protocol.\r
This publication is of high relevance for Smart Grid."""@en,
        "Specifies the data communication protocol (DCP) management requirements. Describes the management services in an abstract way as well as the underlying protocol.nThis publication is of high relevance for Smart Grid."@en ;
    sto:hasAvailableLanguage lang:eng,
        lang:fra ;
    sto:hasDBpediaResource <https://dbpedia.org/resource/IEC_61334> ;
    sto:hasEdition "1.0"^^xsd:float ;
    sto:hasFileSize sto:FileSizeIEC_61334_2000_P4_S511 ;
    sto:hasICS sto:ICS_33_040_40,
        sto:ICS_33_200 ;
    sto:hasOfficialResource <https://webstore.iec.ch/publication/5305> ;
    sto:hasPages "65"^^xsd:int ;
    sto:hasPublicationDate "2000-04-18"^^xsd:date ;
    sto:hasPublisher sto:IEC ;
    sto:hasStabilityDate "2018-01-01"^^xsd:gYear ;
    sto:hasTag "IEC 61334-4-511:2000"@en ;
    sto:hasTechnicalCommittee sto:TC_57 ;
    sto:hasWikipediaArticle <https://en.wikipedia.org/wiki/IEC_61334> .

sto:IEC_61334_P4_S512_2001 a dbont:Work,
        owl:NamedIndividual,
        sto:Standard ;
    rdfs:label "IEC 61334-4-512:2001"@en ;
    dcterms:subject dbrc:Networking_standards,
        dbrc:Wide_area_networks ;
    dcterms:title "Distribution automation using distribution line carrier systems - Part 4-512: Data communication protocols - System management using profile 61334-5-1 - Management Information Base (MIB)"@en ;
    lingg:hypernym dbres:Standard ;
    rdfs:comment """Specifies the Management Information Base (MIB), which is used for the management of the communication profile defined by the following standards: IEC 61334-5-1, IEC 61334-4-32, IEC 61334-4-42, and IEC 61334-4-41.\r
This publication is of high relevance for Smart Grid."""@en,
        "Specifies the Management Information Base (MIB), which is used for the management of the communication profile defined by the following standards: IEC 61334-5-1, IEC 61334-4-32, IEC 61334-4-42, and IEC 61334-4-41.nThis publication is of high relevance for Smart Grid."@en ;
    sto:hasAvailableLanguage lang:eng,
        lang:fra ;
    sto:hasDBpediaResource <https://dbpedia.org/resource/IEC_61334> ;
    sto:hasEdition "1.0"^^xsd:float ;
    sto:hasFileSize sto:FileSizeIEC_61334_2001_P4_S512 ;
    sto:hasICS sto:ICS_33_200 ;
    sto:hasOfficialResource <https://webstore.iec.ch/publication/5306> ;
    sto:hasPages "47"^^xsd:int ;
    sto:hasPublicationDate "2001-10-30"^^xsd:date ;
    sto:hasPublisher sto:IEC ;
    sto:hasStabilityDate "2018-01-01"^^xsd:gYear ;
    sto:hasTag "IEC 61334-4-512:2001"@en ;
    sto:hasTechnicalCommittee sto:TC_57 ;
    sto:hasWikipediaArticle <https://en.wikipedia.org/wiki/IEC_61334> .

sto:IEC_61334_P4_S61_1998 a dbont:Work,
        owl:NamedIndividual,
        sto:Standard ;
    rdfs:label "IEC 61334-4-61:1998"@en ;
    dcterms:subject dbrc:Networking_standards,
        dbrc:Wide_area_networks ;
    dcterms:title "Distribution automation using distribution line carrier systems - Part 4-61: Data communication protocols - Network layer - Connectionless protocol"@en ;
    lingg:hypernym dbres:Standard ;
    rdfs:comment """Covers the services required by the data communication protocol (DCP) network layer (N) sublayer entity at the logical interfaces with the N user layer and the LLC sublayer, using the connectionless N procedures.\r
This publication is of high relevance for Smart Grid."""@en,
        "Covers the services required by the data communication protocol (DCP) network layer (N) sublayer entity at the logical interfaces with the N user layer and the LLC sublayer, using the connectionless N procedures.nThis publication is of high relevance for Smart Grid."@en ;
    sto:hasAvailableLanguage lang:eng,
        lang:fra ;
    sto:hasDBpediaResource <https://dbpedia.org/resource/IEC_61334> ;
    sto:hasEdition "1.0"^^xsd:float ;
    sto:hasFileSize sto:FileSizeIEC_61334_1998_P4_S61 ;
    sto:hasICS sto:ICS_29_240_20,
        sto:ICS_33_200 ;
    sto:hasOfficialResource <https://webstore.iec.ch/publication/5307> ;
    sto:hasPages "63"^^xsd:int ;
    sto:hasPublicationDate "1998-07-10"^^xsd:date ;
    sto:hasPublisher sto:IEC ;
    sto:hasStabilityDate "2018-01-01"^^xsd:gYear ;
    sto:hasTag "IEC 61334-4-61:1998"@en ;
    sto:hasTechnicalCommittee sto:TC_57 ;
    sto:hasWikipediaArticle <https://en.wikipedia.org/wiki/IEC_61334> .

sto:IEC_61334_P5_S1_2001 a dbont:Work,
        owl:NamedIndividual,
        sto:Standard ;
    rdfs:label "IEC 61334-5-1:2001"@en ;
    dcterms:subject dbrc:Networking_standards,
        dbrc:Wide_area_networks ;
    dcterms:title "Distribution automation using distribution line carrier systems - Part 5-1: Lower layer profiles - The spread frequency shift keying (S-FSK) profile"@en ;
    lingg:hypernym dbres:Standard ;
    rdfs:comment """Describes the requirements of S-FSK (frequency shift keying modulation) in conjunction with the services provided by the physical layer entity and the MAC sublayer. The transmission medium is assumed to be the distribution network on both MV or LV level. To be used in conjunction with IEC 61334-4-32.\r
This publication is of high relevance for Smart Grid."""@en,
        "Describes the requirements of S-FSK (frequency shift keying modulation) in conjunction with the services provided by the physical layer entity and the MAC sublayer. The transmission medium is assumed to be the distribution network on both MV or LV level. To be used in conjunction with IEC 61334-4-32.nThis publication is of high relevance for Smart Grid."@en ;
    sto:hasAvailableLanguage lang:eng,
        lang:fra ;
    sto:hasDBpediaResource <https://dbpedia.org/resource/IEC_61334> ;
    sto:hasEdition "2.0"^^xsd:float ;
    sto:hasFileSize sto:FileSizeIEC_61334_2001_P5_S1 ;
    sto:hasICS sto:ICS_33_200 ;
    sto:hasOfficialResource <https://webstore.iec.ch/publication/5308> ;
    sto:hasPages "123"^^xsd:int ;
    sto:hasPublicationDate "2001-05-28"^^xsd:date ;
    sto:hasPublisher sto:IEC ;
    sto:hasStabilityDate "2018-01-01"^^xsd:gYear ;
    sto:hasTag "IEC 61334-5-1:2001"@en ;
    sto:hasTechnicalCommittee sto:TC_57 ;
    sto:hasWikipediaArticle <https://en.wikipedia.org/wiki/IEC_61334> .

sto:IEC_61334_P6_2000 a dbont:Work,
        owl:NamedIndividual,
        sto:Standard ;
    rdfs:label "IEC 61334-6:2000"@en ;
    dcterms:subject dbrc:Networking_standards,
        dbrc:Wide_area_networks ;
    dcterms:title "Distribution automation using distribution line carrier systems - Part 6: A-XDR encoding rule"@en ;
    lingg:hypernym dbres:Standard ;
    rdfs:comment """Defines a set of encoding rules that may be used to derive the specification of a transfer syntax for values of types defined in the DLMS core standard using the ASN.1 notation (see IEC 61334-4-41).\r
This publication is of high relevance for Smart Grid."""@en,
        "Defines a set of encoding rules that may be used to derive the specification of a transfer syntax for values of types defined in the DLMS core standard using the ASN.1 notation (see IEC 61334-4-41).nThis publication is of high relevance for Smart Grid."@en ;
    sto:hasAvailableLanguage lang:eng,
        lang:fra ;
    sto:hasDBpediaResource <https://dbpedia.org/resource/IEC_61334> ;
    sto:hasEdition "1.0"^^xsd:float ;
    sto:hasFileSize sto:FileSizeIEC_61334_2000_P6 ;
    sto:hasICS sto:ICS_29_240_20,
        sto:ICS_33_200 ;
    sto:hasOfficialResource <https://webstore.iec.ch/publication/5313> ;
    sto:hasPages "75"^^xsd:int ;
    sto:hasPublicationDate "2000-06-16"^^xsd:date ;
    sto:hasPublisher sto:IEC ;
    sto:hasStabilityDate "2018-01-01"^^xsd:gYear ;
    sto:hasTag "IEC 61334-6:2000"@en ;
    sto:hasTechnicalCommittee sto:TC_57 ;
    sto:hasWikipediaArticle <https://en.wikipedia.org/wiki/IEC_61334> .

sto:IEC_61400 a dbont:Work,
        owl:NamedIndividual,
        sto:Standard ;
    rdfs:label "IEC 61400"@en ;
    dcterms:subject dbrc:Electric_power_distribution,
        dbrc:Electric_power_transmission_systems,
        dbrc:IEC_standards,
        dbrc:Wind_turbines ;
    lingg:hypernym dbres:Standard ;
    rdfs:comment "IEC 61334 , known as Distribution automation using distribution line carrier systems, is a standard for low-speed reliable power line communications by electricity meters, water meters and SCADA."@en ;
    sto:hasDBpediaResource <http://dbpedia.org/page/IEC_61400> ;
    sto:hasOfficialResource <https://webstore.iec.ch/publication/26603> ;
    sto:hasPublicationDate "2017-03-03"^^xsd:date ;
    sto:hasPublisher sto:IEC ;
    sto:hasWikipediaArticle "http://en.wikipedia.org/wiki/IEC_61400" .

sto:IEC_61400_P25_1 a owl:NamedIndividual,
        sto:Standard ;
    rdfs:label "IEC 61400-25-1:2017"@en ;
    dcterms:title "Wind energy generation systems - Part 25-1: Communications for monitoring and control of wind power plants - Overall description of principles and models"@en ;
    rdfs:comment """IEC 61400-25-1:2017 RLV contains the International Standard and its Redline version. The Redline version is available in English only. The Redline version provides you with a quick and easy way to compare all the changes between this standard and its previous edition. The Redline version is not an official IEC Standard, only the current version of the standard is to be considered the official document.\r
\r
IEC 61400-25-1:2017 gives an overall description of the principles and models used in the IEC 61400�25 series, which is designed for a communication environment supported by a client-server model. Three areas are defined, that are modelled separately to ensure the scalability of implementations: wind power plant information models, information exchange model, and mapping of these two models to a standard communication profile. This new edition includes the following significant technical changes with respect to the previous edition: general harmonization of text and overview models with the other parts of the IEC 61400�25 series, harmonization of definitions in other related standards."""@en,
        "IEC 61400-25-1:2017 RLV contains the International Standard and its Redline version. The Redline version is available in English only. The Redline version provides you with a quick and easy way to compare all the changes between this standard and its previous edition. The Redline version is not an official IEC Standard, only the current version of the standard is to be considered the official document.IEC 61400-25-1:2017 gives an overall description of the principles and models used in the IEC 61400�25 series, which is designed for a communication environment supported by a client-server model. Three areas are defined, that are modelled separately to ensure the scalability of implementations: wind power plant information models, information exchange model, and mapping of these two models to a standard communication profile. This new edition includes the following significant technical changes with respect to the previous edition: general harmonization of text and overview models with the other parts of the IEC 61400�25 series, harmonization of definitions in other related standards."@en,
        "IEC 61400-25-1:2017 RLV contains the International Standard and its Redline version. The Redline version is available in English only. The Redline version provides you with a quick and easy way to compare all the changes between this standard and its previous edition. The Redline version is not an official IEC Standard, only the current version of the standard is to be considered the official document.nnIEC 61400-25-1:2017 gives an overall description of the principles and models used in the IEC 61400�25 series, which is designed for a communication environment supported by a client-server model. Three areas are defined, that are modelled separately to ensure the scalability of implementations: wind power plant information models, information exchange model, and mapping of these two models to a standard communication profile. This new edition includes the following significant technical changes with respect to the previous edition: general harmonization of text and overview models with the other parts of the IEC 61400�25 series, harmonization of definitions in other related standards."@en ;
    sto:hasAvailableLanguage lang:eng ;
    sto:hasEdition "2.0"^^xsd:float ;
    sto:hasFileSize sto:FileSizeIEC_61400_P25_1 ;
    sto:hasICS sto:ICS_27_180 ;
    sto:hasOfficialResource <https://webstore.iec.ch/publication/61087> ;
    sto:hasPages "109"^^xsd:int ;
    sto:hasPublicationDate "2017-07-20"^^xsd:date ;
    sto:hasPublisher sto:IEC ;
    sto:hasStabilityDate "2020-01-01"^^xsd:gYear ;
    sto:hasTag "IEC 61400-25-1:2017"@en ;
    sto:hasTechnicalCommittee sto:TC_88 .

sto:IEC_61400_P25_2 a owl:NamedIndividual,
        sto:Standard ;
    rdfs:label "IEC 61400-25-2:2015 "@en ;
    dcterms:title "Wind turbines - Part 25-2: Communications for monitoring and control of wind power plants - Information models"@en ;
    rdfs:comment """IEC 61400-25-2:2015 specifies the information model of devices and functions related to wind power plant applications. In particular, it specifies the compatible logical node names, and data names for communication between wind power plant components. This includes the relationship between logical devices, logical nodes and data. The names defined in the IEC 61400-25 series are used to build the hierarchical object references applied for communicating with components in wind power plants. Main changes with respect to the previous edition consist of:\r
- harmonization with newer editions of IEC 61850 standards;\r
- reduction of overlap between standards and simplification by increased referencing,\r
- extension of data objects for operation of smart grids,\r
- extended and enhanced semantics for existing data objects, etc."""@en,
        "IEC 61400-25-2:2015 specifies the information model of devices and functions related to wind power plant applications. In particular, it specifies the compatible logical node names, and data names for communication between wind power plant components. This includes the relationship between logical devices, logical nodes and data. The names defined in the IEC 61400-25 series are used to build the hierarchical object references applied for communicating with components in wind power plants. Main changes with respect to the previous edition consist of:- harmonization with newer editions of IEC 61850 standards;- reduction of overlap between standards and simplification by increased referencing,- extension of data objects for operation of smart grids,- extended and enhanced semantics for existing data objects, etc."@en,
        "IEC 61400-25-2:2015 specifies the information model of devices and functions related to wind power plant applications. In particular, it specifies the compatible logical node names, and data names for communication between wind power plant components. This includes the relationship between logical devices, logical nodes and data. The names defined in the IEC 61400-25 series are used to build the hierarchical object references applied for communicating with components in wind power plants. Main changes with respect to the previous edition consist of:n- harmonization with newer editions of IEC 61850 standards;n- reduction of overlap between standards and simplification by increased referencing,n- extension of data objects for operation of smart grids,n- extended and enhanced semantics for existing data objects, etc."@en ;
    sto:hasAvailableLanguage lang:eng,
        lang:fra ;
    sto:hasEdition "2.0"^^xsd:float ;
    sto:hasFileSize sto:FileSizeIEC_61400_P25_2 ;
    sto:hasICS sto:ICS_27_180 ;
    sto:hasOfficialResource <https://webstore.iec.ch/publication/22813> ;
    sto:hasPages "221"^^xsd:int ;
    sto:hasPublicationDate "2015-06-30"^^xsd:date ;
    sto:hasPublisher sto:IEC ;
    sto:hasStabilityDate "2018-01-01"^^xsd:gYear ;
    sto:hasTag "IEC 61400-25-2:2015 "@en ;
    sto:hasTechnicalCommittee sto:TC_88 .

sto:IEC_61400_P25_3 a owl:NamedIndividual,
        sto:Standard ;
    rdfs:label "IEC 61400-25-3:2015"@en ;
    dcterms:title "Wind turbines - Part 25-3: Communications for monitoring and control of wind power plants - Information exchange models"@en ;
    rdfs:comment """IEC 61400-25-3:2015 RLV contains the International Standard and its Redline version. The Redline version is available in English only. The Redline version provides you with a quick and easy way to compare all the changes between this standard and its previous edition. The Redline version is not an official IEC Standard, only the current version of the standard is to be considered the official document.\r
IEC 61400-25-3:2015 specifies an abstract communication service interface describing the information exchange between a client and a server for:\r
- data access and retrieval,\r
- device control,\r
- event reporting and logging,\r
- self-description of devices (device data dictionary),\r
- data typing and discovery of data types.\r
Main changes with respect to the previous edition consist of:\r
- harmonization with newer editions of IEC 61850 standards;\r
- reduction of overlap between standards and simplification by increased referencing, etc."""@en,
        "IEC 61400-25-3:2015 RLV contains the International Standard and its Redline version. The Redline version is available in English only. The Redline version provides you with a quick and easy way to compare all the changes between this standard and its previous edition. The Redline version is not an official IEC Standard, only the current version of the standard is to be considered the official document.IEC 61400-25-3:2015 specifies an abstract communication service interface describing the information exchange between a client and a server for:- data access and retrieval,- device control,- event reporting and logging,- self-description of devices (device data dictionary),- data typing and discovery of data types.Main changes with respect to the previous edition consist of:- harmonization with newer editions of IEC 61850 standards;- reduction of overlap between standards and simplification by increased referencing, etc."@en,
        "IEC 61400-25-3:2015 RLV contains the International Standard and its Redline version. The Redline version is available in English only. The Redline version provides you with a quick and easy way to compare all the changes between this standard and its previous edition. The Redline version is not an official IEC Standard, only the current version of the standard is to be considered the official document.nIEC 61400-25-3:2015 specifies an abstract communication service interface describing the information exchange between a client and a server for:n- data access and retrieval,n- device control,n- event reporting and logging,n- self-description of devices (device data dictionary),n- data typing and discovery of data types.nMain changes with respect to the previous edition consist of:n- harmonization with newer editions of IEC 61850 standards;n- reduction of overlap between standards and simplification by increased referencing, etc."@en ;
    sto:hasAvailableLanguage lang:eng ;
    sto:hasEdition "2.0"^^xsd:float ;
    sto:hasFileSize sto:FileSizeIEC_61400_P25_3 ;
    sto:hasICS sto:ICS_27_180 ;
    sto:hasOfficialResource <https://webstore.iec.ch/publication/22808> ;
    sto:hasPages "103"^^xsd:int ;
    sto:hasPublicationDate "2015-06-30"^^xsd:date ;
    sto:hasPublisher sto:IEC ;
    sto:hasStabilityDate "2018-01-01"^^xsd:gYear ;
    sto:hasTag "IEC 61400-25-3:2015"@en ;
    sto:hasTechnicalCommittee sto:TC_88 .

sto:IEC_61400_P25_4 a owl:NamedIndividual,
        sto:Standard ;
    rdfs:label "IEC 61400-25-4:2016"@en ;
    dcterms:title "Wind energy generation systems - Part 25-4: Communications for monitoring and control of wind power plants - Mapping to communication profile"@en ;
    rdfs:comment """IEC 61400-25-4:2016 RLV contains the International Standard and its Redline version. The Redline version is available in English only. The Redline version provides you with a quick and easy way to compare all the changes between this standard and its previous edition. The Redline version is not an official IEC Standard, only the current version of the standard is to be considered the official document.\r
\r
IEC 61400-25-4:2016 specifies the specific mappings to protocol stacks encoding the messages required for the information exchange between a client and a remote server for: data access and retrieval, device control, event reporting and logging, publisher/subscriber, self-description of devices (device data dictionary), data typing and discovery of data types. The mappings specified in this part of IEC 61400-25 comprise:\r
- a mapping to SOAP-based web services,\r
- a mapping to OPC/XML-DA,\r
- a mapping to IEC 61850-8-1 MMS,\r
- a mapping to IEC 60870-5-104,\r
- a mapping to DNP3.\r
The main technical changes with regard to the previous edition are as follows:\r
- general harmonization with information models in IEC 61400-25-2 and information exchange services in IEC 61400-25-3;\r
- reduction of overlap between standards and simplification by increased referencing."""@en,
        "IEC 61400-25-4:2016 RLV contains the International Standard and its Redline version. The Redline version is available in English only. The Redline version provides you with a quick and easy way to compare all the changes between this standard and its previous edition. The Redline version is not an official IEC Standard, only the current version of the standard is to be considered the official document.nnIEC 61400-25-4:2016 specifies the specific mappings to protocol stacks encoding the messages required for the information exchange between a client and a remote server for: data access and retrieval, device control, event reporting and logging, publisher/subscriber, self-description of devices (device data dictionary), data typing and discovery of data types. The mappings specified in this part of IEC 61400-25 comprise:n- a mapping to SOAP-based web services,n- a mapping to OPC/XML-DA,n- a mapping to IEC 61850-8-1 MMS,n- a mapping to IEC 60870-5-104,n- a mapping to DNP3.nThe main technical changes with regard to the previous edition are as follows:n- general harmonization with information models in IEC 61400-25-2 and information exchange services in IEC 61400-25-3;n- reduction of overlap between standards and simplification by increased referencing."@en ;
    sto:hasAvailableLanguage lang:eng ;
    sto:hasEdition "2.0"^^xsd:float ;
    sto:hasFileSize sto:FileSizeIEC_61400_P25_4 ;
    sto:hasICS sto:ICS_27_180 ;
    sto:hasOfficialResource <https://webstore.iec.ch/publication/59497> ;
    sto:hasPages "829"^^xsd:int ;
    sto:hasPublicationDate "2016-11-30"^^xsd:date ;
    sto:hasPublisher sto:IEC ;
    sto:hasStabilityDate "2018-01-01"^^xsd:gYear ;
    sto:hasTag "IEC 61400-25-4:2016"@en ;
    sto:hasTechnicalCommittee sto:TC_88 .

sto:IEC_61400_P25_5 a owl:NamedIndividual,
        sto:Standard ;
    rdfs:label "IEC 61400-25-5:2017"@en ;
    dcterms:title "Wind energy generation systems - Part 25-5: Communications for monitoring and control of wind power plants - Compliance testing"@en ;
    rdfs:comment """IEC 61400-25-5:2017 specifies standard techniques for testing of compliance of implementations, as well as specific measurement techniques to be applied when declaring performance parameters. The use of these techniques will enhance the ability of users to purchase systems that integrate easily, operate correctly, and support the applications as intended. This part of IEC 61400-25 defines: the methods and abstract test cases for compliance testing of server and client devices used in wind power plants; the metrics to be measured in said devices according to the communication requirements specified in IEC 61400-25 (all parts). This new edition includes the following significant technical changes with respect to the previous edition:\r
- harmonization with structure and test cases in IEC 61850-10:2012;\r
- reduction of overlap between standards and simplification by increased referencing to the IEC 61850 standard series."""@en,
        "IEC 61400-25-5:2017 specifies standard techniques for testing of compliance of implementations, as well as specific measurement techniques to be applied when declaring performance parameters. The use of these techniques will enhance the ability of users to purchase systems that integrate easily, operate correctly, and support the applications as intended. This part of IEC 61400-25 defines: the methods and abstract test cases for compliance testing of server and client devices used in wind power plants; the metrics to be measured in said devices according to the communication requirements specified in IEC 61400-25 (all parts). This new edition includes the following significant technical changes with respect to the previous edition:n- harmonization with structure and test cases in IEC 61850-10:2012;n- reduction of overlap between standards and simplification by increased referencing to the IEC 61850 standard series."@en ;
    sto:hasAvailableLanguage lang:eng ;
    sto:hasEdition "2.0"^^xsd:float ;
    sto:hasFileSize sto:FileSizeIEC_61400_P25_5 ;
    sto:hasICS sto:ICS_27_180 ;
    sto:hasOfficialResource <https://webstore.iec.ch/publication/26560> ;
    sto:hasPages "56"^^xsd:int ;
    sto:hasPublicationDate "2017-09-20"^^xsd:date ;
    sto:hasPublisher sto:IEC ;
    sto:hasStabilityDate "2020-01-01"^^xsd:gYear ;
    sto:hasTag "IEC 61400-25-5:2017"@en ;
    sto:hasTechnicalCommittee sto:TC_88 .

sto:IEC_61400_P25_6 a owl:NamedIndividual,
        sto:Standard ;
    rdfs:label "IEC 61400-25-6:2016"@en ;
    dcterms:title "Wind energy generation systems - Part 25-6: Communications for monitoring and control of wind power plants - Logical node classes and data classes for condition monitoring"@en ;
    rdfs:comment """IEC 61400-25-6:2016(E) specifies the information models related to condition monitoring for wind power plants and the information exchange of data values related to these models. This standard is to be used with other standards of the IEC 61400-25 series. This new edition includes the following significant technical changes with respect to the previous edition:\r
- major restructuring of the data model to accommodate flexibility; removal of UFF58 format;\r
- access to data using the standard reporting and logging functions;\r
- recommendations for creating data names to accommodate flexibility."""@en,
        "IEC 61400-25-6:2016(E) specifies the information models related to condition monitoring for wind power plants and the information exchange of data values related to these models. This standard is to be used with other standards of the IEC 61400-25 series. This new edition includes the following significant technical changes with respect to the previous edition:n- major restructuring of the data model to accommodate flexibility; removal of UFF58 format;n- access to data using the standard reporting and logging functions;n- recommendations for creating data names to accommodate flexibility."@en ;
    sto:hasAvailableLanguage lang:eng ;
    sto:hasEdition "2.0"^^xsd:float ;
    sto:hasFileSize sto:FileSizeIEC_61400_P25_6 ;
    sto:hasICS sto:ICS_27_180 ;
    sto:hasOfficialResource <https://webstore.iec.ch/publication/32580> ;
    sto:hasPages "49"^^xsd:int ;
    sto:hasPublicationDate "2016-12-16"^^xsd:date ;
    sto:hasPublisher sto:IEC ;
    sto:hasStabilityDate "2019-01-01"^^xsd:gYear ;
    sto:hasTag "IEC 61400-25-6:2016"@en ;
    sto:hasTechnicalCommittee sto:TC_88 .

sto:IEC_61506 a owl:NamedIndividual,
        sto:Standard ;
    rdfs:label "IEC 61506:1997"@en ;
    dcterms:title "Industrial-process measurement and control - Documentation ofapplication software"@en ;
    rdfs:comment "Defines the requirements for the documentation of software in industrial process measurement and control systems."@en ;
    sto:hasAvailableLanguage lang:eng,
        lang:fra ;
    sto:hasEdition "1.0"^^xsd:float ;
    sto:hasFileSize sto:FileSizeIEC_61506 ;
    sto:hasICS sto:ICS_25_040_40 ;
    sto:hasOfficialResource <https://webstore.iec.ch/publication/5513> ;
    sto:hasPages "119"^^xsd:int ;
    sto:hasPublicationDate "1997-02-28"^^xsd:date ;
    sto:hasPublisher sto:IEC ;
    sto:hasStabilityDate "2018-01-01"^^xsd:gYear ;
    sto:hasTag "IEC 61506:1997"@en ;
    sto:hasTechnicalCommittee sto:TC_65 .

sto:IEC_61508 a dbpcy:WikicatElectricalStandards,
        dbpcy:WikicatIECStandards,
        owl:NamedIndividual,
        sto:Standard ;
    rdfs:label "IEC 61508"@en ;
    dcterms:hasLicense "Private"@en ;
    dcterms:subject dbrc:Electrical_standards,
        dbrc:IEC_standards,
        dbrc:Safety ;
    rdfs:comment "Functional safety is a concept applicable across all industry sectors. It is fundamental to the enabling of complex technology used for safety-related systems. It provides the assurance that the safety-related systems will offer the necessary risk reduction required to achieve safety for the equipment. The oil and gas industry, nuclear plants and the machinery sector, to name but a few, all rely heavily on functional safety to achieve safety for the equipment giving rise to the hazards."@en ;
    sto:alignesWith sto:Safety ;
    sto:hasClassification iira:Safety,
        rami:Safety,
        idsram:Certification,
        idsram:Safety ;
    sto:hasDBpediaResource dbres:IEC_61508 ;
    sto:hasMotivation "Defines the functional safety requirements established by IEC 61508 in process industry sector terminology"@en ;
    sto:hasOfficialResource <http://www.iec.ch/functionalsafety/> ;
    sto:hasPublicationDate "1997-02-28"^^xsd:date ;
    sto:hasPublisher sto:IEC ;
    sto:hasTag "Functional Safety of Electrical/Electronic/Programmable Electronic Safety-related Systems"@en ;
    sto:hasWikipediaArticle <https://en.wikipedia.org/wiki/IEC_61508> ;
    sto:relatedTo sto:IEC_61511 .

sto:IEC_61512 a dbpcy:WikicatANSIStandards,
        dbpcy:WikicatStandards,
        dbont:Place,
        owl:NamedIndividual,
        sto:Standard ;
    rdfs:label "IEC 61512"@en ;
    dcterms:subject dbrc:ANSI_standards,
        dbrc:Manufacturing ;
    lingg:hypernym dbres:Control ;
    rdfs:comment "Batch control - Models and terminology"@en ;
    sto:hasClassification rami:ControlDevice,
        rami:Product,
        rami:Station,
        rami:WorkCenter ;
    sto:hasDBpediaResource dbres:ISA-88 ;
    sto:hasMotivation "The standard sought to address the following problems: lack of a universal model for batch control, difficulty in communicating user requirement, integration among batch automation suppliers, difficulty in batch control configuration."@en ;
    sto:hasOfficialResource <https://webstore.iec.ch/publication/5528> ;
    sto:hasPublisher sto:IEC ;
    sto:hasTag "ISA-88"@en ;
    sto:hasWikipediaArticle <https://en.wikipedia.org/wiki/ISA-88> .

sto:IEC_61513 a owl:NamedIndividual,
        sto:Standard ;
    rdfs:label "IEC 61513"@en ;
    rdfs:comment "IEC 61508 is intended to be a basic functional safety standard applicable to all kinds of industry. It defines functional safety as: “part of the overall safety relating to the EUC (Equipment Under Control) and the EUC control system which depends on the correct functioning of the E/E/PE safety-related systems, other technology safety-related systems and external risk reduction facilities.\""@en ;
    sto:hasClassification iira:Safety ;
    sto:hasOfficialResource <https://webstore.iec.ch/publication/5532> ;
    sto:hasPublisher sto:IEC ;
    sto:hasWikipediaArticle <https://en.wikipedia.org/wiki/IEC_61508> .

sto:IEC_61690_P1_2000 a owl:NamedIndividual,
        sto:Standard ;
    rdfs:label "IEC 61690-1:2000"@en ;
    dcterms:title "Electronic design interchange format (EDIF) - Part 1: Version 3 0 0. (This publication is available in electronic HTML format only)"@en ;
    rdfs:comment "IEC 61690-1:2000 defines the syntax and semantics for EDIF Version 3 0 0. EDIF Version 3 0 0 addresses EDIF Level 0 and Level 1. EDIF Version 3 0 0 completely addresses the Connectivity and Schematic views, including at Level 1 the ability to represent frames. It includes capabilities formerly found in the Document and Graphics views. A series of releases is planned in the near future to address those views not completely addressed in this version."@en ;
    sto:hasAvailableLanguage lang:eng,
        lang:fra ;
    sto:hasEdition "1.0"^^xsd:float ;
    sto:hasFileSize sto:FileSizeIEC_61690_P1_2000 ;
    sto:hasICS sto:ICS_35_240_50 ;
    sto:hasOfficialResource <https://webstore.iec.ch/publication/5723> ;
    sto:hasPublicationDate "2000-01-31"^^xsd:date ;
    sto:hasPublisher sto:IEC ;
    sto:hasStabilityDate "2018-01-01"^^xsd:gYear ;
    sto:hasTag "IEC 61690-1:2000"@en ;
    sto:hasTechnicalCommittee sto:TC_91 .

sto:IEC_61690_P2_2000 a owl:NamedIndividual,
        sto:Standard ;
    rdfs:label "IEC 61690-2:2000"@en ;
    dcterms:title "Electronic design interchange format (EDIF) - Part 2: Version 4 0 0. (This publication is available in electronic HTML format only)"@en ;
    rdfs:comment "IEC 61690-2:2000 defines the syntax and semantics for EDIF Version 4 0 0. EDIF Version 4 0 0 addresses EDIF Level 0 and Level 1. EDIF Version 3 0 0 provides support for Connectivity and Schematics; EDIF Version 4 0 0 offers additional capability by providing support for the representation of Printed Circuit Boards (PCBs) and Multi-chip Modules (MCMs) including technology rules and assembly drawings."@en ;
    sto:hasAvailableLanguage lang:eng,
        lang:fra ;
    sto:hasEdition "1.0"^^xsd:float ;
    sto:hasFileSize sto:FileSizeIEC_61690_P2_2000 ;
    sto:hasICS sto:ICS_35_240_50 ;
    sto:hasOfficialResource <https://webstore.iec.ch/publication/5724> ;
    sto:hasPublicationDate "2000-01-31"^^xsd:date ;
    sto:hasPublisher sto:IEC ;
    sto:hasStabilityDate "2018-01-01"^^xsd:gYear ;
    sto:hasTag "IEC 61690-2:2000"@en ;
    sto:hasTechnicalCommittee sto:TC_91 .

sto:IEC_61691_P6 a owl:NamedIndividual,
        sto:Standard ;
    rdfs:label "IEC 61691-6:2009"@en ;
    dcterms:title "Behavioural languages - Part 6: VHDL Analog and Mixed-Signal Extensions"@en ;
    rdfs:comment "IEC 61691-6:2009(E) Defines IEC 61691-6/IEEE Std 1076.1 language, a hardware description language for the description and the simulation of analog, digital, and mixed-signal systems. The language, also informally known as VHDLAMS, is built on the IEC 61691-1-1/IEEE 1076 (VHDL) language and extends it to provide capabilities of writing and simulating analog and mixed-signal models."@en ;
    sto:hasAvailableLanguage lang:eng ;
    sto:hasEdition "1.0"^^xsd:float ;
    sto:hasFileSize sto:FileSizeIEC_61691_P6 ;
    sto:hasICS sto:ICS_35_060,
        sto:IECICS_25_040_01 ;
    sto:hasOfficialResource <https://webstore.iec.ch/publication/5726> ;
    sto:hasPages "332"^^xsd:int ;
    sto:hasPublicationDate "2009-12-14"^^xsd:date ;
    sto:hasPublisher sto:IEC ;
    sto:hasStabilityDate "2018-01-01"^^xsd:gYear ;
    sto:hasTag "IEC 61691-6:2009"@en ;
    sto:hasTechnicalCommittee sto:TC_91 .

sto:IEC_61810_P2 a owl:NamedIndividual,
        sto:Standard ;
    rdfs:label "IEC 61810-2:2017"@en ;
    dcterms:title "Electromechanical elementary relays - Part 2: Reliability"@en ;
    rdfs:comment """IEC 61810-2:2017 covers test conditions and provisions for the evaluation of endurance tests using appropriate statistical methods to obtain reliability characteristics for relays.\r
This document applies to electromechanical elementary relays considered as non-repaired items (i.e. items which are not repaired after failure).\r
This document does not cover procedures for electromechanical elementary relays where enhanced requirements for the verification of reliability apply.\r
This edition includes the following significant technical changes with respect to the previous edition:\r
- not only graphical but also numerical methods are added;\r
- reduction of number of samples in specified cases;\r
- new subclauses of confidence intervals are added;\r
- the WeiBayes approach is added to facilitate compliance tests (routine test) with lower effort;\r
- annexes have been restructured into an Annex A for data analysis (normative) and Annex B (informative) where various examples of the data analysis are given;\r
- the former Annex C has been incorporated into the modified Annex B;\r
- a new Annex C replaces the old Annex D."""@en,
        "IEC 61810-2:2017 covers test conditions and provisions for the evaluation of endurance tests using appropriate statistical methods to obtain reliability characteristics for relays.nThis document applies to electromechanical elementary relays considered as non-repaired items (i.e. items which are not repaired after failure).nThis document does not cover procedures for electromechanical elementary relays where enhanced requirements for the verification of reliability apply.nThis edition includes the following significant technical changes with respect to the previous edition:n- not only graphical but also numerical methods are added;n- reduction of number of samples in specified cases;n- new subclauses of confidence intervals are added;n- the WeiBayes approach is added to facilitate compliance tests (routine test) with lower effort;n- annexes have been restructured into an Annex A for data analysis (normative) and Annex B (informative) where various examples of the data analysis are given;n- the former Annex C has been incorporated into the modified Annex B;n- a new Annex C replaces the old Annex D."@en ;
    sto:hasAvailableLanguage lang:eng,
        lang:fra ;
    sto:hasEdition "3.0"^^xsd:float ;
    sto:hasFileSize sto:FileSizeIEC_61810_P2 ;
    sto:hasICS sto:ICS_29_120_70 ;
    sto:hasOfficialResource <https://webstore.iec.ch/publication/33869> ;
    sto:hasPages "86"^^xsd:int ;
    sto:hasPublicationDate "2017-05-30"^^xsd:date ;
    sto:hasPublisher sto:IEC ;
    sto:hasStabilityDate "2020-01-01"^^xsd:gYear ;
    sto:hasTag "IEC 61810-2:2017"@en ;
    sto:hasTechnicalCommittee sto:TC_94 .

sto:IEC_61810_P7 a owl:NamedIndividual,
        sto:Standard ;
    rdfs:label "IEC 61810-7:2006"@en ;
    dcterms:title "Electromechanical elementary relays - Part 7: Test and measurement procedures"@en ;
    rdfs:comment "IEC 61810-7:2006 Lays down the test and measurement procedures for electromechanical elementary relays. Covers basic considerations which are common to all types of electromechanical elementary relays. Supplementary requirements may be necessitated by specific designs or application."@en ;
    sto:hasAvailableLanguage lang:eng,
        lang:fra,
        lang:spa ;
    sto:hasEdition "2.0"^^xsd:float ;
    sto:hasFileSize sto:FileSizeIEC_61810_P7 ;
    sto:hasICS sto:ICS_29_120_70 ;
    sto:hasOfficialResource <https://webstore.iec.ch/publication/5963> ;
    sto:hasPages "176"^^xsd:int ;
    sto:hasPublicationDate "2006-03-14"^^xsd:date ;
    sto:hasPublisher sto:IEC ;
    sto:hasStabilityDate "2018-01-01"^^xsd:gYear ;
    sto:hasTag "IEC 61810-7:2006"@en ;
    sto:hasTechnicalCommittee sto:TC_94 .

sto:IEC_62264 a dbpcy:WikicatIECStandards,
        dbont:Work,
        owl:NamedIndividual,
        sto:Standard ;
    rdfs:label "IEC 62264"@en ;
    dcterms:hasLicense "Private"@en ;
    dcterms:subject dbrc:Control_engineering,
        dbrc:IEC_standards,
        dbrc:Systems_engineering ;
    lingg:hypernym dbres:Standard ;
    rdfs:comment "Enterprise-control system integration - Models and terminology"@en,
        "IEC 62264 is an international standard for enterprise-control system integration. This standard is based upon ANSI/ISA-95."@en ;
    rdfs:seeAlso <https://en.wikipedia.org/wiki/B2MML> ;
    skos:altLabel "B2MML" ;
    sto:hasClassification rami:Functional ;
    sto:hasDBpediaResource dbres:IEC_62264 ;
    sto:hasDeveloper sto:IEC ;
    sto:hasDomain "Enterprise Control"@en ;
    sto:hasMotivation "Informational representation of MES and ERP models."@en ;
    sto:hasOfficialResource <http://www.iso.org/iso/catalogue_detail.htm?csnumber=63740>,
        <https://webstore.iec.ch/publication/6675>,
        <https://www.iso.org/standard/57308.html> ;
    sto:hasPublisher sto:IEC,
        sto:MESA ;
    sto:hasTag "Enterprise control systems"@en,
        "Enterprise-control system integration"@en ;
    sto:hasWikipediaArticle <https://en.wikipedia.org/wiki/IEC_62264> ;
    sto:relatedTo sto:ISA-95 .

sto:IEC_62279 a owl:NamedIndividual,
        sto:Standard ;
    rdfs:label "IEC 62279"@en ;
    rdfs:comment "IEC 62279:2015 specifies the process and technical requirements for the development of software for programmable electronic systems for use in railway control and protection applications. It is aimed at use in any area where there are safety implications. These systems can be implemented using dedicated microprocessors, programmable logic controllers, multiprocessor distributed systems, larger scale central processor systems or other architectures."@en ;
    sto:hasClassification iira:Safety ;
    sto:hasDomain sto:ITSecurity ;
    sto:hasOfficialResource <https://webstore.iec.ch/publication/22781> ;
    sto:hasPublicationDate "2015-06-25"^^xsd:date ;
    sto:hasPublisher sto:IEC .

sto:IEC_62424 a dbpcy:WikicatAbbreviations,
        dbpcy:WikicatComputerFileFormats,
        dbpcy:WikicatIndustry-specificXML-basedStandards,
        dbpcy:WikicatXML-basedStandards,
        dbont:Software,
        owl:NamedIndividual,
        sto:Standard ;
    rdfs:label "IEC 62424"@en ;
    dcterms:hasLicense "Private"@en ;
    dcterms:subject dbrc:Computer_file_formats,
        dbrc:Industry-specific_XML-based_standards ;
    lingg:hypernym dbres:Format ;
    dul:isComponentOf sto:IEC_62714 ;
    rdfs:comment "CAEX (Computer Aided Engineering Exchange) is a neutral data format that allows storage of hierarchical object information, e.g. the hierarchical architecture of a plant. On a certain abstraction level, a plant consists in modules or components that are interconnected. CAEX allows storage of those modules or components by means of objects. Object oriented concepts as encapsulation, classes, class libraries, instances, instance hierarchies, inheritance, relations, attributes and interfaces are explicitly supported. CAEX bases on XML and is defined as XML schema (xsd file). The original intention of developing CAEX was the industrial lack of a common and established data exchange between process engineering tools and process control engineering tools. However, CAEX can be applied to all types of static object information, e.g. plant topologies, document topologies, product topologies, petri nets, but also for non-technical applications like phylogenetic trees."@en ;
    sto:hasDBpediaResource dbres:CAEX ;
    sto:hasOfficialResource <https://webstore.iec.ch/publication/25442> ;
    sto:hasPublisher sto:IEC ;
    sto:hasTag "CAEX"@en ;
    sto:hasWikipediaArticle <https://en.wikipedia.org/wiki/CAEX> .

sto:IEC_62591 a dbont:Company,
        owl:NamedIndividual,
        sto:Standard ;
    rdfs:label "IEC 62591"@en ;
    dcterms:subject dbrc:Wireless_networking,
        dbrc:Wireless_sensor_network ;
    lingg:hypernym dbres:Technology ;
    rdfs:comment "Industrial networks - Wireless communication network and communication profiles."@en ;
    sto:hasDBpediaResource <http://dbpedia.org/page/WirelessHART> ;
    sto:hasOfficialResource <https://webstore.iec.ch/publication/24433> ;
    sto:hasPublisher sto:IEC ;
    sto:hasWikipediaArticle <https://en.wikipedia.org/wiki/WirelessHART> .

sto:IEC_62656 a owl:NamedIndividual,
        sto:Standard ;
    rdfs:label "IEC 62656"@en ;
    rdfs:comment "Specifies the logical structure for a set of spreadsheets, used as data parcels, to define, transfer and register product ontologies"@en ;
    sto:hasOfficialResource <https://webstore.iec.ch/publication/7326> ;
    sto:hasPublisher sto:IEC .

sto:IEC_62832 a owl:NamedIndividual,
        sto:TechnicalSpecification ;
    rdfs:label "IEC TS 62832-1:2016 "@en ;
    rdfs:comment "Industrial-process measurement, control and automation - Digital factory framework - Part 1: General principles"@en ;
    sto:hasAvailableLanguage lang:eng ;
    sto:hasEdition "1.0"^^xsd:float ;
    sto:hasFileSize sto:FileSizeIEC_62832 ;
    sto:hasICS sto:ICS_25_040_40 ;
    sto:hasPages "47"^^xsd:int ;
    sto:hasPublicationDate "2016-12-16"^^xsd:date ;
    sto:hasStabilityDate "2020-01-01"^^xsd:gYear ;
    sto:hasTechnicalCommittee sto:TC_65 .

sto:IEC_62837 a owl:NamedIndividual,
        sto:Standard ;
    rdfs:label "IEC 62837"@en ;
    rdfs:comment "Provides to the technical committees a framework for the development and adaptation of documents in order to improve energy efficiency in manufacturing, process control and industrial facility management."@en ;
    sto:hasOfficialResource <https://webstore.iec.ch/publication/7446> ;
    sto:hasPublisher sto:IEC ;
    sto:hasTag "62837"@en .

sto:IEC_81714 a owl:NamedIndividual,
        sto:Standard ;
    rdfs:label "IEC 81714"@en ;
    rdfs:comment "ISO/IEC 81714 Design of graphical symbols for use in the technical documentation of products -- Part 3: Classification of connect nodes, networks and their encoding-- specifies requirements concerning the classification of connect nodes assigned to graphical symbols, being a representation of functional and product concepts."@en ;
    sto:hasClassification rami:Asset,
        rami:Engineering,
        rami:Identification,
        rami:Product,
        sto:ModelingPractice ;
    sto:hasDomain sto:CAD ;
    sto:hasOfficialResource <https://www.iso.org/standard/40134.html> ;
    sto:hasPublicationDate "2004-10-01"^^xsd:date ;
    sto:hasPublisher sto:IEC,
        sto:ISO .

sto:IEC_PAS_63088 a owl:NamedIndividual,
        sto:Standard ;
    rdfs:label "IEC PAS 63088"@en ;
    rdfs:comment "IEC PAS 63088:2017(E) describes a reference architecture model in the form of a cubic layer model, RAMI model"@en ;
    sto:hasOfficialResource <https://webstore.iec.ch/publication/30082?lipi=urn%3Ali%3Apage%3Ad_flagship3_pulse_read%3B2vZf0%2FOGS2CeRjny8ARziQ%3D%3D> ;
    sto:hasPublicationDate "2017-03-07"^^xsd:date ;
    sto:hasPublisher sto:IEC,
        sto:ISO ;
    sto:hasTag "RAMI 4.0" .

sto:IEC_TR_62794 a owl:NamedIndividual,
        sto:Standard ;
    rdfs:label "IEC TR 62794"@en ;
    dcterms:hasLicense "Private"@en ;
    rdfs:comment "Industrial-process measurement, control and automation - Reference model for representation of production facilities (digital factory)"@en ;
    sto:hasClassification rami:AdminShellGeneral,
        rami:ControlDevice,
        rami:FieldDevice,
        rami:GeneralAdminShell,
        rami:Station,
        rami:WorkCenter ;
    sto:hasMotivation "The standards for Digital Factory define methods and information models, which are required for self description of I40-components. "@en ;
    sto:hasOfficialResource <https://webstore.iec.ch/publication/7433> ;
    sto:hasPublisher sto:IEC ;
    sto:hasTag "DF/TR"@en ;
    sto:relatedTo sto:IEC_TS_62832 .

sto:IEC_TS_62237 a owl:NamedIndividual,
        sto:Standard ;
    rdfs:label "IEC 62237"@en ;
    rdfs:comment "Live working - Insulating hoses with fittings for use with hydraulic tools and equipment."@en ;
    sto:hasClassification rami:ControlDevice,
        rami:FieldDevice,
        rami:GeneralAdminShell,
        rami:Station,
        rami:WorkCenter,
        sto:ProductionSystemModelData ;
    sto:hasDomain sto:IndustrialAutomation ;
    sto:hasOfficialResource <https://webstore.iec.ch/publication/6626> ;
    sto:hasPublicationDate "2003-10-26"^^xsd:date ;
    sto:hasPublisher sto:IEC ;
    sto:relatedTo sto:IEC_62337 .

sto:IEEE_1686 a dbpcy:WikicatInternationalNongovernmentalOrganizations,
        dbpcy:WikicatProfessionalAssociations,
        dbpcy:WikicatStandardsOrganizations,
        dbont:Agent,
        dbont:Organisation,
        schema:Organization,
        dul:Agent,
        dul:SocialPerson,
        owl:NamedIndividual,
        owl:Thing,
        wike:Q24229398,
        wike:Q43229,
        sto:Standard ;
    rdfs:label "IEEE 1686"@en ;
    dcterms:subject dbrc:Emerging_technologies,
        dbrc:Institute_of_Electrical_and_Electronics_Engineers,
        dbrc:Renewable_energy_technology,
        dbrc:Smart_grid,
        dbrc:Standards_organizations ;
    dcterms:title "Standard for Intelligent Electronic Devices Cyber Security Capabilities"@en ;
    lingg:hypernym dbres:Initiative ;
    rdfs:comment "The functions and features to be provided in intelligent electronic devices (IEDs) to accommodate critical infrastructure protection programs are defined in this standard. Security regarding the access, operation, configuration, firmware revision and data retrieval from an IED are addressed. Communications for the purpose of power system protection (teleprotection) are not addressed in this standard."@en ;
    sto:hasClassification idsram:Security ;
    sto:hasDBpediaResource dbres:IEEE_Smart_Grid ;
    sto:hasDeveloper sto:IEEE ;
    sto:hasPublisher sto:IEEE ;
    sto:hasWikipediaArticle <https://en.wikipedia.org/wiki/IEEE_Smart_Grid> .

sto:IIRA a owl:NamedIndividual,
        sto:StandardizationFramework ;
    rdfs:label "IIRA"@en ;
    rdfs:comment "Industrial Internet Reference Architecture"@en ;
    sto:hasOfficialResource <http://www.iiconsortium.org/IIRA.htm> .

sto:ISA_62443 a owl:NamedIndividual ;
    sto:publisher sto:ISA .

sto:ISO_1101 a owl:NamedIndividual,
        sto:Standard ;
    rdfs:label "ISO 1101"@en ;
    rdfs:comment "Geometrical product specifications (GPS) -- Geometrical tolerancing -- Tolerances of form, orientation, location and run-out"@en ;
    sto:hasClassification rami:Asset,
        rami:Product,
        sto:ModelingPractice ;
    sto:hasOfficialResource <https://www.iso.org/standard/66777.html> ;
    sto:hasPublicationDate "2017-02-01"^^xsd:date ;
    sto:hasPublisher sto:ISO .

sto:ISO_11898-1 a dbpcy:WikicatComputerBuses,
        dbpcy:WikicatLinkProtocols,
        dbpcy:WikicatNetworkProtocols,
        dbont:MeanOfTransportation,
        owl:NamedIndividual,
        owl:Thing,
        sto:Standard ;
    rdfs:label "ISO 11898-1"@en ;
    dcterms:subject dbrc:Automation,
        dbrc:Computer_networks,
        dbrc:Industrial_automation,
        dbrc:Industrial_computing,
        dbrc:Robert_Bosch_GmbH,
        dbrc:Serial_buses ;
    lingg:hypernym dbres:Vehicle ;
    rdfs:comment "Used mainly for Road vehicles Controller area network (CAN) Data link layer and physical signalling."@en ;
    sto:hasClassification rami:Communication,
        rami:Engineering,
        rami:Safety ;
    sto:hasDBpediaResource <http://dbpedia.org/page/CAN_bus> ;
    sto:hasDomain sto:IndustrialAutomation ;
    sto:hasOfficialResource <https://www.iso.org/standard/63648.html> ;
    sto:hasPublicationDate "2015-12-01"^^xsd:date ;
    sto:hasPublisher sto:ISO ;
    sto:hasTag "CAN Bus"@en ;
    sto:hasWikipediaArticle "http://en.wikipedia.org/wiki/CAN_bus" ;
    sto:relatedTo sto:ISO_11783 .

sto:ISO_1302 a owl:NamedIndividual,
        sto:Standard ;
    rdfs:label "ISO 1302"@en ;
    rdfs:comment "Geometrical product specifications Standards"@en ;
    sto:hasClassification sto:ModelingPractice ;
    sto:hasOfficialResource <https://www.iso.org/standard/28089.html> ;
    sto:hasPublicationDate "2002-02-01"^^xsd:date .

sto:ISO_13485 a dbpcy:WikicatISOStandards,
        dbont:Organisation,
        owl:NamedIndividual,
        sto:Standard ;
    rdfs:label "ISO 13485"@en ;
    dcterms:subject dbrc:ISO_standards,
        dbrc:Medical_equipment,
        dbrc:Medical_technology,
        dbrc:Regulation_of_medical_devices ;
    lingg:hypernym dbres:Organization ;
    rdfs:comment "Medical devices -- Quality management systems -- Requirements for regulatory purposes."@en ;
    sto:hasClassification rami:Safety ;
    sto:hasDBpediaResource <http://dbpedia.org/page/ISO_13485> ;
    sto:hasOfficialResource <https://www.iso.org/iso-9001-quality-management.html> ;
    sto:hasPublisher sto:ISO ;
    sto:hasWikipediaArticle "http://en.wikipedia.org/wiki/ISO_13485" .

sto:ISO_14739-1 a owl:NamedIndividual,
        sto:Standard ;
    rdfs:label "ISO 14739-1"@en ;
    rdfs:comment "Document management -- 3D use of Product Representation Compact (PRC) format-ISO 14739-1:2014 describes PRC 10001 of a product representation compact (PRC) file format for three dimensional (3D) content data. This format is designed to be included in PDF (ISO 32000) and other similar document formats for the purpose of 3D visualization and exchange. "@en ;
    skos:altLabel "STEP"@en ;
    sto:hasClassification sto:ProductModelDataExchange ;
    sto:hasDomain sto:CAD ;
    sto:hasOfficialResource <https://www.iso.org/standard/54948.html> ;
    sto:hasPublicationDate "2014-12-01"^^xsd:date ;
    sto:hasPublisher sto:ISO .

sto:ISO_15531-2x a owl:NamedIndividual,
        sto:StandardPart ;
    rdfs:label "ISO 15531 2x series"@en ;
    dul:isComponentOf sto:ISO_15531 ;
    rdfs:comment "Production data for external exchanges. refering to the representation of product information to be exchanged with the external environment (customers and suppliers), with the aim to model the main production information exchanged between industrial companies, in order to improve exchanges and integration through the use of EDI protocols."@en ;
    rdfs:isDefinedBy "https://www.researchgate.net/publication/220171079_ISO_15531_MANDATE_a_standardised_data_model_for_manufacturing_management" .

sto:ISO_15531-3x a owl:NamedIndividual,
        sto:StandardPart ;
    rdfs:label "ISO 15531 3x series"@en ;
    dul:isComponentOf sto:ISO_15531 ;
    rdfs:comment "Manufacturing resource usage management data : refering to the way of managing the use of resources, such as resource configuration and capabilities, operation management of manufacturing devices, installations and facilities."@en ;
    rdfs:isDefinedBy "https://www.researchgate.net/publication/220171079_ISO_15531_MANDATE_a_standardised_data_model_for_manufacturing_management" .

sto:ISO_15531-4x a owl:NamedIndividual,
        sto:StandardPart ;
    rdfs:label "ISO 15531 4x series"@en ;
    dul:isComponentOf sto:ISO_15531 ;
    rdfs:comment "Manufacturing flow management data : refering to the material flow control and aiming at the representation of data and elements supporting the control and monitoring of the flow of materials in manufacturing processes."@en ;
    rdfs:isDefinedBy "https://www.researchgate.net/publication/220171079_ISO_15531_MANDATE_a_standardised_data_model_for_manufacturing_management" .

sto:ISO_15704 a owl:NamedIndividual,
        sto:Standard ;
    rdfs:label "ISO 15704"@en ;
    rdfs:comment "Identifies requirements for enterprise-reference architectures and methodologies"@en ;
    sto:hasClassification rami:Business,
        rami:Enterprise,
        rami:Other ;
    sto:hasDomain sto:IndustrialAutomation ;
    sto:hasOfficialResource <https://www.iso.org/standard/28777.html> ;
    sto:hasPublicationDate "2000-06-01"^^xsd:date ;
    sto:hasPublisher sto:ISO ;
    sto:relatedTo sto:ISO_13374,
        sto:ISO_19439 .

sto:ISO_15746 a owl:NamedIndividual,
        sto:Standard ;
    rdfs:label "ISO 15746"@en ;
    rdfs:comment "Automation systems and integration -- Integration of advanced process control and optimization capabilities for manufacturing systems."@en ;
    sto:hasClassification rami:Communication,
        rami:ControlDevice,
        rami:Engineering,
        rami:FieldDevice,
        rami:Functional,
        rami:Information,
        rami:Integration,
        rami:Product,
        sto:ProductLifeCycleManagement ;
    sto:hasDomain sto:IndustrialAutomation ;
    sto:hasOfficialResource <https://www.iso.org/standard/61131.html> ;
    sto:hasPublicationDate "2015-04-01"^^xsd:date ;
    sto:hasPublisher sto:ISO ;
    sto:relatedTo sto:ISO_15926 .

sto:ISO_16739 a owl:NamedIndividual,
        sto:Standard ;
    rdfs:label "ISO 16739"@en ;
    rdfs:comment "Industry Foundation Classes (IFC) for data sharing in the construction and facility management industries."@en ;
    sto:hasClassification rami:LifecycleStatus,
        rami:Station,
        rami:WorkCenter,
        sto:ProductLifeCycleManagement ;
    sto:hasDomain sto:IndustrialAutomation ;
    sto:hasOfficialResource <https://www.iso.org/standard/51622.html> ;
    sto:hasPublicationDate "2013-04-01"^^xsd:date ;
    sto:hasPublisher sto:ISO ;
    sto:relatedTo sto:IEC_62890 .

sto:ISO_16792 a owl:NamedIndividual,
        sto:Standard ;
    rdfs:label "ISO 16792"@en ;
    rdfs:comment "ISO 16792 Technical product documentation -- Digital product definition data practices-It supports two methods of application: model-only and model and drawing in digital format."@en ;
    sto:hasClassification rami:Asset,
        rami:Product,
        sto:ModelingPractice ;
    sto:hasDomain sto:CAD ;
    sto:hasOfficialResource <https://www.iso.org/standard/56865.html> ;
    sto:hasPublicationDate "2015-12-01"^^xsd:date ;
    sto:hasPublisher sto:ISO .

sto:ISO_18629 a owl:NamedIndividual,
        sto:Standard ;
    rdfs:label "ISO 19629"@en ;
    rdfs:comment "ISO 18629-1:2004 provides a general overview of the different series of parts of ISO 18629, which defines a process specification language aimed at identifying, formally defining and structuring the semantic concepts intrinsic to the capture and exchange of process information related to discrete manufacturing."@en ;
    sto:hasClassification rami:Communication,
        rami:Configuration,
        rami:ControlDevice,
        rami:Engineering,
        rami:FieldDevice,
        rami:Functional,
        rami:Information,
        rami:Integration,
        rami:Product,
        sto:ProductModelDataExchange ;
    sto:hasDomain sto:IndustrialAutomation ;
    sto:hasOfficialResource <https://www.iso.org/standard/35431.html> ;
    sto:hasPublicationDate "2004-11-01"^^xsd:date ;
    sto:hasPublisher sto:ISO ;
    sto:hasTag "PSL"@en ;
    sto:hasWikipediaArticle <https://en.wikipedia.org/wiki/Process_Specification_Language> ;
    sto:relatedTo sto:ISO_15926,
        sto:ISO_ASTM_52915 .

sto:ISO_18828-2 a owl:NamedIndividual,
        sto:Standard ;
    rdfs:label "ISO 18828-2"@en ;
    rdfs:comment "Industrial automation systems and integration -- Standardized procedures for production systems engineering."@en ;
    sto:hasClassification rami:ControlDevice,
        rami:Engineering,
        rami:Enterprise,
        rami:FieldDevice,
        rami:Station,
        rami:WorkCenter,
        sto:Prodcut ;
    sto:hasDomain sto:IndustrialAutomation ;
    sto:hasOfficialResource <https://www.iso.org/standard/63505.html> ;
    sto:hasPublicationDate "2016-10-01"^^xsd:date ;
    sto:hasPublisher sto:ISO ;
    sto:relatedTo sto:IEC_61804 .

sto:ISO_19440 a owl:NamedIndividual,
        sto:Standard ;
    rdfs:label "ISO 19440"@en ;
    rdfs:comment "Enterprise integration -- Constructs for enterprise modelling-specifies the characteristics of the core constructs necessary for computer-supported modelling of enterprises conforming to ISO 19439.."@en ;
    sto:hasClassification rami:Engineering,
        rami:Enterprise,
        rami:Integration,
        sto:EnterpriseLevel,
        sto:Product ;
    sto:hasDomain sto:EnterpriseIntegration ;
    sto:hasOfficialResource <https://www.iso.org/standard/33834.html> ;
    sto:hasPublicationDate "2007-12-01"^^xsd:date ;
    sto:hasPublisher sto:ISO ;
    sto:relatedTo sto:BPMN .

sto:ISO_19770 a <http://dbpedia.org/class/yago/WikicatISO/IECStandards>,
        owl:NamedIndividual,
        sto:Standard ;
    rdfs:label "ISO/IEC 19770"@en ;
    dcterms:subject <http://dbpedia.org/resource/Category:ISO/IEC_standards>,
        dbrc:Information_technology_management ;
    dcterms:title "Information technology — Software asset management"@en ;
    rdfs:comment "International standards in the ISO/IEC 19770 family of standards for IT asset management (ITAM) address both the processes and technology for managing software assets and related IT assets. Broadly speaking, the standard family belongs to the set of Software Asset Management (or SAM) standards and is integrated with other Management System Standards."@en ;
    sto:hasClassification iira:Security ;
    sto:hasDBpediaResource <http://dbpedia.org/resource/ISO/IEC_19770> ;
    sto:hasDeveloper sto:ISO ;
    sto:hasPublicationDate "2017-12-01"^^xsd:date ;
    sto:hasPublisher sto:IEC,
        sto:ISO ;
    sto:hasWikipediaArticle <https://en.wikipedia.org/wiki/ISO/IEC_19770> .

sto:ISO_20140_5 a owl:NamedIndividual,
        sto:Standard ;
    rdfs:label "ISO 20140-5"@en ;
    rdfs:comment "Automation systems and integration -- Evaluating energy efficiency and other factors of manufacturing systems that influence the environment"@en ;
    sto:hasClassification rami:EnergyEfficiency ;
    sto:hasOfficialResource <http://www.iso.org/iso/catalogue_detail.htm?csnumber=54809> ;
    sto:hasPublisher sto:ISO ;
    sto:hasTag "Energy Efficiency"@en .

sto:ISO_20546 a owl:NamedIndividual,
        sto:Standard ;
    rdfs:label "ISO/IEC 20546"@en ;
    dcterms:title "Big data -- Overview and vocabulary"@en ;
    rdfs:comment "TODO: check with other reference architecture standards"@en ;
    sto:hasPublisher sto:IEC,
        sto:ISO .

sto:ISO_20547-3 a owl:NamedIndividual,
        sto:Standard ;
    rdfs:label "ISO/IEC DIS 20547-3"@en ;
    dcterms:title "Big data reference architecture -- Part 3: Reference architecture"@en ;
    rdfs:comment "TODO: how is this standard related to other reference architecture description formats?"@en,
        "under development (as from 2018-07-23)"@en ;
    sto:hasOfficialResource <https://www.iso.org/standard/71277.html> ;
    sto:hasPublisher sto:IEC,
        sto:ISO .

sto:ISO_20547-4 a owl:NamedIndividual,
        sto:Standard ;
    rdfs:label "ISO/IEC AWI 20547-4"@en ;
    dcterms:title "Big data reference architecture -- Part 4: Security and privacy"@en ;
    rdfs:comment "TODO: check with other reference architecture description frameworks"@en,
        "under development (as from 2018-07-23)"@en ;
    sto:hasOfficialResource <https://www.iso.org/standard/71278.html> ;
    sto:hasPublisher sto:IEC,
        sto:ISO .

sto:ISO_20922 a dbpcy:WikicatApplicationLayerProtocols,
        dbpcy:WikicatNetworkProtocols,
        owl:NamedIndividual,
        sto:Standard ;
    rdfs:label "ISO 20922"@en ;
    dcterms:subject dbrc:Application_layer_protocols,
        dbrc:Data_transmission,
        dbrc:IBM_WebSphere,
        dbrc:Message-oriented_middleware,
        dbrc:Network_protocols,
        dbrc:Telemetry ;
    rdfs:comment "ISO/IEC 20922:2016 is a Client Server publish/subscribe messaging transport protocol. It is light weight, open, simple, and designed so as to be easy to implement. These characteristics make it ideal for use in many situations, including constrained environments such as for communication in Machine to Machine (M2M) and Internet of Things (IoT) contexts where a small code footprint is required and/or network bandwidth is at a premium."@en ;
    sto:hasClassification iira:InformationDomain,
        iira:TansportLayer ;
    sto:hasDBpediaResource dbres:MQTT ;
    sto:hasDeveloper sto:IBM,
        sto:OASIS ;
    sto:hasDomain sto:M2M ;
    sto:hasOfficialResource <http://mqtt.org/>,
        <https://www.iso.org/standard/69466.html> ;
    sto:hasPublisher sto:IEC,
        sto:ISO ;
    sto:hasTag "MQTT"@en,
        "Message Queue Telemetry Transport"@en ;
    sto:hasWikipediaArticle <https://en.wikipedia.org/wiki/MQTT> ;
    sto:relatedTo sto:IEC_62541 .

sto:ISO_22400 a owl:NamedIndividual,
        sto:Standard ;
    rdfs:label "ISO 22400"@en ;
    rdfs:comment "Automation systems and integration -- Key performance indicators (KPIs) for manufacturing operations management."@en ;
    sto:hasClassification rami:Business,
        rami:Conditional_Monitoring,
        rami:ConnectedWorld,
        rami:ControlDevice,
        rami:Enterprise,
        rami:FieldDevice,
        rami:LifeCycle_Status,
        rami:Station,
        rami:WorkCenter ;
    sto:hasDomain sto:IndustrialAutomation ;
    sto:hasOfficialResource <https://www.iso.org/standard/54497.html> ;
    sto:hasPublicationDate "2014-01-01"^^xsd:date ;
    sto:hasPublisher sto:ISO ;
    sto:relatedTo sto:IEC_62541 .

sto:ISO_22745-11 a owl:NamedIndividual,
        sto:Standard ;
    rdfs:label "ISO 22745-11"@en ;
    rdfs:comment "ISO 22745-11:2010 provides guidelines that are recommended for the development of terminology for concepts in an open technical dictionary (OTD).Compliance with these guidelines is not required in order for a term or definition to be included in an OTD. These guidelines are provided as a framework for developers of industrial terminology to ensure that definitions are consistent and understandable. Terminology that complies with these guidelines will be marked as such in the OTD. This will allow a user to perform a search that filters terminology based on compliance with ISO 22745-11:2010."@en ;
    sto:hasClassification rami:Assest,
        rami:Product,
        sto:ProductCatalogData ;
    sto:hasDomain sto:IndustrialAutomation ;
    sto:hasOfficialResource <https://www.iso.org/standard/53999.html> ;
    sto:hasPublicationDate "2010-02-01"^^xsd:date ;
    sto:hasPublisher sto:ISO .

sto:ISO_26262 a dbpcy:Profession100609953,
        dbpcy:WikicatAutomotiveStandards,
        dbpcy:WikicatAutomotiveTechnologies,
        dbpcy:WikicatISOStandards,
        dbpcy:WikicatInternationalStandards,
        dbpcy:WikicatStandards,
        dbont:Work,
        owl:NamedIndividual,
        owl:Thing,
        sto:Standard ;
    rdfs:label "ISO 26262"@en ;
    dcterms:subject dbrc:Automotive_standards,
        dbrc:Car_safety,
        dbrc:International_standards,
        dbrc:Safety_engineering ;
    dcterms:title "Road vehicles – Functional safety"@en ;
    lingg:hypernym dbres:Standard ;
    rdfs:comment "ISO 26262, titled \"Road vehicles – Functional safety\", is an international standard for functional safety of electrical and/or electronic systems in production automobiles defined by the International Organization for Standardization (ISO) in 2011."@en ;
    sto:hasClassification iira:Safety,
        idsram:Certification,
        idsram:Safety ;
    sto:hasDBpediaResource dbres:ISO_26262 ;
    sto:hasDomain sto:ITSecurity ;
    sto:hasOfficialResource <https://www.iso.org/obp/ui/#iso:std:iso:26262:-1:ed-1:v1:en> ;
    sto:hasPublisher sto:ISO ;
    sto:hasWikipediaArticle <https://en.wikipedia.org/wiki/ISO_26262> .

sto:ISO_27000 a owl:NamedIndividual,
        sto:Standard ;
    rdfs:label "IEC 27000"@en,
        "ISO 27000"@en,
        "ISO/IEC 27000"@en ;
    rdfs:comment "The ISO/IEC 27000 family of standards helps organizations keep information assets secure. Using this family of standards will help your organization manage the security of assets such as financial information, intellectual property, employee details or information entrusted to you by third parties."@en ;
    sto:hasClassification idsram:Security ;
    sto:hasDBpediaResource dbres:IEC_27000 ;
    sto:hasMotivation "Provides best practices for information security management. A critical issue for Industry 4.0 "@en ;
    sto:hasOfficialResource <http://www.27000.org/> ;
    sto:hasPublisher sto:ISO ;
    sto:hasTag "Information Security Management Systems"@en ;
    sto:hasWikipediaArticle <https://en.wikipedia.org/wiki/ISO/IEC_27000> .

sto:ISO_27001 a owl:NamedIndividual,
        sto:Standard ;
    rdfs:label "ISO 27001"@en,
        "ISO/IEC 27001"@en ;
    rdfs:comment "ISO/IEC 27001 is an information security standard, part of the ISO/IEC 27000 family of standards."@en ;
    sto:hasClassification iira:Security,
        idsram:Certification,
        idsram:Security ;
    sto:hasDBpediaResource <http://dbpedia.org/resource/ISO/IEC_27001> ;
    sto:hasDomain sto:ITSecurity ;
    sto:hasOfficialResource <https://www.iso.org/isoiec-27001-information-security.html> ;
    sto:hasPublisher sto:IEC,
        sto:ISO ;
    sto:hasWikipediaArticle <https://en.wikipedia.org/wiki/ISO/IEC_27001> .

sto:ISO_27017 a dbpcy:WikicatComputerSecurityStandards,
        dbpcy:WikicatENStandards,
        dbpcy:WikicatIECStandards,
        <http://dbpedia.org/class/yago/WikicatISO/IECStandards>,
        dbpcy:WikicatISOStandards,
        owl:NamedIndividual,
        sto:Standard ;
    rdfs:label "ISO/IEC 27017"@en ;
    dc11:title "Code of practice for information security controls based on ISO/IEC 27002 for cloud services"@en ;
    dcterms:subject <http://dbpedia.org/resource/Category:ISO/IEC_standards>,
        dbrc:Information_technology_management ;
    rdfs:comment "The ISO/IEC 270172 standard provides guidance on the information security elements of cloud computing. It assists with the implementation of cloud-specific information security controls, supplementing the guidance in ISO 27000 series standards."@en ;
    sto:hasClassification iira:Security ;
    sto:hasDBpediaResource <http://dbpedia.org/resource/ISO/IEC_27000-series> ;
    sto:hasDomain sto:ITSecurity ;
    sto:hasOfficialResource <https://www.iso.org/standard/43757.html> ;
    sto:hasPublicationDate "2015-12-01"^^xsd:date ;
    sto:hasPublisher sto:IEC,
        sto:ISO ;
    sto:hasWikipediaArticle <https://en.wikipedia.org/wiki/ISO/IEC_27000-series> .

sto:ISO_27019 a owl:NamedIndividual,
        sto:Standard ;
    rdfs:label "ISO 27019"@en ;
    dcterms:title "Guidance for information security management of power supply control systems based on ISO/IEC 27002"@en ;
    rdfs:comment "The specification serves as a guidance for introducing ISO/IEC 27002 into the energy domain."@en ;
    sto:hasClassification idsram:Certification ;
    sto:hasOfficialResource <https://www.beuth.de/de/technische-regel/din-iso-iec-tr-27019/223679647> ;
    sto:hasPublisher sto:ISO .

sto:ISO_29002 a owl:NamedIndividual,
        sto:Standard ;
    rdfs:label "ISO 29002"@en ;
    rdfs:comment "ISO 29002 is an interoperability standard, which provides a repository to be used in various ISO XML formats. It is used in ontoML."@en ;
    sto:hasDomain sto:IndustrialProcessMeasurementControl ;
    sto:hasOfficialResource <https://www.iso.org/standard/53617.html> ;
    sto:hasPublicationDate "2010-04-01"^^xsd:date ;
    sto:hasPublisher sto:ISO ;
    sto:relatedTo sto:eClass .

sto:ISO_29101 a owl:NamedIndividual,
        sto:Standard ;
    rdfs:label "ISO/IEC 29101"@en ;
    dcterms:title "Privacy architecture framework"@en,
        "Privacy impact assessment–Guidelines"@en ;
    rdfs:comment "Code of practice for protection of personally identifiable information (PII) in public clouds acting as PII processors"@en ;
    sto:hasClassification iira:Privacy ;
    sto:hasOfficialResource <https://www.iso.org/standard/45124.html> ;
    sto:hasPublicationDate "2013-10-01"^^xsd:date ;
    sto:hasPublisher sto:IEC,
        sto:ISO .

sto:ISO_29134 a owl:NamedIndividual,
        sto:Standard ;
    rdfs:label "ISO/IEC 29134"@en ;
    dc11:title "Privacy impact assessment–Guidelines"@en ;
    rdfs:comment "‘Privacy impact assessment–Guidelines’ proposes a methodology to conduct assessments on the impact of privacy."@en ;
    sto:hasClassification iira:Privacy ;
    sto:hasDomain sto:ITSecurity ;
    sto:hasOfficialResource <https://www.iso.org/standard/62289.html> ;
    sto:hasPublicationDate "2017-06-01"^^xsd:date ;
    sto:hasPublisher sto:IEC,
        sto:ISO .

sto:ISO_42010 a <http://dbpedia.org/class/yago/WikicatISO/IECStandards>,
        dbont:Work,
        owl:NamedIndividual,
        sto:Standard ;
    rdfs:label "ISO/IEC 42010"@en ;
    dcterms:subject dbrc:IEEE_standards,
        <http://dbpedia.org/resource/Category:ISO/IEC_standards>,
        dbrc:Software_architecture ;
    dcterms:title "Systems and software engineering — Architecture description"@en ;
    lingg:hypernym dbres:Standard ;
    rdfs:comment """ISO/IEC/IEEE 42010:2011 defines requirements on the description of system, software and enterprise architectures. It aims to standardise the practice of architecture description by defining standard terms, presenting a conceptual foundation for expressing, communicating and reviewing architectures and specifying requirements that apply to architecture descriptions, architecture frameworks and architecture description languages.\r
\r
Following its predecessor, IEEE Std 1471, the standard makes a strict distinction between Architectures and Architecture Descriptions.\r
\r
The description of ISO/IEC/IEEE 42010 in this article is based upon the standard published in 2011."""@en ;
    sto:domainName "Reference Architecture Description"@en ;
    sto:hasDBpediaResource <http://dbpedia.org/resource/ISO/IEC_42010> ;
    sto:hasOfficialResource <https://www.iso.org/standard/50508.html> ;
    sto:hasPublisher sto:IEC,
        sto:ISO ;
    sto:hasWikipediaArticle <https://en.wikipedia.org/wiki/ISO/IEC_42010> .

sto:ISO_50001 a dbpcy:WikicatISOStandards,
        dbont:Software,
        owl:NamedIndividual,
        sto:Standard ;
    rdfs:label "ISO 50001"@en ;
    dcterms:subject dbrc:Energy_economics,
        dbrc:ISO_standards ;
    lingg:hypernym dbres:Specification ;
    rdfs:comment "Energy management systems – Requirements with guidance for use is a specification created by the International Organization for Standardization (ISO) for an energy management system."@en ;
    sto:hasClassification sto:CrossLevel ;
    sto:hasDBpediaResource <http://dbpedia.org/page/ISO_50001> ;
    sto:hasOfficialResource <https://www.iso.org/iso-50001-energy-management.html> ;
    sto:hasPublisher sto:ISO ;
    sto:hasWikipediaArticle "http://en.wikipedia.org/wiki/ISO_50001" .

sto:ISO_5459 a owl:NamedIndividual,
        sto:Standard ;
    rdfs:label "ISO 5459"@en ;
    rdfs:comment "Geometrical product specifications (GPS) -- Geometrical tolerancing -- Datums and datum systems--ISO 5459:2011 specifies terminology, rules and methodology for the indication and understanding of datums and datum systems in technical product documentation"@en ;
    sto:hasClassification rami:Asset,
        rami:Product,
        sto:ModelingPractice ;
    sto:hasDomain sto:M2M ;
    sto:hasOfficialResource <https://www.iso.org/standard/40358.html> ;
    sto:hasPublicationDate "2011-08-01"^^xsd:date ;
    sto:hasPublisher sto:ISO .

sto:ISO_8062-4 a owl:NamedIndividual,
        sto:Standard ;
    rdfs:label "ISO 8062-4"@en ;
    rdfs:comment "Geometrical product specifications (GPS) -- Dimensional and geometrical tolerances for moulded parts -- General tolerances for castings using profile tolerancing in a general datum system"@en ;
    sto:hasClassification rami:Asset,
        rami:Product,
        sto:ProductionSystemModelData ;
    sto:hasOfficialResource <https://www.iso.org/standard/60774.html> ;
    sto:hasPublicationDate "2017-07-01"^^xsd:date ;
    sto:hasPublisher sto:ISO ;
    sto:hasTag "Automation systems and integration"@en ;
    sto:relatedTo sto:ISO_10303 .

sto:ISO_9000 a dbpcy:WikicatBritishStandards,
        dbpcy:WikicatISOStandards,
        owl:NamedIndividual,
        sto:Standard ;
    rdfs:label "ISO 9000"@en ;
    dcterms:subject dbrc:ISO_standards,
        dbrc:Quality,
        dbrc:Quality_management ;
    rdfs:comment "The ISO 9000 family of quality management systems standards is designed to help organizations ensure that they meet the needs of customers and other stakeholders while meeting statutory and regulatory requirements related to a product or program."@en ;
    sto:hasClassification sto:CrossLevel,
        idsram:Certification ;
    sto:hasDBpediaResource <http://dbpedia.org/page/ISO_9000> ;
    sto:hasOfficialResource <https://www.iso.org/iso-9001-quality-management.html> ;
    sto:hasPublisher sto:ISO ;
    sto:hasWikipediaArticle <https://en.wikipedia.org/wiki/ISO_9000> .

sto:ISO_9594 a owl:NamedIndividual,
        sto:Standard ;
    rdfs:label "ISO/IEC 9594"@en,
        "X.509"@en ;
    sto:hasClassification sto:DataSovereignty,
        idsram:Certification,
        idsram:Security ;
    sto:hasOfficialResource <https://tools.ietf.org/html/rfc5280> ;
    sto:hasPublisher sto:ISO .

sto:ISO_9594-8 a owl:NamedIndividual,
        sto:Standard ;
    rdfs:label "ISO/IEC 9594-8"@en,
        "X.509"@en ;
    dcterms:title "Information technology -- Open Systems Interconnection -- The Directory -- Part 8: Public-key and attribute certificate frameworks"@en ;
    rdfs:comment """ISO/IEC 9594-8:2017 addresses some of the security requirements in the areas of authentication and other security services through the provision of a set of frameworks upon which full services can be based. Specifically, this Recommendation | International Standard defines frameworks for:\r
\r
- public-key certificates; and\r
\r
- attribute certificates."""@en ;
    rdfs:seeAlso "https://tools.ietf.org/html/rfc5280" ;
    sto:hasClassification sto:DataSovereignty,
        idsram:Certification,
        idsram:Security ;
    sto:hasOfficialResource <https://tools.ietf.org/html/rfc5280>,
        <https://www.iso.org/standard/72557.html> ;
    sto:hasPublisher sto:ISO .

sto:ISO_PAS_17506 a dbpcy:Wikicat3DGraphicsFileFormats,
        dbpcy:WikicatCADFileFormats,
        dbpcy:WikicatComputerFileFormats,
        dbpcy:WikicatGraphicsFileFormats,
        dbpcy:WikicatGraphicsStandards,
        dbpcy:WikicatXML-basedStandards,
        dbont:Software,
        owl:NamedIndividual,
        sto:Standard ;
    rdfs:label "ISO PAS 17506"@en ;
    dcterms:subject <http://dbpedia.org/resource/Category:2004_software>,
        <http://dbpedia.org/resource/Category:3D_graphics_file_formats>,
        <http://dbpedia.org/resource/Category:3D_graphics_software>,
        dbrc:CAD_file_formats,
        dbrc:Graphics_standards,
        dbrc:XML-based_standards ;
    lingg:hypernym dbres:Format ;
    dul:isComponentOf sto:IEC_62714 ;
    rdfs:comment "ISO-PAS 17506-2012 describes the COLLADA schema. COLLADA is a COLLAborative Design Activity that defines an XML-based schema to enable 3D authoring applications to freely exchange digital assets without loss of information, enabling multiple software packages to be combined into extremely powerful tool chains."@en,
        "SO/PAS 17506:2012 describes the COLLADA schema. COLLADA is a COLLAborative Design Activity that defines an XML-based schema to enable 3D authoring applications to freely exchange digital assets without loss of information, enabling multiple software packages to be combined into extremely powerful tool chains. The purpose of ISO/PAS 17506:2012 is to provide a specification for the COLLADA schema in sufficient detail to enable software developers to create tools to process COLLADA resources. In particular, it is relevant to those who import to or export from digital content creation (DCC) applications, 3D interactive applications and tool chains, prototyping tools, real-time visualization applications such as those used in the video game and movie industries, and CAD tools. ISO/PAS 17506:2012 covers the initial design and specifications of the COLLADA schema, as well as a minimal set of requirements for COLLADA exporters. "@en ;
    sto:hasDBpediaResource dbres:COLLADA ;
    sto:hasDeveloper sto:ISO ;
    sto:hasOfficialResource <https://www.iso.org/standard/59902.html> ;
    sto:hasPublisher sto:ISO ;
    sto:hasTag "COLLADA"@en ;
    sto:hasWikipediaArticle <https://en.wikipedia.org/wiki/COLLADA> .

sto:ISO_TS_14649-201 a owl:NamedIndividual,
        sto:Standard ;
    rdfs:label "ISO TS 14649-201"@en ;
    rdfs:comment "SO/TS 14649-201:2011 specifies the technology-specific machine tool description data elements needed as process data for manufacturing and machine characteristics. The machine tool descriptions covered in this schema are, initially, milling machines, machining centres, turning machines and multi-tasking machines.ISO/TS 14649-201:2011 is not intended to replace existing machine tool description standards, but to cover the specific needs of manufacturing resource description for manufacturing needs in the technologies described in ISO 14649."@en ;
    sto:hasClassification rami:Assest,
        rami:Configuration,
        rami:Engineering,
        rami:Integration,
        rami:Product,
        rami:Safety,
        sto:ProductionSystemModelData ;
    sto:hasDomain sto:IndustrialAutomation ;
    sto:hasOfficialResource <https://www.iso.org/standard/60042.html> ;
    sto:hasPublicationDate "2011-12-01"^^xsd:date ;
    sto:hasPublisher sto:ISO .

sto:KATS a dbont:Organisation,
        owl:NamedIndividual,
        sto:StandardOrganization ;
    rdfs:label "Korean Agency for Technology and Standards"@en ;
    dcterms:subject dbrc:ISO_member_bodies ;
    lingg:hypernym dbres:Organization ;
    dul:isMemberOf sto:IEC,
        sto:ISO ;
    rdfs:comment "Korean Agency for Technology and Standards is the government standards organization for South Korea. It is part of the Ministry of Knowledge Economy. It is authorized to regulate and manage the legal measures of South Korea by the current Measures Act."@en ;
    sto:abbreviation "KATS"@de ;
    sto:belongsTo dbr:South_Korea ;
    sto:hasDBpediaResource <http://dbpedia.org/page/Korean_Agency_for_Technology_and_Standards> ;
    sto:hasHeadquaterIn dbr:Eumseong ;
    sto:hasWikipediaArticle <https://en.wikipedia.org/wiki/Korean_Agency_for_Technology_and_Standards> ;
    sto:orgName "Korean Agency for Technology and Standards"@en .

sto:MIIT a dbont:Agent,
        dbont:GovernmentAgency,
        dbont:Organisation,
        schema:Organization,
        dul:Agent,
        dul:SocialPerson,
        owl:NamedIndividual,
        owl:Thing,
        wike:Q24229398,
        wike:Q327333,
        wike:Q43229,
        sto:StandardOrganization ;
    dcterms:subject <http://dbpedia.org/resource/Category:2008_establishments_in_China>,
        dbrc:Communications_ministries,
        <http://dbpedia.org/resource/Category:Government_ministries_of_the_People's_Republic_of_China>,
        dbrc:Information_ministries,
        dbrc:Ministries_established_in_2008,
        <http://dbpedia.org/resource/Category:Ministry_of_Industry_and_Information_Technology_of_the_People's_Republic_of_China>,
        dbrc:Organizations_based_in_Beijing ;
    lingg:hypernym dbres:Agency ;
    rdfs:comment "Ministry of Industry and Information Technology (MIIT) of the Chinese government, established in March 2008, is the state agency of the People's Republic of China responsible for regulation and development of the postal service, Internet, wireless, broadcasting, communications, production of electronic and information goods, software industry and the promotion of the national knowledge economy."@en ;
    sto:abbreviation "MIIT" ;
    sto:belongsTo dbr:China ;
    sto:formationDate "2008-03-01"^^xsd:date ;
    sto:hasDBpediaResource <http://dbpedia.org/page/Ministry_of_Industry_and_Information_Technology> ;
    sto:hasHeadquaterIn dbr:Beijing ;
    sto:hasOfficialResource <http://www.miit.gov.cn/> ;
    sto:hasWikipediaArticle <https://en.wikipedia.org/wiki/Ministry_of_Industry_and_Information_Technology> ;
    sto:orgName "Ministry of Industry and Information Technology"@en .

sto:MOMLevel a owl:NamedIndividual,
        sto:ISA95Level ;
    rdfs:label "MOM Level"@en ;
    rdfs:comment "Describes the MOM level according to the ISA95 level classification."@en ;
    skos:definition "Manufacturing Operation Management Level according to ISA 95"@en .

sto:MTConnect a dbpcy:WikicatIndustry-specificXML-basedStandards,
        dbont:Company,
        owl:NamedIndividual,
        sto:Standard ;
    rdfs:label "MTConnect"@en ;
    dcterms:subject dbrc:Automation,
        dbrc:Computer-aided_manufacturing,
        dbrc:Industrial_computing,
        dbrc:Industry-specific_XML-based_standards ;
    lingg:hypernym dbres:Industry ;
    rdfs:comment "MTConnect is a protocol designed for the exchange of data between shop floor equipment and software applications used for monitoring and data analysis. MTConnect is referred to as a read-only standard, meaning that it only defines the extraction (reading) of data from control devices, not the writing of data to a control device. Freely available, open standards are used for all aspects of MTConnect. Data from shop floor devices is presented in XML format, and is retrieved from information providers, called Agents, using Hypertext Transfer Protocol (HTTP) as the underlying transport protocol. MTConnect provides a RESTful interface, which means the interface is stateless. No session must be established to retrieve data from an MTConnect Agent, and no logon or logoff sequence is required (unless overlying security protocols are added which do). Lightweight Directory Access Protocol (LDAP) is recommended for discovery services."@en ;
    sto:hasClassification sto:DeviceLevel ;
    sto:hasDBpediaResource dbres:MTConnect ;
    sto:hasDeveloper sto:MTConnect_Institute ;
    sto:hasOfficialResource <http://www.mtconnect.org/standard-documents> ;
    sto:hasPublisher sto:MTConnect_Institute ;
    sto:hasTag "MTConnect"@en ;
    sto:hasWikipediaArticle <https://en.wikipedia.org/wiki/MTConnect> .

sto:Manufacturing a owl:NamedIndividual .

sto:ModBus a dbpcy:WikicatComputerBuses,
        dbpcy:WikicatNetworkProtocols,
        dbpcy:WikicatOSIProtocols,
        dbont:Software,
        owl:NamedIndividual,
        sto:Standard ;
    rdfs:label "ModBus"@en ;
    dcterms:subject dbrc:Automation,
        dbrc:Building_automation,
        dbrc:Industrial_Ethernet,
        dbrc:Industrial_computing,
        dbrc:Network_protocols ;
    lingg:hypernym dbres:Protocol ;
    rdfs:comment "Modbus is a serial communications protocol to be used in Programmable logic controllers (PLCs)."@en ;
    sto:hasClassification rami:Integration ;
    sto:hasDBpediaResource <http://dbpedia.org/page/Modbus> ;
    sto:hasOfficialResource <http://www.modbus.org/> ;
    sto:hasPublisher sto:SE ;
    sto:hasTag "Modbus"@en ;
    sto:hasWikipediaArticle <https://en.wikipedia.org/wiki/Modbus> .

sto:NERC a owl:NamedIndividual,
        sto:StandardOrganization ;
    dcterms:description "The North American Electric Reliability Corporation (NERC) is a not-for-profit international regulatory authority whose mission is to assure the effective and efficient reduction of risks to the reliability and security of the grid. NERC develops and enforces Reliability Standards; annually assesses seasonal and long‐term reliability; monitors the bulk power system through system awareness; and educates, trains, and certifies industry personnel. NERC’s area of responsibility spans the continental United States, Canada, and the northern portion of Baja California, Mexico. NERC is the electric reliability organization (ERO) for North America, subject to oversight by the Federal Energy Regulatory Commission (FERC) and governmental authorities in Canada. NERC's jurisdiction includes users, owners, and operators of the bulk power system, which serves more than 334 million people."@en ;
    rdfs:seeAlso "https://www.nerc.com/Pages/default.aspx"@en ;
    sto:abbreviation "NERC"@en ;
    sto:hasWikipediaArticle <https://wikipedia.org/wiki/North_American_Electric_Reliability_Corporation> ;
    sto:orgName "North American Electric Reliability Corporation"@en .

sto:NISTIR_8062 a owl:NamedIndividual,
        sto:Standard ;
    rdfs:label "NIST Internal Report (NISTIR) 8062"@en,
        "NISTIR 8062"@en ;
    dc11:title "Privacy Risk Management for Federal Information Systems"@en ;
    rdfs:comment "This document provides an introduction to the concepts of privacy engineering and risk management for federal information systems. These concepts establish the basis for a common vocabulary to facilitate better understanding and communication of privacy risk within federal information systems, and the effective implementation of privacy principles. This publication introduces two key components to support the application of privacy engineering and risk management: privacy engineering objectives and a privacy risk model."@en ;
    sto:hasClassification iira:Privacy ;
    sto:hasOfficialResource <https://doi.org/10.6028/NIST.IR.8062> ;
    sto:hasPublicationDate "2017-04-01"^^xsd:date ;
    sto:hasPublisher sto:NIST .

sto:NISTIR_8107 a owl:NamedIndividual ;
    rdfs:label "NISTIR_8107"@en ;
    rdfs:comment "Describes the NIST Initiative"@en ;
    rdfs:isDefinedBy "http://nvlpubs.nist.gov/nistpubs/ir/2016/NIST.IR.8107.pdf" ;
    skos:note "TODO - improve this classification" ;
    sto:isDescribedin sto:BusinessProcessExecution,
        sto:SCM .

sto:NIST_500-291 a owl:NamedIndividual,
        sto:Standard ;
    rdfs:label "NIST 500-291"@en ;
    dcterms:title "NIST Cloud Computing Standards Roadmap"@en ;
    rdfs:comment "The NIST Cloud Computing Standards Roadmap Working Group has surveyed the existing standards landscape for security, portability, and interoperability standards/models/studies/use cases, etc., relevant to cloud computing. Using this available information, current standards, standards gaps, and standardization priorities are identified in this document. The NIST Definition of Cloud Computing identified cloud computing as a model for enabling ubiquitous, convenient, on-demand network access to a shared pool of configurable computing resources (e.g., networks, servers, storage, applications, and services) that can be rapidly provisioned and released with minimal management effort or service provider interaction."@en ;
    sto:domainName "Cloud Computing"@en ;
    sto:hasClassification iira:Security ;
    sto:hasOfficialResource <https://www.nist.gov/publications/nist-sp-500-291-nist-cloud-computing-standards-roadmap> ;
    sto:hasPublicationDate "2011-08-10"^^xsd:date ;
    sto:hasPublisher sto:NIST .

sto:NIST_500-292 a owl:NamedIndividual,
        sto:Standard ;
    rdfs:label "NIST 500-292"@en ;
    dc11:title "NIST Cloud Computing Reference Architecture"@en ;
    rdfs:comment "The adoption of cloud computing into the Federal Government and its implementation depend upon a variety of technical and non-technical factors. A fundamental reference point, based on the NIST definition of Cloud Computing, is needed to describe an overall framework that can be used government-wide. This document presents the NIST Cloud Computing Reference Architecture (RA) and Taxonomy (Tax) that will accurately communicate the components and offerings of cloud computing."@en ;
    sto:domainName "Cloud Computing"@en ;
    sto:hasClassification iira:Security ;
    sto:hasOfficialResource <https://www.nist.gov/publications/nist-cloud-computing-reference-architecture> ;
    sto:hasPublicationDate "2011-09-09"^^xsd:date ;
    sto:hasPublisher sto:NIST .

sto:NIST_500-293 a owl:NamedIndividual,
        sto:Standard ;
    rdfs:label "NIST 500-293"@en ;
    dcterms:title "US Government Cloud Computing Technology Roadmap"@en ;
    rdfs:comment "The National Institute of Standards and Technology (NIST), consistent with its mission, has a technology leadership role in support of United States Government (USG) secure and effective adoption of the Cloud Computing model to reduce costs and improve services. This role is described in the 2011 Federal Cloud Computing Strategy as “... a central one in defining and advancing standards, and collaborating with USG Agency CIOs, private sector experts, and international bodies to identify and reach consensus on cloud computing technology & standardization priorities.” This NIST Cloud Computing program and initiative to develop a USG Cloud Computing Technology Roadmap is one of several complementary and parallel USG initiatives defined in the broader Federal Cloud Computing Strategy referenced above. The Federal Cloud Computing Strategy characterizes cloud computing as a “profound economic and technical shift (with) great potential to reduce the cost of federal Information Technology (IT) systems while … improving IT capabilities and stimulating innovation in IT solutions.” In the technology vision of Federal Cloud Computing Strategy success, USG agencies will be able to easily locate desired IT services in a mature and competitive marketplace, rapidly procure access to these services, and use them to deliver innovative mission solutions. Cloud services will be secure, interoperable, and reliable. Agencies will be able to switch between providers easily and with minimal cost, and receive equal or superior service."@en ;
    sto:domainName "Cloud Computing"@en ;
    sto:hasAvailableLanguage lang:eng ;
    sto:hasClassification iira:Security ;
    sto:hasOfficialResource <https://www.nist.gov/publications/us-government-cloud-computing-technology-roadmap-volume-i-high-priority-requirements?pub_id=915112> ;
    sto:hasPublicationDate "2014-10-21"^^xsd:date ;
    sto:hasPublisher sto:NIST .

sto:NIST_800-144 a owl:NamedIndividual,
        sto:Standard ;
    rdfs:label "NIST 800-144"@en ;
    dcterms:title "Guidelines on Security and Privacy in Public Cloud Computing"@en ;
    rdfs:comment "Cloud computing can and does mean different things to different people. The common characteristics most interpretations share are on-demand scalability of highly available and reliable pooled computing resources, secure access to metered services from nearly anywhere, and displacement of data and services from inside to outside the organization. While aspects of these characteristics have been realized to a certain extent, cloud computing remains a work in progress. This publication provides an overview of the security and privacy challenges pertinent to public cloud computing and points out considerations organizations should take when outsourcing data, applications, and infrastructure to a public cloud environment."@en ;
    sto:domainName "Cloud Computing"@en ;
    sto:hasClassification iira:Security ;
    sto:hasOfficialResource <https://csrc.nist.gov/publications/detail/sp/800-144/final> ;
    sto:hasPublicationDate "2011-12-01"^^xsd:date ;
    sto:hasPublisher sto:NIST .

sto:NIST_800-146 a owl:NamedIndividual,
        sto:Standard ;
    rdfs:label "NIST 800-146"@en ;
    dc11:title "Cloud Computing Synopsis and Recommendations"@en ;
    rdfs:comment "This document reprises the NIST-established definition of cloud computing, describes cloud computing benefits and open issues, presents an overview of major classes of cloud technology, and provides guidelines and recommendations on how organizations should consider the relative opportunities and risks of cloud computing."@en ;
    sto:hasClassification iira:Security ;
    sto:hasOfficialResource <https://csrc.nist.gov/publications/detail/sp/800-146/final> ;
    sto:hasPublicationDate "2012-05-01"^^xsd:date ;
    sto:hasPublisher sto:NIST .

sto:OAGIS a owl:NamedIndividual,
        sto:Standard ;
    rdfs:label "OAGIS"@en ;
    rdfs:comment "The Open Applications Group Integration Specification (OAGIS) is an effort to provide a canonical business language for information integration. It uses XML as the common alphabet for defining business messages, and for identifying business processes (scenarios) that allow businesses and business applications to communicate."@en ;
    sto:hasOfficialResource <http://www.oagi.org/dnn2/DownloadsandResources/OAGIS100PublicDownload.aspx> ;
    sto:hasPublisher sto:OAGi ;
    sto:hasTag "Open Applications Group Integration Specification"@en ;
    sto:hasWikipediaArticle <https://de.wikipedia.org/wiki/Open_Application_Group_Integration_Specification> .

sto:ODRL a owl:NamedIndividual,
        sto:Standard ;
    rdfs:label "ODRL"@en,
        "Open Digital Rights Language"@en ;
    rdfs:comment """The Open Digital Rights Language (ODRL) is a policy expression language that provides a flexible and interoperable information model, vocabulary, and encoding mechanisms for representing statements about the usage of content and services. The ODRL Information Model describes the underlying concepts, entities, and relationships that form the foundational basis for the semantics of the ODRL policies.\r
Policies are used to represent permitted and prohibited actions over a certain asset, as well as the obligations required to be meet by stakeholders. In addition, policies may be limited by constraints (e.g., temporal or spatial constraints) and duties (e.g. payments) may be imposed on permissions."""@en ;
    sto:hasClassification idsram:InformationLayer,
        idsram:Security ;
    sto:hasOfficialResource <https://www.w3.org/TR/odrl-model/> ;
    sto:hasPublisher sto:W3C .

sto:ODVA a dbpcy:Abstraction100002137,
        dbpcy:Group100031264,
        dbpcy:Organization108008335,
        dbpcy:SocialGroup107950920,
        dbpcy:WikicatComputerNetworkOrganizations,
        dbpcy:YagoLegalActor,
        dbpcy:YagoLegalActorGeo,
        dbpcy:YagoPermanentlyLocatedEntity,
        owl:NamedIndividual,
        sto:StandardOrganization ;
    dcterms:subject dbrc:Computer_network_organizations ;
    rdfs:comment "Founded in 1995, ODVA is a global association whose members comprise the world’s leading automation companies. ODVA’s mission is to advance open, interoperable information and communication technologies in industrial automation. ODVA recognizes its media independent network protocol, the Common Industrial Protocol or “CIP” — and the network adaptations of CIP — EtherNet/IP, DeviceNet, CompoNet and ControlNet — as its core technology and the primary common interest of its membership. For future interoperability of production systems and the integration of the production systems with other systems, ODVA embraces the adoption of commercial-off-the-shelf (COTS) and standard, unmodified Internet and Ethernet technologies as a guiding principle wherever possible. This principle is exemplified by EtherNet/IP — the world’s number one industrial Ethernet network."@en ;
    sto:abbreviation "ODVA" ;
    sto:formationDate "1995-01-01"^^xsd:date ;
    sto:hasDBpediaResource <http://dbpedia.org/resource/ODVA_(company)> ;
    sto:hasHeadquaterIn dbr:_Michigan ;
    sto:hasOfficialResource <https://www.odva.org> ;
    sto:hasWikipediaArticle <https://en.wikipedia.org/wiki/ODVA_(company)> ;
    sto:orgName "ODVA, Inc"@en .

sto:OMG_DDS a dbpcy:WikicatComputerStandards,
        dbont:Software,
        owl:NamedIndividual,
        sto:Standard ;
    rdfs:label "OMG DDS"@en ;
    dcterms:subject dbrc:Computer_standards,
        dbrc:Message-oriented_middleware ;
    lingg:hypernym dbres:Middleware ;
    rdfs:comment "The Data Distribution Service for real-time systems (DDS) is an Object Management Group (OMG) machine-to-machine (sometimes called middleware) standard that aims to enable scalable, real-time, dependable, high-performance and interoperable data exchanges using a publish–subscribe pattern. DDS addresses the needs of applications like financial trading, air-traffic control, smart grid management, and other big data applications. The standard is used in applications such as smartphone operating systems, transportation systems and vehicles, software-defined radio, and by healthcare providers. DDS was promoted for use in the Internet of things."@en ;
    sto:hasClassification sto:FrameworkLayer,
        sto:IIRC ;
    sto:hasDBpediaResource <http://dbpedia.org/page/Data_Distribution_Service> ;
    sto:hasOfficialResource <http://portals.omg.org/dds/> ;
    sto:hasPublisher sto:OMG ;
    sto:hasTag "Data Distribution Service for real-time systems"@en ;
    sto:hasWikipediaArticle <https://en.wikipedia.org/wiki/Data_Distribution_Service> ;
    sto:relatedTo sto:IEC_61158 .

sto:ProductionSystemMaintenance a owl:NamedIndividual,
        sto:ProductionSystemLifeCycle ;
    rdfs:label "Production System Maintenance"@en ;
    rdfs:comment "Classifies standards define data processing, communication, and presentation standards for condition monitoring and diagnostics of machines, for maintaining the adequate performance of the system, and for searching ways to improve performance"@en ;
    sto:isDescribedin sto:NISTInitiative .

sto:QIF a owl:NamedIndividual,
        sto:Standard ;
    rdfs:label "Quality Information Framework"@en ;
    rdfs:comment " Quality Information Framework (QIF) standard defines an integrated set of information models which enable the effective exchange of metrology data throughout the entire manufacturing quality measurement process"@en ;
    rdfs:isDefinedBy "http://qifstandards.org/about-qif/" ;
    skos:note "Is implemented in XML" ;
    sto:hasOfficialResource <http://qifstandards.org/> ;
    sto:hasPublisher sto:DMSC .

sto:RAMI a owl:NamedIndividual ;
    rdfs:label "RAMI"@en ;
    rdfs:comment "Describes the RAMI model"@en ;
    rdfs:isDefinedBy "https://www.plattform-i40.de/I40/Redaktion/EN/Downloads/Publikation/structure-of-the-administration-shell.html" ;
    sto:isDescribedin rami:Information .

sto:RFC_1122 a owl:NamedIndividual,
        sto:Standard ;
    rdfs:label "RFC 1122"@en ;
    dcterms:title "Requirements for Internet Hosts -- Communication Layers"@en ;
    rdfs:comment "This is one RFC of a pair that defines and discusses the requirements for Internet host software.  This RFC covers the communications protocol layers: link layer, IP layer, and transport layer; its companion RFC-1123 covers the application and support protocols."@en ;
    sto:hasClassification iira:Connectivity,
        iira:NetworkLayer ;
    sto:hasOfficialResource <https://tools.ietf.org/html/rfc1122> ;
    sto:hasPublisher sto:IETF .

sto:RFC_2616 a owl:NamedIndividual,
        sto:Standard ;
    rdfs:label "HTTP/1.1"@en,
        "RFC 2616"@en ;
    rdfs:comment "The Hypertext Transfer Protocol (HTTP) is an application-level protocol for distributed, collaborative, hypermedia information systems. It is a generic, stateless, protocol which can be used for many tasks beyond its use for hypertext, such as name servers and distributed object management systems, through extension of its request methods, error codes and headers. A feature of HTTP is the typing and negotiation of data representation, allowing systems to be built independently of the data being transferred."@en ;
    sto:hasClassification iira:FunctionalViewpoint,
        iira:TansportLayer,
        rami:Communication,
        idsram:SystemLayer ;
    sto:hasOfficialResource <https://tools.ietf.org/html/rfc2817>,
        <https://www.ietf.org/rfc/rfc2616> ;
    sto:hasPublisher sto:IETF .

sto:RFC_2818 a owl:NamedIndividual,
        sto:Standard ;
    rdfs:label "HTTPS"@en,
        "RFC 2818"@en ;
    rdfs:comment "This memo describes how to use TLS to secure HTTP connections over  the Internet. Current practice is to layer HTTP over SSL (the predecessor to TLS), distinguishing secured traffic from insecure traffic by the use of a different server port. This document documents that practice using TLS. A companion document describes a method for using HTTP/TLS over the same port as normal HTTP [RFC2817]."@en ;
    sto:hasClassification idsram:Security,
        idsram:SystemLayer ;
    sto:hasPublisher sto:IETF .

sto:RFC_5246 a owl:NamedIndividual,
        sto:Standard ;
    rdfs:label "RFC 5246"@en ;
    dcterms:description "This document specifies Version 1.2 of the Transport Layer Security (TLS) protocol.  The TLS protocol provides communications security over the Internet.  The protocol allows client/server applications to communicate in a way that is designed to prevent eavesdropping, tampering, or message forgery."@en ;
    rdfs:comment "This document specifies Version 1.2 of the Transport Layer Security (TLS) protocol.  The TLS protocol provides communications security over the Internet.  The protocol allows client/server applications to communicate in a way that is designed to prevent eavesdropping, tampering, or message forgery."@en ;
    sto:hasClassification sto:DataSovereignty,
        idsram:Security ;
    sto:hasOfficialResource <https://tools.ietf.org/html/rfc5246> ;
    sto:hasPublisher sto:IETF .

sto:RFC_6750 a owl:NamedIndividual,
        sto:Standard ;
    rdfs:label "RFC 6750"@en ;
    dcterms:description "This specification describes how to use bearer tokens in HTTP requests to access OAuth 2.0 protected resources.  Any party in possession of a bearer token (a \"bearer\") can use it to get access to the associated resources (without demonstrating possession of a cryptographic key).  To prevent misuse, bearer tokens need to be protected from disclosure in storage and in transport."@en ;
    rdfs:comment "This specification describes how to use bearer tokens in HTTP requests to access OAuth 2.0 protected resources.  Any party in possession of a bearer token (a \"bearer\") can use it to get access to the associated resources (without demonstrating possession of a cryptographic key).  To prevent misuse, bearer tokens need to be protected from disclosure in storage and in transport."@en ;
    skos:altLabel "OAuth2.0"@en ;
    sto:hasClassification idsram:Security ;
    sto:hasOfficialResource <https://tools.ietf.org/html/rfc6750> ;
    sto:hasPublisher sto:IETF .

sto:RFC_7252 a owl:NamedIndividual,
        sto:Standard ;
    rdfs:label "RFC 7252"@en ;
    dcterms:title "The Constrained Application Protocol"@en ;
    rdfs:comment "The Constrained Application Protocol (CoAP) is a specialized web transfer protocol for use with constrained nodes and constrained (e.g., low-power, lossy) networks.  The nodes often have 8-bit microcontrollers with small amounts of ROM and RAM, while constrained networks such as IPv6 over Low-Power Wireless Personal Area Networks (6LoWPANs) often have high packet error rates and a typical throughput of 10s of kbit/s.  The protocol is designed for machine-to-machine (M2M) applications such as smart energy and building automation."@en ;
    skos:altLabel "CoAP"@en ;
    sto:hasClassification iira:OperationDomain,
        iira:TansportLayer ;
    sto:hasOfficialResource <https://tools.ietf.org/html/rfc7252> ;
    sto:hasPublicationDate "2014-06-01"^^xsd:date ;
    sto:hasPublisher sto:IETF .

sto:RFC_7519 a owl:NamedIndividual,
        sto:Standard ;
    rdfs:label "JSON Web Token"@en,
        "RFC 7519"@en ;
    dcterms:description "JSON Web Token (JWT) is a compact, URL-safe means of representing claims to be transferred between two parties.  The claims in a JWT are encoded as a JSON object that is used as the payload of a JSON Web Signature (JWS) structure or as the plaintext of a JSON Web Encryption (JWE) structure, enabling the claims to be digitally signed or integrity protected with a Message Authentication Code (MAC) and/or encrypted."@en ;
    rdfs:comment "JSON Web Token (JWT) is a compact, URL-safe means of representing claims to be transferred between two parties.  The claims in a JWT are encoded as a JSON object that is used as the payload of a JSON Web Signature (JWS) structure or as the plaintext of a JSON Web Encryption (JWE) structure, enabling the claims to be digitally signed or integrity protected with a Message Authentication Code (MAC) and/or encrypted."@en ;
    sto:hasClassification sto:DataSovereignty,
        idsram:Security ;
    sto:hasOfficialResource <https://tools.ietf.org/html/rfc7519> ;
    sto:hasPublisher sto:IETF .

sto:RFC_7540 a owl:NamedIndividual,
        sto:Standard ;
    rdfs:label "HTTP/2"@en,
        "RFC 7540"@en ;
    rdfs:comment """This specification describes an optimized expression of the semantics of the Hypertext Transfer Protocol (HTTP), referred to as HTTP version 2 (HTTP/2).  HTTP/2 enables a more efficient use of network resources and a reduced perception of latency by introducing header field compression and allowing multiple concurrent exchanges on the same connection.  It also introduces unsolicited push of  representations from servers to clients.\r
\r
This specification is an alternative to, but does not obsolete, the HTTP/1.1 message syntax.  HTTP's existing semantics remain unchanged."""@en ;
    sto:hasClassification iira:FunctionalViewpoint,
        iira:TansportLayer,
        rami:Communication,
        idsram:Interoperability,
        idsram:SystemLayer ;
    sto:hasPublisher sto:IETF .

sto:RFC_768 a dbpcy:WikicatInternetProtocols,
        dbpcy:WikicatInternetStandards,
        dbpcy:WikicatTransportLayerProtocols,
        owl:NamedIndividual,
        owl:Thing,
        sto:Standard ;
    rdfs:label "RFC 768"@en ;
    dcterms:subject dbrc:Internet_Standards,
        dbrc:Internet_protocols,
        dbrc:Transport_layer_protocols ;
    dcterms:title "User Datagram Protocol (UDP)"@en ;
    lingg:hypernym dbres:Members ;
    rdfs:comment "In computer networking, the User Datagram Protocol (UDP) is one of the core members of the Internet protocol suite. The protocol was designed by David P. Reed in 1980 and formally defined in RFC 768. With UDP, computer applications can send messages, in this case referred to as datagrams, to other hosts on an Internet Protocol (IP) network. Prior communications are not required in order to set up communication channels or data paths."@en ;
    sto:hasClassification iira:TansportLayer ;
    sto:hasDBpediaResource dbres:User_Datagram_Protocol ;
    sto:hasOfficialResource <https://tools.ietf.org/html/rfc768> ;
    sto:hasPublisher sto:IETF ;
    sto:hasWikipediaArticle <https://en.wikipedia.org/wiki/User_Datagram_Protocol> .

sto:RFC_793 a owl:NamedIndividual,
        sto:Standard ;
    rdfs:label "RFC 793"@en ;
    dcterms:title "TRANSMISSION CONTROL PROTOCOL"@en ;
    rdfs:comment """This document describes the DoD Standard Transmission Control Protocol\r
(TCP).  There have been nine earlier editions of the ARPA TCP\r
specification on which this standard is based, and the present text\r
draws heavily from them.  There have been many contributors to this work\r
both in terms of concepts and in terms of text.  This edition clarifies\r
several details and removes the end-of-letter buffer-size adjustments,\r
and redescribes the letter mechanism as a push function."""@en ;
    sto:hasClassification iira:TansportLayer,
        idsram:SystemLayer ;
    sto:hasOfficialResource <https://tools.ietf.org/html/rfc793> ;
    sto:hasPublisher sto:IETF .

sto:SCOR a dbont:Person,
        owl:NamedIndividual,
        sto:Standard ;
    rdfs:label "SCOR"@en ;
    dcterms:subject dbrc:Business_models,
        dbrc:Supply_chain_management ;
    lingg:hypernym dbres:Model ;
    rdfs:comment "APICS Supply Chain Operations Reference."@en ;
    sto:hasClassification sto:SCM ;
    sto:hasDBpediaResource <http://dbpedia.org/page/Supply-chain_operations_reference> ;
    sto:hasDeveloper sto:APICS ;
    sto:hasOfficialResource <http://www.apics.org/apics-for-business/products-and-services/apics-scc-frameworks/scor> ;
    sto:hasTag "SCOR"@en ;
    sto:hasWikipediaArticle <https://en.wikipedia.org/wiki/Supply-chain_operations_reference> .

sto:SecureCommunication a owl:NamedIndividual,
        sto:ISO_42010_Concern .

sto:SysML a dbont:Language,
        owl:NamedIndividual,
        owl:Thing,
        sto:Standard ;
    rdfs:label "Systems Modeling Language"@en ;
    dcterms:subject dbrc:Systems_Modeling_Language,
        dbrc:Systems_engineering,
        dbrc:Unified_Modeling_Language ;
    lingg:hypernym dbres:Language ;
    rdfs:comment "The OMG Systems Modeling Language (OMG SysML) is a general-purpose graphical modeling language for specifying, analyzing, designing, and verifying complex systems that may include hardware, software, information, personnel, procedures, and facilities. In particular, the language provides graphical representations with a semantic foundation for modeling system requirements, behavior, structure, and parametrics, which is used to integrate with other engineering analysis models. It represents a subset of UML 2 with extensions needed to satisfy the requirements of the UML for Systems Engineering RFP as indicated in Figure 1. SysML leverages the OMG XML Metadata Interchange (XMI®) to exchange modeling data between tools, and is also intended to be compatible with the evolving ISO 10303-233 systems engineering data interchange standard."@en ;
    sto:hasDBpediaResource dbres:Systems_Modeling_Language ;
    sto:hasDeveloper sto:OMG ;
    sto:hasOfficialResource <http://sysml.org/>,
        <http://www.omgsysml.org/what-is-sysml.htm> ;
    sto:hasPublisher sto:OMG ;
    sto:hasTag "SysML"@en ;
    sto:hasWikipediaArticle <https://en.wikipedia.org/wiki/Systems_Modeling_Language> ;
    sto:relatedTo sto:IEC_62714 .

sto:TS-0009 a owl:NamedIndividual,
        sto:Standard ;
    rdfs:label "TS-0009"@en ;
    dcterms:title "HTTP Protocol Binding"@en ;
    rdfs:comment """The present document will cover the protocol specific part of communication protocol used by oneM2M compliant systems as RESTful HTTP binding.\r
The scope of the present document is (not limited to as shown below):\r
• Binding oneM2M Protocol primitive types to HTTP method.\r
• Binding oneM2M response status codes (successful/unsuccessful) to HTTP response codes.\r
• Binding oneM2M RESTful resources to HTTP resources.\r
The present document is depending on Core Protocol specification (oneM2M TS-0004) for data types."""@en ;
    sto:hasClassification sto:FrameworkLayer ;
    sto:hasOfficialResource "www.onem2m.org/images/files/deliverables/Release2A/TS-0009-HTTP_Protocol_Binding-v_2_13_1.pdf"^^xsd:anyURI ;
    sto:hasPublisher sto:oneM2M .

sto:VDMA_24582 a owl:NamedIndividual,
        sto:Standard ;
    rdfs:label "VDMA 24582"@en ;
    rdfs:comment "Fieldbus neutral reference architecture for Condition Monitoring in production automation"@en ;
    sto:hasClassification rami:ConditionMonitoring ;
    sto:hasOfficialResource <https://www.vdma.org/documents/105628/2244593/Inhalt+VDMA+24582_en.pdf/> ;
    sto:hasPublisher sto:VDMA ;
    sto:hasTag "Condition Monitoring"@en .

sto:W3C_RIF a dbpcy:WikicatKnowledgeRepresentationLanguages,
        dbpcy:WikicatQueryLanguages,
        dbpcy:WikicatWorldWideWebConsortiumStandards,
        dbont:ProgrammingLanguage,
        owl:NamedIndividual,
        sto:Standard ;
    rdfs:label "Rule Interchange Format"@en ;
    dcterms:hasLicense "Public"@en ;
    dcterms:subject dbrc:Knowledge_representation_languages,
        dbrc:Semantic_Web,
        dbrc:World_Wide_Web ;
    lingg:hypernym dbres:Recommendation ;
    rdfs:comment "The Rule Interchange Format (RIF) is a W3C Recommendation. RIF is part of the infrastructure for the semantic web, along with (principally) SPARQL, RDF and OWL. Although originally envisioned by many as a rules layer for the semantic web, in reality the design of RIF is based on the observation that there are many rules languages in existence, and what is needed is to exchange rules between them."@en ;
    sto:hasDBpediaResource dbres:Rule_Interchange_Format ;
    sto:hasOfficialResource <https://www.w3.org/TR/rif-overview/> ;
    sto:hasPublisher sto:W3C ;
    sto:hasTag "RIF"@en ;
    sto:hasWikipediaArticle <https://en.wikipedia.org/wiki/Rule_Interchange_Format> ;
    sto:relatedTo sto:W3C_OWL .

sto:W3C_SPARQL a dbpcy:WikicatComputerLanguages,
        dbpcy:WikicatDataModelingLanguages,
        dbpcy:WikicatQueryLanguages,
        dbpcy:WikicatWebServices,
        dbpcy:WikicatWorldWideWebConsortiumStandards,
        dbont:Language,
        dbont:ProgrammingLanguage,
        schema:Language,
        owl:NamedIndividual,
        owl:Thing,
        wike:Q315,
        wike:Q34770,
        wike:Q9143,
        sto:Standard ;
    rdfs:label "SPARQL"@en ;
    dcterms:hasLicense "Public"@en ;
    dcterms:subject dbrc:Data_modeling_languages,
        dbrc:Declarative_programming_languages,
        dbrc:Query_languages,
        dbrc:RDF_data_access,
        dbrc:Resource_Description_Framework,
        dbrc:Web_services,
        dbrc:World_Wide_Web_Consortium_standards ;
    lingg:hypernym dbres:Language ;
    rdfs:comment "The SPARQL Protocol and RDF Query Language (SPARQL) is a query language and protocol for RDF. This document specifies the SPARQL Protocol; it describes a means for conveying SPARQL queries and updates to a SPARQL processing service and returning the results via HTTP to the entity that requested them. This protocol was developed by the W3C SPARQL Working Group, part of the Semantic Web Activity as described in the activity statement ."@en ;
    sto:hasDBpediaResource dbres:SPARQL ;
    sto:hasOfficialResource <https://www.w3.org/SPARQL> ;
    sto:hasPublisher sto:W3C ;
    sto:hasTag "SPARQL"@en ;
    sto:hasWikipediaArticle <https://en.wikipedia.org/wiki/SPARQL> ;
    sto:relatedTo sto:W3C_RDF .

sto:Written a dcterms:linguisticSystem,
        owl:NamedIndividual ;
    rdfs:label "Written"@en ;
    rdfs:comment "Describes a Written Linguistic System"@en .

sto:abbreviation a owl:DatatypeProperty ;
    rdfs:label "has Abbreviated Name"@en ;
    rdfs:comment "Abbreviated  name of the thing."@en ;
    rdfs:domain owl:Thing ;
    rdfs:range rdf:PlainLiteral .

sto:alignesWith a owl:ObjectProperty,
        owl:SymmetricProperty ;
    rdfs:label "alignes With"@en ;
    rdfs:comment "indicates that some Standard Classification entity has a similar scope as another. This property most probably is symmetric but not transitive."@en ;
    rdfs:domain sto:StandardClassification ;
    rdfs:range sto:StandardClassification ;
    rdfs:subPropertyOf dul:associatedWith .

sto:belongsTo a owl:ObjectProperty ;
    rdfs:label "belongs To"@en ;
    rdfs:comment "A Standard Organization that belongs to the country"@en ;
    rdfs:domain sto:StandardOrganization ;
    rdfs:range dbo:Country .

sto:domainName a owl:DatatypeProperty ;
    rdfs:label "has Domain Name"@en ;
    rdfs:comment "Points the Standard with the name of the Industrial Domain"@en ;
    rdfs:domain sto:Domain ;
    rdfs:range rdf:PlainLiteral .

sto:ebXML a dbpcy:WikicatAbbreviations,
        dbpcy:WikicatComputerFileFormats,
        dbpcy:WikicatDataInterchangeStandards,
        dbpcy:WikicatDataModelingLanguages,
        dbpcy:WikicatMarkupLanguages,
        dbpcy:WikicatWebServices,
        dbpcy:WikicatWorldWideWebConsortiumStandards,
        dbpcy:WikicatXML-basedStandards,
        owl:NamedIndividual,
        sto:Standard ;
    rdfs:label "ebXML"@en ;
    dcterms:subject dbrc:Computer_file_formats,
        dbrc:Data_modeling_languages,
        dbrc:Technical_communication,
        dbrc:World_Wide_Web_Consortium_standards,
        dbrc:XML-based_standards,
        dbrc:XML_markup_languages ;
    lingg:hypernym dbres:Family ;
    rdfs:comment "Electronic Business using eXtensible Markup Language, commonly known as e-business XML, or ebXML is a family of XML based standards whose mission is to provide an open, XML-based infrastructure that enables the global use of electronic business information in an interoperable, secure, and consistent manner by all trading partners."@en ;
    sto:hasClassification sto:BusinessProcessExecution ;
    sto:hasDBpediaResource dbres:EbXML ;
    sto:hasOfficialResource <https://webstore.iec.ch/publication/24433> ;
    sto:hasPublisher sto:OASIS,
        sto:UN-CEFACT ;
    sto:hasTag "ebXML"@en ;
    sto:hasWikipediaArticle <https://en.wikipedia.org/wiki/EbXML> .

sto:edition a owl:AnnotationProperty .

sto:formationDate a owl:DatatypeProperty,
        owl:FunctionalProperty ;
    rdfs:label "has Formation Date"@en ;
    rdfs:comment "Formation date of the Organization"@en ;
    rdfs:domain sto:StandardOrganization ;
    rdfs:range xsd:date .

sto:hasAvailableLanguage a owl:ObjectProperty ;
    rdfs:label "has Available Language"@en,
        "hasAvailableLanguage"@en ;
    dcterms:creator sto:irlan ;
    rdfs:comment "Languages in which the document of the Standard is available, e.g., English, French, Spanish"@en,
        "Points to Languages in which the standard document is available, e.g., English, French, etc. Defined as subProperty of dcterms:language"@en ;
    rdfs:domain foaf:Document ;
    rdfs:subPropertyOf dcterms:language ;
    skos:note """dcterms:language  rdfs:range dcterms:LinguisticSystem.\r
                         """ .

sto:hasClassification a owl:ObjectProperty ;
    rdfs:label "has Classification"@en ;
    dcterms:creator sto:irlan ;
    rdfs:comment "An Standard is isCategorizedBy a given Categorization Area which is connected to a specific Standarization Initiative"@en ;
    rdfs:domain sto:Standard ;
    rdfs:range sto:StandardClassification .

sto:hasDBpediaResource a owl:DatatypeProperty ;
    rdfs:label "has DBpedia Resource"@en ;
    rdfs:comment "Instance's DBpedia Resource"@en ;
    rdfs:range xsd:anyURI .

sto:hasDeveloper a owl:ObjectProperty ;
    rdfs:label "has Developer"@en ;
    dcterms:creator sto:irlan ;
    rdfs:comment "The organization that developed this Standard"@en ;
    rdfs:domain sto:Publication ;
    rdfs:range sto:StandardOrganization ;
    rdfs:subPropertyOf foaf:maker .

sto:hasDomain a owl:ObjectProperty ;
    rdfs:label "has Domain"@en ;
    dcterms:creator sto:irlan ;
    rdfs:comment "Describes the domain, in which the Publication is used, particularly, standards."@en,
        "Points to the domain in which the standard is used"@en ;
    rdfs:domain sto:Publication ;
    rdfs:range sto:Domain .

sto:hasEdition a owl:DatatypeProperty ;
    rdfs:label "has Edition"@en ;
    rdfs:comment "Indicates the current Edition/Version number of the document."@en ;
    rdfs:domain foaf:Document ;
    rdfs:range xsd:float .

sto:hasFileSize a owl:ObjectProperty ;
    rdfs:label "has File Size"@en ;
    rdfs:comment "The size of document file in some unit, e.g., 104 Kilobyte."@en ;
    rdfs:domain foaf:Document ;
    rdfs:range om2:Measure ;
    rdfs:seeAlso <https://webstore.iec.ch/webstore/webstore.nsf/xpFAQ.xsp?Open&id=ADMN-7NALM5> ;
    skos:note """1. Reference for om2:Measure <http://www.ontology-of-units-of-measure.org/page/om-2/Measure>\r
                         2. om2:Measure om2:hasNumericalValue xsd:float;\r
                         3. om2:Measure om2:hasUnit om2:Unit;\r
                         4. om2:hasUnit om2:InformationCapacityUnit; is another possibility for range that could not be verified.\r
                         5. rdfs:seeAlso <http://www.ontology-of-units-of-measure.org/page/om-2/kilobyte> \r
                         6. Documentation on Measure <https://github.com/HajoRijgersberg/OM>""" .

sto:hasHeadquaterIn a owl:ObjectProperty ;
    rdfs:label "has Headquater In"@en ;
    dcterms:creator sto:irlan ;
    rdfs:comment "Denotes the countries in which the Headquarter of the organization who publishes the Standart"@en ;
    rdfs:domain sto:StandardOrganization ;
    rdfs:range dbo:Place .

sto:hasICS a owl:ObjectProperty ;
    rdfs:label "has ICS"@en ;
    rdfs:comment "Serves as a catalogue of International Classification For Standards"@en ;
    rdfs:domain sto:Publication ;
    rdfs:range sto:InternationalClassificationForStandards .

sto:hasImplementationFormat a owl:DatatypeProperty ;
    rdfs:label "has Implementation Format"@en ;
    rdfs:comment "Describes the name of the implementation or serialization format of the Publication, e.g., XML, Document, binary, batch"@en ;
    rdfs:domain sto:Publication ;
    rdfs:range rdfs:Literal .

sto:hasMotivation a owl:ObjectProperty ;
    rdfs:domain sto:Publication ;
    rdfs:range deo:Motivation .

sto:hasObjective a owl:DatatypeProperty ;
    rdfs:label "has Objective"@en ;
    rdfs:comment "Specifies the objectives for the different ISA 95 levels."@en ;
    rdfs:domain sto:ISA95Level ;
    rdfs:range xsd:string .

sto:hasOfficialResource a owl:DatatypeProperty ;
    rdfs:label "has Official Resource"@en ;
    rdfs:comment "Standard Official Website"@en ;
    rdfs:range xsd:anyURI .

sto:hasOntology a owl:DatatypeProperty ;
    rdfs:label "has Ontology"@en ;
    rdfs:comment "Point to the URL of a recognized Ontology representation of the Standard"@en ;
    rdfs:domain sto:Publication ;
    rdfs:range xsd:anyURI .

sto:hasPages a owl:DatatypeProperty ;
    rdfs:label "has Pages"@en ;
    rdfs:comment "Indicates the number of the pages in the document."@en ;
    rdfs:domain foaf:Document ;
    rdfs:range xsd:integer .

sto:hasPreviousVersion a owl:ObjectProperty ;
    rdfs:label "has Previous Version"@en ;
    rdfs:comment "Indicates the list of Standards that are previous versions of a Standard. For example,IEC 60038:2009 has IEC 60038:1983+AMD1:1994+AMD2:1997,IEC 60038:1983/AMD2:1997,IEC 60038:1983/AMD1:1994,IEC 60038:1983,IEC 60038:1975/AMD1:1977,IEC 60038:1975,IEC 60038:1967,IEC 60038:1954,IEC 60038:1938,IEC 60038:1927 as previous versions."@en ;
    rdfs:subPropertyOf sto:relatedTo .

sto:hasPublicationDate a owl:DatatypeProperty ;
    rdfs:label "has Publication Date"@en ;
    rdfs:comment "Publication date of the Publication"@en ;
    rdfs:domain sto:Publication ;
    rdfs:range xsd:date .

sto:hasPublisher a owl:ObjectProperty ;
    rdfs:label "has Publisher"@en ;
    dcterms:creator sto:irlan ;
    rdfs:comment "The organization that published this Standard"@en ;
    rdfs:domain sto:Publication ;
    rdfs:range sto:StandardOrganization ;
    rdfs:subPropertyOf foaf:maker .

sto:hasStabilityDate a owl:DatatypeProperty ;
    rdfs:label "has Stability Date"@en ;
    rdfs:comment "The contents of the publications will remain unchanged up to the Stability date. At this date, the publication will be either reconfirmed, withdrawn, replaced by a revised edition or amended. If there is a revision or amendment on-going then this is mentioned under the publication in the \"Work in progress\" tab, if you don't see this tab it means that there is no project under development."@en ;
    rdfs:domain sto:Publication ;
    rdfs:range xsd:gYear ;
    rdfs:seeAlso <https://webstore.iec.ch/webstore/webstore.nsf/xpFAQ.xsp?Open&id=ADMN-7NALM5> ;
    skos:note "The data specified is not actually a Date but an Year " .

sto:hasStatus a owl:DatatypeProperty ;
    rdfs:label "has Status"@en ;
    rdfs:comment "Publication status of the Standard, e.g., Valid, Revised, Published, under preparation, Released"@en ;
    rdfs:domain sto:Publication ;
    rdfs:range rdfs:Literal .

sto:hasTag a owl:DatatypeProperty,
        owl:ObjectProperty ;
    rdfs:label "has Tag"@en ;
    rdfs:comment "Points to the identification of the standards"@en ;
    rdfs:domain sto:Publication ;
    rdfs:range muto:Tag,
        rdfs:Literal .

sto:hasTask a owl:DatatypeProperty ;
    rdfs:label "has Task"@en ;
    rdfs:comment "Specifies the tasks for the different ISA 95 levels."@en ;
    rdfs:domain sto:ISA95Level ;
    rdfs:range xsd:string .

sto:hasTechnicalCommittee a owl:ObjectProperty ;
    rdfs:label "has Technical Committee"@en ;
    rdfs:comment "Specifies the Technical Committe or a Sub-Committee that is responsible for creation and maintenance of a standard"@en ;
    rdfs:domain sto:Publication ;
    rdfs:range sto:TechnicalCommittee .

sto:hasWikipediaArticle a owl:DatatypeProperty ;
    rdfs:label "has Wikipedia Article"@en ;
    rdfs:comment "Wikipedia Article about the Standard"@en ;
    rdfs:range xsd:anyURI .

sto:isImplementationOf a owl:ObjectProperty ;
    rdfs:label "is Implementation Of"@en ;
    rdfs:comment "Represent the relation that connects two standards when standard A is the implementation of standard B, e.g., B2MML isImplementationOf ISA-95."@en ;
    rdfs:subPropertyOf sto:relatedTo .

sto:norm a owl:AnnotationProperty .

sto:orgName a owl:DatatypeProperty ;
    rdfs:label "Org Name"@en ;
    rdfs:comment "Name of the Organization"@en ;
    rdfs:domain sto:StandardOrganization ;
    rdfs:range rdf:PlainLiteral .

sto:publisher a owl:AnnotationProperty .

sto:stoPartName a owl:DatatypeProperty ;
    rdfs:label "std Part Name"@en ;
    rdfs:comment "Name of the standard part."@en ;
    rdfs:domain sto:StandardPart ;
    rdfs:range xsd:string .

sto:useStructureOf a owl:ObjectProperty ;
    rdfs:label "use Structure Of"@en ;
    rdfs:comment "Standard A uses the structure of Standard B. For example, OPC UA uses Structure Of IEC_61804 (EDDL)"@en ;
    rdfs:subPropertyOf sto:relatedTo .

sto:uses a owl:ObjectProperty ;
    rdfs:label "uses"@en ;
    rdfs:comment "Defines that Standard A uses Standard B. For example, IEC_62714(AML) uses MathML."@en ;
    rdfs:subPropertyOf sto:relatedTo .

ids:TrustedConnector a owl:NamedIndividual,
        sto:StandardizationFramework ;
    rdfs:label "Trusted Connector"@en ;
    rdfs:comment "TODO: model IDS concepts correctly"@en ;
    sto:alignesWith sto:AdministrationShell ;
    sto:hasPublisher idsram:ReferenceArchitectureModel .

idsram:DataMarket a owl:NamedIndividual,
        sto:StandardClassification ;
    rdfs:label "IDS Data Market"@en ;
    sto:isDescribedin idsram:ReferenceArchitectureModel .

dbo:Country a owl:Class .

dbo:Place a owl:Class .

dbr:Beijing a owl:NamedIndividual .

dbr:Berlin a owl:NamedIndividual .

dbr:Boston a owl:NamedIndividual .

dbr:Chicago a owl:NamedIndividual .

dbr:China a owl:NamedIndividual .

dbr:Cologne a owl:NamedIndividual .

dbr:Eumseong a owl:NamedIndividual .

dbr:Frankfurt a owl:NamedIndividual .

dbr:Höhenkirchen-Siegertsbrunn a owl:NamedIndividual .

dbr:New_York_City a owl:NamedIndividual .

dbr:Paris a owl:NamedIndividual .

dbr:South_Korea a owl:NamedIndividual .

dbr:Switzerland a owl:NamedIndividual .

dbr:United_States a owl:NamedIndividual .

dbr:Valbonne a owl:NamedIndividual .

<http://dbpedia.org/resource#Washington,_D.C.> a owl:NamedIndividual .

dbr:_California a owl:NamedIndividual .

dbr:_Georgia a owl:NamedIndividual .

dbr:_Maryland a owl:NamedIndividual .

dbr:_Michigan a owl:NamedIndividual .

dbr:_New_York a owl:NamedIndividual .

dbr:_North_Carolina a owl:NamedIndividual .

dbr:_Texas a owl:NamedIndividual .

iira:ApplicationDomain a iira:FunctionalDomain,
        owl:NamedIndividual ;
    rdfs:label "IIRA Application Domain"@en ;
    dul:isPartOf iira:FunctionalViewpoint ;
    sto:alignesWith idsram:ProcessLayer ;
    sto:isDescribedin iira:IIRA .

iira:ControlDomain a iira:FunctionalDomain,
        owl:NamedIndividual ;
    rdfs:label "IIRA Control Domain"@en ;
    sto:alignesWith rami:Integration ;
    sto:isDescribedin iira:IIRA .

iira:LinkLayer a owl:NamedIndividual,
        sto:ConnectivityLayer ;
    rdfs:label "IICF Link Layer"@en .

iira:PhysicalLayer a owl:NamedIndividual,
        sto:ConnectivityLayer ;
    rdfs:label "IICF Physical Layer" ;
    sto:hasClassification iira:Connectivity .

dcterms:language a owl:ObjectProperty .

dcterms:linguisticSystem a owl:Class .

muto:Tag a owl:Class .

deo:Motivation a owl:Class .

<http://wikipedia.org/wiki/Common_Criteria_for_Information_Technology_Security_Evaluation> a owl:NamedIndividual .

<http://wikipedia.org/wiki/Institute_of_Electrical_and_Electronics_Engineers> a owl:NamedIndividual .

<http://www.ietf.org/> a owl:NamedIndividual .

dul:associatedWith a owl:ObjectProperty .

xsd:gYear a rdfs:Datatype .

foaf:Organization a owl:Class .

foaf:Person a owl:Class .

rami:CommunicationSubModel a owl:NamedIndividual .

rami:Communications a owl:NamedIndividual ;
    rdfs:label "RAMI Communication Layer"@en .

rami:ConditionMonitoring a owl:NamedIndividual .

rami:EnergyEfficiency a owl:NamedIndividual,
        rami:AdminShellSubmodel ;
    sto:isDescribedin sto:AdministrationShell .

rami:LifeCycle_Status a owl:NamedIndividual .

rami:Lifecycle_Status a owl:NamedIndividual .

rami:Other a owl:NamedIndividual .

rami:Work_Centers a owl:NamedIndividual .

sto: a dbont:Agent,
        dbont:Organisation,
        schema:Organization,
        om2:Measure,
        dul:Agent,
        dul:SocialPerson,
        owl:NamedIndividual,
        owl:Ontology,
        owl:Thing,
        wike:Q24229398,
        wike:Q43229,
        sto:Standard ;
    dcterms:created "2017-01-25"^^xsd:date ;
    dcterms:creator <http://data.semanticweb.org/person/steffen-lohmann>,
        <http://http://sda.cs.uni-bonn.de/people/irlan-grangel-gonzalez/>,
        <https://www.linkedin.com/in/paul-baptista-601177b2> ;
    dcterms:modified "2017-09-08"^^xsd:date ;
    dcterms:publisher <http://de.dbpedia.org/resource/Fraunhofer-Gesellschaft> ;
    dcterms:rights "This work is distributed under a Creative Commons Attribution License (http://creativecommons.org/licenses/by/3.0/)."@en ;
    dcterms:subject dbrc:International_Electrotechnical_Commission,
        dbrc:Standards_organizations ;
    dcterms:title "Standards Ontology"@en ;
    vann:preferredNamespacePrefix "sto" ;
    vann:preferredNamespaceUri "https://w3id.org/i40/sto#" ;
    doap:repository <https://github.com/i40-Tools/StandardsOntology> ;
    rdfs:comment "An ontology to describe standards related to Industry 4.0 and Smart Manufacturing"@en ;
    owl:versionInfo "0.3" ;
    sto:hasDBpediaResource <http://dbpedia.org/page/International_Electrotechnical_Vocabulary> ;
    sto:hasEdition "2.0"^^xsd:float,
        "7.0"^^xsd:float ;
    sto:hasFileSize sto: ;
    sto:hasICS sto:ICS_01_040_07 ;
    sto:hasImplementationFormat "Document"@en ;
    sto:hasOfficialResource <https://webstore.iec.ch/publication/153>,
        <https://webstore.iec.ch/publication/159> ;
    sto:hasPages "26"^^xsd:int,
        "129"^^xsd:int ;
    sto:hasPublicationDate "1998-04-30"^^xsd:date,
        "2009-06-17"^^xsd:date ;
    sto:hasPublisher sto:IEC ;
    sto:hasStabilityDate "2020-01-01"^^xsd:gYear ;
    sto:hasStatus "Valid"@en ;
    sto:hasTag "IEC 60038:2009"@en,
        "IEC 60050-101:1998"@en ;
    sto:hasTechnicalCommittee sto:TC_1,
        sto:TC_8 ;
    sto:hasWikipediaArticle <https://en.wikipedia.org/wiki/International_Electrotechnical_Vocabulary> .

sto:APICS a dbpcy:Abstraction100002137,
        dbpcy:Association108049401,
        dbpcy:Business108061042,
        dbpcy:Enterprise108056231,
        dbpcy:Group100031264,
        dbpcy:Organization108008335,
        dbpcy:ProfessionalAssociation108242675,
        dbpcy:SocialGroup107950920,
        dbpcy:WikicatBusinessOrganizations,
        dbpcy:WikicatNon-profitOrganizations,
        <http://dbpedia.org/class/yago/WikicatOrganizationsBasedInChicago,Illinois>,
        dbpcy:WikicatOrganizationsBasedInTheUnitedStates,
        dbpcy:WikicatOrganizationsEstablishedIn1957,
        dbpcy:WikicatProfessionalAssociations,
        dbpcy:WikicatProfessionalAssociationsBasedInTheUnitedStates,
        dbpcy:WikicatStandardsOrganizations,
        dbpcy:YagoLegalActor,
        dbpcy:YagoLegalActorGeo,
        dbpcy:YagoPermanentlyLocatedEntity,
        dbont:Agent,
        dbont:Company,
        dbont:Organisation,
        schema:Organization,
        dul:Agent,
        dul:SocialPerson,
        owl:NamedIndividual,
        owl:Thing,
        wike:Q24229398,
        wike:Q43229,
        sto:StandardOrganization ;
    rdfs:label "APICS"@en ;
    dcterms:subject <http://dbpedia.org/resource/Category:1957_establishments_in_Ohio>,
        dbrc:Business_and_finance_professional_associations,
        dbrc:Organizations_based_in_Chicago,
        dbrc:Organizations_established_in_1957,
        dbrc:Professional_associations_based_in_the_United_States,
        dbrc:Standards_organizations ;
    lingg:hypernym dbres:Organization ;
    rdfs:comment "American Production and Inventory Control Society."@en ;
    sto:formationDate "1957-01-01"^^xsd:date ;
    sto:hasDBpediaResource <http://dbpedia.org/page/APICS> ;
    sto:hasHeadquaterIn dbr:Chicago ;
    sto:hasOfficialResource <http://www.apics.org/apics> ;
    sto:hasWikipediaArticle <https://en.wikipedia.org/wiki/APICS> ;
    sto:orgName "American Production and Inventory Control Society"@en .

sto:ASAM a dbont:Agent,
        dbont:Organisation,
        schema:Organization,
        dul:Agent,
        dul:SocialPerson,
        owl:NamedIndividual,
        owl:Thing,
        wike:Q24229398,
        wike:Q43229,
        sto:StandardOrganization ;
    rdfs:label "ASAM" ;
    dcterms:subject dbrc:Automotive_standards,
        dbrc:Professional_associations_based_in_Germany ;
    lingg:hypernym dbres:Association ;
    rdfs:comment "Association for Standardization of Automation and Measuring Systems or ASAM is an incorporated association under German law. Its members are primarily international car manufacturers, suppliers and engineering service providers from the automotive industry. The association coordinates the development of technical standards, which are developed by working groups composed of experts from its member companies. ASAM pursues the vision that the tools of a development process chain can be freely interconnected and allow a seamless exchange of data. The standards define protocols, data models, file formats and application programming interfaces (APIs) for the use in the development and testing of automotive electronic control units. A large amount of popular tools in the areas of simulation, measurement, calibration and test automation are compliant to ASAM standards. Compliance shall guarantee interoperability of tools from different vendors, allow data exchange without the need for converters, and facilitate the exchange of unambiguous specification between customers and suppliers."@en ;
    sto:abbreviation "ASAM" ;
    sto:belongsTo dbr:Germany ;
    sto:formationDate "1998-12-01"^^xsd:date ;
    sto:hasDBpediaResource <http://dbpedia.org/page/Association_for_Standardisation_of_Automation_and_Measuring_Systems> ;
    sto:hasHeadquaterIn dbr:Höhenkirchen-Siegertsbrunn ;
    sto:hasOfficialResource <https://www.asam.net/> ;
    sto:hasWikipediaArticle <https://en.wikipedia.org/wiki/Association_for_Standardisation_of_Automation_and_Measuring_Systems> ;
    sto:orgName "Association for Standardization of Automation and Measuring Systems"@en .

sto:ASME a dbpcy:Abstraction100002137,
        dbpcy:Association108049401,
        dbpcy:Company108058098,
        dbpcy:Group100031264,
        dbpcy:Institution108053576,
        dbpcy:Organization108008335,
        dbpcy:ProfessionalAssociation108242675,
        dbpcy:SocialGroup107950920,
        dbpcy:WikicatEngineeringOrganizations,
        dbpcy:WikicatOrganizationsBasedInNewYork,
        dbpcy:WikicatOrganizationsBasedInNewYorkCity,
        dbpcy:WikicatOrganizationsBasedInTheUnitedStates,
        dbpcy:WikicatOrganizationsEstablishedIn1880,
        dbpcy:WikicatProfessionalAssociations,
        dbpcy:WikicatStandardsOrganizations,
        dbpcy:YagoLegalActor,
        dbpcy:YagoLegalActorGeo,
        dbpcy:YagoPermanentlyLocatedEntity,
        dbont:Agent,
        dbont:Organisation,
        schema:Organization,
        dul:Agent,
        dul:SocialPerson,
        owl:NamedIndividual,
        owl:Thing,
        wike:Q24229398,
        wike:Q43229,
        sto:StandardOrganization ;
    dcterms:subject <http://dbpedia.org/resource/Category:1880_establishments_in_New_York>,
        dbrc:American_Society_of_Mechanical_Engineers,
        dbrc:American_engineering_organizations,
        dbrc:American_mechanical_engineers,
        dbrc:Engineering_societies_based_in_the_United_States,
        dbrc:Historic_Mechanical_Engineering_Landmarks,
        dbrc:Mechanical_engineering_organizations,
        dbrc:Organizations_established_in_1880 ;
    lingg:hypernym dbres:Association ;
    rdfs:comment "The American Society of Mechanical Engineers (ASME) is a professional association that, promotes the art, science, and practice of multidisciplinary engineering and allied sciences around the globe via continuing education, training and professional development, codes and standards, research, conferences and publications, government relations, and other forms of outreach."@en ;
    sto:abbreviation "ASME" ;
    sto:formationDate "1880-01-01"^^xsd:date ;
    sto:hasDBpediaResource dbres:ASME ;
    sto:hasHeadquaterIn dbr:New_York_City ;
    sto:hasOfficialResource <https://www.asme.org/> ;
    sto:hasWikipediaArticle <https://en.wikipedia.org/wiki/ASME> ;
    sto:orgName "American Society of Mechanical Engineers"@en .

sto:Authentication a owl:NamedIndividual,
        sto:ISO_42010_Concern .

sto:BPMN a owl:NamedIndividual,
        sto:Standard ;
    rdfs:label "Business Process Model Notation"@en ;
    dcterms:subject dbrc:Business_process_modelling,
        dbrc:Diagrams,
        dbrc:ISO_standards,
        dbrc:Specification_languages,
        dbrc:Workflow_technology ;
    lingg:hypernym dbres:Representation ;
    rdfs:comment "Business Process Model and Notation is a graphical representation for specifying business processes in a business process model."@en ;
    sto:hasClassification sto:SCM ;
    sto:hasDBpediaResource <http://dbpedia.org/page/Business_Process_Model_and_Notation> ;
    sto:hasDeveloper sto:OMG ;
    sto:hasOfficialResource <http://www.bpmn.org/> ;
    sto:hasTag "BPMN"@en ;
    sto:hasWikipediaArticle <https://en.wikipedia.org/wiki/Business_Process_Model_and_Notation> .

sto:Certification a owl:NamedIndividual,
        sto:ISO_42010_Concern .

sto:Communication a owl:NamedIndividual,
        rami:AdminShellSubmodel ;
    sto:isDescribedin sto:AdministrationShell .

sto:DMSC a owl:NamedIndividual,
        sto:StandardOrganization ;
    rdfs:label "Dimensional Metrology Standards Consortium"@en ;
    rdfs:comment "Dimensional Metrology Standards Consortium (DMSC) is to identify urgently needed standards in the field of dimensional metrology, and to promote, foster, and encourage the development and interoperability of these standards, along with related and supporting standards that will benefit the industry as a whole."@en ;
    sto:hasHeadquaterIn dbr:_Texas ;
    sto:hasOfficialResource <http://www.dmis.org/> .

sto:DeviceLevel a owl:NamedIndividual,
        sto:ISA95Level ;
    rdfs:label "Device Level"@en ;
    rdfs:comment "Describes the device level according to the ISA95 level classification."@en .

sto:ENISA a owl:NamedIndividual,
        sto:StandardOrganization ;
    rdfs:label "ENISA"@en ;
    dcterms:title "European Union Agency for Network and Information Security"@en ;
    rdfs:comment "ENISA provides recommendations on cybersecurity, supports policy development and its implementation, and collaborates with operational teams throughout Europe."@en ;
    sto:hasOfficialResource <https://www.enisa.europa.eu/> .

sto:EnterpriseIntegration a owl:NamedIndividual .

sto:FileSizeIEC_60027_2006 a om2:Measure,
        owl:NamedIndividual ;
    rdfs:label "FileSize IEC 60027:2006"@en ;
    om2:hasNumericalValue "661.0"^^xsd:float ;
    om2:hasUnit om2:kilobyte ;
    rdfs:comment "Specifies the file size of the document for standard IEC 60027:2006"@en .

sto:FileSizeIEC_60038_2009 a om2:Measure,
        owl:NamedIndividual ;
    rdfs:label "FileSize IEC 60038:2009"@en ;
    om2:hasNumericalValue "946.0"^^xsd:float ;
    om2:hasUnit om2:kilobyte ;
    rdfs:comment "Specifies the file size of the document for standard IEC 60038:2009"@en .

sto:FileSizeIEC_60050_1984 a om2:Measure,
        owl:NamedIndividual ;
    rdfs:label "FileSize IEC 60050-371:1984"@en ;
    om2:hasNumericalValue "2485.0"^^xsd:float ;
    om2:hasUnit om2:kilobyte ;
    rdfs:comment "Specifies the file size of the document for standard IEC 60050-101:1998 "@en .

sto:FileSizeIEC_60050_1998 a om2:Measure,
        owl:NamedIndividual ;
    rdfs:label "FileSize IEC 60050-101:1998"@en ;
    om2:hasNumericalValue "1712.0"^^xsd:float ;
    om2:hasUnit om2:kilobyte ;
    rdfs:comment "Specifies the file size of the document for standard IEC 60050-101:1998 "@en .

sto:FileSizeIEC_60050_2013 a om2:Measure,
        owl:NamedIndividual ;
    rdfs:label "FileSize IEC 60050-351:2013"@en ;
    om2:hasNumericalValue "3999.0"^^xsd:float ;
    om2:hasUnit om2:kilobyte ;
    rdfs:comment "Specifies the file size of the document for standard IEC 60050-351:2013 "@en .

sto:FileSizeIEC_60073_2002 a om2:Measure,
        owl:NamedIndividual ;
    rdfs:label "FileSize IEC 60073:2002"@en ;
    om2:hasNumericalValue "525.0"^^xsd:float ;
    om2:hasUnit om2:kilobyte ;
    rdfs:comment "Specifies the file size of the document for standard IEC 60073:2002"@en .

sto:FileSizeIEC_60204_2000 a om2:Measure,
        owl:NamedIndividual ;
    rdfs:label "FileSize IEC 60204:2000"@en ;
    om2:hasNumericalValue "494.0"^^xsd:float ;
    om2:hasUnit om2:kilobyte ;
    rdfs:comment "Specifies the file size of the document for standard IEC 60204:2000"@en .

sto:FileSizeIEC_60255_149_2013 a om2:Measure,
        owl:NamedIndividual ;
    rdfs:label "FileSize 60255-149:2013"@en ;
    om2:hasNumericalValue "1722.0"^^xsd:float ;
    om2:hasUnit om2:kilobyte ;
    rdfs:comment "Specifies the file size of the document for standard IEC 60255-149:2013 "@en .

sto:FileSizeIEC_60255_151_2009 a om2:Measure,
        owl:NamedIndividual ;
    rdfs:label "FileSize IEC 60255-151:2009 "@en ;
    om2:hasNumericalValue "1341.0"^^xsd:float ;
    om2:hasUnit om2:kilobyte ;
    rdfs:comment "Specifies the file size of the document for standard IEC IEC 60255-151:2009"@en .

sto:FileSizeIEC_60255_2009 a om2:Measure,
        owl:NamedIndividual ;
    rdfs:label "FileSize IEC 60255-1:2009"@en ;
    om2:hasNumericalValue "1411.0"^^xsd:float ;
    om2:hasUnit om2:kilobyte ;
    rdfs:comment "Specifies the file size of the document for standard 60255-1:2009"@en .

sto:FileSizeIEC_60255_2010 a om2:Measure,
        owl:NamedIndividual ;
    rdfs:label "FileSize 60255-127:2010"@en ;
    om2:hasNumericalValue "1215.0"^^xsd:float ;
    om2:hasUnit om2:kilobyte ;
    rdfs:comment "Specifies the file size of the document for standard IEC 60255-127:2010 "@en .

sto:FileSizeIEC_60255_2013 a om2:Measure,
        owl:NamedIndividual ;
    rdfs:label "FileSize IEC 60255-27:2013"@en ;
    om2:hasNumericalValue "2520.0"^^xsd:float ;
    om2:hasUnit om2:kilobyte ;
    rdfs:comment "Specifies the file size of the document for standard IEC 60255-27:2013"@en .

sto:FileSizeIEC_60286_3_2013 a om2:Measure,
        owl:NamedIndividual ;
    rdfs:label "FileSize IEC 60286-3:2013  "@en ;
    om2:hasNumericalValue "1764.0"^^xsd:float ;
    om2:hasUnit om2:kilobyte ;
    rdfs:comment "Specifies the file size of the document for standard IEC IEC 60286-3:2013 "@en .

sto:FileSizeIEC_60286_4_2013 a om2:Measure,
        owl:NamedIndividual ;
    rdfs:label "FileSize IEC 60286-4:2013  "@en ;
    om2:hasNumericalValue "1129.0"^^xsd:float ;
    om2:hasUnit om2:kilobyte ;
    rdfs:comment "Specifies the file size of the document for standard IEC IEC 60286-4:2013 "@en .

sto:FileSizeIEC_60286_5_2018 a om2:Measure,
        owl:NamedIndividual ;
    rdfs:label "FileSize IEC 60286-5:2018  "@en ;
    om2:hasNumericalValue "3481.0"^^xsd:float ;
    om2:hasUnit om2:kilobyte ;
    rdfs:comment "Specifies the file size of the document for standard IEC IEC 60286-5:2018 "@en .

sto:FileSizeIEC_60381_1978 a om2:Measure,
        owl:NamedIndividual ;
    rdfs:label "FileSize IEC 60381-2:1978"@en ;
    om2:hasNumericalValue "483.0"^^xsd:float ;
    om2:hasUnit om2:kilobyte ;
    rdfs:comment "Specifies the file size of the document for standard IEC 60381-2:1978"@en .

sto:FileSizeIEC_60381_1982 a om2:Measure,
        owl:NamedIndividual ;
    rdfs:label "FileSize IEC 60381-1:1982"@en ;
    om2:hasNumericalValue "507.0"^^xsd:float ;
    om2:hasUnit om2:kilobyte ;
    rdfs:comment "Specifies the file size of the document for standard IEC 60381-1:1982 "@en .

sto:FileSizeIEC_60382 a om2:Measure,
        owl:NamedIndividual ;
    rdfs:label "FileSize IEC 60382:1991"@en ;
    om2:hasNumericalValue "557.0"^^xsd:float ;
    om2:hasUnit om2:kilobyte ;
    rdfs:comment "Specifies the file size of the document for standard  IEC 60382:1991."@en .

sto:FileSizeIEC_60382_1991 a om2:Measure,
        owl:NamedIndividual ;
    rdfs:label "FileSize IEC 60382:1991"@en ;
    om2:hasNumericalValue "557.0"^^xsd:float ;
    om2:hasUnit om2:kilobyte ;
    rdfs:comment "Specifies the file size of the document for standard IEC 60382:1991"@en .

sto:FileSizeIEC_60839_P7_1 a om2:Measure,
        owl:NamedIndividual ;
    rdfs:label "FileSize IEC 60839-7-1:2001"@en ;
    om2:hasNumericalValue "1137.0"^^xsd:float ;
    om2:hasUnit om2:kilobyte ;
    rdfs:comment "Specifies the file size of the document for standard IEC 60839-7-1:2001"@en .

sto:FileSizeIEC_60839_P7_2 a om2:Measure,
        owl:NamedIndividual ;
    rdfs:label "FileSize IEC 60839-7-2:2001"@en ;
    om2:hasNumericalValue "1047.0"^^xsd:float ;
    om2:hasUnit om2:kilobyte ;
    rdfs:comment "Specifies the file size of the document for standard IEC 60839-7-2:2001"@en .

sto:FileSizeIEC_60839_P7_3 a om2:Measure,
        owl:NamedIndividual ;
    rdfs:label "FileSize IEC 60839-7-3:2001"@en ;
    om2:hasNumericalValue "975.0"^^xsd:float ;
    om2:hasUnit om2:kilobyte ;
    rdfs:comment "Specifies the file size of the document for standard IEC 60839-7-3:2001"@en .

sto:FileSizeIEC_60839_P7_4 a om2:Measure,
        owl:NamedIndividual ;
    rdfs:label "FileSize IEC 60839-7-4:2001"@en ;
    om2:hasNumericalValue "967.0"^^xsd:float ;
    om2:hasUnit om2:kilobyte ;
    rdfs:comment "Specifies the file size of the document for standard IEC 60839-7-4:2001"@en .

sto:FileSizeIEC_60839_P7_5 a om2:Measure,
        owl:NamedIndividual ;
    rdfs:label "FileSize IEC 60839-7-5:2001"@en ;
    om2:hasNumericalValue "939.0"^^xsd:float ;
    om2:hasUnit om2:kilobyte ;
    rdfs:comment "Specifies the file size of the document for standard IEC 60839-7-5:2001"@en .

sto:FileSizeIEC_60839_P7_6 a om2:Measure,
        owl:NamedIndividual ;
    rdfs:label "FileSize IEC 60839-7-6:2001"@en ;
    om2:hasNumericalValue "926.0"^^xsd:float ;
    om2:hasUnit om2:kilobyte ;
    rdfs:comment "Specifies the file size of the document for standard IEC 60839-7-6:2001"@en .

sto:FileSizeIEC_60839_P7_7 a om2:Measure,
        owl:NamedIndividual ;
    rdfs:label "FileSize IEC 60839-7-7:2001"@en ;
    om2:hasNumericalValue "964.0"^^xsd:float ;
    om2:hasUnit om2:kilobyte ;
    rdfs:comment "Specifies the file size of the document for standard IEC 60839-7-7:2001"@en .

sto:FileSizeIEC_60848 a om2:Measure,
        owl:NamedIndividual ;
    rdfs:label "FileSize IEC 60848:2013"@en ;
    om2:hasNumericalValue "1784.0"^^xsd:float ;
    om2:hasUnit om2:kilobyte ;
    rdfs:comment "Specifies the file size of the document for standard IEC 60848:2013"@en .

sto:FileSizeIEC_60864_P1 a om2:Measure,
        owl:NamedIndividual ;
    rdfs:label "FileSizeIEC 60864-1:1986"@en ;
    om2:hasNumericalValue "1540.0"^^xsd:float ;
    om2:hasUnit om2:kilobyte ;
    rdfs:comment "Specifies the file size of the document for standard IEC 60864-1:1986 "@en .

sto:FileSizeIEC_60864_P2 a om2:Measure,
        owl:NamedIndividual ;
    rdfs:label "FileSize IEC 60864-2:1997"@en ;
    om2:hasNumericalValue "283.0"^^xsd:float ;
    om2:hasUnit om2:kilobyte ;
    rdfs:comment "Specifies the file size of the document for standard IEC 60864-2:1997"@en .

sto:FileSizeIEC_60870_1990_P5_S1 a om2:Measure,
        owl:NamedIndividual ;
    rdfs:label "FileSize IEC 60870-5-1:1990"@en ;
    om2:hasNumericalValue "2954.0"^^xsd:float ;
    om2:hasUnit om2:kilobyte ;
    rdfs:comment "Specifies the file size of the document for standard IEC 60870-5-1:1990"@en .

sto:FileSizeIEC_60870_1992_P5_S2 a om2:Measure,
        owl:NamedIndividual ;
    rdfs:label "FileSize IEC 60870-5-2:1992"@en ;
    om2:hasNumericalValue "3658.0"^^xsd:float ;
    om2:hasUnit om2:kilobyte ;
    rdfs:comment "Specifies the file size of the document for standard IEC 60870-5-2:1992"@en .

sto:FileSizeIEC_60870_1992_P5_S3 a om2:Measure,
        owl:NamedIndividual ;
    rdfs:label "FileSize IEC 60870-5-3:1992"@en ;
    om2:hasNumericalValue "1629.0"^^xsd:float ;
    om2:hasUnit om2:kilobyte ;
    rdfs:comment "Specifies the file size of the document for standard IEC 60870-5-3:1992"@en .

sto:FileSizeIEC_60870_1995_P2_S1 a om2:Measure,
        owl:NamedIndividual ;
    rdfs:label "FileSize IEC 60870-2-1:1995"@en ;
    om2:hasNumericalValue "1674.0"^^xsd:float ;
    om2:hasUnit om2:kilobyte ;
    rdfs:comment "Specifies the file size of the document for standard IEC 60870-2-1:1995"@en .

sto:FileSizeIEC_60870_1996_P2_S2 a owl:NamedIndividual .

sto:FileSizeIEC_60870_P5_S101_2003 a om2:Measure,
        owl:NamedIndividual ;
    rdfs:label "FileSize IEC 60870-5-101:2003"@en ;
    om2:hasNumericalValue "2651.0"^^xsd:float ;
    om2:hasUnit om2:kilobyte ;
    rdfs:comment "Specifies the file size of the document for standard IEC 60870-5-101:2003"@en .

sto:FileSizeIEC_60870_P5_S102_1996 a om2:Measure,
        owl:NamedIndividual ;
    rdfs:label "FileSize IEC 60870-5-102:1996"@en ;
    om2:hasNumericalValue "505.0"^^xsd:float ;
    om2:hasUnit om2:kilobyte ;
    rdfs:comment "Specifies the file size of the document for standard IEC 60870-5-102:1996"@en .

sto:FileSizeIEC_60870_P5_S103_1997 a om2:Measure,
        owl:NamedIndividual ;
    rdfs:label "FileSize IEC 60870-5-103:1997"@en ;
    om2:hasNumericalValue "964.0"^^xsd:float ;
    om2:hasUnit om2:kilobyte ;
    rdfs:comment "Specifies the file size of the document for standard IEC 60870-5-103:1997"@en .

sto:FileSizeIEC_60870_P5_S104_2016 a om2:Measure,
        owl:NamedIndividual ;
    rdfs:label "FileSize IEC 60870-5-104:2006"@en ;
    om2:hasNumericalValue "2994.0"^^xsd:float ;
    om2:hasUnit om2:kilobyte ;
    rdfs:comment "Specifies the file size of the document for standard IEC 60870-5-104:2006"@en .

sto:FileSizeIEC_60870_P5_S4_1993 a om2:Measure,
        owl:NamedIndividual ;
    rdfs:label "FileSize IEC 60870-5-4:1993"@en ;
    om2:hasNumericalValue "1776.0"^^xsd:float ;
    om2:hasUnit om2:kilobyte ;
    rdfs:comment "Specifies the file size of the document for standard IEC 60870-5-4:1993"@en .

sto:FileSizeIEC_60870_P5_S5_1995 a om2:Measure,
        owl:NamedIndividual ;
    rdfs:label "FileSize IEC 60870-5-5:1995"@en ;
    om2:hasNumericalValue "3347.0"^^xsd:float ;
    om2:hasUnit om2:kilobyte ;
    rdfs:comment "Specifies the file size of the document for standard IEC 60870-5-5:1995"@en .

sto:FileSizeIEC_60870_P5_S6_2006 a om2:Measure,
        owl:NamedIndividual ;
    rdfs:label "FileSize IEC 60870-5-6:2006"@en ;
    om2:hasNumericalValue "1342.0"^^xsd:float ;
    om2:hasUnit om2:kilobyte ;
    rdfs:comment "Specifies the file size of the document for standard IEC 60870-5-6::2006."@en .

sto:FileSizeIEC_60870_P6_S2_1995 a om2:Measure,
        owl:NamedIndividual ;
    rdfs:label "FileSize IEC 60870-6-2:1995"@en ;
    om2:hasNumericalValue "3524.0"^^xsd:float ;
    om2:hasUnit om2:kilobyte ;
    rdfs:comment "Specifies the file size of the document for standard IEC 60870-6-2:1995"@en .

sto:FileSizeIEC_60870_P6_S501_1995 a om2:Measure,
        owl:NamedIndividual ;
    rdfs:label "FileSize IEC 60870-6-501:1995"@en ;
    om2:hasNumericalValue "578.0"^^xsd:float ;
    om2:hasUnit om2:kilobyte ;
    rdfs:comment "Specifies the file size of the document for standard IEC 60870-6-501:1995"@en .

sto:FileSizeIEC_60870_P6_S502_1995 a om2:Measure,
        owl:NamedIndividual ;
    rdfs:label "FileSize IEC 60870-6-502:1995"@en ;
    om2:hasNumericalValue "1963.0"^^xsd:float ;
    om2:hasUnit om2:kilobyte ;
    rdfs:comment "Specifies the file size of the document for standard IEC 60870-6-502:1995"@en .

sto:FileSizeIEC_60870_P6_S503_2014 a om2:Measure,
        owl:NamedIndividual ;
    rdfs:label "FileSize IEC 60870-6-503:2014"@en ;
    om2:hasNumericalValue "2630.0"^^xsd:float ;
    om2:hasUnit om2:kilobyte ;
    rdfs:comment "Specifies the file size of the document for standard IEC 60870-6-503:2014"@en .

sto:FileSizeIEC_60870_P6_S601_1994 a om2:Measure,
        owl:NamedIndividual ;
    rdfs:label "FileSize IEC 60870-6-601:1994"@en ;
    om2:hasNumericalValue "1112.0"^^xsd:float ;
    om2:hasUnit om2:kilobyte ;
    rdfs:comment "Specifies the file size of the document for standard IEC 60870-6-601:1994"@en .

sto:FileSizeIEC_60870_P6_S701_1998 a om2:Measure,
        owl:NamedIndividual ;
    rdfs:label "FileSize IEC 60870-6-701:1998"@en ;
    om2:hasNumericalValue "130.0"^^xsd:float ;
    om2:hasUnit om2:kilobyte ;
    rdfs:comment "Specifies the file size of the document for standard IEC 60870-6-701:1998"@en .

sto:FileSizeIEC_60870_P6_S702_2014 a om2:Measure,
        owl:NamedIndividual ;
    rdfs:label "FileSize IEC 60870-6-702:2014"@en ;
    om2:hasNumericalValue "1374.0"^^xsd:float ;
    om2:hasUnit om2:kilobyte ;
    rdfs:comment "Specifies the file size of the document for standard IEC 60870-6-702:2014"@en .

sto:FileSizeIEC_60870_P6_S802_2014 a om2:Measure,
        owl:NamedIndividual ;
    rdfs:label "FileSize IEC 60870-6-802:2014"@en ;
    om2:hasNumericalValue "1678.0"^^xsd:float ;
    om2:hasUnit om2:kilobyte ;
    rdfs:comment "Specifies the file size of the document for standard IEC 60870-6-802:2014"@en .

sto:FileSizeIEC_60946 a om2:Measure,
        owl:NamedIndividual ;
    rdfs:label "FileSize IEC 60946"@en ;
    om2:hasNumericalValue "546.0"^^xsd:float ;
    om2:hasUnit om2:kilobyte ;
    rdfs:comment "Specifies the file size of the document for standard IEC 60946"@en .

sto:FileSizeIEC_61000_P6_S2_2016 a om2:Measure,
        owl:NamedIndividual ;
    rdfs:label "FileSize IEC 61000-6-2:2016"@en ;
    om2:hasNumericalValue "2028.0"^^xsd:float ;
    om2:hasUnit om2:kilobyte ;
    rdfs:comment "Specifies the file size of the document for standard IEC 61000-6-2:2016."@en .

sto:FileSizeIEC_61010_P2_S012_2016 a om2:Measure,
        owl:NamedIndividual ;
    rdfs:label "FileSize IEC 61010-2-012:2016"@en ;
    om2:hasNumericalValue "2717.0"^^xsd:float ;
    om2:hasUnit om2:kilobyte ;
    rdfs:comment "Specifies the file size of the document for standard IEC 61010-2-012:2016."@en .

sto:FileSizeIEC_61010_P2_S201_2017 a om2:Measure,
        owl:NamedIndividual ;
    rdfs:label "FileSize IEC 61010-2-201:2017"@en ;
    om2:hasNumericalValue "5743.0"^^xsd:float ;
    om2:hasUnit om2:kilobyte ;
    rdfs:comment "Specifies the file size of the document for standard IEC 61010-2-201:2017."@en .

sto:FileSizeIEC_61010_P2_S202_2016 a om2:Measure,
        owl:NamedIndividual ;
    rdfs:label "FileSize IEC 61010-2-202:2016"@en ;
    om2:hasNumericalValue "1027.0"^^xsd:float ;
    om2:hasUnit om2:kilobyte ;
    rdfs:comment "Specifies the file size of the document for standard IEC 61010-2-202:2016."@en .

sto:FileSizeIEC_61160 a om2:Measure,
        owl:NamedIndividual ;
    rdfs:label "FileSize IEC 61160:2005"@en ;
    om2:hasNumericalValue "69.0"^^xsd:float ;
    om2:hasUnit om2:kilobyte ;
    rdfs:comment "Specifies the file size of the document for standard  IEC 61160:2005."@en .

sto:FileSizeIEC_61310_P1 a om2:Measure,
        owl:NamedIndividual ;
    rdfs:label "FileSize IEC 61310-1:2007"@en ;
    om2:hasNumericalValue "763.0"^^xsd:float ;
    om2:hasUnit om2:kilobyte ;
    rdfs:comment "Specifies the file size of the document for standard IEC 61310-1:2007."@en .

sto:FileSizeIEC_61310_P2 a om2:Measure,
        owl:NamedIndividual ;
    rdfs:label "FileSize IEC 61310-2:2007"@en ;
    om2:hasNumericalValue "724.0"^^xsd:float ;
    om2:hasUnit om2:kilobyte ;
    rdfs:comment "Specifies the file size of the document for standard IEC 61310-2:2007."@en .

sto:FileSizeIEC_61310_P3 a om2:Measure,
        owl:NamedIndividual ;
    rdfs:label "FileSize IEC 61310-3:2007"@en ;
    om2:hasNumericalValue "716.0"^^xsd:float ;
    om2:hasUnit om2:kilobyte ;
    rdfs:comment "Specifies the file size of the document for standard IEC 61310-3:2007."@en .

sto:FileSizeIEC_61334_1996_P3_S1 a owl:NamedIndividual .

sto:FileSizeIEC_61334_1996_P3_S22 a om2:Measure,
        owl:NamedIndividual ;
    rdfs:label "FileSize IEC 61334-4-1:1996"@en ;
    om2:hasNumericalValue "165.0"^^xsd:float ;
    om2:hasUnit om2:kilobyte ;
    rdfs:comment "Specifies the file size of the document for standard IEC 61334-3-22:2001"@en .

sto:FileSizeIEC_61334_1996_P4_S1 a om2:Measure,
        owl:NamedIndividual ;
    rdfs:label "FileSize IEC 61334-3-22:2000"@en ;
    om2:hasNumericalValue "1707.0"^^xsd:float ;
    om2:hasUnit om2:kilobyte ;
    rdfs:comment "Specifies the file size of the document for standard IEC 61334-4-1:1996"@en .

sto:FileSizeIEC_61334_1996_P4_S32 a om2:Measure,
        owl:NamedIndividual ;
    rdfs:label "FileSize IEC 61334-4-32:1996 "@en ;
    om2:hasNumericalValue "869.0"^^xsd:float ;
    om2:hasUnit om2:kilobyte ;
    rdfs:comment "Specifies the file size of the document for standard IEC 61334-4-32:1996 "@en .

sto:FileSizeIEC_61334_1996_P4_S41 a om2:Measure,
        owl:NamedIndividual ;
    rdfs:label "FileSize IEC 61334-4-41:1996"@en ;
    om2:hasNumericalValue "834.0"^^xsd:float ;
    om2:hasUnit om2:kilobyte ;
    rdfs:comment "Specifies the file size of the document for standard IEC 61334-4-41:1996"@en .

sto:FileSizeIEC_61334_1996_P4_S42 a om2:Measure,
        owl:NamedIndividual ;
    rdfs:label "FileSize IEC 61334-4-42:1996"@en ;
    om2:hasNumericalValue "305.0"^^xsd:float ;
    om2:hasUnit om2:kilobyte ;
    rdfs:comment "Specifies the file size of the document for standard IEC 61334-4-42:1996"@en .

sto:FileSizeIEC_61334_1998_P3_S1 a om2:Measure,
        owl:NamedIndividual ;
    rdfs:label "FileSize IEC 61334-3-1:1998 "@en ;
    om2:hasNumericalValue "147.0"^^xsd:float ;
    om2:hasUnit om2:kilobyte ;
    rdfs:comment "Specifies the file size of the document for standard IEC 61334-3-1:1998 "@en .

sto:FileSizeIEC_61334_1998_P4_S3 a om2:Measure,
        owl:NamedIndividual ;
    rdfs:label "FileSize IEC 61334-4-33:1998"@en ;
    om2:hasNumericalValue "135.0"^^xsd:float ;
    om2:hasUnit om2:kilobyte ;
    rdfs:comment "Specifies the file size of the document for standard IEC 61334-4-33:1998 "@en .

sto:FileSizeIEC_61334_1998_P4_S61 a om2:Measure,
        owl:NamedIndividual ;
    rdfs:label "FileSize IEC 61334-4-61:1998"@en ;
    om2:hasNumericalValue "753.0"^^xsd:float ;
    om2:hasUnit om2:kilobyte ;
    rdfs:comment "Specifies the file size of the document for standard IEC 61334-4-61:1998"@en .

sto:FileSizeIEC_61334_2000_P4_S511 a om2:Measure,
        owl:NamedIndividual ;
    rdfs:label "FileSize IEC 61334-4-511:2000"@en ;
    om2:hasNumericalValue "203.0"^^xsd:float ;
    om2:hasUnit om2:kilobyte ;
    rdfs:comment "Specifies the file size of the document for standard IEC 61334-4-511:2000"@en .

sto:FileSizeIEC_61334_2000_P6 a om2:Measure,
        owl:NamedIndividual ;
    rdfs:label "FileSize IEC 61334-6:2000"@en ;
    om2:hasNumericalValue "294.0"^^xsd:float ;
    om2:hasUnit om2:kilobyte ;
    rdfs:comment "Specifies the file size of the document for standard IEC 61334-6:2000"@en .

sto:FileSizeIEC_61334_2001_P4_S512 a om2:Measure,
        owl:NamedIndividual ;
    rdfs:label "FileSize IEC 61334-4-512:2001"@en ;
    om2:hasNumericalValue "459.0"^^xsd:float ;
    om2:hasUnit om2:kilobyte ;
    rdfs:comment "Specifies the file size of the document for standard IEC 61334-4-512:2001"@en .

sto:FileSizeIEC_61334_2001_P5_S1 a om2:Measure,
        owl:NamedIndividual ;
    rdfs:label "FileSize IEC 61334-5-1:2001"@en ;
    om2:hasNumericalValue "723.0"^^xsd:float ;
    om2:hasUnit om2:kilobyte ;
    rdfs:comment "Specifies the file size of the document for standard IEC 61334-5-1:2001"@en .

sto:FileSizeIEC_61400_P25_1 a om2:Measure,
        owl:NamedIndividual ;
    rdfs:label "FileSize IEC 61400-25-1:2017"@en ;
    om2:hasNumericalValue "3644.0"^^xsd:float ;
    om2:hasUnit om2:kilobyte ;
    rdfs:comment "Specifies the file size of the document for standard  IEC 61400-25-1:2017."@en .

sto:FileSizeIEC_61400_P25_2 a om2:Measure,
        owl:NamedIndividual ;
    rdfs:label "FileSize IEC 61400-25-2:2015"@en ;
    om2:hasNumericalValue "3707.0"^^xsd:float ;
    om2:hasUnit om2:kilobyte ;
    rdfs:comment "Specifies the file size of the document for standard IEC 61400-25-2:2015."@en .

sto:FileSizeIEC_61400_P25_3 a om2:Measure,
        owl:NamedIndividual ;
    rdfs:label "FileSize IEC 61400-25-3:2015"@en ;
    om2:hasNumericalValue "2027.0"^^xsd:float ;
    om2:hasUnit om2:kilobyte ;
    rdfs:comment "Specifies the file size of the document for standard IEC 61400-25-3:2015."@en .

sto:FileSizeIEC_61400_P25_4 a om2:Measure,
        owl:NamedIndividual ;
    rdfs:label "FileSize IEC 61400-25-4:2016"@en ;
    om2:hasNumericalValue "7800.0"^^xsd:float ;
    om2:hasUnit om2:kilobyte ;
    rdfs:comment "Specifies the file size of the document for standard IEC 61400-25-4:2016."@en .

sto:FileSizeIEC_61400_P25_5 a om2:Measure,
        owl:NamedIndividual ;
    rdfs:label "FileSize IEC 61400-25-5:2017"@en ;
    om2:hasNumericalValue "1567.0"^^xsd:float ;
    om2:hasUnit om2:kilobyte ;
    rdfs:comment "Specifies the file size of the document for standard IEC 61400-25-5:2017."@en .

sto:FileSizeIEC_61400_P25_6 a om2:Measure,
        owl:NamedIndividual ;
    rdfs:label "FileSize IEC 61400-25-5:2017"@en ;
    om2:hasNumericalValue "1673.0"^^xsd:float ;
    om2:hasUnit om2:kilobyte ;
    rdfs:comment "Specifies the file size of the document for standard IEC 61400-25-5:2017."@en .

sto:FileSizeIEC_61506 a om2:Measure,
        owl:NamedIndividual ;
    rdfs:label "FileSize IEC 61506:1997"@en ;
    om2:hasNumericalValue "294.0"^^xsd:float ;
    om2:hasUnit om2:kilobyte ;
    rdfs:comment "Specifies the file size of the document for standard  IEC 61506:1997."@en .

sto:FileSizeIEC_61690_P1_2000 a om2:Measure,
        owl:NamedIndividual ;
    rdfs:label "FileSize IEC 61690-1:2000 "@en ;
    om2:hasNumericalValue "1676.0"^^xsd:float ;
    om2:hasUnit om2:kilobyte ;
    rdfs:comment "Specifies the file size of the document for standard IEC 61690-1:2000 ."@en .

sto:FileSizeIEC_61690_P2_2000 a om2:Measure,
        owl:NamedIndividual ;
    rdfs:label "FileSize IEC 61690-2:2000 "@en ;
    om2:hasNumericalValue "6700.0"^^xsd:float ;
    om2:hasUnit om2:kilobyte ;
    rdfs:comment "Specifies the file size of the document for standard IEC 61690-2:2000 ."@en .

sto:FileSizeIEC_61691_P6 a om2:Measure,
        owl:NamedIndividual ;
    rdfs:label "FileSize IEC 61691-6:2009"@en ;
    om2:hasNumericalValue "5004.0"^^xsd:float ;
    om2:hasUnit om2:kilobyte ;
    rdfs:comment "Specifies the file size of the document for standard IEC 61691-6:2009."@en .

sto:FileSizeIEC_61810_P2 a om2:Measure,
        owl:NamedIndividual ;
    rdfs:label "FileSize IEC 61810-2:2017"@en ;
    om2:hasNumericalValue "4364.0"^^xsd:float ;
    om2:hasUnit om2:kilobyte ;
    rdfs:comment "Specifies the file size of the document for standard IEC 61810-2:2017."@en .

sto:FileSizeIEC_61810_P7 a om2:Measure,
        owl:NamedIndividual ;
    rdfs:label "FileSize IEC 61810-7:2006"@en ;
    om2:hasNumericalValue "2204.0"^^xsd:float ;
    om2:hasUnit om2:kilobyte ;
    rdfs:comment "Specifies the file size of the document for standard IEC 61810-7:2006."@en .

sto:FileSizeIEC_62832 a om2:Measure,
        owl:NamedIndividual ;
    om2:hasNumericalValue "2722.0"^^xsd:float ;
    om2:hasUnit om2:kilobyte .

sto:FunctionalSafety a owl:NamedIndividual,
        sto:Domain ;
    rdfs:label "Functional Safety"@en ;
    rdfs:comment "Functional Safety"@en .

sto:GPLv2 a dcterms:LicenseDocument,
        owl:NamedIndividual ;
    rdfs:label "GNU General Public License"@en ;
    rdfs:comment "Published under Open Content License."@en ;
    rdfs:seeAlso <https://opcfoundation.org/license/gpl.htm> ;
    skos:prefLabel "OCL 1.0" .

sto:IBM a dbpcy:Abstraction100002137,
        dbpcy:Company108058098,
        dbpcy:ElectronicsCompany108003035,
        dbpcy:Group100031264,
        dbpcy:Institution108053576,
        dbpcy:Organization108008335,
        dbpcy:SocialGroup107950920,
        dbpcy:WikicatCompaniesBasedInNewYork,
        <http://dbpedia.org/class/yago/WikicatCompaniesBasedInWestchesterCounty,NewYork>,
        dbpcy:WikicatCompaniesEstablishedIn1896,
        dbpcy:WikicatCompaniesEstablishedIn1911,
        dbpcy:WikicatCompaniesInTheDowJonesIndustrialAverage,
        dbpcy:WikicatCompaniesListedOnNASDAQ,
        dbpcy:WikicatCompaniesListedOnTheNewYorkStockExchange,
        dbpcy:WikicatComputerCompaniesOfTheUnitedStates,
        dbpcy:WikicatComputerHardwareCompanies,
        dbpcy:WikicatComputerStorageCompanies,
        dbpcy:WikicatDisplayTechnologyCompanies,
        dbpcy:WikicatElectronicsCompaniesOfTheUnitedStates,
        dbpcy:WikicatFoundrySemiconductorCompanies,
        dbpcy:WikicatMultinationalCompanies,
        dbpcy:WikicatMultinationalCompaniesHeadquarteredInTheUnitedStates,
        dbpcy:WikicatOutsourcingCompanies,
        dbpcy:WikicatPubliclyTradedCompaniesOfTheUnitedStates,
        dbpcy:WikicatSemiconductorCompanies,
        dbpcy:WikicatSoftwareCompanies,
        dbpcy:WikicatSoftwareCompaniesBasedInNewYork,
        dbpcy:WikicatSoftwareCompaniesOfTheUnitedStates,
        dbpcy:YagoLegalActor,
        dbpcy:YagoLegalActorGeo,
        dbpcy:YagoPermanentlyLocatedEntity,
        dbont:Agent,
        dbont:Company,
        dbont:Organisation,
        schema:Organization,
        <http://umbel.org/umbel/rc/Business>,
        <http://umbel.org/umbel/rc/Organization>,
        dul:Agent,
        dul:SocialPerson,
        owl:NamedIndividual,
        owl:Thing,
        wike:Q24229398,
        wike:Q43229,
        sto:StandardOrganization ;
    dcterms:subject <http://dbpedia.org/resource/Category:1896_establishments_in_the_United_States>,
        <http://dbpedia.org/resource/Category:1911_establishments_in_New_York>,
        dbrc:American_brands,
        dbrc:Cloud_computing_providers,
        dbrc:Collier_Trophy_recipients,
        <http://dbpedia.org/resource/Category:Companies_based_in_Westchester_County,_New_York>,
        dbrc:Companies_established_in_1896,
        dbrc:Companies_in_the_Dow_Jones_Industrial_Average,
        dbrc:Companies_listed_on_the_New_York_Stock_Exchange,
        dbrc:Computer_companies_of_the_United_States,
        dbrc:Computer_hardware_companies,
        dbrc:Computer_storage_companies,
        dbrc:Display_technology_companies,
        dbrc:Electronics_companies_of_the_United_States,
        dbrc:Foundry_semiconductor_companies,
        dbrc:IBM,
        dbrc:Multinational_companies_headquartered_in_the_United_States,
        dbrc:National_Medal_of_Technology_recipients,
        dbrc:Outsourcing_companies,
        dbrc:Point_of_sale_companies,
        dbrc:Semiconductor_companies,
        dbrc:Software_companies_based_in_New_York,
        dbrc:Storage_Area_Network_companies,
        dbrc:Technology_companies_established_in_1911 ;
    lingg:hypernym dbres:Technology ;
    rdfs:comment "International Business Machines Corporation (commonly referred to as IBM) is an American multinational technology and consulting corporation, with corporate headquarters in Armonk, New York. IBM manufactures and markets computer hardware, middleware and software, and offers infrastructure, hosting and consulting services in areas ranging from mainframe computers to nanotechnology.On August 6, 2015, IBM announced that it will buy Merge Healthcare Inc for $1 billion." ;
    sto:abbreviation "IBM" ;
    sto:formationDate "1911-06-16"^^xsd:date ;
    sto:hasDBpediaResource dbres:IBM ;
    sto:hasHeadquaterIn dbr:_New_York ;
    sto:hasOfficialResource <http://www.ibm.com> ;
    sto:hasWikipediaArticle <https://en.wikipedia.org/wiki/IBM> ;
    sto:orgName "International Business Machines Corporation"@en .

sto:ICS_01_040_35 a owl:NamedIndividual,
        sto:InternationalClassificationForStandards ;
    rdfs:label "ICS 01.040.35"@en ;
    dcterms:title " Information technology. Office machines (Vocabularies)"@en ;
    rdfs:comment "This is ICS for  Information technology. Office machines (Vocabularies)"@en .

sto:ICS_01_060 a owl:NamedIndividual,
        sto:InternationalClassificationForStandards ;
    rdfs:label "ICS 01.060"@en ;
    dcterms:title "Quantities and units "@en ;
    rdfs:comment "This is ICS for Quantities and units"@en .

sto:ICS_01_070 a owl:NamedIndividual,
        sto:InternationalClassificationForStandards ;
    rdfs:label "ICS 01.070"@en ;
    dcterms:title "Colour coding  "@en ;
    rdfs:comment "This is ICS for Colour coding "@en .

sto:ICS_03_100_40 a owl:NamedIndividual,
        sto:InternationalClassificationForStandards ;
    rdfs:label "ICS 03.100.40"@en ;
    dcterms:title "Research and development"@en ;
    rdfs:comment "This is ICS for “Research and development  ”"@en .

sto:ICS_03_120_01 a owl:NamedIndividual,
        sto:InternationalClassificationForStandards ;
    rdfs:label "ICS 03.120.01"@en ;
    dcterms:title "Quality in general "@en ;
    rdfs:comment "This is ICS for “Quality in general  ”"@en .

sto:ICS_19_08 a owl:NamedIndividual,
        sto:InternationalClassificationForStandards ;
    rdfs:label "ICS 19.08"@en ;
    dcterms:title "Electrical and electronic testing"@en ;
    rdfs:comment "This is ICS for “Electrical and electronic testing”"@en .

sto:ICS_33_040_40 a owl:NamedIndividual,
        sto:InternationalClassificationForStandards ;
    rdfs:label "ICS 33.040.40"@en ;
    dcterms:title "Data communication networks "@en ;
    rdfs:comment "This is ICS for “Data communication networks”"@en .

sto:ICS_33_100_10 a owl:NamedIndividual,
        sto:InternationalClassificationForStandards ;
    rdfs:label "ICS 33.100.10"@en ;
    dcterms:title "Emission"@en ;
    rdfs:comment "This is ICS for “Emission”"@en .

sto:ICS_33_100_20 a owl:NamedIndividual,
        sto:InternationalClassificationForStandards ;
    rdfs:label "ICS 33.100.20"@en ;
    dcterms:title "Immunity"@en ;
    rdfs:comment "This is ICS for “Immunity”"@en .

sto:ICS_35_060 a owl:NamedIndividual,
        sto:InternationalClassificationForStandards ;
    rdfs:label "ICS 35.060"@en ;
    dcterms:title "Languages used in information technology"@en ;
    rdfs:comment "This is ICS for “Languages used in information technology”"@en .

sto:IECICS_25_040_01 a owl:NamedIndividual .

sto:IEC_61131 a dbpcy:WikicatENStandards,
        dbpcy:WikicatIECStandards,
        owl:NamedIndividual,
        sto:Standard ;
    rdfs:label "IEC 61131"@en ;
    dcterms:subject dbrc:Electronic_engineering,
        dbrc:IEC_standards,
        dbrc:Programmable_logic_controllers ;
    lingg:hypernym dbres:IEC ;
    dul:isComponentOf sto:IEC_62714 ;
    rdfs:comment "IEC 61131 is an IEC standard for programmable controllers. It was known as IEC 1131 before the change in numbering system by IEC. The parts of the IEC 61131 standard are prepared and maintained working group 7, programmable control systems, of subcommittee SC 65B of Technical Committee TC65 of the IEC."@en ;
    sto:hasClassification rami:ControlDevice,
        rami:Station,
        rami:WorkCenter ;
    sto:hasDBpediaResource <http://dbpedia.org/page/IEC_61131> ;
    sto:hasOfficialResource <https://webstore.iec.ch/publication/4550> ;
    sto:hasPublisher sto:IEC ;
    sto:hasTag "PLC Open"@en ;
    sto:hasWikipediaArticle <https://en.wikipedia.org/wiki/IEC_61131> ;
    sto:relatedTo sto:IEC_61499 .

sto:IEC_61511 a dbpcy:WikicatElectricalStandards,
        owl:NamedIndividual,
        sto:Standard ;
    rdfs:label "IEC 61511" ;
    dcterms:hasLicense "Private"@en ;
    dcterms:subject dbrc:Electrical_standards,
        dbrc:Industrial_processes,
        dbrc:Manufacturing,
        dbrc:Safety ;
    rdfs:comment "IEC 61511 is a technical standard which sets out practices in the engineering of systems that ensure the safety of an industrial process through the use of instrumentation."@en ;
    sto:hasClassification idsram:Certification,
        idsram:Safety ;
    sto:hasDBpediaResource dbres:IEC_61511 ;
    sto:hasDomain sto:FunctionalSafety ;
    sto:hasMotivation "Defines the functional safety requirements established by IEC 61508 in process industry sector terminology"@en ;
    sto:hasOfficialResource <https://webstore.iec.ch/publication/24241> ;
    sto:hasPublicationDate "2016-02-24"^^xsd:date ;
    sto:hasPublisher sto:IEC ;
    sto:hasTag "Functional safety - Safety instrumented systems for the process industry sector"@en ;
    sto:hasWikipediaArticle <https://en.wikipedia.org/wiki/IEC_61511> ;
    sto:relatedTo sto:IEC_62061,
        sto:ISO_13849 .

sto:IEC_61784 a dbpcy:WikicatComputerBuses,
        dbont:Work,
        owl:NamedIndividual,
        sto:Standard ;
    rdfs:label "IEC 61784"@en ;
    dcterms:hasLicense "Private"@en ;
    dcterms:subject dbrc:Automation,
        dbrc:Industrial_automation,
        dbrc:Industrial_computing,
        dbrc:Production_and_manufacturing,
        dbrc:Serial_buses ;
    lingg:hypernym dbres:Standard ;
    rdfs:comment "Industrial communication networks - Profiles - Ethernet-real-time-enabled"@en ;
    sto:hasClassification rami:Communication,
        rami:CommunicationSubModel,
        rami:ControlDevice,
        rami:FieldDevice ;
    sto:hasDBpediaResource <http://dbpedia.org/page/Profibus> ;
    sto:hasMotivation "Information description and communication mapping for fieldbus profiles"@en ;
    sto:hasOfficialResource <https://webstore.iec.ch/publication/5878> ;
    sto:hasPublicationDate "2014-08-19"^^xsd:date ;
    sto:hasPublisher sto:IEC ;
    sto:hasTag "IEC Fieldbus (Profibus)"@en ;
    sto:hasWikipediaArticle "http://en.wikipedia.org/wiki/Profibus" ;
    sto:relatedTo sto:IEC_61158 .

sto:IEC_61850 a dbpcy:WikicatIECStandards,
        dbpcy:WikicatNetworkProtocols,
        dbont:Agent,
        owl:NamedIndividual,
        sto:Standard ;
    rdfs:label "IEC 61850"@en ;
    dcterms:subject dbrc:Electric_power,
        dbrc:IEC_standards,
        dbrc:Smart_grid ;
    lingg:hypernym dbres:Communication ;
    rdfs:comment "IEC 61850 is a standard for vendor-agnostic engineering of the configuration of Intelligent Electronic Devices for electrical substation automation systems to be able to communicate with each other.."@en ;
    sto:hasDBpediaResource <http://dbpedia.org/page/IEC_61850> ;
    sto:hasOfficialResource <https://webstore.iec.ch/publication/4550> ;
    sto:hasPublisher sto:IEC ;
    sto:hasWikipediaArticle <https://en.wikipedia.org/wiki/IEC_61850> .

sto:IEC_61987_X a owl:NamedIndividual,
        sto:Standard ;
    rdfs:label "IEC 61987_X"@en ;
    dcterms:hasLicense "Private"@en ;
    rdfs:comment "Industrial-process measurement and control - Data structures and elements in process equipment catalogs - Measuring equipment with analogue and digital output"@en ;
    sto:hasClassification rami:ControlDevice,
        rami:Engineering,
        rami:Enterprise,
        rami:FieldDevice,
        rami:Product,
        rami:Station,
        rami:WorkCenter ;
    sto:hasMotivation "Properties and LOPs as an informational representation of the features of measuring equipment. The referenced standards define general principles (e.g. part 11) as well as specific LOPs for specific device types. These international standards also may serve as examples for description of products."@en ;
    sto:hasOfficialResource <https://webstore.iec.ch/publication/6225> ;
    sto:hasPublisher sto:IEC ;
    sto:hasTag "LOPs in PA"@en .

sto:IEC_62061 a dbpcy:WikicatElectricalStandards,
        dbpcy:WikicatIECStandards,
        dbont:Software,
        owl:NamedIndividual,
        sto:Standard ;
    rdfs:label "IEC 60061"@en ;
    dcterms:subject dbrc:Electrical_standards,
        dbrc:IEC_standards,
        dbrc:Safety ;
    lingg:hypernym dbres:Implementation ;
    rdfs:comment "provides requirements that are applicable to the system level design of all types of machinery safety-related electrical control systems and also for the design of non-complex subsystems or devices."@en ;
    sto:hasClassification rami:Safety ;
    sto:hasDBpediaResource dbres:IEC_62061 ;
    sto:hasOfficialResource <https://webstore.iec.ch/publication/22797> ;
    sto:hasPublisher sto:IEC ;
    sto:hasTag "Safety of machinery"@en ;
    sto:hasWikipediaArticle <https://en.wikipedia.org/wiki/IEC_62061> .

sto:IEC_62337 a owl:NamedIndividual,
        sto:Standard ;
    rdfs:label "IEC 62337"@en ;
    rdfs:comment "Commissioning of electrical, instrumentation and control systems in the process industry - Specific phases and milestones."@en ;
    sto:hasClassification rami:Conditional_Monitoring,
        rami:Enterprise,
        rami:Functional,
        rami:Lifecycle_Status,
        rami:Work_Centers,
        sto:ProductionSystemModelData ;
    sto:hasDomain sto:IndustrialAutomation ;
    sto:hasOfficialResource <https://webstore.iec.ch/publication/6871> ;
    sto:hasPublicationDate "2012-02-22"^^xsd:date ;
    sto:hasPublisher sto:IEC .

sto:IEC_62443 a owl:NamedIndividual,
        sto:Standard ;
    rdfs:label "IEC 62443"@en ;
    dcterms:hasLicense "Private"@en ;
    rdfs:comment "Defines procedures for implementing electronically secure Industrial Automation and Control Systems."@en,
        "ISA/IEC-62443 is a series of standards, technical reports, and related information that define procedures for implementing electronically secure Industrial Automation and Control Systems (IACS). This guidance applies to end-users (i.e. asset owner), system integrators, security practitioners, and control systems manufacturers responsible for manufacturing, designing, implementing, or managing industrial automation and control systems."@en ;
    skos:altLabel "ISA 99" ;
    skos:note "TODO" ;
    sto:alignesWith sto:Identification ;
    sto:hasClassification iira:Security,
        rami:Security,
        sto:CrossLevel,
        idsram:Certification ;
    sto:hasDBpediaResource <http://dbpedia.org/page/Cyber_security_standards#ISA/IEC-62443_(formerly_ISA-99)> ;
    sto:hasDeveloper sto:ANSI,
        sto:ISA ;
    sto:hasMotivation "Cyber attacks threat the industry and can cause damage to property and personal injury and affect the image of companies. The Standard allows to define procedures for implementing electronically secure Industrial Automation and Control Systems (IACS). This guidance applies to end-users, system integrators, security practitioners, and control systems manufacturers responsible for manufacturing, designing, implementing, or managing industrial automation and control systems"@en ;
    sto:hasOfficialResource <https://webstore.iec.ch/publication/7029>,
        <https://webstore.iec.ch/publication/7033> ;
    sto:hasPublisher sto:ANSI,
        sto:IEC,
        sto:ISA ;
    sto:hasTag "Electronically secure Industrial Automation and Control Systems"@en,
        "Network and system security for industrial-process measurement and control"@en ;
    sto:hasWikipediaArticle <https://en.wikipedia.org/wiki/Cyber_security_standards#ISA.2FIEC-62443_.28formerly_ISA-99.29> .

sto:IEC_62453 a owl:NamedIndividual,
        sto:Standard ;
    rdfs:label "IEC 62453"@en ;
    rdfs:comment "Field device tool (FDT) interface specification - Overview and guidance"@en ;
    sto:hasClassification rami:Configuration,
        rami:ControlDevice,
        rami:FieldDevice,
        rami:Station ;
    sto:hasMotivation "FDT is an interface for integration of devices into a system (e.g. control system or engineering system). The standard supports factory automation as well as process automation with a wide range of fieldbus protocols. The interface defines fieldbus-independent mechanisms for accessing data and functions of the devices."@en ;
    sto:hasOfficialResource <https://webstore.iec.ch/publication/7040> ;
    sto:hasPublisher sto:IEC ;
    sto:hasTag "FDT"@en .

sto:IEC_62890 a owl:NamedIndividual,
        sto:Standard ;
    rdfs:label "IEC 62890"@en ;
    dcterms:hasLicense "Private"@en ;
    rdfs:comment "Defines standards for lifecycle management for systems and products used in industrial process measurement, control and automation"@en,
        "MES KPIs"@en ;
    sto:hasClassification rami:LifecycleStatus,
        rami:Station,
        rami:WorkCenter,
        sto:ProductionLifeCycleDataManagement ;
    sto:hasMotivation "Stations need to describe their operational state and performance parameters towards superior I4.0-Components"@en ;
    sto:hasOfficialResource <http://www.iec.ch/dyn/www/f?p=103:38:16824039984463::::FSP_ORG_ID,FSP_APEX_PAGE,FSP_PROJECT_ID:1250,23,20929> ;
    sto:hasPublisher sto:IEC ;
    sto:hasTag "IEC 62890"@en .

sto:IEC_TS_62832 a owl:NamedIndividual,
        sto:Standard ;
    rdfs:label "IEC TS 62832"@en ;
    dcterms:hasLicense "Private"@en ;
    rdfs:comment "Digital Factory Reference model TS"@en ;
    sto:hasClassification rami:AdminShellGeneral,
        rami:ControlDevice,
        rami:FieldDevice,
        rami:GeneralAdminShell,
        rami:Station,
        rami:WorkCenter ;
    sto:hasMotivation "The standards for Digital Factory define methods and information models, which are required for self description of I40-components. IEC TS 62832 defines methods, which allow to validate or plan connections between assets."@en ;
    sto:hasOfficialResource <https://webstore.iec.ch/publication/33023> ;
    sto:hasPublisher sto:IEC ;
    sto:hasTag "DF/TS"@en .

sto:ISO_10303 a dbpcy:WikicatCADFileFormats,
        dbpcy:WikicatGraphicsFileFormats,
        dbpcy:WikicatISOStandards,
        dbont:Organisation,
        owl:NamedIndividual,
        sto:Standard ;
    rdfs:label "ISO 10303"@en ;
    dcterms:subject dbrc:CAD_file_formats,
        dbrc:ISO_standards ;
    lingg:hypernym dbres:ISO ;
    rdfs:comment "Standard for the Exchange of Product model data. ISO 10303 can represent 3D objects in Computer-aided design (CAD) and related information."@en ;
    skos:note "TODO - Split properly and classify it - check the NIST paper" ;
    sto:hasClassification sto:ProductLifeCycleManagement ;
    sto:hasDBpediaResource <http://dbpedia.org/page/ISO_10303> ;
    sto:hasOfficialResource <https://www.steptools.com/stds/step/> ;
    sto:hasPublisher sto:ISO ;
    sto:hasTag "STEP"@en ;
    sto:hasWikipediaArticle <https://en.wikipedia.org/wiki/ISO_10303> .

sto:ISO_11404 a owl:NamedIndividual ;
    rdfs:label "ISO/IEC 11404"@en ;
    sto:hasClassification idsram:InformationLayer ;
    sto:hasDeveloper sto:IEC,
        sto:ISO .

sto:ISO_11783 a dbpcy:WikicatISOStandards,
        dbpcy:WikicatNetworkProtocols,
        dbont:Software,
        owl:NamedIndividual,
        sto:Standard ;
    rdfs:label "ISO 11783"@en ;
    dcterms:subject dbrc:ISO_standards,
        dbrc:Network_protocols ;
    lingg:hypernym dbres:Protocol ;
    rdfs:comment "ISO 11783, known as Tractors and machinery for agriculture and forestry—Serial control and communications data network is a communication protocol for the agriculture industry based on the SAE J1939 protocol (which includes CANbus)."@en ;
    sto:hasDBpediaResource dbres:ISO_11783 ;
    sto:hasOfficialResource <https://www.iso.org/standard/61646.html> ;
    sto:hasPublisher sto:ISO ;
    sto:hasTag "ISOBUS"@en ;
    sto:hasWikipediaArticle <https://en.wikipedia.org/wiki/ISO_11783> .

sto:ISO_13374 a owl:NamedIndividual,
        sto:Standard ;
    rdfs:label "ISO 13374"@en ;
    rdfs:comment "Condition monitoring and diagnostics of machines -- Data processing, communication and presentation"@en ;
    sto:hasClassification rami:Business,
        rami:Conditional_Monitoring,
        rami:Enterprise,
        sto:ProductionSystemEngineering ;
    sto:hasDomain sto:IndustrialAutomation ;
    sto:hasOfficialResource <https://www.iso.org/standard/61131.html> ;
    sto:hasPublicationDate "2012-02-01"^^xsd:date ;
    sto:hasPublisher sto:ISO .

sto:ISO_13849 a dbpcy:WikicatISOStandards,
        dbpcy:WikicatSafetyCodes,
        owl:NamedIndividual,
        sto:Standard ;
    rdfs:label "ISO 13849"@en ;
    dcterms:subject dbrc:ISO_standards,
        dbrc:Safety_codes ;
    rdfs:comment "Provides safety requirements and guidance on the principles for the design and integration of safety-related parts of control systems (SRP/CS), including the design of software."@en ;
    sto:hasClassification iira:Security,
        rami:Safety,
        idsram:Certification,
        idsram:Safety ;
    sto:hasDBpediaResource dbres:ISO_13849 ;
    sto:hasDomain "Safety of machinery"@en ;
    sto:hasOfficialResource <http://www.iso.org/iso/home/store/catalogue_tc/catalogue_detail.htm?csnumber=69883> ;
    sto:hasPublisher sto:ISO ;
    sto:hasWikipediaArticle <https://en.wikipedia.org/wiki/ISO_13849> .

sto:ISO_14306 a owl:NamedIndividual,
        sto:Standard ;
    rdfs:label "ISO 14306"@en ;
    rdfs:comment "It provides the description of the structure and content for a binary file having the extension of .jt. A binary file with the .jt extension is generally referred to as a JT file. The JT format described in ISO 14306:2012 is used primarily in industrial use cases as the means for capturing and repurposing lightweight 3D product definition data"@en ;
    sto:hasClassification rami:Asset,
        rami:Engineering,
        rami:Identification,
        rami:Product,
        sto:ProcessPlanning,
        sto:ProductionSystemModelData ;
    sto:hasDomain sto:CAD ;
    sto:hasOfficialResource <https://www.iso.org/standard/60572.html> ;
    sto:hasPublicationDate "2017-07-01"^^xsd:date ;
    sto:hasPublisher sto:ISO ;
    sto:relatedTo sto:IEC_62541 .

sto:ISO_14443 a owl:NamedIndividual,
        sto:Standard ;
    rdfs:label "ISO 14443"@en ;
    rdfs:comment "ISO 14443 Identification cards -- Contactless integrated circuit cards -- Proximity cards is an international standard that defines proximity cards used for identification, and the transmission protocols for communicating with it"@en .

sto:ISO_15408 a owl:NamedIndividual,
        sto:Standard ;
    rdfs:label "ISO/IEC 15408"@en ;
    dc11:title "Common Criteria for Information Technology Security Evaluation"@en ;
    rdfs:comment "The Common Criteria for Information Technology Security Evaluation (abbreviated as Common Criteria or CC) is an international standard (ISO/IEC 15408) for computer security certification"@en ;
    sto:hasClassification iira:Security ;
    sto:hasOfficialResource <https://www.niap-ccevs.org/Documents_and_Guidance/cc_docs.cfm> ;
    sto:hasPublisher sto:ISO ;
    sto:hasWikipediaArticle <http://wikipedia.org/wiki/Common_Criteria_for_Information_Technology_Security_Evaluation> .

sto:ISO_15459 a owl:NamedIndividual .

sto:ISO_19439 a dbpcy:WikicatISOStandards,
        dbont:Work,
        owl:NamedIndividual,
        sto:Standard ;
    rdfs:label "ISO 19439"@en ;
    dcterms:subject dbrc:Enterprise_modelling,
        dbrc:ISO_standards ;
    lingg:hypernym dbres:Standard ;
    dul:associatedWith sto:Certification ;
    rdfs:comment "Provides a unified conceptual basis for model-based enterprise engineering that enables consistency, convergence and interoperability of the various modelling methodologies and supporting tools."@en ;
    sto:hasClassification rami:Business ;
    sto:hasDBpediaResource <http://dbpedia.org/page/ISO_19439> ;
    sto:hasOfficialResource <https://www.iso.org/standard/33833.html> ;
    sto:hasPublisher sto:ISO ;
    sto:hasTag "19439"@en ;
    sto:hasWikipediaArticle <https://en.wikipedia.org/wiki/ISO_19439> .

sto:ISO_24760 a owl:NamedIndividual .

sto:ISO_27018 a dbpcy:WikicatComputerSecurityStandards,
        dbpcy:WikicatENStandards,
        dbpcy:WikicatIECStandards,
        <http://dbpedia.org/class/yago/WikicatISO/IECStandards>,
        dbpcy:WikicatISOStandards,
        owl:NamedIndividual,
        sto:Standard ;
    rdfs:label "ISO/IEC 27018"@en ;
    dc11:title "Information technology -- Security techniques -- Code of practice for protection of personally identifiable information (PII) in public clouds acting as PII processors"@en ;
    dcterms:subject <http://dbpedia.org/resource/Category:ISO/IEC_standards>,
        dbrc:Information_technology_management ;
    rdfs:comment "ISO/IEC 27018:2014 establishes commonly accepted control objectives, controls and guidelines for implementing measures to protect Personally Identifiable Information (PII) in accordance with the privacy principles in ISO/IEC 29100 for the public cloud computing environment."@en ;
    sto:hasClassification iira:Privacy,
        iira:Security ;
    sto:hasDBpediaResource <http://dbpedia.org/resource/ISO/IEC_27000-series> ;
    sto:hasOfficialResource <https://www.iso.org/standard/61498.html> ;
    sto:hasPublicationDate "2014-08-01"^^xsd:date ;
    sto:hasPublisher sto:IEC,
        sto:ISO ;
    sto:hasWikipediaArticle <https://en.wikipedia.org/wiki/ISO/IEC_27000-series> .

sto:ISO_27031 a owl:NamedIndividual,
        sto:Standard ;
    rdfs:label "ISO/IEC 27031"@en ;
    dc11:title "Guidelines for information and communication technology readiness for business continuity"@en ;
    rdfs:comment "ISO/IEC 27031:2011 describes the concepts and principles of information and comunication technology (ICT) readiness for business continuity, and provides a framework of methods and processes to identify and specify all aspects (such as performance criteria, design, and implementation) for improving an organization's ICT readiness to ensure business continuity."@en ;
    sto:domainName "Business Continuity"@en ;
    sto:hasClassification iira:Security ;
    sto:hasOfficialResource <https://www.iso.org/standard/44374.html> ;
    sto:hasPublicationDate "2011-03-01"^^xsd:date ;
    sto:hasPublisher sto:IEC,
        sto:ISO .

sto:ISO_27036 a dbpcy:WikicatComputerSecurityStandards,
        dbpcy:WikicatENStandards,
        dbpcy:WikicatIECStandards,
        <http://dbpedia.org/class/yago/WikicatISO/IECStandards>,
        dbpcy:WikicatISOStandards,
        owl:NamedIndividual,
        sto:Standard ;
    rdfs:label "ISO/IEC 27036"@en ;
    dc11:title "Information security for supplier relationships"@en ;
    dcterms:subject <http://dbpedia.org/resource/Category:ISO/IEC_standards>,
        dbrc:Information_technology_management ;
    rdfs:comment """ISO/IEC 27036-4:2016 provides cloud service customers and cloud service providers with guidance on\r
\r
a) gaining visibility into the information security risks associated with the use of cloud services and managing those risks effectively, and\r
\r
b) responding to risks specific to the acquisition or provision of cloud services that can have an information security impact on organizations using these services."""@en ;
    sto:hasClassification iira:Security ;
    sto:hasDBpediaResource <http://dbpedia.org/resource/ISO/IEC_27000-series> ;
    sto:hasOfficialResource <https://www.iso.org/standard/59689.html> ;
    sto:hasPublicationDate "2016-10-01"^^xsd:date ;
    sto:hasPublisher sto:IEC,
        sto:ISO ;
    sto:hasWikipediaArticle <https://en.wikipedia.org/wiki/ISO/IEC_27000-series> .

sto:ISO_29100 a owl:NamedIndividual,
        sto:Standard ;
    rdfs:label "ISO/IEC 29100"@en ;
    dcterms:title "Privacy framework"@en ;
    rdfs:comment """‘Privacy framework’1 provides a guideline that specifies a common privacy terminology, defines actors and roles in processing PII, describes privacy safeguarding considerations, and includes references to known privacy principles for Information technology.\r
source: IIC SF"""@en ;
    sto:hasClassification iira:Privacy,
        iira:Security ;
    sto:hasOfficialResource <https://www.iso.org/standard/45123.html> ;
    sto:hasPublicationDate "2011-12-01"^^xsd:date ;
    sto:hasPublisher sto:IEC,
        sto:ISO .

sto:ISO_29115 a owl:NamedIndividual ;
    rdfs:label "ISO/IEC 29115"@en ;
    sto:alignesWith sto:Authentication,
        sto:Identification ;
    sto:hasClassification iira:Security ;
    sto:hasPublisher sto:ISO .

sto:ISO_29161 a owl:NamedIndividual,
        sto:Standard ;
    rdfs:label "ISO 29161" ;
    rdfs:comment "ISO/IEC 29161:2016 establishes a unique identification scheme for the Internet of Things (IoT), based on existing and evolving data structures."@en ;
    sto:hasOfficialResource <https://www.iso.org/standard/45240.html> .

sto:ISO_29190 a owl:NamedIndividual,
        sto:Standard ;
    rdfs:label "ISO/IEC 29190"@en ;
    dcterms:title "Privacy capability assessment model"@en ;
    rdfs:comment "‘Privacy capability assessment model’ provides high-level guidance to organizations about assessing their capability to manage privacy-related processes."@en ;
    sto:hasClassification iira:Privacy,
        iira:Security ;
    sto:hasOfficialResource <https://www.iso.org/standard/45269.html> ;
    sto:hasPublicationDate "2015-08-01"^^xsd:date ;
    sto:hasPublisher sto:IEC,
        sto:ISO .

sto:IndustrialDataSpace a owl:NamedIndividual,
        sto:StandardizationFramework .

sto:ManufacturingModelData a owl:NamedIndividual,
        sto:ProductDevelopmentLifeCycle ;
    rdfs:label "Manufacturing Model Data"@en ;
    rdfs:comment "Manufacturing Model Data Standards define the data needed to manufacture a product from a design."@en ;
    sto:isDescribedin sto:NISTInitiative .

sto:MathML a dbpcy:WikicatMarkupLanguages,
        dbpcy:WikicatMathematicalMarkupLanguages,
        dbpcy:WikicatWebBrowsers,
        dbpcy:WikicatWebStandards,
        dbpcy:WikicatWorldWideWebConsortiumStandards,
        dbpcy:WikicatXML-basedStandards,
        dbont:Language,
        owl:NamedIndividual,
        owl:Thing,
        sto:Standard ;
    rdfs:label "MathML"@en ;
    dcterms:subject dbrc:Articles_with_example_Scheme_code,
        dbrc:MathML,
        dbrc:Mathematical_markup_languages,
        dbrc:World_Wide_Web_Consortium_standards,
        dbrc:XML-based_standards,
        dbrc:XML_markup_languages ;
    lingg:hypernym dbres:Language ;
    rdfs:comment "MathML is a low-level specification for mathematical and scientific content on the Web and beyond"@en ;
    sto:hasDBpediaResource <http://dbpedia.org/page/MathML> ;
    sto:hasOfficialResource <https://www.w3.org/Math/> ;
    sto:hasPublisher sto:W3C ;
    sto:hasWikipediaArticle <https://en.wikipedia.org/wiki/MathML> .

sto:OAGi a owl:NamedIndividual,
        sto:StandardOrganization ;
    rdfs:label "OAGi"@en ;
    rdfs:comment "The Open Applications Group is a not-for-profit standards development organization. Founded in 1994, is focused on building enterprise ready process-based data exchange standards for both B2B and A2A integration."@en ;
    sto:abbreviation "OAGi" ;
    sto:formationDate "1994-01-01"^^xsd:date ;
    sto:hasHeadquaterIn dbr:_Georgia ;
    sto:hasOfficialResource <http://www.oagi.org/dnn2/Home.aspx> ;
    sto:orgName "Open Applications Group"@en .

sto:OPC_Foundation a dbpcy:Abstraction100002137,
        dbpcy:Group100031264,
        dbpcy:Organization108008335,
        dbpcy:SocialGroup107950920,
        dbpcy:WikicatStandardsOrganizations,
        dbpcy:YagoLegalActor,
        dbpcy:YagoLegalActorGeo,
        dbpcy:YagoPermanentlyLocatedEntity,
        dbont:Organisation,
        owl:NamedIndividual,
        sto:StandardOrganization ;
    rdfs:label "OPC Foundation"@en ;
    dcterms:subject dbrc:Automation ;
    lingg:hypernym dbres:Consortium ;
    rdfs:comment "Is an industry consortium that creates and maintains standards for open connectivity of industrial automation devices and systems, such as industrial control systems and process control generally"@en ;
    sto:abbreviation "OPC" ;
    sto:formationDate "1994-01-01"^^xsd:date ;
    sto:hasDBpediaResource <http://dbpedia.org/page/OPC_Foundation> ;
    sto:hasHeadquaterIn dbr:_Arizona ;
    sto:hasOfficialResource <https://opcfoundation.org/> ;
    sto:hasWikipediaArticle <https://en.wikipedia.org/wiki/OPC_Foundation> ;
    sto:orgName "OPC Foundation"@en .

sto:ProcessPlanning a owl:NamedIndividual .

sto:Prodcut a owl:NamedIndividual .

sto:Product a owl:NamedIndividual .

sto:ProductionLifeCycleDataManagement a owl:NamedIndividual,
        sto:ProductionSystemLifeCycle ;
    rdfs:label "Production Life Cycle Data Management"@en ;
    rdfs:comment "Production lifecycle data management standards define general models of data integration, sharing, exchange, and hand-over for lifecycle support of production facilities."@en ;
    sto:isDescribedin sto:NISTInitiative .

sto:SCADALevel a owl:NamedIndividual,
        sto:ISA95Level ;
    rdfs:label "SCADA Level"@en ;
    rdfs:comment "Describes the SCADA level according to the ISA95 level classification."@en ;
    skos:definition "Supervisory control and data acquisition according to ISA 95"@en ;
    sto:isDescribedin sto:ISA95 .

sto:SE a dbpcy:Abstraction100002137,
        dbpcy:Business108061042,
        dbpcy:Company108058098,
        dbpcy:ElectronicsCompany108003035,
        dbpcy:Enterprise108056231,
        dbpcy:Group100031264,
        dbpcy:Institution108053576,
        dbpcy:Manufacturer108060446,
        dbpcy:Organization108008335,
        dbpcy:SocialGroup107950920,
        dbpcy:WikicatCompaniesBasedInParis,
        dbpcy:WikicatCompaniesEstablishedIn1836,
        dbpcy:WikicatCompaniesListedOnTheEuronextExchanges,
        dbpcy:WikicatCompaniesListedOnTheEuronextParis,
        dbpcy:WikicatCompaniesListedOnTheFrankfurtStockExchange,
        dbpcy:WikicatCompaniesOfFrance,
        dbpcy:WikicatDefenceCompaniesOfFrance,
        dbpcy:WikicatElectricalEquipmentManufacturers,
        dbpcy:WikicatElectronicsCompaniesOfFrance,
        dbpcy:WikicatLocomotiveManufacturersOfFrance,
        dbpcy:WikicatManufacturersOfIndustrialAutomation,
        dbpcy:WikicatManufacturingCompaniesOfFrance,
        dbpcy:WikicatMultinationalCompaniesHeadquarteredInFrance,
        dbpcy:YagoLegalActor,
        dbpcy:YagoLegalActorGeo,
        dbpcy:YagoPermanentlyLocatedEntity,
        dbont:Agent,
        dbont:Company,
        dbont:Organisation,
        schema:Organization,
        dul:Agent,
        dul:SocialPerson,
        owl:NamedIndividual,
        owl:Thing,
        wike:Q24229398,
        wike:Q43229,
        sto:StandardOrganization ;
    dcterms:subject <http://dbpedia.org/resource/Category:1836_establishments_in_France>,
        dbrc:CAC_40,
        dbrc:Companies_established_in_1836,
        dbrc:Companies_in_the_Euro_Stoxx_50,
        dbrc:Conglomerate_companies_of_France,
        dbrc:Electrical_engineering_companies_of_France,
        dbrc:Electrical_wiring_and_construction_supplies_manufacturers,
        dbrc:French_brands,
        dbrc:Locomotive_manufacturers_of_France,
        dbrc:MES_software,
        dbrc:Manufacturers_of_industrial_automation,
        dbrc:Manufacturing_companies_of_France,
        dbrc:Multinational_companies_headquartered_in_France,
        dbrc:Power_engineering,
        dbrc:Schneider_Electric,
        dbrc:Societates_Europaeae ;
    lingg:hypernym dbres:Corporation ;
    rdfs:comment "The Broadband Forum is a non-profit industry consortium dedicated to developing broadband network specifications. Members include telecommunications networking and service provider companies, broadband device and equipment vendors, consultants and independent testing labs (ITLs). Service provider members are primarily wire-line service providers (non-mobile) telephone companies."@en ;
    sto:abbreviation "SE" ;
    sto:formationDate "1936-01-01"^^xsd:date ;
    sto:hasDBpediaResource <http://dbpedia.org/page/Schneider_Electric> ;
    sto:hasHeadquaterIn dbr:Paris ;
    sto:hasOfficialResource <http://www.schneider-electric.com/ww/en/> ;
    sto:hasWikipediaArticle <https://en.wikipedia.org/wiki/Schneider_Electric> ;
    sto:orgName "Schneider Electric"@en .

sto:Safety a owl:NamedIndividual,
        sto:ISO_42010_Concern .

sto:TC_25 a owl:NamedIndividual,
        sto:TechnicalCommittee ;
    rdfs:label "TC 25"@en ;
    dcterms:title "Quantities and units"@en ;
    rdfs:comment "To prepare international standards on quantities and units to be used in electrical technology. Such standards may relate to their definitions, names, letter symbols and use; to the relations in which they appear; and to the signs and symbols used with them."@en .

sto:TC_56 a owl:NamedIndividual,
        sto:TechnicalCommittee ;
    rdfs:label "TC 56"@en ;
    dcterms:title "Dependability"@en ;
    rdfs:comment """To prepare international standards in the field of dependability, in all appropriate technological areas, including those not normally dealt with by IEC Technical Committees. Dependability covers the availability performance and its influencing factors: reliability performance, maintainability performance and maintenance support performance (including management of obsolescence). The standards provide systematic methods and tools for the dependability assessment and management of equipment, services and systems throughout their life cycles.\r
The standards cover generic aspects on reliability and maintainability programme management, testing and analytical techniques, software and system dependability, life cycle costing, technical risk analysis and project risk management. This includes standards related to product issues from component reliability to guidance for engineering dependability of systems, standards related to process issues from technological risk analysis to integrated logistics support and standards related to management issues from dependability program management to managing for obsolescence.\r
The application of these standards may raise safety related issues, though the standards themselves do not cover safety. They may be applied to business risk analysis but these risk areas are not dealt with by TC 56."""@en .

sto:TC_66 a owl:NamedIndividual,
        sto:TechnicalCommittee ;
    rdfs:label "TC 66"@en ;
    dcterms:title "Safety of measuring"@en,
        "control and laboratory equipment"@en ;
    rdfs:comment """To prepare safety standards for test and measurement equipment, industrial-process control equipment, and laboratory equipment wherever they are used.\r
Such equipment includes:\r
a) equipment and systems to measure, test, generate, and analyse, simple and complex electromagnetic quantities and equipment that by electromagnetic means measure physical quantities.\r
Note: Aspects of this equipment other than safety are covered by other technical committees.\r
b) equipment and systems for industrial-process measurement and control.\r
Note: Aspects of this equipment other than safety are covered by TC 65 except that SC 65A has a Horizontal Safety Function relating to the functional safety of electrical/electronic/ programmable electronic systems and SC 65B is responsible for the functional safety of programmable controllers.\r
c) laboratory equipment for analysis, handling and preparation of materials.\r
Note: This equipment includes measuring instruments, systems and their accessories, for preparation, treatment and analysis of materials in the fields of research, medicine, industry and education, and for environmental monitoring.\r
TC 66 has a Group Safety Function in accordance with IEC Guide 104 for the equipment in categories a) to c) above."""@en .

sto:TC_77 a owl:NamedIndividual,
        sto:TechnicalCommittee ;
    rdfs:label "TC 77"@en ;
    dcterms:title "Electromagnetic compatibility"@en ;
    rdfs:comment """Standardization - to prepare standards and technical reports - in the field of electromagnetic compatibility (EMC), with\r
particular emphasis on general application and use by product committees. (Horizontal function). The scope covers the following aspects of EMC:\r
- Immunity and related items, over the whole frequency range: basic and generic standards, - emission in the low frequency range (f <= 9 kHz, e.g. harmonics and voltage fluctuations): basic, generic and product (family) standards,\r
- emission in the high frequency range (f > 9 kHz): disturbances not covered by CISPR 10 (1992), in co-ordination with CISPR (e.g. mains signalling).\r
Product immunity standards are not included. However, at the request of product committees, TC 77 may also prepare such standards under the co-ordination of ACEC.\r
Horizontal Safety Function: Electromagnetic compatibility in so far as safety aspects are involved."""@en .

sto:TechnicalSpecification a owl:Class,
        owl:NamedIndividual ;
    rdfs:label "Technical Specification"@en ;
    cc:attributionURL "http://www.iec.ch" ;
    rdfs:comment "Specifies that a given Publication is a Technical Specification"@en,
        "Technical Specifications are often published when the subject under question is still under development or when insufficient consensus for approval of an International Standard is available.Technical Specifications approach International Standards in terms of detail and completeness, but have not yet passed through all approval stages either because consensus has not been reached or because standardization is seen to be premature."@en ;
    rdfs:isDefinedBy sto:IEC ;
    rdfs:seeAlso <http://www.iec.ch/standardsdev/publications/ts.htm> ;
    rdfs:subClassOf sto:Publication ;
    sto:abbreviation "TS" .

sto:UN-CEFACT a dbpcy:Abstraction100002137,
        dbpcy:Group100031264,
        dbpcy:Organization108008335,
        dbpcy:SocialGroup107950920,
        dbpcy:WikicatInternationalEconomicOrganizations,
        dbpcy:WikicatOrganizationsEstablishedByTheUnitedNations,
        dbpcy:YagoLegalActor,
        dbpcy:YagoLegalActorGeo,
        dbpcy:YagoPermanentlyLocatedEntity,
        dbont:Organisation,
        owl:NamedIndividual,
        owl:Thing,
        sto:StandardOrganization ;
    dcterms:subject dbrc:Accounting,
        dbrc:Computer_file_formats,
        dbrc:E-commerce,
        dbrc:International_trade,
        dbrc:United_Nations_Economic_Commission_for_Europe ;
    lingg:hypernym dbres:Organisation ;
    rdfs:comment "UN/CEFACT is the United Nations Centre for Trade Facilitation and Electronic Business. It was established as an intergovernmental body of the United Nations Economic Commission for Europe (UNECE) in 1996 and evolved from UNECE’s long tradition of work in trade facilitation."@en ;
    sto:abbreviation "UN/CEFACT" ;
    sto:hasDBpediaResource <http://dbpedia.org/page/UN/CEFACT> ;
    sto:hasHeadquaterIn dbr:Geneva ;
    sto:hasOfficialResource <https://www.unece.org/cefact/> ;
    sto:hasWikipediaArticle <https://en.wikipedia.org/wiki/UN/CEFACT> ;
    sto:orgName "United Nations Centre for Trade Facilitation and Electronic Business"@en .

sto:VDMA a dbpcy:Abstraction100002137,
        dbpcy:Association108049401,
        dbpcy:Group100031264,
        dbpcy:Organization108008335,
        dbpcy:ProfessionalAssociation108242675,
        dbpcy:SocialGroup107950920,
        dbpcy:WikicatProfessionalAssociations,
        dbpcy:WikicatProfessionalAssociationsBasedInGermany,
        dbpcy:YagoLegalActor,
        dbpcy:YagoLegalActorGeo,
        dbpcy:YagoPermanentlyLocatedEntity,
        dbont:Organisation,
        owl:NamedIndividual,
        sto:StandardOrganization ;
    lingg:hypernym dbres:Association ;
    rdfs:comment "The Mechanical Engineering Industry Association (Verband Deutscher Maschinen- und Anlagenbau – VDMA) has its headquarters in Frankfurt am Main, Germany, and represents around 3,200 members, making it the largest industry association in Europe. The Association represents the interests of the predominantly medium-sized companies in the mechanical engineering industry towards policymakers and society, as well as towards business, the scientific community, public authorities and the media. With more than one million employees and a turnover of around EUR 218 billion (2015), mechanical and plant engineering is Germany’s largest employer in the industrial sector.In addition, VDMA sees itself as a platform that provides its member companies with various networks where they can discuss technological challenges, interdisciplinary issues and many other topics."@en ;
    sto:abbreviation "VDMA" ;
    sto:formationDate "1892-11-15"^^xsd:date ;
    sto:hasDBpediaResource dbres:VDMA ;
    sto:hasHeadquaterIn dbr:Frankfurt ;
    sto:hasOfficialResource <http://www.vdma.org> ;
    sto:hasWikipediaArticle <https://en.wikipedia.org/wiki/Mechanical_Engineering_Industry_Association>,
        "http://en.wikipedia.org/wiki/VDMA" ;
    sto:orgName "Verband Deutscher Maschinen- und Anlagenbau"@de,
        "Mechanical Engineering Industry Association"@en .

sto:Viewpoint a owl:Class ;
    rdfs:label "Viewpoint" ;
    rdfs:comment "ISO 42010 definition of a Viewpoint"@en ;
    rdfs:seeAlso "https://www.iso.org/standard/50508.html" .

sto:W3C_OWL a dbpcy:WikicatOntologyLanguages,
        dbpcy:WikicatWebStandards,
        dbpcy:WikicatWorldWideWebConsortiumStandards,
        dbpcy:WikicatXML-basedStandards,
        owl:NamedIndividual,
        owl:Thing,
        sto:Standard ;
    rdfs:label "Web Ontology Language"@en ;
    dcterms:hasLicense "Public"@en ;
    dcterms:subject dbrc:Declarative_programming_languages,
        dbrc:Ontology_languages,
        dbrc:Resource_Description_Framework,
        <http://dbpedia.org/resource/Category:School_of_Computer_Science,_University_of_Manchester>,
        dbrc:Semantic_Web,
        dbrc:Web_Ontology_Language,
        dbrc:World_Wide_Web_Consortium_standards,
        dbrc:XML-based_standards ;
    lingg:hypernym dbres:Family ;
    rdfs:comment "The W3C Web Ontology Language (OWL) is a Semantic Web language designed to represent rich and complex knowledge about things, groups of things, and relations between things. OWL is a computational logic-based language such that knowledge expressed in OWL can be exploited by computer programs, e.g., to verify the consistency of that knowledge or to make implicit knowledge explicit. OWL documents, known as ontologies, can be published in the World Wide Web and may refer to or be referred from other OWL ontologies. OWL is part of the W3C’s Semantic Web technology stack, which includes RDF, RDFS, SPARQL, etc."@en ;
    sto:hasDBpediaResource dbres:Web_Ontology_Language ;
    sto:hasOfficialResource <https://www.w3.org/OWL/> ;
    sto:hasPublisher sto:W3C ;
    sto:hasTag "OWL"@en ;
    sto:hasWikipediaArticle <https://en.wikipedia.org/wiki/Web_Ontology_Language?oldformat=true>,
        "http://en.wikipedia.org/wiki/Web_Ontology_Language" ;
    sto:relatedTo sto:W3C_RDF .

sto:isDescribedin a owl:ObjectProperty ;
    rdfs:label "is Described in"@en ;
    rdfs:comment "Links the Standarization Frameworks with the Classification of Standards"@en ;
    rdfs:domain sto:StandardClassification ;
    rdfs:range sto:StandardizationFramework .

sto:oneM2M a owl:NamedIndividual,
        sto:StandardOrganization ;
    rdfs:label "oneM2M"@en ;
    rdfs:comment "The purpose and goal of oneM2M is to develop technical specifications which address the need for a common M2M Service Layer that can be readily embedded within various hardware and software, and relied upon to connect the myriad of devices in the field with M2M application servers worldwide. A critical objective of oneM2M is to attract and actively involve organizations from M2M-related business domains such as: telematics and intelligent transportation, healthcare, utilities, industrial automation, smart homes, etc."@en ;
    sto:hasOfficialResource "http://www.onem2m.org/about-onem2m/why-onem2m"^^xsd:anyURI .

idsram:DataSovereignty a owl:NamedIndividual,
        sto:StandardClassification .

idsram:FunctionalLayer a owl:NamedIndividual,
        idsram:Layer ;
    rdfs:label "IDS RAM Functional Layer"@en ;
    dul:associatedWith sto:DataSovereignty,
        sto:Interoperability ;
    sto:isDescribedin idsram:ReferenceArchitectureModel .

idsram:Interoperability a owl:NamedIndividual,
        sto:StandardClassification ;
    rdfs:label "IDS Interoperability"@en ;
    sto:isDescribedin idsram:ReferenceArchitectureModel .

<https://wikipedia.org/wiki/North_American_Electric_Reliability_Corporation> a owl:NamedIndividual .

<ids:TrustedConnector> a owl:NamedIndividual .

dbr:Germany a owl:NamedIndividual .

dbr:_Arizona a owl:NamedIndividual .

dbr:_Massachusetts a owl:NamedIndividual .

iira:BusinessDomain a iira:FunctionalDomain,
        owl:NamedIndividual ;
    rdfs:label "IIRA Business Domain"@en ;
    sto:alignesWith rami:Business,
        idsram:BusinessLayer .

iira:Connectivity a iira:CrosscuttingFunction,
        owl:NamedIndividual ;
    rdfs:label "IIRA Connectivity"@en ;
    dul:associatedWith iira:LinkLayer,
        iira:NetworkLayer,
        iira:PhysicalLayer,
        iira:TansportLayer,
        sto:FrameworkLayer,
        sto:IIRC ;
    dul:isPartOf rami:Asset .

iira:NetworkLayer a owl:NamedIndividual,
        sto:ConnectivityLayer ;
    rdfs:label "IICF Network Layer"@en .

lang:en a owl:NamedIndividual .

lang:rus a owl:NamedIndividual .

dcterms:LicenseDocument a owl:Class ;
    rdfs:label "License Document"@en ;
    rdfs:comment "A legal document giving official permission to do something with a Resource."@en ;
    rdfs:isDefinedBy dcterms: .

<http://wikipedia.org/wiki/Internet_Engineering_Task_Force> a owl:NamedIndividual .

dul:isPartOf a owl:ObjectProperty .

xsd:date a rdfs:Datatype .

foaf:maker a owl:ObjectProperty .

rami:AdminShellGeneral a owl:NamedIndividual,
        rami:AdminShellSubmodel ;
    sto:isDescribedin sto:AdministrationShell .

rami:Assest a owl:NamedIndividual .

rami:LifecycleStatus a owl:NamedIndividual,
        rami:AdminShellSubmodel ;
    sto:isDescribedin sto:AdministrationShell .

sto:BBF a dbpcy:Abstraction100002137,
        dbpcy:Association108049401,
        dbpcy:Consortium108236438,
        dbpcy:Group100031264,
        dbpcy:Organization108008335,
        dbpcy:SocialGroup107950920,
        dbpcy:WikicatConsortia,
        dbpcy:YagoLegalActor,
        dbpcy:YagoLegalActorGeo,
        dbpcy:YagoPermanentlyLocatedEntity,
        dbont:Agent,
        dbont:Organisation,
        schema:Organization,
        dul:Agent,
        dul:SocialPerson,
        owl:NamedIndividual,
        owl:Thing,
        wike:Q24229398,
        wike:Q43229,
        sto:StandardOrganization ;
    rdfs:label "Broadband Forum"@en ;
    dcterms:subject dbrc:Broadband,
        dbrc:Digital_subscriber_line,
        dbrc:Digital_television,
        dbrc:Technology_consortia ;
    lingg:hypernym dbres:Consortium ;
    rdfs:comment "The Broadband Forum is a non-profit industry consortium dedicated to developing broadband network specifications. Members include telecommunications networking and service provider companies, broadband device and equipment vendors, consultants and independent testing labs (ITLs). Service provider members are primarily wire-line service providers (non-mobile) telephone companies."@en ;
    sto:abbreviation "BBF" ;
    sto:formationDate "2008-01-01"^^xsd:date ;
    sto:hasDBpediaResource dbres:Broadband_Forum ;
    sto:hasHeadquaterIn dbr:_California ;
    sto:hasOfficialResource <https://www.broadband-forum.org/> ;
    sto:hasWikipediaArticle <https://en.wikipedia.org/wiki/Broadband_Forum> ;
    sto:orgName "Broadband Forum"@en .

sto:BusinessCycleSCM a owl:Class ;
    rdfs:label "Business Cycle SCM"@en ;
    rdfs:comment "Suply Chain Management Business Cycle."@en ;
    rdfs:isDefinedBy "http://nvlpubs.nist.gov/nistpubs/ir/2016/NIST.IR.8107.pdf" ;
    rdfs:seeAlso "https://en.wikipedia.org/wiki/Supply_chain_management" ;
    rdfs:subClassOf sto:StandardClassification .

sto:ETSI_DECT a dbpcy:WikicatMobileTelecommunicationsStandards,
        dbont:Work,
        owl:NamedIndividual,
        owl:Thing,
        sto:Standard ;
    rdfs:label "ETSI DECT" ;
    dcterms:subject dbrc:Broadband,
        dbrc:Local_loop,
        dbrc:Mobile_telecommunications_standards,
        dbrc:Software-defined_radio ;
    lingg:hypernym dbres:Standard ;
    rdfs:comment "Digital Enhanced Cordless Telecommunications (DECT) is the ETSI standard for short-range cordless communications, which can be adapted for many applications and can be used over unlicensed frequency allocations world-wide."@en ;
    sto:hasDBpediaResource dbres:Digital_Enhanced_Cordless_Telecommunications ;
    sto:hasDeveloper sto:ETSI ;
    sto:hasOfficialResource <http://www.etsi.org/technologies-clusters/technologies/dect> ;
    sto:hasPublisher sto:ETSI ;
    sto:hasTag "Digital Enhanced Cordless Telecommunications"@en ;
    sto:hasWikipediaArticle <https://en.wikipedia.org/wiki/Digital_Enhanced_Cordless_Telecommunications> .

sto:EnterpriseLevel a owl:NamedIndividual,
        sto:ISA95Level ;
    rdfs:label "Enterprise Level"@en ;
    rdfs:comment "Describes the Enterprise level according to the ISA95 level classification."@en .

sto:ICS_17_020 a owl:NamedIndividual,
        sto:InternationalClassificationForStandards ;
    rdfs:label "ICS 17.020"@en ;
    dcterms:title "Metrology and measurement in general "@en ;
    rdfs:comment "This is ICS for “Metrology and measurement in general ”"@en .

sto:ICS_19_020 a owl:NamedIndividual,
        sto:InternationalClassificationForStandards ;
    rdfs:label "ICS 19.020"@en ;
    dcterms:title "Test conditions and procedures in general"@en ;
    rdfs:comment "This is ICS for “Test conditions and procedures in general"@en .

sto:ICS_31_240 a owl:NamedIndividual,
        sto:InternationalClassificationForStandards ;
    rdfs:label "ICS 31.240"@en ;
    dcterms:title "Mechanical structures for electronic equipment"@en ;
    rdfs:comment "This is ICS for  Mechanical structures for electronic equipment"@en .

sto:ICS_33_060_20 a owl:NamedIndividual,
        sto:InternationalClassificationForStandards ;
    rdfs:label "ICS 33.060.20"@en ;
    dcterms:title "Receiving and transmitting equipment"@en ;
    rdfs:comment "This is ICS for Receiving and transmitting equipment"@en .

sto:IEC_61499 a dbpcy:WikicatENStandards,
        dbpcy:WikicatIECStandards,
        owl:NamedIndividual,
        sto:Standard ;
    rdfs:label "IEC 61499"@en ;
    dcterms:subject dbrc:IEC_standards ;
    rdfs:comment "Function Blocks - Architecture Related Applications http://www.eclipse.org/4diac/ (sourceforge.net/projects/oooneida-fbench/) http://timeme.io/  not accepted by the Industry yet. http://www.holobloc.com/Proposed for IEC to overcome the restricctions of IEC 61131"@en ;
    sto:hasClassification rami:ControlDevice,
        rami:FieldDevice ;
    sto:hasDBpediaResource dbres:IEC_61499 ;
    sto:hasMotivation "Functional description, informational representation and communication mapping of application functionality. This standard describes how a distributed control application is composed of functional units (FB), which are executed in different context. It may help to describe how functions are distributed between different I40-Components and how the execution of the functions between the different I40-Components is controled."@en ;
    sto:hasOfficialResource <https://webstore.iec.ch/publication/5506> ;
    sto:hasPublicationDate "2012-11-07"^^xsd:date ;
    sto:hasPublisher sto:IEC ;
    sto:hasTag "FBs distributed systems"@en ;
    sto:hasWikipediaArticle <https://en.wikipedia.org/wiki/IEC_61499> ;
    sto:relatedTo sto:IEC_61131,
        sto:IEC_62541 .

sto:IEC_61804 a dbont:Language,
        owl:NamedIndividual,
        sto:Standard ;
    rdfs:label "IEC 61804"@en ;
    dcterms:subject dbrc:Automation ;
    lingg:hypernym dbres:Language ;
    rdfs:comment "Function blocks (FB) for process control - Overview of system aspects "@en ;
    sto:hasClassification rami:Configuration,
        rami:ControlDevice,
        rami:FieldDevice ;
    sto:hasDBpediaResource dbres:Device_Description_Language ;
    sto:hasOfficialResource <https://webstore.iec.ch/publication/5953> ;
    sto:hasPublisher sto:IEC ;
    sto:hasTag "EDDL"@en ;
    sto:hasWikipediaArticle <https://en.wikipedia.org/wiki/Device_Description_Language> ;
    sto:relatedTo sto:IEC_62453 .

sto:IEEE a owl:NamedIndividual,
        sto:StandardOrganization ;
    dcterms:description "IEEE and its members inspire a global community to innovate for a better tomorrow through highly cited publications, conferences, technology standards, and professional and educational activities. IEEE is the trusted “voice” for engineering, computing, and technology information around the globe."@en ;
    rdfs:seeAlso "https://www.ieee.org/"@en ;
    sto:abbreviation "IEEE"@en ;
    sto:hasWikipediaArticle <http://wikipedia.org/wiki/Institute_of_Electrical_and_Electronics_Engineers> ;
    sto:orgName "Institute of Electrical and Electronics Engineers"@en .

sto:IIRC a owl:NamedIndividual,
        sto:StandardizationFramework ;
    rdfs:label "IICF"@en ;
    rdfs:comment "Industrial Internet Connectivity Framework"@en ;
    rdfs:isDefinedBy "https://www.iiconsortium.org/IICF.htm"@en ;
    rdfs:seeAlso "https://www.iiconsortium.org/pdf/IIC_PUB_G5_V1.01_PB_20180228.pdf" .

sto:ISA-95 a dbpcy:WikicatANSIStandards,
        dbpcy:WikicatStandards,
        dbont:Work,
        owl:NamedIndividual,
        sto:Standard ;
    rdfs:label "ISA 95"@en ;
    dcterms:subject dbrc:ANSI_standards,
        dbrc:Manufacturing ;
    lingg:hypernym dbres:Standard ;
    rdfs:comment "ANSI/ISA-95, or ISA-95 as it is more commonly referred, is an international standard from the International Society of Automation for developing an automated interface between enterprise and control systems. This standard has been developed for global manufacturers. It was developed to be applied in all industries, and in all sorts of processes, like batch processes, continuous and repetitive processes.There are 5 parts of the ISA-95 standard.ISA-95 Models"@en ;
    sto:hasDBpediaResource <http://dbpedia.org/resource/ANSI/ISA-95> ;
    sto:hasDeveloper sto:ANSI,
        sto:ISA ;
    sto:hasOfficialResource <https://www.isa.org/isa95/> ;
    sto:hasPublisher sto:ANSI,
        sto:ISA ;
    sto:hasTag "Enterprise-Control System Integration"@en ;
    sto:hasWikipediaArticle <https://en.wikipedia.org/wiki/ANSI/ISA-95> .

sto:ISA95 a owl:NamedIndividual,
        sto:StandardizationFramework ;
    rdfs:label "ISA 95"@en ;
    rdfs:comment "Describes the ISA95 as a Standarization Initiative that classifies Standards"@en .

sto:ISO_13584 a dbpcy:WikicatISOStandards,
        dbont:Place,
        owl:NamedIndividual,
        sto:Standard ;
    rdfs:label "ISO 13584"@en ;
    dcterms:hasLicense "Private"@en ;
    dcterms:subject dbrc:ISO_standards ;
    lingg:hypernym dbres:Systems ;
    rdfs:comment "ISO 13584 is a series of International Standards for the computer-sensible representation and exchange of parts library data. The objective is to provide a mechanism capable of transferring parts library data, independent from any particular system. The nature of this description makes it suitable not only for the exchange of files containing parts libraries, but also as a basis for implementing and sharing databases of parts library data, and archiving"@en ;
    sto:hasClassification sto:ProductCatalogData ;
    sto:hasDBpediaResource dbres:ISO_13584 ;
    sto:hasMotivation "Standard data elements (properties) are used as elements in administration shell"@en ;
    sto:hasOfficialResource <https://webstore.iec.ch/publication/5380%0Ahttp://www.iso.org/iso/catalogue_detail.htm?csnumber=43423> ;
    sto:hasPublisher sto:ISO ;
    sto:hasTag "Industrial automation systems and integration"@en ;
    sto:hasWikipediaArticle <https://en.wikipedia.org/wiki/ISO_13584> ;
    sto:relatedTo sto:IEC_61360,
        sto:eClass .

sto:ISO_15926 a owl:NamedIndividual,
        sto:Standard ;
    rdfs:label "ISO 15926"@en ;
    rdfs:comment "Industrial automation systems and integration -- Integration of life-cycle data for process plants including oil and gas production facilities."@en ;
    sto:hasClassification rami:Configuration,
        rami:Engineering,
        rami:Integration,
        rami:Product,
        sto:ProductLifeCycleManagement ;
    sto:hasDomain sto:IndustrialAutomation ;
    sto:hasOfficialResource <https://www.iso.org/standard/29557.html> ;
    sto:hasPublicationDate "2003-12-01"^^xsd:date ;
    sto:hasPublisher sto:ISO ;
    sto:relatedTo sto:ISO_ASTM_52915 .

sto:ISO_ASTM_52915 a owl:NamedIndividual,
        sto:Standard ;
    rdfs:label "ISO ASTM 52915"@en ;
    rdfs:comment "ISO ASTM 52915:2016 provides the specification for the Additive Manufacturing File Format (AMF), an interchange format to address the current and future needs of additive manufacturing technology."@en ;
    sto:hasClassification rami:Asset,
        rami:Engineering,
        rami:Identification,
        rami:Product,
        sto:ProductionSystemEngineering ;
    sto:hasDomain sto:IndustrialAutomation ;
    sto:hasOfficialResource <https://www.iso.org/standard/60572.html> ;
    sto:hasPublicationDate "2016-02-01"^^xsd:date ;
    sto:hasPublisher sto:ISO ;
    sto:relatedTo sto:IEC_62541,
        sto:ISO_14306 .

sto:IndustrialProcessMeasurementControl a owl:NamedIndividual,
        sto:Domain ;
    rdfs:comment "Industrial process measurement and control"@en ;
    sto:domainName "Industrial process measurement and control"@en .

sto:Interoperability a owl:NamedIndividual,
        sto:ISO_42010_Concern ;
    rdfs:label "Interoperability"@en ;
    rdfs:comment "A systems ability to connect with other systems."@en .

sto:MTConnect_Institute a owl:NamedIndividual,
        sto:StandardOrganization ;
    rdfs:comment "MTConnect Institute is a collaborative effort to develop technical standards and specifications intended to foster greater interoperability between automation/control applications, field systems/devices, and business/office applications in the manufacturing industry (\"MTConnect Specifications\"), as well as schema, prototype software examples, and related documentation in order to facilitate the implementation of the MTConnect Specifications in compliant applications, drivers, and other services"@en ;
    sto:abbreviation "MTC" ;
    sto:formationDate "2006-01-01"^^xsd:date ;
    sto:hasOfficialResource <https://w3id.org/i40/www.mtconnect.org> ;
    sto:orgName "MTConnect Institute"@en .

sto:ProductCatalogData a owl:NamedIndividual,
        sto:ProductDevelopmentLifeCycle ;
    rdfs:label "Product Catalog Data"@en ;
    rdfs:comment "Product catalog data standards support the description of particular instances of products or parts in a uniform, vendor-neutral way."@en ;
    sto:isDescribedin sto:NISTInitiative .

sto:TC_103 a owl:NamedIndividual,
        sto:TechnicalCommittee ;
    rdfs:label "TC 103"@en ;
    dcterms:title "Transmitting equipment for radiocommunication"@en ;
    rdfs:comment """Standardization of transmitting equipment for radiocommunications purposes and electronic devices employing similar\r
techniques. The standardization work deals with methods of measurement, safety requirements and transmitter control and Interconnection"""@en .

sto:TC_3 a owl:NamedIndividual,
        sto:TechnicalCommittee ;
    rdfs:label "TC 3"@en ;
    dcterms:title "Information structures and elements, identification and marking principles, documentation and graphical symbols"@en ;
    rdfs:comment "To prepare standards for the electrotechnical and related fields regarding:1) methods and rules associated with the human interpretation of information. This refers to:- presentation of information in technical documentation,- graphical symbols for use in technical documentation,- graphical symbols for the human interaction with equipment,2) methods and rules associated with the handling of information in computer sensible form. This refers to:- information models for the purpose of technical documentation and the exchange of technical information, and the identification of further needs for such models,- definition of data element types and data sets for use in information models and technical documentation, and for exchange of technical information.It includes definition and co-ordination of the information required during the whole life cycle of a device, system, or plant.3) General and safety application concerning the man-machine interface, marking and identification in electrical installations and equipment, marking systems and general rules for:- the meanings of colours and alternative means, when used for marking and identification,- the arrangement of indicating devices and actuators,- coding principles for indicating and actuating devices,- terminal designation of electrical and electronic components, apparatus and equipment,- the termination designation of certain designated conductors,- marking of electrical and electronic equipment with ratings related to supply and to its properties,- marking of bare and insulated conductors.These standards are principally intended for use by technical committees in the preparation of standards in accordance with the principles laid down in IEC Guide 104: Guide to the drafting of Safety Standards, and the role of committees with Safety Pilot Functions and Safety Group Functions, and in ISO/IEC Guide 51: Guidelines for the inclusion of safety aspects in standards."@en .

sto:TC_8 a owl:NamedIndividual,
        sto:TechnicalCommittee ;
    rdfs:label "TC 8"@en ;
    dcterms:title "Systems aspects of electrical energy supply"@en ;
    rdfs:comment "To prepare and coordinate, in co-operation with other TC/SCs, the development of international standards and other deliverables with emphasis on overall system aspects of electricity supply systems and acceptable balance between cost and quality for the users of electrical energy. Electricity supply system encompasses transmission and distribution networks, generators and loads with their network interfaces."@en .

sto:TC_94 a owl:NamedIndividual,
        sto:TechnicalCommittee ;
    rdfs:label "TC 94"@en ;
    dcterms:title "All-or-nothing electrical relays"@en ;
    rdfs:comment """To prepare international standards applicable to all-or-nothing electrical relays used in the various fields of Electrical Engineering covered by the IEC, normally produced in very large\r
numbers as components of electromechanical or electronic\r
equipment and eventually submitted to Quality Assurance requirements based on sampling techniques."""@en .

sto:W3C_RDF a dbpcy:WikicatBibliographyFileFormats,
        dbpcy:WikicatComputerFileFormats,
        dbpcy:WikicatFilenameExtensions,
        dbpcy:WikicatMarkupLanguages,
        dbpcy:WikicatOpenFormats,
        dbpcy:WikicatWebStandards,
        dbpcy:WikicatWorldWideWebConsortiumStandards,
        dbpcy:WikicatXML-basedStandards,
        owl:NamedIndividual,
        owl:Thing,
        sto:Standard ;
    rdfs:label "Resource Description Framework"@en ;
    dcterms:hasLicense "Public"@en ;
    dcterms:subject dbrc:Bibliography_file_formats,
        dbrc:Knowledge_representation,
        dbrc:Metadata,
        dbrc:Resource_Description_Framework,
        dbrc:Semantic_Web,
        dbrc:World_Wide_Web_Consortium_standards,
        dbrc:XML,
        dbrc:XML-based_standards ;
    lingg:hypernym dbres:Family ;
    rdfs:comment "RDF is a standard model for data interchange on the Web. RDF has features that facilitate data merging even if the underlying schemas differ, and it specifically supports the evolution of schemas over time without requiring all the data consumers to be changed. "@en ;
    sto:hasDBpediaResource dbres:Resource_Description_Framework ;
    sto:hasOfficialResource <https://www.w3.org/RDF/> ;
    sto:hasPublisher sto:W3C ;
    sto:hasTag "RDF"@en ;
    sto:hasWikipediaArticle <https://en.wikipedia.org/wiki/Resource_Description_Framework> .

sto:_020 a owl:NamedIndividual .

sto:eClassAssoc a owl:NamedIndividual,
        sto:StandardOrganization ;
    rdfs:comment "Der eCl@ss e. V. ist eine Non-Profit-Organisation, die den gleichnamigen Klassifikationsstandard branchenübergreifend international definiert, weiterentwickelt und verbreitet. Der Verein wird getragen von ordentlichen und fördernden Mitgliedern aus Unternehmen, Verbänden und Institutionen."@de ;
    sto:abbreviation "eCl@ss",
        "eClass" ;
    sto:formationDate "2000-11-14"^^xsd:date ;
    sto:hasHeadquaterIn dbr:Cologne ;
    sto:hasOfficialResource <https://www.eclass.eu> ;
    sto:hasWikipediaArticle <https://www.wikiwand.com/de/ECl@ss> ;
    sto:orgName "eCl@ss e. V."@de .

idsram:Governance a <http://w3id.org/ids/ram/Perspective>,
        owl:NamedIndividual ;
    rdfs:label "IDS RAM Governance Perspective"@en ;
    sto:isDescribedin idsram:ReferenceArchitectureModel .

dbr:Geneva a owl:NamedIndividual .

iira:InformationDomain a iira:FunctionalDomain,
        owl:NamedIndividual ;
    rdfs:label "IIRA Information Domain"@en ;
    sto:alignesWith rami:Information ;
    sto:isDescribedin iira:IIRA .

iira:OperationDomain a iira:FunctionalDomain,
        owl:NamedIndividual ;
    rdfs:label "IIRA Operation Domain"@en ;
    sto:alignesWith rami:Functional ;
    sto:isDescribedin iira:IIRA .

<http://w3id.org/ids/ram/Perspective> a owl:Class ;
    rdfs:label "IDS RAM Perspective"@en ;
    rdfs:subClassOf sto:StandardClassification ;
    owl:equivalentClass [ a owl:Class ;
            owl:oneOf ( idsram:Certification idsram:Governance idsram:Security ) ] .

xsd:string a owl:NamedIndividual .

rami:Conditional_Monitoring a owl:NamedIndividual .

rami:GeneralAdminShell a owl:NamedIndividual .

rami:Identification a owl:NamedIndividual,
        rami:AdminShellSubmodel ;
    rdfs:label "RAMI Identification"@en ;
    sto:alignesWith sto:Identification ;
    sto:isDescribedin sto:AdministrationShell .

rami:Security a owl:NamedIndividual,
        rami:AdminShellSubmodel ;
    rdfs:label "RAMI Security"@en ;
    sto:isDescribedin sto:AdministrationShell .

sto:CrossLevel a owl:NamedIndividual,
        sto:ISA95Level ;
    rdfs:label "Cross Level"@en ;
    rdfs:comment "Describes the cross-level according to the ISA95 level classification. It means standards that are used at more than one level, e.g., manufacturing system security, etc"@en ;
    sto:isDescribedin sto:ISA95 .

sto:ICS_01_040_07 a owl:NamedIndividual,
        sto:InternationalClassificationForStandards ;
    rdfs:label "ICS 01.040.07"@en ;
    dcterms:title "Natural and applied sciences (Vocabularies)"@en ;
    rdfs:comment "This is ICS for Natural and applied sciences (Vocabularies)"@en .

sto:ICS_31_020 a owl:NamedIndividual,
        sto:InternationalClassificationForStandards ;
    rdfs:label "ICS 31.020"@en ;
    dcterms:title "Electronic components in general "@en ;
    rdfs:comment "This is ICS for Electronic components in general "@en .

sto:IEC_61158 a dbpcy:WikicatIECStandards,
        owl:NamedIndividual,
        sto:Standard ;
    rdfs:label "IEC 61158"@en ;
    dcterms:subject dbrc:Industrial_computing,
        dbrc:Production_and_manufacturing,
        dbrc:Serial_buses ;
    lingg:hypernym dbres:Family ;
    rdfs:comment "Fieldbus is the name of a family of industrial computer network protocols used for real-time distributed control, standardized as IEC 61158. A complex automated industrial system such as manufacturing assembly line usually needs a distributed control system an organized hierarchy of controller systems to function. In this hierarchy, there is usually a Human Machine Interface (HMI) at the top, where an operator can monitor or operate the system. This is typically linked to a middle layer of programmable logic controllers (PLC) via a non-time-critical communications system (e.g. Ethernet). At the bottom of the control chain is the fieldbus that links the PLCs to the components that actually do the work, such as sensors, actuators, electric motors, console lights, switches, valves and contactors"@en ;
    sto:hasDBpediaResource <http://dbpedia.org/page/Fieldbus> ;
    sto:hasOfficialResource <http://www.fieldbus.org/> ;
    sto:hasPublisher sto:IEC ;
    sto:hasTag "Fieldbus"@en ;
    sto:hasWikipediaArticle <https://en.wikipedia.org/wiki/Fieldbus> ;
    sto:relatedTo sto:IEC_61784 .

sto:IEC_61360 a owl:NamedIndividual,
        sto:Standard ;
    rdfs:label "IEC 61360"@en ;
    rdfs:comment "IEC Common Data Dictionary (IEC CDD) is a common repository of concepts for all electrotechnical domains based on the methodology and the information model of IEC 61360 series. Standard data elements types with associated classification scheme for electric items."@en ;
    sto:hasClassification rami:Asset,
        rami:Engineering,
        sto:ManufacturingModelData,
        idsram:InformationLayer ;
    sto:hasDomain "Electrotechnical"@en ;
    sto:hasMotivation "Standard data elements (properties) are used as elements in administration shell"@en ;
    sto:hasOfficialResource <http://cdd.iec.ch/cdd/iec61360/iec61360.nsf>,
        <https://webstore.iec.ch/publication/5380> ;
    sto:hasPublisher sto:IEC ;
    sto:hasTag "IEC Common Data Dictionary"@en ;
    sto:relatedTo sto:ISO_13584,
        sto:eClass .

sto:ISO_15531 a owl:NamedIndividual,
        sto:Standard ;
    rdfs:label "ISO 15531"@en ;
    rdfs:comment "This Standard models manufacturing management data such as, Resources management data (Resource model); Time related features (Time model); Flow management data in manufacturing (Flow management model)."@en ;
    rdfs:isDefinedBy "https://www.researchgate.net/publication/220171079_ISO_15531_MANDATE_a_standardised_data_model_for_manufacturing_management" ;
    sto:hasDomain sto:IndustrialProcessMeasurementControl ;
    sto:hasOfficialResource <https://www.iso.org/standard/28144.html> ;
    sto:hasPublisher sto:ISO ;
    sto:hasTag "MANDATE" .

sto:MESA a dbont:Settlement,
        owl:NamedIndividual,
        sto:StandardOrganization ;
    dcterms:subject dbrc:MES_software ;
    lingg:hypernym dbres:Community ;
    rdfs:comment "The Manufacturing Enterprise Solutions Association International is a global community of manufacturers, producers, industry leaders, and solution providers who are focused on driving business results from manufacturing information."@en ;
    sto:abbreviation "MESA" ;
    sto:formationDate "1992-01-01"^^xsd:date ;
    sto:hasDBpediaResource <http://dbpedia.org/page/Manufacturing_Enterprise_Solutions_Association> ;
    sto:hasHeadquaterIn dbr:_Arizona ;
    sto:hasOfficialResource <http://www.mesa.org/en/index.asp> ;
    sto:hasWikipediaArticle <https://en.wikipedia.org/wiki/Manufacturing_Enterprise_Solutions_Association> ;
    sto:orgName "Manufacturing Enterprise Solutions Association"@en .

sto:OASIS a dbpcy:Abstraction100002137,
        dbpcy:Group100031264,
        dbpcy:NongovernmentalOrganization108009834,
        dbpcy:Organization108008335,
        dbpcy:SocialGroup107950920,
        dbpcy:WikicatComputerScienceOrganizations,
        dbpcy:WikicatInformationTechnologyOrganisations,
        dbpcy:WikicatInternationalNongovernmentalOrganizations,
        dbpcy:WikicatStandardsOrganizations,
        dbpcy:WikicatXMLOrganizations,
        dbpcy:YagoLegalActor,
        dbpcy:YagoLegalActorGeo,
        dbpcy:YagoPermanentlyLocatedEntity,
        dbont:Agent,
        dbont:Non-ProfitOrganisation,
        dbont:Organisation,
        schema:Organization,
        dul:Agent,
        dul:SocialPerson,
        owl:NamedIndividual,
        owl:Thing,
        wike:Q163740,
        wike:Q24229398,
        wike:Q43229,
        sto:StandardOrganization ;
    dcterms:subject dbrc:Standards_organizations,
        dbrc:Web_services,
        dbrc:XML_organizations ;
    lingg:hypernym dbres:Consortium ;
    rdfs:comment "The Organization for the Advancement of Structured Information Standards (OASIS) is a global nonprofit consortium that works on the development, convergence, and adoption of standards for security, Internet of Things, energy, content technologies, emergency management, and other areas."@en ;
    sto:abbreviation "OASIS" ;
    sto:formationDate "1993-01-01"^^xsd:date ;
    sto:hasDBpediaResource <http://dbpedia.org/page/OASIS_(organization)> ;
    sto:hasHeadquaterIn dbr:Boston ;
    sto:hasOfficialResource <https://www.oasis-open.org/> ;
    sto:hasWikipediaArticle <https://en.wikipedia.org/wiki/OASIS_(organization)> ;
    sto:orgName "Organization for the Advancement of Structured Information Standards"@en .

sto:ProductModelDataExchange a owl:NamedIndividual,
        sto:ProductDevelopmentLifeCycle ;
    rdfs:label "Product Model Data Exchange"@en ;
    rdfs:comment "These standards capture the representation of product and engineering information to enable data exchange between CAD software from different vendors."@en ;
    sto:isDescribedin sto:NISTInitiative .

sto:ProductionSystemEngineering a owl:NamedIndividual,
        sto:ProductionSystemLifeCycle ;
    rdfs:label "Production System Engineering"@en ;
    rdfs:comment "Standards can interconnect engineering tools from different disciplines, e.g., system engineering, mechanical plant engineering, electrical design, process engineering, process control engineering, Human Machine Interface (HMI) development, PLC programming, and robotic programming."@en ;
    sto:isDescribedin sto:NISTInitiative .

sto:SCM a owl:NamedIndividual,
        sto:BusinessCycleSCM ;
    rdfs:label "Supply Chain Management"@en ;
    rdfs:comment "Describes Plan-Source-Make-Deliver-Return cycle for managing the manufacturing supply chain."@en ;
    sto:isDescribedin sto:NISTInitiative .

sto:TC_91 a owl:NamedIndividual,
        sto:TechnicalCommittee ;
    rdfs:label "TC 91"@en ;
    dcterms:title "Electronics assembly technology"@en ;
    rdfs:comment "To prepare international standards on design, manufacturing and testing of electronic assemblies including the requirements and tests for materials and components used to manufacture circuit boards and electronic assemblies, as well as the formats of electronic data and libraries for describing these products and processes."@en .

idsram:BusinessLayer a owl:NamedIndividual,
        idsram:Layer ;
    rdfs:label "IDS RAM Business Layer"@en ;
    sto:alignesWith iira:BusinessDomain,
        rami:Business ;
    sto:isDescribedin idsram:ReferenceArchitectureModel .

idsram:ProcessLayer a owl:NamedIndividual,
        idsram:Layer ;
    rdfs:label "IDS RAM Process Layer"@en ;
    sto:isDescribedin idsram:ReferenceArchitectureModel .

iira:CrosscuttingFunction a owl:Class ;
    rdfs:label "IIRA Crosscutting Function"@en ;
    rdfs:subClassOf [ a owl:Restriction ;
            owl:hasValue iira:FunctionalViewpoint ;
            owl:onProperty dul:isPartOf ],
        sto:StandardClassification .

iira:Safety a iira:SystemCharacteristics,
        owl:NamedIndividual ;
    rdfs:label "IIRA Safety"@en .

iira:Viewpoint a owl:Class ;
    rdfs:label "IIRA Viewpoint"@en ;
    rdfs:subClassOf sto:StandardClassification .

rami:ConnectedWorld a owl:NamedIndividual,
        rami:RAMIHierarchyLevel ;
    sto:isDescribedin sto:RAMI40 .

rami:RAMILifeCycleLayer a owl:Class ;
    rdfs:label "RAMI Life Cycle Layer"@en ;
    rdfs:seeAlso "http://www.zvei.org/en/subjects/Industry-40/Pages/The-Reference-Architectural-Model-RAMI-40-and-the-Industrie-40-Component.aspx" ;
    rdfs:subClassOf sto:StandardClassification ;
    skos:definition "It describes the different Life Cycle and Value Stream layers for the RAMI model according to the IEC 62890 Standard."@en ;
    skos:prefLabel "RAMI Life Cycle Layer"@en .

sto:ANSI a dbpcy:Abstraction100002137,
        dbpcy:Association108049401,
        dbpcy:Group100031264,
        dbpcy:Institute108407330,
        dbpcy:Organization108008335,
        dbpcy:SocialGroup107950920,
        dbpcy:WikicatInstitutes,
        dbpcy:WikicatOrganizations,
        dbpcy:WikicatOrganizationsBasedInTheUnitedStates,
        dbpcy:WikicatOrganizationsBasedInTheUnitedStatesByActivity,
        dbpcy:WikicatOrganizationsEstablishedIn1918,
        dbpcy:WikicatResearchInstitutesInTheUnitedStates,
        dbpcy:WikicatStandardsOrganizations,
        dbpcy:YagoLegalActor,
        dbpcy:YagoLegalActorGeo,
        dbpcy:YagoPermanentlyLocatedEntity,
        dbont:Agent,
        dbont:Organisation,
        schema:Organization,
        dul:Agent,
        dul:SocialPerson,
        owl:NamedIndividual,
        owl:Thing,
        wike:Q24229398,
        wike:Q43229,
        sto:StandardOrganization ;
    rdfs:label "ANSI"@en ;
    dcterms:subject <http://dbpedia.org/resource/Category:1918_establishments_in_the_United_States>,
        dbrc:ANSI_standards,
        <http://dbpedia.org/resource/Category:Charities_based_in_Washington,_D.C.>,
        dbrc:ISO_member_bodies,
        dbrc:Organizations_established_in_1918,
        dbrc:Standards_organizations,
        dbrc:Technical_specifications ;
    lingg:hypernym dbres:Organization ;
    rdfs:comment "The American National Standards Institute is a private non-profit organization that oversees the development of voluntary consensus standards for products, services, processes, systems, and personnel in the United States. The organization also coordinates U.S. standards with international standards so that American products can be used worldwide. ANSI accredits standards that are developed by representatives of other standards organizations, government agencies, consumer groups, companies, and others. These standards ensure that the characteristics and performance of products are consistent, that people use the same definitions and terms, and that products are tested the same way. ANSI also accredits organizations that carry out product or personnel certification in accordance with requirements defined in international standards."@en ;
    sto:abbreviation "ANSI" ;
    sto:formationDate "1918-05-14"^^xsd:date ;
    sto:hasDBpediaResource dbres:American_National_Standards_Institute ;
    sto:hasHeadquaterIn <http://dbpedia.org/resource#Washington,_D.C.> ;
    sto:hasOfficialResource <https://www.ansi.org/> ;
    sto:hasWikipediaArticle <https://en.wikipedia.org/wiki/American_National_Standards_Institute?oldformat=true>,
        "http://en.wikipedia.org/wiki/American_National_Standards_Institute" ;
    sto:orgName "American National Standards Institute"@en .

sto:BusinessProcessExecution a owl:NamedIndividual,
        sto:BusinessCycleSCM ;
    rdfs:label "Business Process Execution"@en ;
    rdfs:comment "Describes Business Process Execution concept."@en ;
    sto:isDescribedin sto:NISTInitiative .

sto:CAD a owl:NamedIndividual,
        owl:Thing,
        sto:Domain ;
    rdfs:label "CAD" ;
    dcterms:subject dbrc:Computer-aided_design,
        dbrc:Design_engineering,
        dbrc:Free_computer-aided_design_software ;
    lingg:hypernym dbres:Use ;
    rdfs:comment "Computer-Aided Design"@en ;
    rdfs:isDefinedBy <https://en.wikipedia.org/wiki/Computer-aided_design> ;
    sto:domainName "Computer-Aided Design"@en ;
    sto:hasDBpediaResource dbres:Computer-aided_design ;
    sto:hasWikipediaArticle "http://en.wikipedia.org/wiki/Computer-aided_design" .

sto:FrameworkLayer a owl:NamedIndividual,
        sto:ConnectivityLayer ;
    rdfs:label "IICF Framework Layer"@en ;
    dul:associatedWith sto:Interoperability ;
    rdfs:comment "Framework Layer"@en,
        "Framework Layer an instance of the Connectivity Layer"@en ;
    rdfs:isDefinedBy "https://www.iiconsortium.org/pdf/IIC_PUB_G5_V1.01_PB_20180228.pdf" ;
    sto:alignesWith idsram:Governance,
        idsram:SystemLayer .

sto:ICS_35_240_50 a owl:NamedIndividual,
        sto:InternationalClassificationForStandards ;
    rdfs:label "ICS 35.240.50"@en ;
    dcterms:title "IT applications in industry"@en ;
    rdfs:comment "This is ICS for IT applications in industry"@en,
        "This is ICS for “IT applications in industry)”"@en .

sto:Identification a owl:NamedIndividual,
        sto:ISO_42010_Concern ;
    rdfs:label "Identification"@en ;
    dc11:description "The concern how to identify a participant (client, endpoint etc.) in the internet."@en .

sto:M2M a dbpcy:Abstraction100002137,
        dbpcy:Buzzword106608277,
        dbpcy:Communication100033020,
        dbpcy:Group100031264,
        dbpcy:Message106598915,
        dbpcy:Network108434259,
        dbpcy:Nonsense106607339,
        dbpcy:System108435388,
        dbpcy:WikicatBuzzwords,
        dbpcy:WikicatNetworks,
        owl:NamedIndividual,
        sto:Domain ;
    rdfs:label "Machine to Machine"@en ;
    dcterms:subject dbrc:Buzzwords,
        dbrc:Machine_to_machine,
        <http://dbpedia.org/resource/Category:Service-oriented_(business_computing)> ;
    rdfs:comment "Machine to machine refers to direct communication between devices using any communications channel, including wired and wireless"@en ;
    sto:domainName "Machine to machine Communication"@en ;
    sto:hasDBpediaResource dbres:Machine_to_machine ;
    sto:hasWikipediaArticle <https://en.wikipedia.org/wiki/Machine_to_machine> .

sto:OMG a dbpcy:Abstraction100002137,
        dbpcy:Company108058098,
        dbpcy:Group100031264,
        dbpcy:Institution108053576,
        dbpcy:Organization108008335,
        dbpcy:SocialGroup107950920,
        dbpcy:WikicatComputerScienceOrganizations,
        dbpcy:WikicatInformationTechnologyOrganisations,
        dbpcy:WikicatSoftwareCompanies,
        dbpcy:WikicatStandardsOrganizations,
        dbpcy:YagoLegalActor,
        dbpcy:YagoLegalActorGeo,
        dbpcy:YagoPermanentlyLocatedEntity,
        dbont:Agent,
        dbont:Organisation,
        schema:Organization,
        dul:Agent,
        dul:SocialPerson,
        owl:NamedIndividual,
        owl:Thing,
        wike:Q24229398,
        wike:Q43229,
        sto:StandardOrganization ;
    dcterms:subject dbrc:Standards_organizations,
        dbrc:Unified_Modeling_Language ;
    lingg:hypernym dbres:Membership ;
    rdfs:comment "The Object Management Group (OMG) is an international, open membership, not-for-profit technology standards consortium. OMG Task Forces develop enterprise integration standards for a wide range of technologies and industries. OMG modeling standards enable visual design, execution and maintenance of software and other processes. Originally aimed at standardizing distributed object-oriented systems, the company now focuses on modeling (programs, systems and business processes) and model-based standards." ;
    sto:abbreviation "OMG" ;
    sto:formationDate "1989-01-01"^^xsd:date ;
    sto:hasDBpediaResource dbres:Object_Management_Group ;
    sto:hasHeadquaterIn dbr:_Massachusetts ;
    sto:hasOfficialResource <http://www.omg.org/> ;
    sto:hasWikipediaArticle <https://en.wikipedia.org/wiki/Object_Management_Group> ;
    sto:orgName "Object Management Group"@en .

sto:ProductLifeCycleManagement a owl:NamedIndividual,
        sto:ProductDevelopmentLifeCycle ;
    rdfs:label "Production Life Cycle Management"@en ;
    rdfs:comment "Product lifecycle data management focuses on the needs of long-term retention and access to data consistently throughout the product lifecycle."@en ;
    sto:isDescribedin sto:NISTInitiative .

sto:ProductionSystemLifeCycle a owl:Class ;
    rdfs:label "Production System Life Cycle"@en ;
    rdfs:comment "Collections of machines, equipment, and auxiliary systems organized to create goods and services from various resources."@en ;
    rdfs:isDefinedBy "http://nvlpubs.nist.gov/nistpubs/ir/2016/NIST.IR.8107.pdf" ;
    rdfs:subClassOf sto:StandardClassification .

sto:StandardPart a owl:Class ;
    rdfs:label "StandardPart" ;
    rdfs:comment "Typically Standards are divided into parts. E.g., ISA 95 has part Part 1: Models and Terminology, Part 2: Object Model Attributes, etc."@en ;
    rdfs:subClassOf foaf:Document .

sto:TC_1 a owl:NamedIndividual,
        sto:TechnicalCommittee ;
    rdfs:label "TC 1"@en ;
    dcterms:title "Terminology" ;
    rdfs:comment "To sanction the terms and definitions used in the different electrotechnical fields and to determine the equivalence of the terms used in the different languages. As a consequence, to prepare an International Electrotechnical Vocabulary aiming at the standardization and coordination of the terms relating to electrical sciences and techniques for use in the technical language and literature, in teaching, in technical specifications and in commercial exchanges, and at giving their equivalents in the different languages."@en .

sto:TC_40 a owl:NamedIndividual,
        sto:TechnicalCommittee ;
    rdfs:label "TC 40"@en ;
    dcterms:title "Capacitors and resistors for electronic equipment"@en ;
    rdfs:comment "To prepare international standards for:a) Capacitors, resistors, thermistors and varistors intended for use in electronic equipment.b) Capacitors, resistors and inductors and complete electromagnetic interference (EMI) suppression filter units for EMI suppression (see note).c) Passive integrated circuits or networks containing resistors, capacitors, inductors or their combinations. For the dimensional standardization of the final package, requirements laid down by TC 47 shall be adopted whenever possible.d) Packaging of electronic components for automatic handling, which is an activity undertaken on behalf of all relevant component technical committees.e) Electric double layer capacitors for use in electric and electronic equipment.Note: In this work, use has to be made as far as possible of any relevant work of TC 51 on inductors, the CISPR on the measurement of EMI suppression characteristics and TC 77 on electromagnetic compatibility (EMC). Liaison has also to be maintained with TC 61, TC 66, TC 108 and other appropriate IEC Technical Committees on the safety aspects of EMI suppression components and filter units."@en .

sto:TC_44 a owl:NamedIndividual,
        sto:TechnicalCommittee ;
    rdfs:label "TC 44"@en ;
    dcterms:title "Safety of machinery - Electrotechnical aspects"@en ;
    rdfs:comment "Standardization in the field of the application of electro-technical equipment and systems to machinery (including a group of machines working together in a coordinated manner, excluding higher-level systems aspects) not portable by hand while working, but which may include mobile equipment. The equipment covered commences at the point of connection of the electrical supply to the machinery.Standardization of interfaces (excluding local area networks and fieldbus) between control equipment and the electro-technical equipment of machinery.Standardization of electrotechnical equipment and systems relating to the safeguarding of persons from hazards of the machinery, its associated equipment and the environment.To coordinate with ISO all matters concerning the safety of machinery.."@en .

sto:eClass a owl:NamedIndividual,
        sto:Standard ;
    rdfs:label "eClass"@en ;
    rdfs:comment "eCl@ss is the cross-industry product data standard for classification and clear description of products and services."@en ;
    sto:hasClassification rami:ConnectedWorld,
        rami:ControlDevice,
        rami:Engineering,
        rami:Enterprise,
        rami:Product,
        rami:Station,
        rami:WorkCenter ;
    sto:hasDBpediaResource <http://de.dbpedia.org/page/ECl@ss> ;
    sto:hasDeveloper sto:eClassAssoc ;
    sto:hasMotivation "Global identification, semantic description and automatic product classification"@en ;
    sto:hasOfficialResource <https://www.eclass.eu/eclasscontent/standard/overview.html.en> ;
    sto:hasPublisher sto:eClassAssoc ;
    sto:hasTag "eClass"@en ;
    sto:hasWikipediaArticle <https://de.wikipedia.org/wiki/ECl@ss> ;
    sto:relatedTo sto:IEC_61360,
        sto:ISO_13584 .

iira:FunctionalDomain a owl:Class ;
    rdfs:label "IIRA Functional Domain"@en ;
    rdfs:subClassOf [ a owl:Restriction ;
            owl:hasValue iira:IIRA ;
            owl:onProperty sto:isDescribedin ],
        sto:StandardClassification .

rami:Configuration a owl:NamedIndividual .

sto:ConnectivityLayer a owl:Class ;
    rdfs:label "Connectivity Layer"@en ;
    rdfs:comment "Connectivity Layer of the Internet Connectivity Framework"@en ;
    rdfs:isDefinedBy "https://www.iiconsortium.org/pdf/IIC_PUB_G5_V1.01_PB_20180228.pdf" ;
    rdfs:subClassOf sto:StandardClassification .

sto:DataSovereignty a owl:NamedIndividual .

sto:ICS_13_110 a owl:NamedIndividual,
        sto:InternationalClassificationForStandards ;
    rdfs:label "ICS 13.110"@en ;
    dcterms:title "Safety of machinery"@en ;
    rdfs:comment "This is ICS for Safety of machinery "@en .

sto:ISA a dbpcy:Abstraction100002137,
        dbpcy:Association108049401,
        dbpcy:Group100031264,
        dbpcy:NongovernmentalOrganization108009834,
        dbpcy:Organization108008335,
        dbpcy:ProfessionalAssociation108242675,
        dbpcy:SocialGroup107950920,
        dbpcy:WikicatInternationalNon-profitOrganizations,
        dbpcy:WikicatInternationalNongovernmentalOrganizations,
        dbpcy:WikicatProfessionalAssociations,
        dbpcy:WikicatStandardsOrganizations,
        dbpcy:YagoLegalActor,
        dbpcy:YagoLegalActorGeo,
        dbpcy:YagoPermanentlyLocatedEntity,
        dbont:Organisation,
        owl:NamedIndividual,
        sto:StandardOrganization ;
    dcterms:subject dbrc:Engineering_organizations,
        dbrc:International_organizations_based_in_the_United_States,
        dbrc:Organizations_based_in_North_Carolina,
        dbrc:Standards_organizations ;
    lingg:hypernym dbres:Society ;
    rdfs:comment "The International Society of Automation (www.isa.org) is a nonprofit professional association that sets the standard for those who apply engineering and technology to improve the management, safety, and cybersecurity of modern automation and control systems used across industry and critical infrastructure. Founded in 1945, ISA develops widely used global standards; certifies industry professionals; provides education and training; publishes books and technical articles; hosts conferences and exhibits; and provides networking and career development programs for its 40,000 members and 400,000 customers around the world."@en ;
    sto:abbreviation "ISA" ;
    sto:formationDate "1945-04-28"^^xsd:date ;
    sto:hasDBpediaResource dbres:International_Society_of_Automation ;
    sto:hasHeadquaterIn dbr:_North_Carolina ;
    sto:hasOfficialResource <https://www.isa.org/> ;
    sto:hasWikipediaArticle <https://en.wikipedia.org/wiki/International_Society_of_Automation> ;
    sto:orgName "International Society of Automation"@en .

sto:ProductDevelopmentLifeCycle a owl:Class ;
    rdfs:label "Product Development Life Cycle"@en ;
    rdfs:comment "PLM is the process of managing the entire lifecycle of a product from inception, through engineering design and manufacture, to service and disposal of manufactured products. Related areas are PLMManagement, Modeling Practice, Product Model Data exchange, Manufacturing Model Data, Product Catalog Data."@en,
        "Product Development Life-Cycle Phase"@en ;
    rdfs:isDefinedBy "https://en.wikipedia.org/wiki/Product_lifecycle" ;
    rdfs:subClassOf sto:StandardClassification .

sto:TC_95 a owl:NamedIndividual,
        sto:TechnicalCommittee ;
    rdfs:label "TC 95"@en ;
    dcterms:title "Measuring relays and protection equipment"@en ;
    rdfs:comment "Standardisation of measuring relays and protection equipment used in various fields of electrical engineering covered by IEC, taking into a ccount combinations of devices to form schemes for power system protection including the control, monitoring and process interface equipment used with those systems.Excluded are the following:All devices covered by standards prepared by other IEC Technical Committees, for example instrument transformers (TC 38)."@en .

idsram:InformationLayer a owl:NamedIndividual,
        idsram:Layer ;
    rdfs:label "IDS RAM Information Layer"@en ;
    sto:isDescribedin idsram:ReferenceArchitectureModel .

idsram:Layer a owl:Class ;
    rdfs:label "IDS RAM Layer"@en ;
    rdfs:subClassOf sto:StandardClassification ;
    owl:equivalentClass [ a owl:Class ;
            owl:oneOf ( idsram:BusinessLayer idsram:FunctionalLayer idsram:InformationLayer idsram:ProcessLayer idsram:SystemLayer ) ] .

iira:FunctionalViewpoint a iira:Viewpoint,
        owl:NamedIndividual ;
    rdfs:label "IIRA Functional Viewpoint"@en ;
    sto:alignesWith idsram:ReferenceArchitectureModel ;
    sto:isDescribedin iira:IIRA .

iira:Privacy a iira:SystemCharacteristics,
        owl:NamedIndividual ;
    rdfs:label "IIRA Privacy"@en .

iira:SystemCharacteristics a owl:Class ;
    rdfs:label "IIRA System Characteristic"@en ;
    rdfs:subClassOf [ a owl:Restriction ;
            owl:hasValue iira:FunctionalViewpoint ;
            owl:onProperty dul:isPartOf ],
        sto:StandardClassification .

foaf:Document a owl:Class .

rami:Functional a owl:NamedIndividual,
        rami:RAMIITLayer ;
    rdfs:label "RAMI Functional Layer"@en ;
    sto:alignesWith iira:OperationDomain,
        idsram:ProcessLayer ;
    sto:isDescribedin sto:RAMI40 .

rami:RAMIITLayer a owl:Class ;
    rdfs:label "RAMI IT Layer"@en ;
    rdfs:subClassOf sto:StandardClassification ;
    owl:equivalentClass [ a owl:Class ;
            owl:oneOf ( rami:Asset rami:Business rami:Communication rami:Functional rami:Information rami:Integration ) ] .

sto:ETSI a dbpcy:Abstraction100002137,
        dbpcy:Group100031264,
        dbpcy:Organization108008335,
        dbpcy:SocialGroup107950920,
        dbpcy:WikicatOrganizationsEstablishedIn1988,
        dbpcy:WikicatStandardsOrganizations,
        dbpcy:WikicatTelecommunicationsOrganizations,
        dbpcy:YagoLegalActor,
        dbpcy:YagoLegalActorGeo,
        dbpcy:YagoPermanentlyLocatedEntity,
        dbont:Organisation,
        owl:NamedIndividual,
        owl:Thing,
        sto:StandardOrganization ;
    rdfs:label "ETSI"@en ;
    dcterms:subject dbrc:Organizations_established_in_1988,
        dbrc:Standards_organizations,
        dbrc:Telecommunications_in_Europe,
        dbrc:Telecommunications_organizations ;
    lingg:hypernym dbres:Organization ;
    rdfs:comment "The European Telecommunications Standards Institute (ETSI) is an independent, not-for-profit, standardization organization in the telecommunications industry (equipment makers and network operators) in Europe, headquartered in Sophia-Antipolis, France, with worldwide projection. ETSI produces globally-applicable standards for Information and Communications Technologies (ICT), including fixed, mobile, radio, converged, broadcast and internet technologies."@en ;
    sto:abbreviation "ETSI"@en ;
    sto:formationDate "1988-01-01"^^xsd:date ;
    sto:hasDBpediaResource dbres:ETSI ;
    sto:hasHeadquaterIn dbr:Valbonne ;
    sto:hasOfficialResource <http://www.etsi.org/> ;
    sto:hasWikipediaArticle <https://en.wikipedia.org/wiki/ETSI> ;
    sto:orgName "European Telecommunications Standards Institute"@en .

sto:ICS_27_180 a owl:NamedIndividual,
        sto:InternationalClassificationForStandards ;
    rdfs:label "ICS 27.180"@en ;
    dcterms:title "Wind turbine energy systems"@en ;
    rdfs:comment "This is ICS for “Wind turbine energy systems”"@en .

sto:ICS_29_020 a owl:NamedIndividual,
        sto:InternationalClassificationForStandards ;
    rdfs:label "ICS 29.020"@en ;
    dcterms:title "Electrical engineering in general "@en ;
    rdfs:comment "This is ICS for Electrical engineering in general"@en .

sto:IEC_62714 a dbpcy:WikicatComputerFileFormats,
        dbpcy:WikicatIndustry-specificXML-basedStandards,
        dbpcy:WikicatMarkupLanguages,
        dbpcy:WikicatXML-basedStandards,
        dbont:Software,
        owl:NamedIndividual,
        sto:Standard ;
    rdfs:label "IEC 62714"@en ;
    dcterms:hasLicense "Open"@en ;
    dcterms:subject dbrc:Computer_file_formats,
        dbrc:Industry-specific_XML-based_standards,
        dbrc:XML_markup_languages ;
    lingg:hypernym dbres:Format ;
    rdfs:comment "Engineering data exchange format for use in industrial automation systems engineering - Automation markup language - Architecture and general requirements"@en ;
    sto:hasClassification rami:ControlDevice,
        rami:Engineering,
        rami:FieldDevice,
        rami:Information,
        rami:Product,
        sto:ProductionSystemEngineering ;
    sto:hasDBpediaResource dbres:AutomationML ;
    sto:hasOfficialResource <https://www.automationml.org/> ;
    sto:hasPublisher sto:IEC ;
    sto:hasTag "AML"@en,
        "AutomationML"@en ;
    sto:hasWikipediaArticle <https://en.wikipedia.org/wiki/AutomationML> ;
    sto:relatedTo sto:IEC_61360,
        sto:IEC_61987_X,
        sto:IEC_62541,
        sto:eClass ;
    sto:uses sto:MathML .

sto:ISO_42010_Concern a owl:Class ;
    rdfs:label "Concern" .

sto:ITSecurity a owl:NamedIndividual,
        sto:Domain ;
    rdfs:label "IT Security"@en ;
    skos:altLabel "Information Security Management"@en .

sto:ModelingPractice a owl:NamedIndividual,
        sto:ProductDevelopmentLifeCycle ;
    rdfs:label "Modeling Practice"@en ;
    rdfs:comment "Modeling practice standards define digital product-definition data practices for both two-dimensional (2D) drawings and three-dimensional (3D) models."@en ;
    sto:isDescribedin sto:NISTInitiative .

sto:NIST a dbont:Agent,
        dbont:GovernmentAgency,
        dbont:Organisation,
        schema:Organization,
        dul:Agent,
        dul:SocialPerson,
        owl:NamedIndividual,
        owl:Thing,
        wike:Q24229398,
        wike:Q327333,
        wike:Q43229,
        sto:StandardOrganization ;
    dcterms:subject <http://dbpedia.org/resource/Category:1901_establishments_in_the_United_States>,
        <http://dbpedia.org/resource/Category:Buildings_and_structures_in_Gaithersburg,_Maryland>,
        dbrc:Cryptography_organizations,
        dbrc:Government_agencies_established_in_1901,
        dbrc:National_Institute_of_Standards_and_Technology,
        dbrc:Standards_organizations,
        dbrc:United_States_Department_of_Commerce_agencies ;
    lingg:hypernym dbres:Laboratory ;
    rdfs:comment "The National Institute of Standards and Technology (NIST) is a measurement standards laboratory, and a non-regulatory agency of the United States Department of Commerce."@en ;
    sto:abbreviation "NIST" ;
    sto:belongsTo dbr:United_States ;
    sto:formationDate "1901-01-01"^^xsd:date ;
    sto:hasDBpediaResource <http://dbpedia.org/page/National_Institute_of_Standards_and_Technology> ;
    sto:hasHeadquaterIn dbr:_Maryland ;
    sto:hasOfficialResource <https://www.nist.gov/> ;
    sto:hasWikipediaArticle <https://en.wikipedia.org/wiki/National_Institute_of_Standards_and_Technology> ;
    sto:orgName "National Institute of Standards and Technology"@en .

sto:ProductionSystemModelData a owl:NamedIndividual,
        sto:ProductionSystemLifeCycle ;
    rdfs:label "Production System Model Data"@en ;
    rdfs:comment "Provide information models for factory and production system design. They enhance information exchange among stakeholders, and enable virtual commissioning, which can improve manufacturing agility and reduce manufacturing cost."@en ;
    sto:isDescribedin sto:NISTInitiative .

sto:TC_88 a owl:NamedIndividual,
        sto:TechnicalCommittee ;
    rdfs:label "TC 88"@en ;
    dcterms:title "Wind energy generation systems"@en ;
    rdfs:comment """TC 88 standardization in the field of wind energy generation systems including wind turbines, wind power plants onshore and offshore and interaction with the electrical system(s) to which energy is supplied.\r
\r
These standards address site suitability and resource assessment, design\r
requirements, engineering integrity, modeling requirements, measurement techniques, test procedures, operation and maintenance. Their purpose is to provide a basis for design, quality assurance and technical aspects for certification. The standards address site-specific conditions, all systems and subsystems of wind turbines and wind power plants, such as mechanical, and electrical systems, support structures, control and protection as well as communication systems for monitoring, centralized and distributed control and evaluation, implementation of grid connection requirements for wind power plants, and environmental aspects of wind power development. The TC 88 standards will be developed based on and in agreement with appropriate IEC/ISO standards."""@en .

sto:W3C a dbpcy:Abstraction100002137,
        dbpcy:Association108049401,
        dbpcy:Consortium108236438,
        dbpcy:Group100031264,
        dbpcy:NongovernmentalOrganization108009834,
        dbpcy:Organization108008335,
        dbpcy:SocialGroup107950920,
        dbpcy:WikicatConsortia,
        dbpcy:WikicatInternationalNongovernmentalOrganizations,
        dbpcy:WikicatOrganizations,
        dbpcy:WikicatOrganizationsEstablishedIn1994,
        dbpcy:WikicatStandardsOrganizations,
        dbpcy:YagoLegalActor,
        dbpcy:YagoLegalActorGeo,
        dbpcy:YagoPermanentlyLocatedEntity,
        dbont:Agent,
        dbont:Organisation,
        schema:Organization,
        <http://umbel.org/umbel/rc/Organization>,
        dul:Agent,
        dul:SocialPerson,
        owl:NamedIndividual,
        owl:Thing,
        wike:Q24229398,
        wike:Q43229,
        sto:StandardOrganization ;
    rdfs:label "W3C"@en ;
    dcterms:subject dbrc:Organizations_established_in_1994,
        dbrc:Standards_organizations,
        dbrc:Technology_consortia,
        dbrc:Web_development,
        dbrc:Web_services,
        dbrc:World_Wide_Web_Consortium ;
    lingg:hypernym dbres:Organization ;
    rdfs:comment "The World Wide Web Consortium (W3C) is the main international standards organization for the World Wide Web (abbreviated WWW or W3). Founded and currently led by Tim Berners-Lee, the consortium is made up of member organizations which maintain full-time staff for the purpose of working together in the development of standards for the World Wide Web. As of 4 November 2015, the World Wide Web Consortium (W3C) has 408 members. The W3C also engages in education and outreach, develops software and serves as an open forum for discussion about the Web."@en ;
    sto:abbreviation "W3C" ;
    sto:formationDate "1994-10-01"^^xsd:date ;
    sto:hasDBpediaResource dbres:World_Wide_Web_Consortium ;
    sto:hasHeadquaterIn dbr:_Massachusetts ;
    sto:hasOfficialResource <https://www.w3.org/> ;
    sto:hasWikipediaArticle <https://en.wikipedia.org/wiki/World_Wide_Web_Consortium> ;
    sto:orgName "World Wide Web Consortium"@en .

sto:relatedTo a owl:ObjectProperty,
        owl:SymmetricProperty,
        owl:TransitiveProperty ;
    rdfs:label "related To"@en ;
    rdfs:comment "Represent any type of relation that connects two standards."@en ;
    rdfs:domain sto:Standard ;
    rdfs:range sto:Standard ;
    skos:altLabel "has Associated Standard"@en .

iira:TansportLayer a owl:NamedIndividual,
        sto:ConnectivityLayer ;
    rdfs:label "IICF Transport Layer"@en .

rami:Business a owl:NamedIndividual,
        rami:RAMIITLayer ;
    rdfs:label "RAMI Business Layer"@en ;
    sto:alignesWith iira:BusinessDomain,
        idsram:BusinessLayer ;
    sto:isDescribedin sto:RAMI40 .

rami:Information a owl:NamedIndividual,
        rami:RAMIITLayer ;
    rdfs:label "RAMI Information Layer"@en ;
    sto:alignesWith iira:InformationDomain,
        idsram:InformationLayer ;
    sto:isDescribedin sto:RAMI40 .

rami:RAMIHierarchyLevel a owl:Class ;
    rdfs:label "RAMI Hierarchy Level"@en ;
    rdfs:subClassOf sto:StandardClassification ;
    owl:equivalentClass [ a owl:Class ;
            owl:oneOf ( rami:ConnectedWorld rami:ControlDevice rami:Enterprise rami:FieldDevice rami:Product rami:Station rami:WorkCenter ) ] .

rami:Safety a owl:NamedIndividual,
        rami:AdminShellSubmodel ;
    rdfs:label "RAMI Safety"@en ;
    sto:isDescribedin sto:AdministrationShell .

sto:ICS_13_320 a owl:NamedIndividual,
        sto:InternationalClassificationForStandards ;
    rdfs:label "ICS 13.320"@en ;
    dcterms:title "Alarm and warning systems"@en ;
    rdfs:comment "This is ICS for Alarm and warning systems"@en .

sto:ICS_25_040_40 a owl:NamedIndividual,
        sto:InternationalClassificationForStandards ;
    rdfs:label "ICS 25.040.40"@en ;
    dcterms:title "Industrial process measurement and control"@en ;
    rdfs:comment "This is ICS for industrial process measurement and control"@en .

sto:ICS_29_120_70 a owl:NamedIndividual,
        sto:InternationalClassificationForStandards ;
    rdfs:label "ICS 29.120.70"@en ;
    dcterms:title "Relays"@en ;
    rdfs:comment "This is ICS for Relays"@en,
        "This is ICS for “Relays”"@en .

sto:IEC_62541 a dbpcy:WikicatComputerStandards,
        dbpcy:WikicatNetworkProtocols,
        dbont:Software,
        owl:NamedIndividual,
        sto:Standard ;
    rdfs:label "IEC 62541"@en ;
    dcterms:hasLicense sto:GPLv2,
        "Open"@en ;
    dcterms:subject dbrc:Application_programming_interfaces,
        dbrc:Automation,
        dbrc:Computer_standards ;
    lingg:hypernym dbres:Protocol ;
    rdfs:comment "OPC Unified Architecture (OPC UA) is an industrial M2M communication protocol for interoperability developed by the OPC Foundation. It is the successor to Open Platform Communications (OPC). Although developed by the same organization, OPC UA differs significantly from its predecessor. The Foundation's goal for this project was to provide a path forward from the original OPC communications model (namely the Microsoft Windows only process exchange COM/DCOM) to a cross-platform service-oriented architecture (SOA) for process control, while enhancing security and providing an information model."@en ;
    sto:hasClassification iira:ApplicationDomain,
        iira:InformationDomain,
        iira:OperationDomain,
        rami:Communication,
        rami:ConnectedWorld,
        rami:ControlDevice,
        rami:Enterprise,
        rami:FieldDevice,
        rami:Station,
        rami:WorkCenter,
        sto:Communication,
        sto:FrameworkLayer,
        sto:SCADALevel,
        idsram:DataSovereignty,
        idsram:SystemLayer ;
    sto:hasDBpediaResource dbres:OPC_Unified_Architecture ;
    sto:hasDeveloper sto:OPC_Foundation ;
    sto:hasDomain sto:IndustrialAutomation ;
    sto:hasOfficialResource <https://opcfoundation.org/about/opc-technologies/opc-ua/> ;
    sto:hasPublisher sto:IEC ;
    sto:hasTag "OPC UA"@en ;
    sto:hasWikipediaArticle <https://en.wikipedia.org/wiki/OPC_Unified_Architecture> ;
    sto:relatedTo sto:IEC_61499,
        sto:IEC_61850,
        sto:IEC_62714 ;
    sto:useStructureOf sto:IEC_61804 .

sto:ISA95Level a owl:Class ;
    rdfs:label "ISA 95 Level"@en ;
    rdfs:comment "Describes the ISA95 levels to classify the industry Standards according to those levels. Eg., Device, SCADA, etc. It has strong relation to the RAMI Hierarchy levels"@en ;
    rdfs:subClassOf sto:StandardClassification .

sto:TC_79 a owl:NamedIndividual,
        sto:TechnicalCommittee ;
    rdfs:label "TC 79"@en ;
    dcterms:title "Alarm and electronic security systems"@en ;
    rdfs:comment "To prepare international standards for the protection of buildings, persons, areas and properties against fraudulent actions having the purpose to enter in a place or to take or to use something without permission and other threat related to persons.The scope includes, but is not limited to equipment and systems, either used by ordinary persons or by trained people in the following residential and non residential applications:- Access control systems- Alarm transmission systems- Video surveillance systems- Combined and/or integrated systems even including fire alarm systems*- Fire detection and fire alarm systems*- Intruder and hold-up alarm systems- Remote receiving and/or surveillance centres- Social alarm systems.These systems can be used for providing a local or remote alarm; they can be used for calling private guards, social assistance, fire brigade or police force. They can be used for recording and transmission of dated or undated information, sounds, pictures of places and people for surveillance purposes. The standards cover:- terminology;- technical characteristics regarding performance criteria, reliable operation, installation, maintenance;- testing for detection, monitoring, recording, triggering an alarm and transmission to a remote centre including procedures and protocols for communication.Electrical safety, environmental conditions and behaviour of alarm systems regarding electromagnetic compatibility are also considered with reference to the appropriate standards (e.g. Guide ISO/IEC 51).* ISO/TC21/SC3 is in charge of the production of standards for \"Fire detection and alarm systems\"."@en .

rami:Integration a owl:NamedIndividual,
        rami:RAMIITLayer ;
    rdfs:label "RAMI Integration Layer"@en ;
    sto:alignesWith iira:ControlDomain,
        idsram:SystemLayer ;
    sto:isDescribedin sto:RAMI40 .

sto:Domain a owl:Class ;
    rdfs:label "Domain"@en ;
    rdfs:comment "Represents the Domains in which the Standards can be used"@en .

sto:TC_65 a owl:NamedIndividual,
        sto:TechnicalCommittee ;
    rdfs:label "TC 65"@en ;
    dcterms:title "Industrial-process measurement, control and automation"@en ;
    rdfs:comment "To prepare international standards for systems and elements used for industrial-process measurement and control concerning continuous and batch processes."@en .

sto:irlan a owl:NamedIndividual,
        foaf:Person ;
    rdfs:label "Irlan Grangel" ;
    foaf:familyName "Grangel" ;
    foaf:mbox "irlangrangel2003@gmail.com" ;
    foaf:name "Irlan" .

rami:Communication a owl:NamedIndividual,
        rami:RAMIITLayer ;
    rdfs:label "RAMI Communication Layer"@en ;
    sto:alignesWith idsram:SystemLayer ;
    sto:isDescribedin sto:RAMI40 .

sto:DIN a owl:NamedIndividual,
        sto:StandardOrganization ;
    rdfs:label "Deutsches Institut für Normung"@de,
        "DIN"@en,
        "German Institute for Standardization"@en ;
    rdfs:comment "Deutsches Institut für Normung e.V. (DIN; in English, the German Institute for Standardization) is the German national organization for standardization and is the German ISO member body. DIN is a German Registered Association (e.V.) headquartered in Berlin. There are currently around thirty thousand DIN Standards, covering nearly every field of technology"@en ;
    sto:abbreviation "DIN"@de ;
    sto:belongsTo dbr:Germany ;
    sto:formationDate "1918-01-01"^^xsd:date ;
    sto:hasDBpediaResource <http://dbpedia.org/page/Deutsches_Institut_f%C3%BCr_Normung> ;
    sto:hasHeadquaterIn dbr:Berlin ;
    sto:hasOfficialResource <http://www.din.de/en/about-standards/din-standards> ;
    sto:hasWikipediaArticle <https://en.wikipedia.org/wiki/Deutsches_Institut_f%C3%BCr_Normung> ;
    sto:orgName "Deutsches Institut für Normung"@en .

idsram:SystemLayer a owl:NamedIndividual,
        idsram:Layer ;
    rdfs:label "IDS RAM System Layer"@en ;
    sto:isDescribedin idsram:ReferenceArchitectureModel .

iira:IIRA a owl:NamedIndividual,
        sto:StandardizationFramework ;
    rdfs:label "IIRA"@en ;
    rdfs:comment "Industrial Internet Reference Architecture"@en ;
    sto:hasOfficialResource <http://www.iiconsortium.org/IIRA.htm> .

rami:AdminShellSubmodel a owl:Class ;
    rdfs:label "Admin Shell Sub Model"@en ;
    rdfs:comment "Describes the Administration Shell concept to organize/classify standards into submodels"@en ;
    rdfs:isDefinedBy <https://www.plattform-i40.de/I40/Redaktion/EN/Downloads/Publikation/structure-of-the-administration-shell.pdf?__blob=publicationFile&v=7> ;
    rdfs:subClassOf sto:StandardClassification .

rami:Enterprise a owl:NamedIndividual,
        rami:RAMIHierarchyLevel ;
    sto:isDescribedin sto:RAMI40 .

sto:ICS_29_240_20 a owl:NamedIndividual,
        sto:InternationalClassificationForStandards ;
    rdfs:label "ICS 29.240.20"@en ;
    dcterms:title "Power transmission and distribution lines"@en ;
    rdfs:comment "This is ICS for “Power transmission and distribution lines”"@en .

sto:IETF a owl:NamedIndividual,
        sto:StandardOrganization ;
    rdfs:label "IETF"@en ;
    rdfs:comment "TODO: complete annotations etc." ;
    rdfs:seeAlso <http://wikipedia.org/wiki/Internet_Engineering_Task_Force>,
        <http://www.ietf.org/> ;
    sto:abbreviation "IETF"@en ;
    sto:hasWikipediaArticle <http://wikipedia.org/wiki/Internet_Engineering_Task_Force> ;
    sto:orgName "Internet Engineering Task Force"@en .

idsram:Safety a owl:NamedIndividual,
        sto:StandardClassification ;
    rdfs:label "IDS RAM Safety"@en,
        "IDS Safety"@en ;
    sto:isDescribedin sto:IndustrialDataSpace,
        idsram:ReferenceArchitectureModel .

rami:Asset a owl:NamedIndividual,
        rami:RAMIITLayer ;
    rdfs:label "RAMI Asset Layer"@en ;
    sto:isDescribedin sto:RAMI40 .

sto:NISTInitiative a owl:NamedIndividual,
        sto:StandardizationFramework ;
    rdfs:label "NIST Initiative"@en ;
    rdfs:comment "Describes the National Institute of Standards and Technology Initiative, i.e., NIST which provides a standard landascape"@en ;
    rdfs:isDefinedBy "http://nvlpubs.nist.gov/nistpubs/ir/2016/NIST.IR.8107.pdf" .

lang:spa a owl:NamedIndividual .

rami:WorkCenter a owl:NamedIndividual,
        rami:RAMIHierarchyLevel ;
    sto:isDescribedin sto:RAMI40 .

sto:AdministrationShell a owl:NamedIndividual,
        sto:StandardizationFramework ;
    rdfs:label "Administration Shell"@en ;
    rdfs:comment "Represents the classifications of the standards according to the submodels of the administration shell."@en .

sto:RAMI40 a owl:NamedIndividual,
        sto:StandardizationFramework ;
    rdfs:label "RAMI 4.0"@en ;
    rdfs:comment "Describes the Reference Architecture Model for Industry 4.0, i.e., the RAMI Initiative."@en .

idsram:ReferenceArchitectureModel a owl:NamedIndividual,
        sto:StandardizationFramework ;
    rdfs:label "IDS RAM"@en,
        "Industrial Data Space Reference Architecture Model"@en .

idsram:Security a <http://w3id.org/ids/ram/Perspective>,
        owl:NamedIndividual ;
    rdfs:label "IDS RAM Security Perspective"@en ;
    sto:alignesWith iira:Security ;
    sto:isDescribedin idsram:ReferenceArchitectureModel .

rami:Engineering a owl:NamedIndividual,
        rami:AdminShellSubmodel ;
    sto:isDescribedin sto:AdministrationShell .

sto:Publication a owl:Class ;
    rdfs:label "Publication"@en ;
    rdfs:comment """Specifies a Publication. E.g., International Standards,Technical Specifications,Publicly Available Specifications,Amendments\r
                Technical Corrigenda,Interpretation Sheets,Technical Reports,Guides"""@en ;
    rdfs:isDefinedBy sto:IEC ;
    rdfs:seeAlso <http://www.iec.ch/standardsdev/publications/> ;
    rdfs:subClassOf foaf:Document .

sto:StandardizationFramework a owl:Class ;
    rdfs:label "Standarization Framework"@en ;
    dcterms:creator sto:irlan ;
    rdfs:comment "Describes existings Standardizations Initiatives, e.g, RAMI, NIST."@en ;
    skos:altLabel "Reference Architecture"@en .

rami:Station a owl:NamedIndividual,
        rami:RAMIHierarchyLevel ;
    sto:isDescribedin sto:RAMI40 .

sto:IndustrialAutomation a owl:NamedIndividual,
        sto:Domain ;
    rdfs:label "Industrial Automation"@en ;
    rdfs:comment "Industrial automation deals primarily with the automation of manufacturing, quality control and material handling processes. General purpose controllers for industrial processes include Programmable logic controllers, stand-alone I/O modules, and computers. Industrial automation is to replace the decision making of humans and manual command-response activities with the use of mechanized equipment and logical programming commands. One trend is increased use of Machine vision to provide automatic inspection and robot guidance functions, another is a continuing increase in the use of robots. Industrial automation is simply done at the industrial level."@en ;
    sto:domainName "Industrial Automation"@en ;
    sto:hasDBpediaResource dbrc:IndustrialAutomation ;
    sto:hasWikipediaArticle <https://en.wikipedia.org/wiki/Automation> .

rami:FieldDevice a owl:NamedIndividual,
        rami:RAMIHierarchyLevel ;
    sto:isDescribedin sto:RAMI40 .

rami:Product a owl:NamedIndividual,
        rami:RAMIHierarchyLevel ;
    sto:isDescribedin sto:RAMI40 .

sto:TechnicalCommittee a owl:Class,
        owl:NamedIndividual ;
    rdfs:label "Technical Committe"@en ;
    rdfs:comment "Specifies the representitive code name of the Technical Committee that covers a Standard for e.g, TC 1, SC 3C. Many thousand experts carry out standardization work in the IEC in TCs (technical committees) and SCs (subcommittees), in hundreds of working groups, project and maintenance teams. They represent the national electrotechnical needs of IEC Member countries and of many Affiliates at the global level in the IEC. These technical experts are sent by industry, governments, test and research laboratories, academia and even consumer groups to work on the global, neutral and independent platform of the IEC. That's where they develop globally relevant, voluntary, consensus based IEC International Standards."@en ;
    rdfs:isDefinedBy sto:IEC ;
    rdfs:seeAlso <http://www.iec.ch/dyn/www/f?p=103:62:9979528650478:::62:FSP_ORG_ID,FSP_LANG_ID:,25> ;
    skos:note "1.sto:       a property explaining that TC and SC are managed by SMB (Standardization Management Board) needs to be added" ;
    sto:abbreviation "TC" .

idsram:Certification a <http://w3id.org/ids/ram/Perspective>,
        owl:NamedIndividual ;
    rdfs:label "IDS RAM Certification Perspective"@en ;
    sto:isDescribedin idsram:ReferenceArchitectureModel .

iira:Security a iira:SystemCharacteristics,
        owl:NamedIndividual ;
    rdfs:label "IIRA Security"@en .

rami:ControlDevice a owl:NamedIndividual,
        rami:RAMIHierarchyLevel ;
    sto:isDescribedin sto:RAMI40 .

sto:StandardClassification a owl:Class ;
    rdfs:label "Standard Classification"@en ;
    rdfs:comment "Describes categorization areas that the different Standardizations Initiatives use to category Standards."@en ;
    owl:equivalentClass sto:Viewpoint .

sto:InternationalClassificationForStandards a owl:Class,
        owl:NamedIndividual ;
    rdfs:label "International Classification For Standards"@en ;
    rdfs:comment "Serves as a structure for catalogues of international, regional and national standards and other normative documents, and as a basis for standing-order systems."@en ;
    rdfs:seeAlso <https://www.iso.org/publication/PUB100033.html> ;
    sto:abbreviation "ICS"@en .

owl:Thing a owl:Class .

sto:TC_57 a owl:NamedIndividual,
        sto:TechnicalCommittee ;
    rdfs:label "TC 57"@en ;
    dcterms:title "Power systems management and associated information exchange"@en ;
    rdfs:comment """To prepare international standards for power systems control equipment and systems including EMS (Energy Management Systems), SCADA (Supervisory Control And Data Acquisition), distribution automation, teleprotection, and associated information exchange for real-time and non-real-time information, used in the planning, operation and maintenance of power systems. Power systems management comprises control within control centres, substations and individual pieces of primary equipment including telecontrol and interfaces to equipment, systems and databases, which may be outside the scope of TC 57. The special conditions in a high voltage environment have to be taken into consideration.\r
Note 1: Standards prepared by other technical committees of the IEC and organizations such as ITU and ISO shall be used where applicable.\r
Note 2: Although the work of TC 57 is chiefly concerned with standards for electric power systems, these standards may also be useful for application by the relevant bodies to other geographical widespread processes.\r
Note 3: Whereas standards related to measuring and protection relays and to the control and monitoring equipment used with these systems are treated by TC 95, TC 57 deals with the interface to the control systems and the transmission aspects for teleprotection systems. Whereas standards related to equipment for electrical measurement and load control are treated by TC 13, TC 57 deals with the interface of equipment for interconnection lines and industrial consumers and producers requiring energy management type interfaces to the control system."""@en .

sto:ICS_33_200 a owl:NamedIndividual,
        sto:InternationalClassificationForStandards ;
    rdfs:label "ICS 33.200"@en ;
    dcterms:title "Telecontrol. Telemetering Including Supervising, Control and Data Acquisition System (SCADA)"@en ;
    rdfs:comment "This is ICS for Telecontrol. Telemetering Including Supervising, Control and Data Acquisition System (SCADA)"@en .

sto:StandardOrganization a owl:Class ;
    rdfs:label "StandardOrganization"@en ;
    dcterms:creator sto:irlan ;
    rdfs:comment "Define the standards organizations that develop and publish industry standards"@en ;
    rdfs:subClassOf foaf:Organization .

sto:ISO a dbpcy:Abstraction100002137,
        dbpcy:Alliance108293982,
        dbpcy:Group100031264,
        dbpcy:Measure100033615,
        dbpcy:NongovernmentalOrganization108009834,
        dbpcy:Organization108008335,
        dbpcy:SocialGroup107950920,
        dbpcy:Standard107260623,
        dbpcy:SystemOfMeasurement113577171,
        dbpcy:WikicatInternationalNongovernmentalOrganizations,
        dbpcy:WikicatInternationalOrganizations,
        dbpcy:WikicatNon-governmentalOrganizations,
        dbpcy:WikicatOrganisationsBasedInGeneva,
        dbpcy:WikicatOrganizationsEstablishedIn1947,
        dbpcy:WikicatOrganizationsWithGeneralConsultativeStatusToTheUnitedNationsEconomicAndSocialCouncil,
        dbpcy:WikicatSocialResponsibilityOrganizations,
        dbpcy:WikicatStandardsOrganizations,
        dbpcy:WikicatWithdrawnISOStandards,
        dbpcy:WorldOrganization108294696,
        dbpcy:YagoLegalActor,
        dbpcy:YagoLegalActorGeo,
        dbpcy:YagoPermanentlyLocatedEntity,
        dbont:Agent,
        dbont:Organisation,
        schema:Organization,
        <http://umbel.org/umbel/rc/Organization>,
        dul:Agent,
        dul:SocialPerson,
        owl:NamedIndividual,
        owl:Thing,
        wike:Q24229398,
        wike:Q43229,
        sto:StandardOrganization ;
    dcterms:subject dbrc:International_Organization_for_Standardization,
        dbrc:Organisations_based_in_Geneva,
        dbrc:Organizations_established_in_1947,
        dbrc:Organizations_with_general_consultative_status_to_the_United_Nations_Economic_and_Social_Council,
        dbrc:Social_responsibility_organizations,
        dbrc:Standards_organizations,
        dbrc:Technical_specifications ;
    lingg:hypernym dbres:Body ;
    rdfs:comment "Is an independent, non-governmental organization, the members of which are the standards organizations of the 162 member countries. It is the world's largest developer of voluntary international standards and facilitates world trade by providing common standards between nations. Nearly twenty thousand standards have been set covering everything from manufactured products and technology to food safety, agriculture and healthcare."@en,
        "The International Organization for Standardization (ISO) is an international standard-setting body composed of representatives from various national standards organizations."@en ;
    sto:abbreviation "ISO" ;
    sto:belongsTo dbr:Switzerland ;
    sto:formationDate "1947-02-23"^^xsd:date ;
    sto:hasDBpediaResource <http://dbpedia.org/page/International_Organization_for_Standardization> ;
    sto:hasHeadquaterIn dbr:Geneva ;
    sto:hasOfficialResource <https://www.iso.org>,
        <https://www.iso.org/about-us.html> ;
    sto:hasWikipediaArticle <https://en.wikipedia.org/wiki/International_Organization_for_Standardization> ;
    sto:orgName "Internationale Organisation für Normung"@de,
        "International Organization for Standardization"@en,
        "The International Organization for Standardization"@en,
        "Organisation internationale de normalisation"@fr,
        "Международная организация по стандартизации"@ru .

lang:fra a owl:NamedIndividual .

lang:eng a owl:NamedIndividual .

om2:Measure a owl:Class .

sto:IEC a dbpcy:Abstraction100002137,
        dbpcy:Alliance108293982,
        dbpcy:Association108049401,
        dbpcy:Company108058098,
        dbpcy:Group100031264,
        dbpcy:Institute108407330,
        dbpcy:Institution108053576,
        dbpcy:Organization108008335,
        dbpcy:SocialGroup107950920,
        dbpcy:WikicatComputerScienceOrganizations,
        dbpcy:WikicatInstitutes,
        dbpcy:WikicatInternationalOrganizations,
        dbpcy:WikicatOrganisationsBasedInGeneva,
        dbpcy:WikicatOrganizationsEstablishedIn1906,
        dbpcy:WikicatStandardsOrganizations,
        dbpcy:WorldOrganization108294696,
        dbpcy:YagoLegalActor,
        dbpcy:YagoLegalActorGeo,
        dbpcy:YagoPermanentlyLocatedEntity,
        dbont:Agent,
        dbont:Organisation,
        schema:Organization,
        dul:Agent,
        dul:SocialPerson,
        owl:NamedIndividual,
        owl:Thing,
        wike:Q24229398,
        wike:Q43229,
        sto:StandardOrganization ;
    dcterms:subject dbrc:Electrical_engineering_organizations,
        dbrc:International_Electrotechnical_Commission,
        dbrc:Standards_organizations ;
    lingg:hypernym dbres:Organization ;
    rdfs:comment "Is a non-profit, non-governmental international standards organization that prepares and publishes International Standards for all electrical, electronic and related technologies – collectively known as \"electrotechnology\". IEC standards cover a vast range of technologies from power generation, transmission and distribution to home appliances and office equipment, semiconductors, fiber optics, batteries, solar energy, nanotechnology and marine energy as well as many others. The IEC also manages three global conformity assessment systems that certify whether equipment, system or components conform to its International Standards."@en ;
    sto:abbreviation "IEC" ;
    sto:formationDate "1906-06-26"^^xsd:date ;
    sto:hasDBpediaResource dbres:International_Electrotechnical_Commission ;
    sto:hasHeadquaterIn dbr:Geneva ;
    sto:hasOfficialResource <http://www.iec.ch/> ;
    sto:hasWikipediaArticle <https://en.wikipedia.org/wiki/International_Electrotechnical_Commission> ;
    sto:orgName "International Electrotechnical Commission"@en,
        "Commission électrotechnique internationale"@fr .

sto:Standard a owl:Class,
        owl:NamedIndividual ;
    rdfs:label "Standard"@en ;
    cc:attributionName "Copyright © 2016 IEC Geneva, Switzerland." ;
    cc:attributionURL <http://www.iec.ch> ;
    rdfs:comment "A document, established by consensus and approved by a recognized body, that provides, for common and repeated use, rules, guidelines or characteristics for activities or their results, aimed at the achievement of the optimum degree of order in a given context."@en ;
    rdfs:isDefinedBy sto:IEC ;
    rdfs:seeAlso <http://www.iec.ch/standardsdev/publications/is.htm> ;
    rdfs:subClassOf sto:Publication ;
    sto:abbreviation "IS" .

