@prefix : <https://w3id.org/i40/sto##> .
@prefix cc: <http://creativecommons.org/ns#> .
@prefix dbo: <http://dbpedia.org/ontology#> .
@prefix dbont: <http://dbpedia.org/ontology/> .
@prefix dbpcy: <http://dbpedia.org/class/yago/> .
@prefix dbprop: <http://dbpedia.org/property/> .
@prefix dbr: <http://dbpedia.org/resource#> .
@prefix dbrc: <http://dbpedia.org/resource/Category:> .
@prefix dbres: <http://dbpedia.org/resource/> .
@prefix dc11: <http://purl.org/dc/elements/1.1/> .
@prefix dcterms: <http://purl.org/dc/terms/> .
@prefix deo: <http://purl.org/spar/deo/> .
@prefix doap: <http://usefulinc.com/ns/doap#> .
@prefix dul: <http://www.ontologydesignpatterns.org/ont/dul/DUL.owl#> .
@prefix foaf: <http://xmlns.com/foaf/0.1/> .
@prefix geo: <http://www.geonames.org/ontology#> .
@prefix lingg: <http://purl.org/linguistics/gold/> .
@prefix muto: <http://purl.org/muto/core#> .
@prefix om2: <http://www.ontology-of-units-of-measure.org/resource/om-2/> .
@prefix owl: <http://www.w3.org/2002/07/owl#> .
@prefix prov: <http://www.w3.org/ns/prov#> .
@prefix rami: <https://w3id.org/i40/rami#> .
@prefix rdf: <http://www.w3.org/1999/02/22-rdf-syntax-ns#> .
@prefix rdfs: <http://www.w3.org/2000/01/rdf-schema#> .
@prefix schema: <http://schema.org/> .
@prefix skos: <http://www.w3.org/2004/02/skos/core#> .
@prefix sto: <https://w3id.org/i40/sto#> .
@prefix vann: <http://purl.org/vocab/vann/> .
@prefix voaf: <http://purl.org/vocommons/voaf#> .
@prefix vocvr: <http://purl.org/voc/vrank#> .
@prefix wike: <http://www.wikidata.org/entity/> .
@prefix xml: <http://www.w3.org/XML/1998/namespace> .
@prefix xsd: <http://www.w3.org/2001/XMLSchema#> .

cc:attributionName a owl:AnnotationProperty .

cc:attributionURL a owl:AnnotationProperty .

dc11:rights a owl:AnnotationProperty .

dcterms:hasLicense a owl:ObjectProperty ;
    rdfs:label "has License"@en ;
    dcterms:hasVersion <http://dublincore.org/usage/terms/history/#license-002> ;
    dcterms:issued "2004-06-14"^^xsd:date ;
    dcterms:modified "2017-12-19"^^xsd:date ;
    rdfs:comment "A legal document giving official permission to do something with the resource."@en,
        "A legal document giving official permission to do something with the resource. In this ontology denotes the license of a Standard."@en,
        "Represent the license document for a given Standard"@en ;
    rdfs:domain sto:Standard ;
    rdfs:isDefinedBy dcterms: ;
    rdfs:range dcterms:LicenseDocument .

dcterms:hasVersion a owl:AnnotationProperty .

dcterms:issued a owl:AnnotationProperty .

dcterms:modified a owl:AnnotationProperty .

dul:isMemberOf a owl:AnnotationProperty .

rdfs:commment a owl:AnnotationProperty .

skos:altLabel a owl:AnnotationProperty .

skos:definition a owl:AnnotationProperty .

skos:note a owl:AnnotationProperty .

skos:prefLabel a owl:AnnotationProperty .

prov:wasGeneratedBy a owl:ObjectProperty ;
    rdfs:comment "Standard A has influences in Standard B. For example, IEC_61499 hasInfluenceIn IEC_61804-2(EDDL)"@en ;
    rdfs:subPropertyOf sto:relatedTo .

rami:Asst a owl:NamedIndividual .

rami:InstanceMaintenance a owl:NamedIndividual,
        rami:RAMILifeCycleLayer ;
    rdfs:label "Instance Maintenance"@en .

rami:InstanceProduction a owl:NamedIndividual,
        rami:RAMILifeCycleLayer ;
    rdfs:label "Instance Production"@en .

rami:TypeDevelopment a owl:NamedIndividual,
        rami:RAMILifeCycleLayer ;
    rdfs:label "Type Development"@en .

rami:TypeMaintenance a owl:NamedIndividual,
        rami:RAMILifeCycleLayer ;
    rdfs:label "Type Maintenance"@en .

rami:safety a owl:NamedIndividual .

sto:ASAM_ODS a owl:NamedIndividual,
        sto:Standard ;
    rdfs:label "ASAM ODS"@en ;
    rdfs:comment "Set up a test data management system on top of test systems that produce measured or calculated data from testing activities"@en ;
    sto:hasOfficialResource "https://wiki.asam.net/display/STANDARDS/ASAM+ODS" ;
    sto:hasPublisher sto:ASAM .

sto:ASME_Y1441 a owl:NamedIndividual,
        sto:Standard ;
    rdfs:label "ASME Y14.41"@en ;
    dcterms:subject dbrc:American_Society_of_Mechanical_Engineers ;
    rdfs:comment "ASME Y14.41 establishs requirements for model-based definition upon CAD software and those who use CAD software to create product definition within the 3D model."@en ;
    sto:hasClassification sto:ModelingPractice ;
    sto:hasDBpediaResource "http://dbpedia.org/resource/ASME_Y14.41" ;
    sto:hasOfficialResource "https://www.asme.org/products/codes-standards/y1441-2012-digital-product-definition-data" ;
    sto:hasPublisher sto:ASME ;
    sto:hasWikipediaArticle "http://en.wikipedia.org/wiki/ASME_Y14.41",
        "https://en.wikipedia.org/wiki/ASME_Y14.41" .

sto:B2MML a dbpcy:Abstraction100002137,
        dbpcy:Measure100033615,
        dbpcy:Standard107260623,
        dbpcy:SystemOfMeasurement113577171,
        dbpcy:WikicatANSIStandards,
        dbpcy:WikicatStandards,
        dbpcy:WikicatXML-basedStandards,
        dbont:Language,
        dbont:ProgrammingLanguage,
        dbont:Software,
        schema:Language,
        owl:NamedIndividual,
        owl:Thing,
        wike:Q315,
        wike:Q34770,
        wike:Q9143,
        sto:Standard ;
    rdfs:label "Business To Manufacturing Markup Language" ;
    dcterms:subject dbrc:ANSI_standards,
        dbrc:Manufacturing,
        dbrc:Supply_chain_management ;
    lingg:hypernym dbres:Implementation ;
    rdfs:comment "B2MML or Business To Manufacturing Markup Language is an XML implementation of the ANSI/ISA-95 family of standards (ISA-95)"@en ;
    skos:altLabel "IEC 62264"@en ;
    sto:hasClassification sto:BusinessProcessExecution,
        sto:EnterpriseLevel ;
    sto:hasDBpediaResource "http://dbpedia.org/resource/B2MML" ;
    sto:hasDeveloper sto:MESA ;
    sto:hasOfficialResource "https://services.mesa.org/ResourceLibrary/ShowResource/0f47758b-60f0-40c6-a71b-fa7b2363fb3a" ;
    sto:hasPublisher sto:MESA ;
    sto:hasTag "B2MML"@en ;
    sto:hasWikipediaArticle "http://en.wikipedia.org/wiki/B2MML",
        "https://en.wikipedia.org/wiki/B2MML" ;
    sto:isImplementationOf sto:ISA-95 .

sto:BBF_TR-069 a dbpcy:Abstraction100002137,
        dbpcy:Accomplishment100035189,
        dbpcy:Act100030358,
        dbpcy:Action100037396,
        dbpcy:Communication100033020,
        dbpcy:Direction106786629,
        dbpcy:Event100029378,
        dbpcy:Feat100036762,
        dbpcy:Measure100033615,
        dbpcy:Message106598915,
        dbpcy:Protocol106665108,
        dbpcy:PsychologicalFeature100023100,
        dbpcy:Rule106652242,
        dbpcy:Standard107260623,
        dbpcy:SystemOfMeasurement113577171,
        dbpcy:WikicatApplicationLayerProtocols,
        dbpcy:WikicatComputerSecurityExploits,
        dbpcy:WikicatInternetStandards,
        dbpcy:WikicatStandards,
        dbpcy:YagoPermanentlyLocatedEntity,
        dbont:Software,
        owl:NamedIndividual,
        sto:Standard ;
    rdfs:label "BBF TR-069"@en ;
    dcterms:subject dbrc:Digital_subscriber_line,
        dbrc:Internet_Standards ;
    lingg:hypernym dbres:Specification ;
    rdfs:comment "Digital Enhanced Cordless Telecommunications (DECT™) is the ETSI standard for short-range cordless communications, which can be adapted for many applications and can be used over unlicensed frequency allocations world-wide."@en ;
    sto:hasDBpediaResource "http://dbpedia.org/resource/TR-069" ;
    sto:hasDeveloper sto:BBF ;
    sto:hasOfficialResource "https://www.broadband-forum.org/standards-and-software/technical-specifications/tr-069-files-tools" ;
    sto:hasPublisher sto:BBF ;
    sto:hasTag "CPE WAN Management Protocol"@en ;
    sto:hasWikipediaArticle "http://en.wikipedia.org/wiki/TR-069",
        "https://en.wikipedia.org/wiki/TR-069" .

sto:BPEL a dbpcy:Abstraction100002137,
        dbpcy:Act100030358,
        dbpcy:Activity100407535,
        dbpcy:ArtificialLanguage106894544,
        dbpcy:Communication100033020,
        dbpcy:Description106724763,
        dbpcy:Event100029378,
        dbpcy:Language106282651,
        dbpcy:LanguageUnit106284225,
        dbpcy:MarkupLanguage106787835,
        dbpcy:Measure100033615,
        dbpcy:Message106598915,
        dbpcy:Part113809207,
        dbpcy:ProgrammingLanguage106898352,
        dbpcy:PsychologicalFeature100023100,
        dbpcy:Relation100031921,
        dbpcy:Service100577525,
        dbpcy:Specification106725067,
        dbpcy:Standard107260623,
        dbpcy:Statement106722453,
        dbpcy:SystemOfMeasurement113577171,
        dbpcy:Terminology106304059,
        dbpcy:WikicatMarkupLanguages,
        dbpcy:WikicatProgrammingLanguages,
        dbpcy:WikicatSpecificationLanguages,
        dbpcy:WikicatWebServiceSpecifications,
        dbpcy:WikicatWebServices,
        dbpcy:WikicatXML-basedStandards,
        dbpcy:Word106286395,
        dbpcy:Work100575741,
        dbpcy:YagoPermanentlyLocatedEntity,
        dbont:Language,
        owl:NamedIndividual,
        sto:Standard ;
    rdfs:label "Business Process Execution Language"@en ;
    dcterms:subject dbrc:Process_management,
        dbrc:Specification_languages,
        dbrc:Web_service_specifications,
        dbrc:Workflow_technology,
        dbrc:XML-based_standards ;
    lingg:hypernym dbres:Language ;
    rdfs:comment "The Web Services Business Process Execution Language (WS-BPEL), commonly known as BPEL Business Process Execution Language, is a standard executable language for specifying actions within business processes with web services."@en ;
    sto:hasClassification sto:BusinessProcessExecution ;
    sto:hasDBpediaResource "http://dbpedia.org/resource/Business_Process_Execution_Language" ;
    sto:hasOfficialResource "https://www.oasis-open.org/committees/tc_home.php?wg_abbrev=wsbpel" ;
    sto:hasPublisher sto:OASIS ;
    sto:hasTag "BPEL"@en ;
    sto:hasWikipediaArticle "http://en.wikipedia.org/wiki/Business_Process_Execution_Language",
        "https://en.wikipedia.org/wiki/Business_Process_Execution_Language" .

sto:ConditionMonitoring a owl:NamedIndividual,
        rami:AdminShellSubmodel ;
    sto:isDescribedin sto:AdministrationShell .

sto:Configuration a owl:NamedIndividual,
        rami:AdminShellSubmodel ;
    sto:isDescribedin sto:AdministrationShell .

sto:DIN_SPEC_16592 a owl:NamedIndividual,
        sto:Standard ;
    rdfs:label "DIN SPEC 16592"@en ;
    rdfs:comment "Combining OPC Unified Architecture and Automation Markup Language."@en ;
    prov:wasGeneratedBy sto:IEC_62541,
        sto:IEC_62714 ;
    sto:hasDeveloper sto:DIN ;
    sto:hasOfficialResource <https://www.beuth.de/de/technische-regel/din-spec-16592/265597431> ;
    sto:hasPublisher sto:DIN .

sto:ETSI_LTN a owl:NamedIndividual,
        sto:Standard ;
    rdfs:label "ETSI LTN"@en ;
    rdfs:comment "Machine-to-Machine communications and the Internet of Things (IoT) involve the connection of potentially billions of connected objects which need only low throughput connectivity. The anticipated benefits of creating new dedicated IoT Low Throughput Networks (LTN) include lower costs, the creation of new applications, a reduction in electromagnetic radiation by improving data transmission efficiency LTN are expected to be crucial to the success of IoT standardization and implementation, and to provide the basis for many new and innovative applications. "@en ;
    sto:hasDeveloper sto:ETSI ;
    sto:hasDomain sto:M2M ;
    sto:hasOfficialResource "http://www.etsi.org/technologies-clusters/technologies/low-throughput-networks" ;
    sto:hasPublisher sto:ETSI ;
    sto:hasTag "Low Throughput Networks"@en ;
    sto:relatedTo sto:ETSI_DECT .

sto:ETSI_ULE a dbpcy:Abstraction100002137,
        dbpcy:Measure100033615,
        dbpcy:Standard107260623,
        dbpcy:SystemOfMeasurement113577171,
        dbpcy:WikicatMobileTelecommunicationsStandards,
        dbont:Work,
        owl:NamedIndividual,
        sto:Standard ;
    rdfs:label "Ultra Low Energy"@en ;
    dcterms:subject dbrc:Mobile_telecommunications_standards ;
    lingg:hypernym dbres:Standard ;
    rdfs:comment "DECT Ultra Low Energy (DECT ULE) is a technology based on DECT, and intended for Machine-to-Machine communications such as Home and Industrial automation. The main characteristics of the technology are ultra-low power consumption (much lower than IEEE 802.11) and wider coverage (much wider than IEEE 802.15 and Bluetooth Low Energy)."@en ;
    sto:hasDBpediaResource "http://dbpedia.org/resource/ULE_-_Ultra_Low_Energy" ;
    sto:hasDeveloper sto:ETSI ;
    sto:hasOfficialResource "http://www.etsi.org/technologies-clusters/technologies/dect/dect-ule" ;
    sto:hasPublisher sto:ETSI ;
    sto:hasTag "ETSI ULE"@en ;
    sto:hasWikipediaArticle "http://en.wikipedia.org/wiki/ULE_-_Ultra_Low_Energy",
        "https://en.wikipedia.org/wiki/DECT_Ultra_Low_Energy" ;
    sto:relatedTo sto:ETSI_DECT .

sto:EndOfLifeReclying a owl:NamedIndividual .

sto:IEC_14443 a dbpcy:Abstraction100002137,
        dbpcy:Assets113329641,
        dbpcy:Communication100033020,
        dbpcy:ConsumerCredit113374426,
        dbpcy:Credit113378518,
        dbpcy:CreditLine113379413,
        dbpcy:Evidence106643408,
        dbpcy:Identification106885083,
        dbpcy:Indication106797169,
        dbpcy:Measure100033615,
        dbpcy:Open-endCredit113375323,
        dbpcy:PositiveIdentification106885389,
        dbpcy:Possession100032613,
        dbpcy:Relation100031921,
        dbpcy:SmartCard113377003,
        dbpcy:Standard107260623,
        dbpcy:SystemOfMeasurement113577171,
        dbpcy:WikicatContactlessSmartCards,
        dbpcy:WikicatIECStandards,
        <http://dbpedia.org/class/yago/WikicatISO/IECStandards>,
        dbpcy:WikicatISOStandards,
        dbpcy:WikicatSmartCards,
        dbont:Work,
        owl:NamedIndividual,
        sto:Standard ;
    rdfs:label "ISO/IEC 14443"@en ;
    dcterms:subject dbrc:Contactless_smart_cards,
        <http://dbpedia.org/resource/Category:ISO/IEC_standards> ;
    lingg:hypernym dbres:Standard ;
    rdfs:comment "The ISO/IEC 14443 standard is a four-part international standard for contact-less smart cards operating at 13.56 MHz in close proximity (~10cm) with a reader antenna. This ISO standard describes the modulation and transmission protocols between card and reader to create interoperability for contact-less smart card products. There are two main communication protocols supported by the ISO/IEC 14443 standard, they are addressed as Type A and Type B. Most High Frequency (13.56 MHz) proximity tags are using these guidelines for their communication."@en ;
    owl:sameAs sto:ISO_14443 ;
    sto:hasDBpediaResource "http://dbpedia.org/resource/ISO/IEC_14443" ;
    sto:hasOfficialResource "https://www.iso.org/standard/70170.html" ;
    sto:hasPublisher sto:IEC,
        sto:ISO ;
    sto:hasTag "IEC 14443"@en ;
    sto:hasWikipediaArticle "http://en.wikipedia.org/wiki/ISO/IEC_14443",
        "https://en.wikipedia.org/wiki/ISO/IEC_14443" .

sto:IEC_15459 a owl:NamedIndividual,
        sto:Standard ;
    rdfs:label "IEC 15459"@en ;
    rdfs:comment "ISO/IEC 15459-1:2014 specifies a unique string of characters for the identification of individual transport units. The character string is intended to be represented in a bar code label or other AIDC media attached to the entity to meet management needs. To address management needs, different types of entities are recognized in the various parts of ISO/IEC 15459, which allows different requirements to be met by the identities associated with each type. The rules for the unique identification for individual transport units, to identify physical logistical transfers, with the identity relevant for the duration of one or more items in the load being held or transported as part of that load, are defined and supported by example."@en ;
    owl:sameAs sto:ISO_15459 ;
    sto:hasOfficialResource "https://www.iso.org/standard/54779.html" ;
    sto:hasPublisher sto:IEC,
        sto:ISO ;
    sto:hasTag "Information technology -- Automatic identification and data capture techniques -- Unique identification"@en .

sto:IEC_24760 a owl:NamedIndividual,
        sto:Standard ;
    rdfs:label "IEC 24760"@en ;
    rdfs:comment "ISO/IEC 24760: it defines terms for identity management, and also specifies core concepts of identity and identity management and their relationships. It is applicable to any information system that processes identity information. A bibliography of documents describing various aspects of identity information management is provided."@en ;
    sto:hasClassification rami:ControlDevice,
        rami:FieldDevice,
        rami:Information,
        rami:Product,
        rami:Safety,
        rami:Security,
        rami:Station,
        sto:ProductModelDataExchange ;
    sto:hasDomain sto:ITSecurity ;
    sto:hasOfficialResource "https://www.iso.org/standard/57914.html" ;
    sto:hasPublicationDate "2011-01-12"^^xsd:date ;
    sto:hasPublisher sto:IEC ;
    sto:relatedTo sto:IEC_62443 .

sto:IEC_29161 a owl:NamedIndividual,
        sto:Standard ;
    rdfs:label "IEC 29161"@en ;
    rdfs:comment "ISO/IEC 29161:2016 establishes a unique identification scheme for the Internet of Things (IoT), based on existing and evolving data structures. This International Standard specifies the common rules applicable for unique identification that are required to ensure full compatibility across different identities. The unique identification is a universal construct for any physical object, virtual object, or person. It is used in IoT information systems that need to track or otherwise refer to entities. It is intended for use with any IoT media."@en ;
    owl:sameAs sto:ISO_29161 ;
    sto:hasDomain "Automatic identification and data capture techniques"@en ;
    sto:hasOfficialResource "https://www.iso.org/standard/45240.html" ;
    sto:hasPublicationDate "2016-08-01"^^xsd:date ;
    sto:hasPublisher sto:IEC,
        sto:ISO ;
    sto:hasTag "Information technology -- Data structure -- Unique identification for the Internet of Things"@en .

sto:IEC_29182-1 a owl:NamedIndividual,
        sto:Standard ;
    rdfs:label "IEC 29182-1"@en ;
    rdfs:comment "ISO/IEC 29182-1: provides a general overview of the characteristics of a sensor network and the organization of the entities that comprise such a network. It also describes the general requirements that are identified for sensor networks."@en ;
    sto:hasClassification rami:Communications,
        rami:ControlDevice,
        rami:FieldDevice,
        sto:ProductionSystemModelData ;
    sto:hasDomain sto:M2M ;
    sto:hasOfficialResource "https://www.iso.org/standard/45261.html" ;
    sto:hasPublicationDate "2013-06-01"^^xsd:date ;
    sto:hasPublisher sto:IEC,
        sto:ISO ;
    sto:relatedTo sto:IEC_61158 .

sto:IEC_42010 a dbpcy:Abstraction100002137,
        dbpcy:Measure100033615,
        dbpcy:Standard107260623,
        dbpcy:SystemOfMeasurement113577171,
        <http://dbpedia.org/class/yago/WikicatISO/IECStandards>,
        dbont:Work,
        owl:NamedIndividual,
        sto:Standard ;
    rdfs:label "IEC 42010"@en ;
    dcterms:subject dbrc:IEEE_standards,
        <http://dbpedia.org/resource/Category:ISO/IEC_standards>,
        dbrc:Software_architecture ;
    lingg:hypernym dbres:Standard ;
    rdfs:comment "ISO/IEC/IEEE 42010:2011 defines requirements on the description of system, software and enterprise architectures. It aims to standardise the practice of architecture description by defining standard terms, presenting a conceptual foundation for expressing, communicating and reviewing architectures and specifying requirements that apply to architecture descriptions, architecture frameworks and architecture description languages."@en ;
    skos:note "The IIRA is based in this standards" ;
    sto:hasDBpediaResource "http://dbpedia.org/page/ISO/IEC_42010" ;
    sto:hasOfficialResource "http://www.iso-architecture.org/ieee-1471/" ;
    sto:hasPublisher sto:IEC,
        sto:ISO ;
    sto:hasTag "ISO/IEC/IEEE 42010"@en ;
    sto:hasWikipediaArticle "http://en.wikipedia.org/wiki/ISO/IEC_42010",
        "https://en.wikipedia.org/wiki/ISO/IEC_42010" .

sto:IEC_60086 a owl:NamedIndividual,
        sto:Standard ;
    rdfs:label "IEC 60086"@en ;
    rdfs:comment "Standard battery nomenclature describes portable dry cell batteries that have physical dimensions and electrical characteristics interchangeable between manufacturers."@en ;
    sto:hasDBpediaResource "http://dbpedia.org/page/Battery_nomenclature#IEC_60086" ;
    sto:hasOfficialResource "https://webstore.iec.ch/publication/22991" ;
    sto:hasPublisher sto:IEC ;
    sto:hasWikipediaArticle "https://en.wikipedia.org/wiki/Battery_nomenclature#IEC_60086" .

sto:IEC_60364 a dbpcy:Abstraction100002137,
        dbpcy:Measure100033615,
        dbpcy:Standard107260623,
        dbpcy:SystemOfMeasurement113577171,
        dbpcy:WikicatIECStandards,
        dbont:Organisation,
        owl:NamedIndividual,
        sto:Standard ;
    rdfs:label "IEC 60364"@en ;
    dcterms:subject dbrc:Electric_power_distribution,
        dbrc:IEC_standards ;
    lingg:hypernym dbres:Commission ;
    rdfs:comment "Electrical Installations for Buildings is the International Electrotechnical Commission's international standard on electrical installations of buildings"@en ;
    sto:hasDBpediaResource "http://dbpedia.org/page/IEC_60364" ;
    sto:hasPublisher sto:IEC ;
    sto:hasWikipediaArticle "http://en.wikipedia.org/wiki/IEC_60364",
        "https://en.wikipedia.org/wiki/IEC_60364" .

sto:IEC_60839-5-2 a owl:NamedIndividual,
        sto:Standard ;
    rdfs:label "IEC 60839-5-2"@en ;
    rdfs:comment "IEC 60839-5-2:2016 specifies the general equipment requirements for the performance, reliability, resilience, security and safety characteristics of supervised premises transceiver (SPT) installed in supervised premises and used in alarm transmission systems (ATS). A supervised premises transceiver can be a stand-alone device or an integrated part of an alarm system. These requirements also apply to the SPT sharing means of interconnection, control, communication and power supplies with other applications. The alarm transmission system requirements and classifications are defined within IEC 60839-5-1. This new edition includes the following significant technical changes with respect to the previous edition: reflects the current technological state of art (IP networks) ,harmonizes with the ATS categories introduced in IEC 60839-5-1:2014; introduces test requirements."@en ;
    sto:hasClassification rami:Communication,
        rami:ControlDevice,
        rami:FieldDevice,
        rami:Security ;
    sto:hasOfficialResource "https://webstore.iec.ch/publication/24120" ;
    sto:hasPublicationDate "2016-02-03"^^xsd:date ;
    sto:hasPublisher sto:IEC .

sto:IEC_60870 a dbpcy:Abstraction100002137,
        dbpcy:Communication100033020,
        dbpcy:Direction106786629,
        dbpcy:Measure100033615,
        dbpcy:Message106598915,
        dbpcy:Protocol106665108,
        dbpcy:Rule106652242,
        dbpcy:Standard107260623,
        dbpcy:SystemOfMeasurement113577171,
        dbpcy:WikicatIECStandards,
        dbpcy:WikicatNetworkProtocols,
        owl:NamedIndividual,
        sto:Standard ;
    rdfs:label "IEC 60870"@en ;
    dcterms:subject dbrc:Electric_power,
        dbrc:IEC_standards ;
    rdfs:comment "In electrical engineering and power system automation, the IEC 60870 series define systems used for telecontrol (supervisory control and data acquisition)"@en ;
    sto:hasDBpediaResource "http://dbpedia.org/page/IEC_60870" ;
    sto:hasPublisher sto:IEC ;
    sto:hasWikipediaArticle "http://en.wikipedia.org/wiki/IEC_60870",
        "https://en.wikipedia.org/wiki/IEC_60870" .

sto:IEC_60904 a owl:NamedIndividual,
        sto:Standard ;
    rdfs:label "IEC 60904"@en ;
    rdfs:comment "Photovoltaic devices"@en ;
    sto:hasOfficialResource "https://webstore.iec.ch/publication/3881" ;
    sto:hasPublicationDate "2017-05-18"^^xsd:date ;
    sto:hasPublisher sto:IEC .

sto:IEC_61334 a dbpcy:Artifact100021939,
        dbpcy:ComputerNetwork103085333,
        dbpcy:Instrumentality103575240,
        dbpcy:Network103820728,
        dbpcy:Object100002684,
        dbpcy:PhysicalEntity100001930,
        dbpcy:System104377057,
        dbpcy:Whole100003553,
        dbpcy:WideAreaNetwork104583477,
        dbpcy:WikicatWideAreaNetworks,
        dbont:Work,
        owl:NamedIndividual,
        sto:Standard ;
    rdfs:label "IEC 61334"@en ;
    dcterms:subject dbrc:Networking_standards,
        dbrc:Wide_area_networks ;
    lingg:hypernym dbres:Standard ;
    rdfs:comment "IEC 61334 , known as Distribution automation using distribution line carrier systems, is a standard for low-speed reliable power line communications by electricity meters, water meters and SCADA."@en ;
    sto:hasDBpediaResource "http://dbpedia.org/page/IEC_61334" ;
    sto:hasOfficialResource "https://webstore.iec.ch/publication/5308" ;
    sto:hasPublisher sto:IEC ;
    sto:hasWikipediaArticle "http://en.wikipedia.org/wiki/IEC_61334" .

sto:IEC_61400 a dbpcy:Artifact100021939,
        dbpcy:Device103183080,
        dbpcy:Engine103287733,
        dbpcy:Gear103431243,
        dbpcy:HeatEngine103507963,
        dbpcy:Instrumentality103575240,
        dbpcy:Internal-combustionEngine103579982,
        dbpcy:Machine103699975,
        dbpcy:Mechanism103738472,
        dbpcy:Motor103789946,
        dbpcy:Object100002684,
        dbpcy:PhysicalEntity100001930,
        dbpcy:RotaryEngine104110654,
        dbpcy:Transmission104472243,
        dbpcy:Turbine104498523,
        dbpcy:Whole100003553,
        dbpcy:WikicatElectricPowerTransmissionSystems,
        dbpcy:WikicatWindTurbines,
        dbpcy:WindTurbine104591517,
        dbont:Work,
        owl:NamedIndividual,
        sto:Standard ;
    rdfs:label "IEC 61400"@en ;
    dcterms:subject dbrc:Electric_power_distribution,
        dbrc:Electric_power_transmission_systems,
        dbrc:IEC_standards,
        dbrc:Wind_turbines ;
    lingg:hypernym dbres:Standard ;
    rdfs:comment "IEC 61334 , known as Distribution automation using distribution line carrier systems, is a standard for low-speed reliable power line communications by electricity meters, water meters and SCADA."@en ;
    sto:hasDBpediaResource "http://dbpedia.org/page/IEC_61400" ;
    sto:hasOfficialResource "https://webstore.iec.ch/publication/26603" ;
    sto:hasPublicationDate "2017-03-03"^^xsd:date ;
    sto:hasPublisher sto:IEC ;
    sto:hasWikipediaArticle "http://en.wikipedia.org/wiki/IEC_61400" .

sto:IEC_61508 a dbpcy:Abstraction100002137,
        dbpcy:Measure100033615,
        dbpcy:Standard107260623,
        dbpcy:SystemOfMeasurement113577171,
        dbpcy:WikicatElectricalStandards,
        dbpcy:WikicatIECStandards,
        owl:NamedIndividual,
        sto:Standard ;
    rdfs:label "IEC 60508"@en ;
    dcterms:hasLicense "Private"@en ;
    dcterms:subject dbrc:Electrical_standards,
        dbrc:IEC_standards,
        dbrc:Safety ;
    rdfs:comment "Functional safety is a concept applicable across all industry sectors. It is fundamental to the enabling of complex technology used for safety-related systems. It provides the assurance that the safety-related systems will offer the necessary risk reduction required to achieve safety for the equipment. The oil and gas industry, nuclear plants and the machinery sector, to name but a few, all rely heavily on functional safety to achieve safety for the equipment giving rise to the hazards."@en ;
    sto:hasClassification rami:Safety ;
    sto:hasDBpediaResource "http://dbpedia.org/resource/IEC_61508" ;
    sto:hasMotivation "Defines the functional safety requirements established by IEC 61508 in process industry sector terminology"@en ;
    sto:hasOfficialResource "http://www.iec.ch/functionalsafety/" ;
    sto:hasPublisher sto:IEC ;
    sto:hasTag "Functional Safety of Electrical/Electronic/Programmable Electronic Safety-related Systems"@en ;
    sto:hasWikipediaArticle "http://en.wikipedia.org/wiki/IEC_61508",
        "https://en.wikipedia.org/wiki/IEC_61508" ;
    sto:relatedTo sto:IEC_61511 .

sto:IEC_61512 a dbpcy:Abstraction100002137,
        dbpcy:Measure100033615,
        dbpcy:Standard107260623,
        dbpcy:SystemOfMeasurement113577171,
        dbpcy:WikicatANSIStandards,
        dbpcy:WikicatStandards,
        dbont:Place,
        owl:NamedIndividual,
        sto:Standard ;
    rdfs:label "IEC 61512"@en ;
    dcterms:subject dbrc:ANSI_standards,
        dbrc:Manufacturing ;
    lingg:hypernym dbres:Control ;
    rdfs:comment "Batch control - Models and terminology"@en ;
    sto:hasClassification rami:ControlDevice,
        rami:Product,
        rami:Station,
        rami:WorkCenter ;
    sto:hasDBpediaResource "http://dbpedia.org/resource/ISA-88" ;
    sto:hasMotivation "The standard sought to address the following problems: lack of a universal model for batch control, difficulty in communicating user requirement, integration among batch automation suppliers, difficulty in batch control configuration."@en ;
    sto:hasOfficialResource "https://webstore.iec.ch/publication/5528" ;
    sto:hasPublisher sto:IEC ;
    sto:hasTag "ISA-88"@en ;
    sto:hasWikipediaArticle "http://en.wikipedia.org/wiki/ISA-88",
        "https://en.wikipedia.org/wiki/ISA-88" .

sto:IEC_62264 a dbpcy:Abstraction100002137,
        dbpcy:Measure100033615,
        dbpcy:Standard107260623,
        dbpcy:SystemOfMeasurement113577171,
        dbpcy:WikicatIECStandards,
        dbont:Work,
        owl:NamedIndividual,
        sto:Standard ;
    rdfs:label "IEC 62264"@en ;
    dcterms:hasLicense "Private"@en ;
    dcterms:subject dbrc:Control_engineering,
        dbrc:IEC_standards,
        dbrc:Systems_engineering ;
    lingg:hypernym dbres:Standard ;
    rdfs:comment "Enterprise-control system integration - Models and terminology"@en,
        "IEC 62264 is an international standard for enterprise-control system integration. This standard is based upon ANSI/ISA-95."@en ;
    rdfs:seeAlso "https://en.wikipedia.org/wiki/B2MML" ;
    skos:altLabel "B2MML" ;
    sto:hasClassification rami:Functional ;
    sto:hasDBpediaResource "http://dbpedia.org/resource/IEC_62264" ;
    sto:hasDeveloper sto:IEC ;
    sto:hasDomain "Enterprise Control"@en ;
    sto:hasMotivation "Informational representation of MES and ERP models."@en ;
    sto:hasOfficialResource "http://www.iso.org/iso/catalogue_detail.htm?csnumber=63740",
        "https://webstore.iec.ch/publication/6675",
        "https://www.iso.org/standard/57308.html" ;
    sto:hasPublisher sto:IEC,
        sto:MESA ;
    sto:hasTag "Enterprise control systems"@en,
        "Enterprise-control system integration"@en ;
    sto:hasWikipediaArticle "http://en.wikipedia.org/wiki/IEC_62264",
        "https://en.wikipedia.org/wiki/IEC_62264" ;
    sto:relatedTo sto:ISA-95 .

sto:IEC_62424 a dbpcy:Abbreviation107091587,
        dbpcy:Abstraction100002137,
        dbpcy:Communication100033020,
        dbpcy:Form106290637,
        dbpcy:Format106636806,
        dbpcy:Information106634376,
        dbpcy:LanguageUnit106284225,
        dbpcy:Measure100033615,
        dbpcy:Message106598915,
        dbpcy:Part113809207,
        dbpcy:Relation100031921,
        dbpcy:Standard107260623,
        dbpcy:SystemOfMeasurement113577171,
        dbpcy:WikicatAbbreviations,
        dbpcy:WikicatComputerFileFormats,
        dbpcy:WikicatIndustry-specificXML-basedStandards,
        dbpcy:WikicatXML-basedStandards,
        dbpcy:Word106286395,
        dbont:Software,
        owl:NamedIndividual,
        sto:Standard ;
    rdfs:label "IEC 62424"@en ;
    dcterms:hasLicense "Private"@en ;
    dcterms:subject dbrc:Computer_file_formats,
        dbrc:Industry-specific_XML-based_standards ;
    lingg:hypernym dbres:Format ;
    rdfs:comment "CAEX (Computer Aided Engineering Exchange) is a neutral data format that allows storage of hierarchical object information, e.g. the hierarchical architecture of a plant. On a certain abstraction level, a plant consists in modules or components that are interconnected. CAEX allows storage of those modules or components by means of objects. Object oriented concepts as encapsulation, classes, class libraries, instances, instance hierarchies, inheritance, relations, attributes and interfaces are explicitly supported. CAEX bases on XML and is defined as XML schema (xsd file). The original intention of developing CAEX was the industrial lack of a common and established data exchange between process engineering tools and process control engineering tools. However, CAEX can be applied to all types of static object information, e.g. plant topologies, document topologies, product topologies, petri nets, but also for non-technical applications like phylogenetic trees."@en ;
    sto:hasDBpediaResource "http://dbpedia.org/resource/CAEX" ;
    sto:hasOfficialResource "https://webstore.iec.ch/publication/25442" ;
    sto:hasPublisher sto:IEC ;
    sto:hasTag "CAEX"@en ;
    sto:hasWikipediaArticle "http://en.wikipedia.org/wiki/CAEX",
        "https://en.wikipedia.org/wiki/CAEX" ;
    sto:isPartOf sto:IEC_62714 .

sto:IEC_62591 a dbpcy:Abstraction100002137,
        dbpcy:Communication100033020,
        dbpcy:Direction106786629,
        dbpcy:Message106598915,
        dbpcy:Protocol106665108,
        dbpcy:Rule106652242,
        dbont:Company,
        owl:NamedIndividual,
        sto:Standard ;
    rdfs:label "IEC 62591"@en ;
    dcterms:subject dbrc:Wireless_networking,
        dbrc:Wireless_sensor_network ;
    lingg:hypernym dbres:Technology ;
    rdfs:comment "Industrial networks - Wireless communication network and communication profiles."@en ;
    sto:hasDBpediaResource "http://dbpedia.org/page/WirelessHART" ;
    sto:hasOfficialResource "https://webstore.iec.ch/publication/24433" ;
    sto:hasPublisher sto:IEC ;
    sto:hasWikipediaArticle "http://en.wikipedia.org/wiki/WirelessHART",
        "https://en.wikipedia.org/wiki/WirelessHART" .

sto:IEC_62656 a owl:NamedIndividual,
        sto:Standard ;
    rdfs:label "IEC 62656"@en ;
    rdfs:comment "Specifies the logical structure for a set of spreadsheets, used as data parcels, to define, transfer and register product ontologies"@en ;
    sto:hasOfficialResource "https://webstore.iec.ch/publication/7326" ;
    sto:hasPublisher sto:IEC .

sto:IEC_62837 a owl:NamedIndividual,
        sto:Standard ;
    rdfs:label "IEC 62837"@en ;
    rdfs:comment "Provides to the technical committees a framework for the development and adaptation of documents in order to improve energy efficiency in manufacturing, process control and industrial facility management."@en ;
    sto:hasOfficialResource "https://webstore.iec.ch/publication/7446" ;
    sto:hasPublisher sto:IEC ;
    sto:hasTag "62837"@en .

sto:IEC_81714 a owl:NamedIndividual,
        sto:Standard ;
    rdfs:label "IEC 81714"@en ;
    rdfs:comment "ISO/IEC 81714 Design of graphical symbols for use in the technical documentation of products -- Part 3: Classification of connect nodes, networks and their encoding-- specifies requirements concerning the classification of connect nodes assigned to graphical symbols, being a representation of functional and product concepts."@en ;
    sto:hasClassification rami:Asset,
        rami:Engineering,
        rami:Identification,
        rami:Product,
        sto:ModelingPractice ;
    sto:hasDomain sto:CAD ;
    sto:hasOfficialResource "https://www.iso.org/standard/40134.html" ;
    sto:hasPublicationDate "2004-10-01"^^xsd:date ;
    sto:hasPublisher sto:IEC,
        sto:ISO .

sto:IEC_PAS_63088 a owl:NamedIndividual,
        sto:Standard ;
    rdfs:label "IEC PAS 63088"@en ;
    rdfs:comment "IEC PAS 63088:2017(E) describes a reference architecture model in the form of a cubic layer model, RAMI model"@en ;
    sto:hasOfficialResource "https://webstore.iec.ch/publication/30082?lipi=urn%3Ali%3Apage%3Ad_flagship3_pulse_read%3B2vZf0%2FOGS2CeRjny8ARziQ%3D%3D" ;
    sto:hasPublicationDate "2017-03-07"^^xsd:date ;
    sto:hasPublisher sto:IEC,
        sto:ISO ;
    sto:hasTag "RAMI 4.0" .

sto:IEC_TR_62794 a owl:NamedIndividual,
        sto:Standard ;
    rdfs:label "IEC TR 62794"@en ;
    dcterms:hasLicense "Private"@en ;
    rdfs:comment "Industrial-process measurement, control and automation - Reference model for representation of production facilities (digital factory)"@en ;
    sto:hasClassification rami:AdminShellGeneral,
        rami:ControlDevice,
        rami:FieldDevice,
        rami:GeneralAdminShell,
        rami:Station,
        rami:WorkCenter ;
    sto:hasMotivation "The standards for Digital Factory define methods and information models, which are required for self description of I40-components. "@en ;
    sto:hasOfficialResource <https://webstore.iec.ch/publication/7433> ;
    sto:hasPublisher sto:IEC ;
    sto:hasTag "DF/TR"@en ;
    sto:relatedTo sto:IEC_TS_62832 .

sto:IEC_TS_62237 a owl:NamedIndividual,
        sto:Standard ;
    rdfs:label "IEC 62237"@en ;
    rdfs:comment "Live working - Insulating hoses with fittings for use with hydraulic tools and equipment."@en ;
    sto:hasClassification rami:ControlDevice,
        rami:FieldDevice,
        rami:GeneralAdminShell,
        rami:Station,
        rami:WorkCenter,
        sto:ProductionSystemModelData ;
    sto:hasDomain sto:IndustrialAutomation ;
    sto:hasOfficialResource "https://webstore.iec.ch/publication/6626" ;
    sto:hasPublicationDate "2003-10-26"^^xsd:date ;
    sto:hasPublisher sto:IEC ;
    sto:relatedTo sto:IEC_62337 .

sto:IIRA a owl:NamedIndividual,
        sto:StandardizationFramework ;
    rdfs:label "IIRA"@en ;
    rdfs:comment "Industrial Internet Reference Architecture"@en ;
    sto:hasOfficialResource "http://www.iiconsortium.org/IIRA.htm" .

sto:ISO_1101 a owl:NamedIndividual,
        sto:Standard ;
    rdfs:label "ISO 1101"@en ;
    rdfs:comment "Geometrical product specifications (GPS) -- Geometrical tolerancing -- Tolerances of form, orientation, location and run-out"@en ;
    sto:hasClassification rami:Asset,
        rami:Product,
        sto:ModelingPractice ;
    sto:hasOfficialResource "https://www.iso.org/standard/66777.html" ;
    sto:hasPublicationDate "2017-02-01"^^xsd:date ;
    sto:hasPublisher sto:ISO .

sto:ISO_11898-1 a dbpcy:Abstraction100002137,
        dbpcy:Arrangement105726596,
        dbpcy:Artifact100021939,
        dbpcy:Bus102924116,
        dbpcy:BusTopology105730591,
        dbpcy:Cognition100023271,
        dbpcy:Communication100033020,
        dbpcy:ComputerNetwork103085333,
        dbpcy:Configuration105731779,
        dbpcy:Conveyance103100490,
        dbpcy:Design105728678,
        dbpcy:Direction106786629,
        dbpcy:Instrumentality103575240,
        dbpcy:Message106598915,
        dbpcy:Network103820728,
        dbpcy:Object100002684,
        dbpcy:PhysicalEntity100001930,
        dbpcy:Protocol106665108,
        dbpcy:PsychologicalFeature100023100,
        dbpcy:PublicTransport104019101,
        dbpcy:Rule106652242,
        dbpcy:Structure105726345,
        dbpcy:System104377057,
        dbpcy:Topology105730365,
        dbpcy:Whole100003553,
        dbpcy:WikicatComputerBuses,
        dbpcy:WikicatComputerNetworks,
        dbpcy:WikicatLinkProtocols,
        dbpcy:WikicatNetworkProtocols,
        dbpcy:WikicatSerialBuses,
        dbont:MeanOfTransportation,
        owl:NamedIndividual,
        owl:Thing,
        sto:Standard ;
    rdfs:label "ISO 11898-1"@en ;
    dcterms:subject dbrc:Automation,
        dbrc:Computer_networks,
        dbrc:Industrial_automation,
        dbrc:Industrial_computing,
        dbrc:Robert_Bosch_GmbH,
        dbrc:Serial_buses ;
    lingg:hypernym dbres:Vehicle ;
    rdfs:comment "Used mainly for Road vehicles Controller area network (CAN) Data link layer and physical signalling."@en ;
    sto:hasClassification rami:Communication,
        rami:Engineering,
        rami:Safety ;
    sto:hasDBpediaResource "http://dbpedia.org/page/CAN_bus" ;
    sto:hasDomain sto:IndustrialAutomation ;
    sto:hasOfficialResource "https://www.iso.org/standard/63648.html" ;
    sto:hasPublicationDate "2015-12-01"^^xsd:date ;
    sto:hasPublisher sto:ISO ;
    sto:hasTag "CAN Bus"@en ;
    sto:hasWikipediaArticle "http://en.wikipedia.org/wiki/CAN_bus" ;
    sto:relatedTo sto:ISO_11783 .

sto:ISO_1302 a owl:NamedIndividual,
        sto:Standard ;
    rdfs:label "ISO 1302"@en ;
    rdfs:comment "Geometrical product specifications Standards"@en ;
    sto:hasClassification sto:ModelingPractice ;
    sto:hasOfficialResource "https://www.iso.org/standard/28089.html" ;
    sto:hasPublicationDate "2002-02-01"^^xsd:date .

sto:ISO_13485 a dbpcy:Abstraction100002137,
        dbpcy:Measure100033615,
        dbpcy:Standard107260623,
        dbpcy:SystemOfMeasurement113577171,
        dbpcy:WikicatISOStandards,
        dbont:Organisation,
        owl:NamedIndividual,
        sto:Standard ;
    rdfs:label "ISO 13485"@en ;
    dcterms:subject dbrc:ISO_standards,
        dbrc:Medical_equipment,
        dbrc:Medical_technology,
        dbrc:Regulation_of_medical_devices ;
    lingg:hypernym dbres:Organization ;
    rdfs:comment "Medical devices -- Quality management systems -- Requirements for regulatory purposes."@en ;
    sto:hasClassification rami:Safety ;
    sto:hasDBpediaResource "http://dbpedia.org/page/ISO_13485" ;
    sto:hasOfficialResource "https://www.iso.org/iso-9001-quality-management.html" ;
    sto:hasPublisher sto:ISO ;
    sto:hasWikipediaArticle "http://en.wikipedia.org/wiki/ISO_13485" .

sto:ISO_14739-1 a owl:NamedIndividual,
        sto:Standard ;
    rdfs:label "ISO 14739-1"@en ;
    rdfs:comment "Document management -- 3D use of Product Representation Compact (PRC) format-ISO 14739-1:2014 describes PRC 10001 of a product representation compact (PRC) file format for three dimensional (3D) content data. This format is designed to be included in PDF (ISO 32000) and other similar document formats for the purpose of 3D visualization and exchange. "@en ;
    skos:altLabel "STEP"@en ;
    sto:hasClassification sto:ProductModelDataExchange ;
    sto:hasDomain sto:CAD ;
    sto:hasOfficialResource "https://www.iso.org/standard/54948.html" ;
    sto:hasPublicationDate "2014-12-01"^^xsd:date ;
    sto:hasPublisher sto:ISO .

sto:ISO_15531-2x a owl:NamedIndividual,
        sto:StandardPart ;
    rdfs:label "ISO 15531 2x series"@en ;
    rdfs:comment "Production data for external exchanges. refering to the representation of product information to be exchanged with the external environment (customers and suppliers), with the aim to model the main production information exchanged between industrial companies, in order to improve exchanges and integration through the use of EDI protocols."@en ;
    rdfs:isDefinedBy "https://www.researchgate.net/publication/220171079_ISO_15531_MANDATE_a_standardised_data_model_for_manufacturing_management" ;
    sto:isPartOf sto:ISO_15531 .

sto:ISO_15531-3x a owl:NamedIndividual,
        sto:StandardPart ;
    rdfs:label "ISO 15531 3x series"@en ;
    rdfs:comment "Manufacturing resource usage management data : refering to the way of managing the use of resources, such as resource configuration and capabilities, operation management of manufacturing devices, installations and facilities."@en ;
    rdfs:isDefinedBy "https://www.researchgate.net/publication/220171079_ISO_15531_MANDATE_a_standardised_data_model_for_manufacturing_management" ;
    sto:isPartOf sto:ISO_15531 .

sto:ISO_15531-4x a owl:NamedIndividual,
        sto:StandardPart ;
    rdfs:label "ISO 15531 4x series"@en ;
    rdfs:comment "Manufacturing flow management data : refering to the material flow control and aiming at the representation of data and elements supporting the control and monitoring of the flow of materials in manufacturing processes."@en ;
    rdfs:isDefinedBy "https://www.researchgate.net/publication/220171079_ISO_15531_MANDATE_a_standardised_data_model_for_manufacturing_management" ;
    sto:isPartOf sto:ISO_15531 .

sto:ISO_15704 a owl:NamedIndividual,
        sto:Standard ;
    rdfs:label "ISO 15704"@en ;
    rdfs:comment "Identifies requirements for enterprise-reference architectures and methodologies"@en ;
    sto:hasClassification rami:Business,
        rami:Enterprise,
        rami:Other ;
    sto:hasDomain sto:IndustrialAutomation ;
    sto:hasOfficialResource "https://www.iso.org/standard/28777.html" ;
    sto:hasPublicationDate "2000-06-01"^^xsd:date ;
    sto:hasPublisher sto:ISO ;
    sto:relatedTo sto:ISO_13374,
        sto:ISO_19439 .

sto:ISO_15746 a owl:NamedIndividual,
        sto:Standard ;
    rdfs:label "ISO 15746"@en ;
    rdfs:comment "Automation systems and integration -- Integration of advanced process control and optimization capabilities for manufacturing systems."@en ;
    sto:hasClassification rami:Communication,
        rami:ControlDevice,
        rami:Engineering,
        rami:FieldDevice,
        rami:Functional,
        rami:Information,
        rami:Integration,
        rami:Product,
        sto:ProductLifeCycleManagement ;
    sto:hasDomain sto:IndustrialAutomation ;
    sto:hasOfficialResource "https://www.iso.org/standard/61131.html" ;
    sto:hasPublicationDate "2015-04-01"^^xsd:date ;
    sto:hasPublisher sto:ISO ;
    sto:relatedTo sto:ISO_15926 .

sto:ISO_16739 a owl:NamedIndividual,
        sto:Standard ;
    rdfs:label "ISO 16739"@en ;
    rdfs:comment "Industry Foundation Classes (IFC) for data sharing in the construction and facility management industries."@en ;
    sto:hasClassification rami:LifecycleStatus,
        rami:Station,
        rami:WorkCenter,
        sto:ProductLifeCycleManagement ;
    sto:hasDomain sto:IndustrialAutomation ;
    sto:hasOfficialResource "https://www.iso.org/standard/51622.html" ;
    sto:hasPublicationDate "2013-04-01"^^xsd:date ;
    sto:hasPublisher sto:ISO ;
    sto:relatedTo sto:IEC_62890 .

sto:ISO_16792 a owl:NamedIndividual,
        sto:Standard ;
    rdfs:label "ISO 16792"@en ;
    rdfs:comment "ISO 16792 Technical product documentation -- Digital product definition data practices-It supports two methods of application: model-only and model and drawing in digital format."@en ;
    sto:hasClassification rami:Asset,
        rami:Product,
        sto:ModelingPractice ;
    sto:hasDomain sto:CAD ;
    sto:hasOfficialResource "https://www.iso.org/standard/56865.html" ;
    sto:hasPublicationDate "2015-12-01"^^xsd:date ;
    sto:hasPublisher sto:ISO .

sto:ISO_18629 a owl:NamedIndividual,
        sto:Standard ;
    rdfs:label "ISO 19629"@en ;
    rdfs:comment "ISO 18629-1:2004 provides a general overview of the different series of parts of ISO 18629, which defines a process specification language aimed at identifying, formally defining and structuring the semantic concepts intrinsic to the capture and exchange of process information related to discrete manufacturing."@en ;
    sto:hasClassification rami:Communication,
        rami:Configuration,
        rami:ControlDevice,
        rami:Engineering,
        rami:FieldDevice,
        rami:Functional,
        rami:Information,
        rami:Integration,
        rami:Product,
        sto:ProductModelDataExchange ;
    sto:hasDomain sto:IndustrialAutomation ;
    sto:hasOfficialResource "https://www.iso.org/standard/35431.html" ;
    sto:hasPublicationDate "2004-11-01"^^xsd:date ;
    sto:hasPublisher sto:ISO ;
    sto:hasTag "PSL"@en ;
    sto:hasWikipediaArticle "https://en.wikipedia.org/wiki/Process_Specification_Language" ;
    sto:relatedTo sto:ISO_15926,
        sto:ISO_ASTM_52915 .

sto:ISO_18828-2 a owl:NamedIndividual,
        sto:Standard ;
    rdfs:label "ISO 18828-2"@en ;
    rdfs:comment "Industrial automation systems and integration -- Standardized procedures for production systems engineering."@en ;
    sto:hasClassification rami:ControlDevice,
        rami:Engineering,
        rami:Enterprise,
        rami:FieldDevice,
        rami:Station,
        rami:WorkCenter,
        sto:Prodcut ;
    sto:hasDomain sto:IndustrialAutomation ;
    sto:hasOfficialResource "https://www.iso.org/standard/63505.html" ;
    sto:hasPublicationDate "2016-10-01"^^xsd:date ;
    sto:hasPublisher sto:ISO ;
    sto:relatedTo sto:IEC_61804 .

sto:ISO_19440 a owl:NamedIndividual,
        sto:Standard ;
    rdfs:label "ISO 19440"@en ;
    rdfs:comment "Enterprise integration -- Constructs for enterprise modelling-specifies the characteristics of the core constructs necessary for computer-supported modelling of enterprises conforming to ISO 19439.."@en ;
    sto:hasClassification rami:Engineering,
        rami:Enterprise,
        rami:Integration,
        sto:EnterpriseLevel,
        sto:Product ;
    sto:hasDomain sto:EnterpriseIntegration ;
    sto:hasOfficialResource "https://www.iso.org/standard/33834.html" ;
    sto:hasPublicationDate "2007-12-01"^^xsd:date ;
    sto:hasPublisher sto:ISO ;
    sto:relatedTo sto:BPMN .

sto:ISO_20140_5 a owl:NamedIndividual,
        sto:Standard ;
    rdfs:label "ISO 20140-5"@en ;
    rdfs:comment "Automation systems and integration -- Evaluating energy efficiency and other factors of manufacturing systems that influence the environment"@en ;
    sto:hasClassification rami:EnergyEfficiency ;
    sto:hasOfficialResource "http://www.iso.org/iso/catalogue_detail.htm?csnumber=54809" ;
    sto:hasPublisher sto:ISO ;
    sto:hasTag "Energy Efficiency"@en .

sto:ISO_20922 a dbpcy:Abstraction100002137,
        dbpcy:Communication100033020,
        dbpcy:Direction106786629,
        dbpcy:Message106598915,
        dbpcy:Protocol106665108,
        dbpcy:Rule106652242,
        dbpcy:WikicatApplicationLayerProtocols,
        dbpcy:WikicatNetworkProtocols,
        owl:NamedIndividual,
        sto:Standard ;
    rdfs:label "ISO 20922"@en ;
    dcterms:subject dbrc:Application_layer_protocols,
        dbrc:Data_transmission,
        dbrc:IBM_WebSphere,
        dbrc:Message-oriented_middleware,
        dbrc:Network_protocols,
        dbrc:Telemetry ;
    rdfs:comment "ISO/IEC 20922:2016 is a Client Server publish/subscribe messaging transport protocol. It is light weight, open, simple, and designed so as to be easy to implement. These characteristics make it ideal for use in many situations, including constrained environments such as for communication in Machine to Machine (M2M) and Internet of Things (IoT) contexts where a small code footprint is required and/or network bandwidth is at a premium."@en ;
    sto:hasDBpediaResource "http://dbpedia.org/resource/MQTT" ;
    sto:hasDeveloper sto:IBM,
        sto:OASIS ;
    sto:hasDomain sto:M2M ;
    sto:hasOfficialResource "http://mqtt.org/",
        "https://www.iso.org/standard/69466.html" ;
    sto:hasPublisher sto:IEC,
        sto:ISO ;
    sto:hasTag "MQTT"@en,
        "Message Queue Telemetry Transport"@en ;
    sto:hasWikipediaArticle "http://en.wikipedia.org/wiki/MQTT",
        "https://en.wikipedia.org/wiki/MQTT" ;
    sto:relatedTo sto:IEC_62541 .

sto:ISO_22400 a owl:NamedIndividual,
        sto:Standard ;
    rdfs:label "ISO 22400"@en ;
    rdfs:comment "Automation systems and integration -- Key performance indicators (KPIs) for manufacturing operations management."@en ;
    sto:hasClassification rami:Business,
        rami:Conditional_Monitoring,
        rami:ConnectedWorld,
        rami:ControlDevice,
        rami:Enterprise,
        rami:FieldDevice,
        rami:LifeCycle_Status,
        rami:Station,
        rami:WorkCenter ;
    sto:hasDomain sto:IndustrialAutomation ;
    sto:hasOfficialResource "https://www.iso.org/standard/54497.html" ;
    sto:hasPublicationDate "2014-01-01"^^xsd:date ;
    sto:hasPublisher sto:ISO ;
    sto:relatedTo sto:IEC_62541 .

sto:ISO_22745-11 a owl:NamedIndividual,
        sto:Standard ;
    rdfs:label "ISO 22745-11"@en ;
    rdfs:comment "ISO 22745-11:2010 provides guidelines that are recommended for the development of terminology for concepts in an open technical dictionary (OTD).Compliance with these guidelines is not required in order for a term or definition to be included in an OTD. These guidelines are provided as a framework for developers of industrial terminology to ensure that definitions are consistent and understandable. Terminology that complies with these guidelines will be marked as such in the OTD. This will allow a user to perform a search that filters terminology based on compliance with ISO 22745-11:2010."@en ;
    sto:hasClassification rami:Assest,
        rami:Product,
        sto:ProductCatalogData ;
    sto:hasDomain sto:IndustrialAutomation ;
    sto:hasOfficialResource "https://www.iso.org/standard/53999.html" ;
    sto:hasPublicationDate "2010-02-01"^^xsd:date ;
    sto:hasPublisher sto:ISO .

sto:ISO_27000 a owl:NamedIndividual,
        sto:Standard ;
    rdfs:label "IEC 27000"@en,
        "ISO 27000"@en,
        "ISO/IEC 27000"@en ;
    rdfs:comment "The ISO/IEC 27000 family of standards helps organizations keep information assets secure. Using this family of standards will help your organization manage the security of assets such as financial information, intellectual property, employee details or information entrusted to you by third parties."@en ;
    sto:hasDBpediaResource "http://dbpedia.org/resource/IEC_27000" ;
    sto:hasMotivation "Provides best practices for information security management. A critical issue for Industry 4.0 "@en ;
    sto:hasOfficialResource "http://www.27000.org/" ;
    sto:hasPublisher sto:ISO ;
    sto:hasTag "Information Security Management Systems"@en ;
    sto:hasWikipediaArticle "https://en.wikipedia.org/wiki/ISO/IEC_27000" .

sto:ISO_29002 a owl:NamedIndividual,
        sto:Standard ;
    rdfs:label "ISO 29002"@en ;
    rdfs:comment "ISO 29002 is an interoperability standard, which provides a repository to be used in various ISO XML formats. It is used in ontoML."@en ;
    sto:hasDomain sto:IndustrialProcessMeasurementControl ;
    sto:hasOfficialResource "https://www.iso.org/standard/53617.html" ;
    sto:hasPublicationDate "2010-04-01"^^xsd:date ;
    sto:hasPublisher sto:ISO ;
    sto:relatedTo sto:eClass .

sto:ISO_50001 a dbpcy:Abstraction100002137,
        dbpcy:Measure100033615,
        dbpcy:Standard107260623,
        dbpcy:SystemOfMeasurement113577171,
        dbpcy:WikicatISOStandards,
        dbont:Software,
        owl:NamedIndividual,
        sto:Standard ;
    rdfs:label "ISO 50001"@en ;
    dcterms:subject dbrc:Energy_economics,
        dbrc:ISO_standards ;
    lingg:hypernym dbres:Specification ;
    rdfs:comment "Energy management systems – Requirements with guidance for use is a specification created by the International Organization for Standardization (ISO) for an energy management system."@en ;
    sto:hasClassification sto:CrossLevel ;
    sto:hasDBpediaResource "http://dbpedia.org/page/ISO_50001" ;
    sto:hasOfficialResource "https://www.iso.org/iso-50001-energy-management.html" ;
    sto:hasPublisher sto:ISO ;
    sto:hasWikipediaArticle "http://en.wikipedia.org/wiki/ISO_50001" .

sto:ISO_5459 a owl:NamedIndividual,
        sto:Standard ;
    rdfs:label "ISO 5459"@en ;
    rdfs:comment "Geometrical product specifications (GPS) -- Geometrical tolerancing -- Datums and datum systems--ISO 5459:2011 specifies terminology, rules and methodology for the indication and understanding of datums and datum systems in technical product documentation"@en ;
    sto:hasClassification rami:Asset,
        rami:Product,
        sto:ModelingPractice ;
    sto:hasDomain sto:M2M ;
    sto:hasOfficialResource "https://www.iso.org/standard/40358.html" ;
    sto:hasPublicationDate "2011-08-01"^^xsd:date ;
    sto:hasPublisher sto:ISO .

sto:ISO_8062-4 a owl:NamedIndividual,
        sto:Standard ;
    rdfs:label "ISO 8062-4"@en ;
    rdfs:comment "Geometrical product specifications (GPS) -- Dimensional and geometrical tolerances for moulded parts -- General tolerances for castings using profile tolerancing in a general datum system"@en ;
    sto:hasClassification rami:Asset,
        rami:Product,
        sto:ProductionSystemModelData ;
    sto:hasOfficialResource "https://www.iso.org/standard/60774.html" ;
    sto:hasPublicationDate "2017-07-01"^^xsd:date ;
    sto:hasPublisher sto:ISO ;
    sto:hasTag "Automation systems and integration"@en ;
    sto:relatedTo sto:ISO_10303 .

sto:ISO_9000 a dbpcy:Abstraction100002137,
        dbpcy:Measure100033615,
        dbpcy:Standard107260623,
        dbpcy:SystemOfMeasurement113577171,
        dbpcy:WikicatBritishStandards,
        dbpcy:WikicatISOStandards,
        owl:NamedIndividual,
        sto:Standard ;
    rdfs:label "ISO 9000"@en ;
    dcterms:subject dbrc:ISO_standards,
        dbrc:Quality,
        dbrc:Quality_management ;
    rdfs:comment "The ISO 9000 family of quality management systems standards is designed to help organizations ensure that they meet the needs of customers and other stakeholders while meeting statutory and regulatory requirements related to a product or program."@en ;
    sto:hasClassification sto:CrossLevel ;
    sto:hasDBpediaResource "http://dbpedia.org/page/ISO_9000" ;
    sto:hasOfficialResource "https://www.iso.org/iso-9001-quality-management.html" ;
    sto:hasPublisher sto:ISO ;
    sto:hasWikipediaArticle "http://en.wikipedia.org/wiki/ISO_9000",
        "https://en.wikipedia.org/wiki/ISO_9000" .

sto:ISO_PAS_17506 a dbpcy:Abstraction100002137,
        dbpcy:Communication100033020,
        dbpcy:Format106636806,
        dbpcy:Information106634376,
        dbpcy:Measure100033615,
        dbpcy:Message106598915,
        dbpcy:Standard107260623,
        dbpcy:SystemOfMeasurement113577171,
        dbpcy:Wikicat3DGraphicsFileFormats,
        dbpcy:WikicatCADFileFormats,
        dbpcy:WikicatComputerFileFormats,
        dbpcy:WikicatGraphicsFileFormats,
        dbpcy:WikicatGraphicsStandards,
        dbpcy:WikicatXML-basedStandards,
        dbont:Software,
        owl:NamedIndividual,
        sto:Standard ;
    rdfs:label "ISO PAS 17506"@en ;
    dcterms:subject <http://dbpedia.org/resource/Category:2004_software>,
        <http://dbpedia.org/resource/Category:3D_graphics_file_formats>,
        <http://dbpedia.org/resource/Category:3D_graphics_software>,
        dbrc:CAD_file_formats,
        dbrc:Graphics_standards,
        dbrc:XML-based_standards ;
    lingg:hypernym dbres:Format ;
    rdfs:comment "ISO-PAS 17506-2012 describes the COLLADA schema. COLLADA is a COLLAborative Design Activity that defines an XML-based schema to enable 3D authoring applications to freely exchange digital assets without loss of information, enabling multiple software packages to be combined into extremely powerful tool chains."@en,
        "SO/PAS 17506:2012 describes the COLLADA schema. COLLADA is a COLLAborative Design Activity that defines an XML-based schema to enable 3D authoring applications to freely exchange digital assets without loss of information, enabling multiple software packages to be combined into extremely powerful tool chains. The purpose of ISO/PAS 17506:2012 is to provide a specification for the COLLADA schema in sufficient detail to enable software developers to create tools to process COLLADA resources. In particular, it is relevant to those who import to or export from digital content creation (DCC) applications, 3D interactive applications and tool chains, prototyping tools, real-time visualization applications such as those used in the video game and movie industries, and CAD tools. ISO/PAS 17506:2012 covers the initial design and specifications of the COLLADA schema, as well as a minimal set of requirements for COLLADA exporters. "@en ;
    sto:hasDBpediaResource "http://dbpedia.org/resource/COLLADA" ;
    sto:hasDeveloper sto:ISO ;
    sto:hasOfficialResource "https://www.iso.org/standard/59902.html" ;
    sto:hasPublisher sto:ISO ;
    sto:hasTag "COLLADA"@en ;
    sto:hasWikipediaArticle "http://en.wikipedia.org/wiki/COLLADA",
        "https://en.wikipedia.org/wiki/COLLADA" ;
    sto:isPartOf sto:IEC_62714 .

sto:ISO_TS_14649-201 a owl:NamedIndividual,
        sto:Standard ;
    rdfs:label "ISO TS 14649-201"@en ;
    rdfs:comment "SO/TS 14649-201:2011 specifies the technology-specific machine tool description data elements needed as process data for manufacturing and machine characteristics. The machine tool descriptions covered in this schema are, initially, milling machines, machining centres, turning machines and multi-tasking machines.ISO/TS 14649-201:2011 is not intended to replace existing machine tool description standards, but to cover the specific needs of manufacturing resource description for manufacturing needs in the technologies described in ISO 14649."@en ;
    sto:hasClassification rami:Assest,
        rami:Configuration,
        rami:Engineering,
        rami:Integration,
        rami:Product,
        rami:Safety,
        sto:ProductionSystemModelData ;
    sto:hasDomain sto:IndustrialAutomation ;
    sto:hasOfficialResource "https://www.iso.org/standard/60042.html" ;
    sto:hasPublicationDate "2011-12-01"^^xsd:date ;
    sto:hasPublisher sto:ISO .

sto:KATS a dbont:Organisation,
        owl:NamedIndividual,
        sto:StandardOrganization ;
    rdfs:label "Korean Agency for Technology and Standards"@en ;
    dcterms:subject dbrc:ISO_member_bodies ;
    lingg:hypernym dbres:Organization ;
    dul:isMemberOf sto:IEC,
        sto:ISO ;
    rdfs:comment "Korean Agency for Technology and Standards is the government standards organization for South Korea. It is part of the Ministry of Knowledge Economy. It is authorized to regulate and manage the legal measures of South Korea by the current Measures Act."@en ;
    sto:abbreviation "KATS"@de ;
    sto:belongsTo dbr:South_Korea ;
    sto:hasDBpediaResource "http://dbpedia.org/page/Korean_Agency_for_Technology_and_Standards" ;
    sto:hasHeadquaterIn dbr:Eumseong ;
    sto:hasWikipediaArticle "http://en.wikipedia.org/wiki/Korean_Agency_for_Technology_and_Standards",
        "https://en.wikipedia.org/wiki/Korean_Agency_for_Technology_and_Standards" ;
    sto:orgName "Korean Agency for Technology and Standards"@en .

sto:MIIT a dbont:Agent,
        dbont:GovernmentAgency,
        dbont:Organisation,
        schema:Organization,
        dul:Agent,
        dul:SocialPerson,
        owl:NamedIndividual,
        owl:Thing,
        wike:Q24229398,
        wike:Q327333,
        wike:Q43229,
        sto:StandardOrganization ;
    dcterms:subject <http://dbpedia.org/resource/Category:2008_establishments_in_China>,
        dbrc:Communications_ministries,
        <http://dbpedia.org/resource/Category:Government_ministries_of_the_People's_Republic_of_China>,
        dbrc:Information_ministries,
        dbrc:Ministries_established_in_2008,
        <http://dbpedia.org/resource/Category:Ministry_of_Industry_and_Information_Technology_of_the_People's_Republic_of_China>,
        dbrc:Organizations_based_in_Beijing ;
    lingg:hypernym dbres:Agency ;
    rdfs:comment "Ministry of Industry and Information Technology (MIIT) of the Chinese government, established in March 2008, is the state agency of the People's Republic of China responsible for regulation and development of the postal service, Internet, wireless, broadcasting, communications, production of electronic and information goods, software industry and the promotion of the national knowledge economy."@en ;
    sto:abbreviation "MIIT" ;
    sto:belongsTo dbr:China ;
    sto:formationDate "2008-03-01"^^xsd:date ;
    sto:hasDBpediaResource "http://dbpedia.org/page/Ministry_of_Industry_and_Information_Technology" ;
    sto:hasHeadquaterIn dbr:Beijing ;
    sto:hasOfficialResource "http://www.miit.gov.cn/" ;
    sto:hasWikipediaArticle "http://en.wikipedia.org/wiki/Ministry_of_Industry_and_Information_Technology",
        "https://en.wikipedia.org/wiki/Ministry_of_Industry_and_Information_Technology" ;
    sto:orgName "Ministry of Industry and Information Technology"@en .

sto:MOMLevel a owl:NamedIndividual,
        sto:ISA95Level ;
    rdfs:label "MOM Level"@en ;
    rdfs:comment "Describes the MOM level according to the ISA95 level classification."@en ;
    skos:definition "Manufacturing Operation Management Level according to ISA 95"@en .

sto:MTConnect a dbpcy:Abstraction100002137,
        dbpcy:Measure100033615,
        dbpcy:Standard107260623,
        dbpcy:SystemOfMeasurement113577171,
        dbpcy:WikicatIndustry-specificXML-basedStandards,
        dbont:Company,
        owl:NamedIndividual,
        sto:Standard ;
    rdfs:label "MTConnect"@en ;
    dcterms:subject dbrc:Automation,
        dbrc:Computer-aided_manufacturing,
        dbrc:Industrial_computing,
        dbrc:Industry-specific_XML-based_standards ;
    lingg:hypernym dbres:Industry ;
    rdfs:comment "MTConnect is a protocol designed for the exchange of data between shop floor equipment and software applications used for monitoring and data analysis. MTConnect is referred to as a read-only standard, meaning that it only defines the extraction (reading) of data from control devices, not the writing of data to a control device. Freely available, open standards are used for all aspects of MTConnect. Data from shop floor devices is presented in XML format, and is retrieved from information providers, called Agents, using Hypertext Transfer Protocol (HTTP) as the underlying transport protocol. MTConnect provides a RESTful interface, which means the interface is stateless. No session must be established to retrieve data from an MTConnect Agent, and no logon or logoff sequence is required (unless overlying security protocols are added which do). Lightweight Directory Access Protocol (LDAP) is recommended for discovery services."@en ;
    sto:hasClassification sto:DeviceLevel ;
    sto:hasDBpediaResource "http://dbpedia.org/resource/MTConnect" ;
    sto:hasDeveloper sto:MTConnect_Institute ;
    sto:hasOfficialResource "http://www.mtconnect.org/standard-documents" ;
    sto:hasPublisher sto:MTConnect_Institute ;
    sto:hasTag "MTConnect"@en ;
    sto:hasWikipediaArticle "http://en.wikipedia.org/wiki/MTConnect",
        "https://en.wikipedia.org/wiki/MTConnect" .

sto:Manufacturing a owl:NamedIndividual .

sto:ModBus a dbpcy:Abstraction100002137,
        dbpcy:Arrangement105726596,
        dbpcy:BusTopology105730591,
        dbpcy:Cognition100023271,
        dbpcy:Communication100033020,
        dbpcy:Configuration105731779,
        dbpcy:Design105728678,
        dbpcy:Direction106786629,
        dbpcy:Message106598915,
        dbpcy:Protocol106665108,
        dbpcy:PsychologicalFeature100023100,
        dbpcy:Rule106652242,
        dbpcy:Structure105726345,
        dbpcy:Topology105730365,
        dbpcy:WikicatComputerBuses,
        dbpcy:WikicatNetworkProtocols,
        dbpcy:WikicatOSIProtocols,
        dbont:Software,
        owl:NamedIndividual,
        sto:Standard ;
    rdfs:label "ModBus"@en ;
    dcterms:subject dbrc:Automation,
        dbrc:Building_automation,
        dbrc:Industrial_Ethernet,
        dbrc:Industrial_computing,
        dbrc:Network_protocols ;
    lingg:hypernym dbres:Protocol ;
    rdfs:comment "Modbus is a serial communications protocol to be used in Programmable logic controllers (PLCs)."@en ;
    sto:hasClassification rami:Integration ;
    sto:hasDBpediaResource "http://dbpedia.org/page/Modbus" ;
    sto:hasOfficialResource "http://www.modbus.org/" ;
    sto:hasPublisher sto:SE ;
    sto:hasTag "Modbus"@en ;
    sto:hasWikipediaArticle "http://en.wikipedia.org/wiki/Modbus",
        "https://en.wikipedia.org/wiki/Modbus" .

sto:NIST a dbont:Agent,
        dbont:GovernmentAgency,
        dbont:Organisation,
        schema:Organization,
        dul:Agent,
        dul:SocialPerson,
        owl:NamedIndividual,
        owl:Thing,
        wike:Q24229398,
        wike:Q327333,
        wike:Q43229,
        sto:StandardOrganization ;
    dcterms:subject <http://dbpedia.org/resource/Category:1901_establishments_in_the_United_States>,
        <http://dbpedia.org/resource/Category:Buildings_and_structures_in_Gaithersburg,_Maryland>,
        dbrc:Cryptography_organizations,
        dbrc:Government_agencies_established_in_1901,
        dbrc:National_Institute_of_Standards_and_Technology,
        dbrc:Standards_organizations,
        dbrc:United_States_Department_of_Commerce_agencies ;
    lingg:hypernym dbres:Laboratory ;
    rdfs:comment "The National Institute of Standards and Technology (NIST) is a measurement standards laboratory, and a non-regulatory agency of the United States Department of Commerce."@en ;
    sto:abbreviation "NIST" ;
    sto:belongsTo dbr:United_States ;
    sto:formationDate "1901-01-01"^^xsd:date ;
    sto:hasDBpediaResource "http://dbpedia.org/page/National_Institute_of_Standards_and_Technology" ;
    sto:hasHeadquaterIn dbr:_Maryland ;
    sto:hasOfficialResource "https://www.nist.gov/" ;
    sto:hasWikipediaArticle "http://en.wikipedia.org/wiki/National_Institute_of_Standards_and_Technology",
        "https://en.wikipedia.org/wiki/National_Institute_of_Standards_and_Technology" ;
    sto:orgName "National Institute of Standards and Technology"@en .

sto:NISTIR_8107 a owl:NamedIndividual ;
    rdfs:label "NISTIR_8107"@en ;
    rdfs:comment "Describes the NIST Initiative"@en ;
    rdfs:isDefinedBy "http://nvlpubs.nist.gov/nistpubs/ir/2016/NIST.IR.8107.pdf" ;
    skos:note "TODO - improve this classification" ;
    sto:isDescribedin sto:BusinessProcessExecution,
        sto:SCM .

sto:OAGIS a owl:NamedIndividual,
        sto:Standard ;
    rdfs:label "OAGIS"@en ;
    rdfs:comment "The Open Applications Group Integration Specification (OAGIS) is an effort to provide a canonical business language for information integration. It uses XML as the common alphabet for defining business messages, and for identifying business processes (scenarios) that allow businesses and business applications to communicate."@en ;
    sto:hasOfficialResource "http://www.oagi.org/dnn2/DownloadsandResources/OAGIS100PublicDownload.aspx" ;
    sto:hasPublisher sto:OAGi ;
    sto:hasTag "Open Applications Group Integration Specification"@en ;
    sto:hasWikipediaArticle "https://de.wikipedia.org/wiki/Open_Application_Group_Integration_Specification" .

sto:ODVA a dbpcy:Abstraction100002137,
        dbpcy:Group100031264,
        dbpcy:Organization108008335,
        dbpcy:SocialGroup107950920,
        dbpcy:WikicatComputerNetworkOrganizations,
        dbpcy:YagoLegalActor,
        dbpcy:YagoLegalActorGeo,
        dbpcy:YagoPermanentlyLocatedEntity,
        owl:NamedIndividual,
        sto:StandardOrganization ;
    dcterms:subject dbrc:Computer_network_organizations ;
    rdfs:comment "Founded in 1995, ODVA is a global association whose members comprise the world’s leading automation companies. ODVA’s mission is to advance open, interoperable information and communication technologies in industrial automation. ODVA recognizes its media independent network protocol, the Common Industrial Protocol or “CIP” — and the network adaptations of CIP — EtherNet/IP, DeviceNet, CompoNet and ControlNet — as its core technology and the primary common interest of its membership. For future interoperability of production systems and the integration of the production systems with other systems, ODVA embraces the adoption of commercial-off-the-shelf (COTS) and standard, unmodified Internet and Ethernet technologies as a guiding principle wherever possible. This principle is exemplified by EtherNet/IP — the world’s number one industrial Ethernet network."@en ;
    sto:abbreviation "ODVA" ;
    sto:formationDate "1995-01-01"^^xsd:date ;
    sto:hasDBpediaResource "http://dbpedia.org/resource/ODVA_(company)" ;
    sto:hasHeadquaterIn dbr:_Michigan ;
    sto:hasOfficialResource "https://www.odva.org" ;
    sto:hasWikipediaArticle "http://en.wikipedia.org/wiki/ODVA_(company)",
        "https://en.wikipedia.org/wiki/ODVA_(company)" ;
    sto:orgName "ODVA, Inc"@en .

sto:OMG_DDS a dbpcy:Abstraction100002137,
        dbpcy:Measure100033615,
        dbpcy:Standard107260623,
        dbpcy:SystemOfMeasurement113577171,
        dbpcy:WikicatComputerStandards,
        dbont:Software,
        owl:NamedIndividual,
        sto:Standard ;
    rdfs:label "OMG DDS"@en ;
    dcterms:subject dbrc:Computer_standards,
        dbrc:Message-oriented_middleware ;
    lingg:hypernym dbres:Middleware ;
    rdfs:comment "The Data Distribution Service for real-time systems (DDS) is an Object Management Group (OMG) machine-to-machine (sometimes called middleware) standard that aims to enable scalable, real-time, dependable, high-performance and interoperable data exchanges using a publish–subscribe pattern. DDS addresses the needs of applications like financial trading, air-traffic control, smart grid management, and other big data applications. The standard is used in applications such as smartphone operating systems, transportation systems and vehicles, software-defined radio, and by healthcare providers. DDS was promoted for use in the Internet of things."@en ;
    sto:hasDBpediaResource "http://dbpedia.org/page/Data_Distribution_Service" ;
    sto:hasOfficialResource "http://portals.omg.org/dds/" ;
    sto:hasPublisher sto:OMG ;
    sto:hasTag "Data Distribution Service for real-time systems"@en ;
    sto:hasWikipediaArticle "http://en.wikipedia.org/wiki/Data_Distribution_Service",
        "https://en.wikipedia.org/wiki/Data_Distribution_Service" ;
    sto:relatedTo sto:IEC_61158 .

sto:ProductionSystemMaintenance a owl:NamedIndividual,
        sto:ProductionSystemLifeCycle ;
    rdfs:label "Production System Maintenance"@en ;
    rdfs:comment "Classifies standards define data processing, communication, and presentation standards for condition monitoring and diagnostics of machines, for maintaining the adequate performance of the system, and for searching ways to improve performance"@en ;
    sto:isDescribedin sto:NISTInitiative .

sto:QIF a owl:NamedIndividual,
        sto:Standard ;
    rdfs:label "Quality Information Framework"@en ;
    rdfs:comment " Quality Information Framework (QIF) standard defines an integrated set of information models which enable the effective exchange of metrology data throughout the entire manufacturing quality measurement process"@en ;
    rdfs:isDefinedBy "http://qifstandards.org/about-qif/" ;
    skos:note "Is implemented in XML" ;
    sto:hasOfficialResource "http://qifstandards.org/" ;
    sto:hasPublisher sto:DMSC .

sto:RAMI a owl:NamedIndividual ;
    rdfs:label "RAMI"@en ;
    rdfs:comment "Describes the RAMI model"@en ;
    rdfs:isDefinedBy "https://www.plattform-i40.de/I40/Redaktion/EN/Downloads/Publikation/structure-of-the-administration-shell.html" ;
    sto:isDescribedin rami:InformationLayer .

sto:SCOR a dbpcy:Assistant109815790,
        dbpcy:CausalAgent100007347,
        dbpcy:LivingThing100004258,
        dbpcy:Model110324560,
        dbpcy:Object100002684,
        dbpcy:Organism100004475,
        dbpcy:Person100007846,
        dbpcy:PhysicalEntity100001930,
        dbpcy:Whole100003553,
        dbpcy:WikicatBusinessModels,
        dbpcy:Worker109632518,
        dbpcy:YagoLegalActor,
        dbpcy:YagoLegalActorGeo,
        dbont:Person,
        owl:NamedIndividual,
        sto:Standard ;
    rdfs:label "SCOR"@en ;
    dcterms:subject dbrc:Business_models,
        dbrc:Supply_chain_management ;
    lingg:hypernym dbres:Model ;
    rdfs:comment "APICS Supply Chain Operations Reference."@en ;
    sto:hasClassification sto:SCM ;
    sto:hasDBpediaResource "http://dbpedia.org/page/Supply-chain_operations_reference" ;
    sto:hasDeveloper sto:APICS ;
    sto:hasOfficialResource "http://www.apics.org/apics-for-business/products-and-services/apics-scc-frameworks/scor" ;
    sto:hasTag "SCOR"@en ;
    sto:hasWikipediaArticle "http://en.wikipedia.org/wiki/Supply-chain_operations_reference",
        "https://en.wikipedia.org/wiki/Supply-chain_operations_reference" .

sto:SysML a dbpcy:Artifact100021939,
        dbpcy:Instrumentality103575240,
        dbpcy:Object100002684,
        dbpcy:PhysicalEntity100001930,
        dbpcy:System104377057,
        dbpcy:Whole100003553,
        dbpcy:WikicatSystemsModelingLanguage,
        dbont:Language,
        owl:NamedIndividual,
        owl:Thing,
        sto:Standard ;
    rdfs:label "Systems Modeling Language"@en ;
    dcterms:subject dbrc:Systems_Modeling_Language,
        dbrc:Systems_engineering,
        dbrc:Unified_Modeling_Language ;
    lingg:hypernym dbres:Language ;
    rdfs:comment "The OMG Systems Modeling Language (OMG SysML) is a general-purpose graphical modeling language for specifying, analyzing, designing, and verifying complex systems that may include hardware, software, information, personnel, procedures, and facilities. In particular, the language provides graphical representations with a semantic foundation for modeling system requirements, behavior, structure, and parametrics, which is used to integrate with other engineering analysis models. It represents a subset of UML 2 with extensions needed to satisfy the requirements of the UML for Systems Engineering RFP as indicated in Figure 1. SysML leverages the OMG XML Metadata Interchange (XMI®) to exchange modeling data between tools, and is also intended to be compatible with the evolving ISO 10303-233 systems engineering data interchange standard."@en ;
    sto:hasDBpediaResource "http://dbpedia.org/resource/Systems_Modeling_Language" ;
    sto:hasDeveloper sto:OMG ;
    sto:hasOfficialResource "http://sysml.org/",
        "http://www.omgsysml.org/what-is-sysml.htm" ;
    sto:hasPublisher sto:OMG ;
    sto:hasTag "SysML"@en ;
    sto:hasWikipediaArticle "http://en.wikipedia.org/wiki/Systems_Modeling_Language",
        "https://en.wikipedia.org/wiki/Systems_Modeling_Language" ;
    sto:relatedTo sto:IEC_62714 .

sto:VDMA_24582 a owl:NamedIndividual,
        sto:Standard ;
    rdfs:label "VDMA 24582"@en ;
    rdfs:comment "Fieldbus neutral reference architecture for Condition Monitoring in production automation"@en ;
    sto:hasClassification rami:ConditionMonitoring ;
    sto:hasOfficialResource "https://www.vdma.org/documents/105628/2244593/Inhalt+VDMA+24582_en.pdf/" ;
    sto:hasPublisher sto:VDMA ;
    sto:hasTag "Condition Monitoring"@en .

sto:W3C_RIF a dbpcy:Abstraction100002137,
        dbpcy:CommandLanguage106899446,
        dbpcy:Communication100033020,
        dbpcy:Language106282651,
        dbpcy:Measure100033615,
        dbpcy:SourceLanguage106283912,
        dbpcy:Standard107260623,
        dbpcy:SystemOfMeasurement113577171,
        dbpcy:WikicatKnowledgeRepresentationLanguages,
        dbpcy:WikicatQueryLanguages,
        dbpcy:WikicatWorldWideWebConsortiumStandards,
        dbont:ProgrammingLanguage,
        owl:NamedIndividual,
        sto:Standard ;
    rdfs:label "Rule Interchange Format"@en ;
    dcterms:hasLicense "Public"@en ;
    dcterms:subject dbrc:Knowledge_representation_languages,
        dbrc:Semantic_Web,
        dbrc:World_Wide_Web ;
    lingg:hypernym dbres:Recommendation ;
    rdfs:comment "The Rule Interchange Format (RIF) is a W3C Recommendation. RIF is part of the infrastructure for the semantic web, along with (principally) SPARQL, RDF and OWL. Although originally envisioned by many as a rules layer for the semantic web, in reality the design of RIF is based on the observation that there are many rules languages in existence, and what is needed is to exchange rules between them."@en ;
    sto:hasDBpediaResource "http://dbpedia.org/resource/Rule_Interchange_Format" ;
    sto:hasOfficialResource "https://www.w3.org/TR/rif-overview/" ;
    sto:hasPublisher sto:W3C ;
    sto:hasTag "RIF"@en ;
    sto:hasWikipediaArticle "http://en.wikipedia.org/wiki/Rule_Interchange_Format",
        "https://en.wikipedia.org/wiki/Rule_Interchange_Format" ;
    sto:relatedTo sto:W3C_OWL .

sto:W3C_SPARQL a dbpcy:Abstraction100002137,
        dbpcy:Act100030358,
        dbpcy:Activity100407535,
        dbpcy:ArtificialLanguage106894544,
        dbpcy:Cognition100023271,
        dbpcy:CommandLanguage106899446,
        dbpcy:Communication100033020,
        dbpcy:ComputerLanguage106899633,
        dbpcy:Datum105816622,
        dbpcy:Event100029378,
        dbpcy:Information105816287,
        dbpcy:Language106282651,
        dbpcy:Measure100033615,
        dbpcy:ProgrammingLanguage106898352,
        dbpcy:PsychologicalFeature100023100,
        dbpcy:Service100577525,
        dbpcy:SourceLanguage106283912,
        dbpcy:Standard107260623,
        dbpcy:SystemOfMeasurement113577171,
        dbpcy:WikicatComputerLanguages,
        dbpcy:WikicatDataModelingLanguages,
        dbpcy:WikicatQueryLanguages,
        dbpcy:WikicatWebServices,
        dbpcy:WikicatWorldWideWebConsortiumStandards,
        dbpcy:Work100575741,
        dbpcy:YagoPermanentlyLocatedEntity,
        dbont:Language,
        dbont:ProgrammingLanguage,
        schema:Language,
        owl:NamedIndividual,
        owl:Thing,
        wike:Q315,
        wike:Q34770,
        wike:Q9143,
        sto:Standard ;
    rdfs:label "SPARQL"@en ;
    dcterms:hasLicense "Public"@en ;
    dcterms:subject dbrc:Data_modeling_languages,
        dbrc:Declarative_programming_languages,
        dbrc:Query_languages,
        dbrc:RDF_data_access,
        dbrc:Resource_Description_Framework,
        dbrc:Web_services,
        dbrc:World_Wide_Web_Consortium_standards ;
    lingg:hypernym dbres:Language ;
    rdfs:comment "The SPARQL Protocol and RDF Query Language (SPARQL) is a query language and protocol for RDF. This document specifies the SPARQL Protocol; it describes a means for conveying SPARQL queries and updates to a SPARQL processing service and returning the results via HTTP to the entity that requested them. This protocol was developed by the W3C SPARQL Working Group, part of the Semantic Web Activity as described in the activity statement ."@en ;
    sto:hasDBpediaResource "http://dbpedia.org/resource/SPARQL" ;
    sto:hasOfficialResource "https://www.w3.org/SPARQL" ;
    sto:hasPublisher sto:W3C ;
    sto:hasTag "SPARQL"@en ;
    sto:hasWikipediaArticle "http://en.wikipedia.org/wiki/SPARQL",
        "https://en.wikipedia.org/wiki/SPARQL" ;
    sto:relatedTo sto:W3C_RDF .

sto:abbreviation a owl:DatatypeProperty ;
    rdfs:label "has Abbreviated Name"@en ;
    rdfs:comment "Abbreviated  name of the organization"@en ;
    rdfs:domain owl:thing ;
    rdfs:range rdf:PlainLiteral .

sto:belongsTo a owl:ObjectProperty ;
    rdfs:label "belongs To"@en ;
    rdfs:comment "A Standard Organization that belongs to the country"@en ;
    rdfs:domain sto:StandardOrganization ;
    rdfs:range dbo:Country .

sto:domainName a owl:DatatypeProperty ;
    rdfs:label "has Domain Name"@en ;
    rdfs:comment "Points the Standard with the name of the Industrial Domain"@en ;
    rdfs:domain sto:Domain ;
    rdfs:range rdf:PlainLiteral .

sto:ebXML a dbpcy:Abbreviation107091587,
        dbpcy:Abstraction100002137,
        dbpcy:Act100030358,
        dbpcy:Activity100407535,
        dbpcy:Cognition100023271,
        dbpcy:Communication100033020,
        dbpcy:Datum105816622,
        dbpcy:Event100029378,
        dbpcy:Form106290637,
        dbpcy:Format106636806,
        dbpcy:Information105816287,
        dbpcy:Information106634376,
        dbpcy:LanguageUnit106284225,
        dbpcy:MarkupLanguage106787835,
        dbpcy:Measure100033615,
        dbpcy:Message106598915,
        dbpcy:Part113809207,
        dbpcy:PsychologicalFeature100023100,
        dbpcy:Relation100031921,
        dbpcy:Service100577525,
        dbpcy:Standard107260623,
        dbpcy:SystemOfMeasurement113577171,
        dbpcy:Terminology106304059,
        dbpcy:WikicatAbbreviations,
        dbpcy:WikicatComputerFileFormats,
        dbpcy:WikicatDataInterchangeStandards,
        dbpcy:WikicatDataModelingLanguages,
        dbpcy:WikicatMarkupLanguages,
        dbpcy:WikicatWebServices,
        dbpcy:WikicatWorldWideWebConsortiumStandards,
        dbpcy:WikicatXML-basedStandards,
        dbpcy:Word106286395,
        dbpcy:Work100575741,
        dbpcy:YagoPermanentlyLocatedEntity,
        owl:NamedIndividual,
        sto:Standard ;
    rdfs:label "ebXML"@en ;
    dcterms:subject dbrc:Computer_file_formats,
        dbrc:Data_modeling_languages,
        dbrc:Technical_communication,
        dbrc:World_Wide_Web_Consortium_standards,
        dbrc:XML-based_standards,
        dbrc:XML_markup_languages ;
    lingg:hypernym dbres:Family ;
    rdfs:comment "Electronic Business using eXtensible Markup Language, commonly known as e-business XML, or ebXML is a family of XML based standards whose mission is to provide an open, XML-based infrastructure that enables the global use of electronic business information in an interoperable, secure, and consistent manner by all trading partners."@en ;
    sto:hasClassification sto:BusinessProcessExecution ;
    sto:hasDBpediaResource "http://dbpedia.org/resource/EbXML" ;
    sto:hasOfficialResource "https://webstore.iec.ch/publication/24433" ;
    sto:hasPublisher sto:OASIS,
        sto:UN-CEFACT ;
    sto:hasTag "ebXML"@en ;
    sto:hasWikipediaArticle "http://en.wikipedia.org/wiki/EbXML",
        "https://en.wikipedia.org/wiki/EbXML" .

sto:edition a owl:AnnotationProperty .

sto:formationDate a owl:DatatypeProperty ;
    rdfs:label "has Formation Date"@en ;
    rdfs:comment "Formation date of the Organization"@en ;
    rdfs:domain sto:StandardOrganization ;
    rdfs:range xsd:date .

sto:hasAvailableLanguage a owl:DatatypeProperty ;
    rdfs:label "has Available Language"@en ;
    rdfs:comment "Languages in which the document of the Standard is available, e.g., English, French, Spanish"@en ;
    rdfs:subPropertyOf dcterms:language .

sto:hasClassification a owl:ObjectProperty ;
    rdfs:label "has Classification"@en ;
    rdfs:comment "An Standard is isCategorizedBy a given Categorization Area which is connected to a specific Standarization Initiative"@en ;
    rdfs:domain sto:Standard ;
    rdfs:range sto:StandardClassification .

sto:hasDBpediaResource a owl:DatatypeProperty ;
    rdfs:label "has DBpedia Resource"@en ;
    rdfs:comment "Instance's DBpedia Resource"@en ;
    rdfs:range xsd:string .

sto:hasDeveloper a owl:ObjectProperty ;
    rdfs:label "has Developer"@en ;
    rdfs:comment "The organization that developed this Standard"@en ;
    rdfs:domain sto:Standard ;
    rdfs:range sto:StandardOrganization ;
    rdfs:subPropertyOf foaf:maker .

sto:hasDomain a owl:ObjectProperty ;
    rdfs:label "has Domain"@en ;
    rdfs:comment "Describes the domain, in which the standard is used"@en ;
    rdfs:domain sto:Standard ;
    rdfs:range sto:Domain .

sto:hasFileSize a owl:ObjectProperty ;
    rdfs:label "has File Size"@en ;
    rdfs:comment "The size of document file in some unit e.g. 104 Kilobyte."@en ;
    rdfs:domain foaf:Document ;
    rdfs:range om2:Measure ;
    rdfs:seeAlso <https://webstore.iec.ch/webstore/webstore.nsf/xpFAQ.xsp?Open&id=ADMN-7NALM5> ;
    skos:note """1. Reference for om2:Measure <http://www.ontology-of-units-of-measure.org/page/om-2/Measure>
                         2. om2:Measure om2:hasNumericalValue xsd:float;
                         3. om2:Measure om2:hasUnit om2:Unit;
                         4. om2:hasUnit om2:InformationCapacityUnit; is another possibility for range that could not be verified.
                         5. rdfs:seeAlso <http://www.ontology-of-units-of-measure.org/page/om-2/kilobyte> 
                         6. Documentation on Measure <https://github.com/HajoRijgersberg/OM>""" .

sto:hasHeadquaterIn a owl:ObjectProperty ;
    rdfs:label "has Headquater In"@en ;
    rdfs:comment "Denotes the countries in which the Headquarter of the organization who publishes the Standart"@en ;
    rdfs:domain sto:StandardOrganization ;
    rdfs:range dbo:Place .

sto:hasImplementationFormat a owl:DatatypeProperty ;
    rdfs:label "has Implementation Format"@en ;
    rdfs:comment "Describes the name of the implementation or serialization format of the standard, e.g., XML, Document, binary, batch"@en ;
    rdfs:domain sto:Standard ;
    rdfs:range xsd:string .

sto:hasMotivation a owl:ObjectProperty ;
    rdfs:label "has Motivation"@en ;
    rdfs:comment "Describes the motivation of the standards"@en ;
    rdfs:domain sto:Standard ;
    rdfs:range deo:Motivation .

sto:hasObjective a owl:DatatypeProperty ;
    rdfs:label "has Objective"@en ;
    rdfs:comment "Specifies the objectives for the different ISA 95 levels."@en ;
    rdfs:domain sto:ISA95Level ;
    rdfs:range xsd:string .

sto:hasOfficialResource a owl:DatatypeProperty ;
    rdfs:label "has Official Resource"@en ;
    rdfs:comment "Standard Official Website"@en ;
    rdfs:range xsd:string .

sto:hasOntology a owl:DatatypeProperty ;
    rdfs:label "has Ontology"@en ;
    rdfs:comment "Point to the URL of a recognized Ontology representation of the Standard"@en ;
    rdfs:domain sto:Standard ;
    rdfs:range xsd:anyURI .

sto:hasPublicationDate a owl:DatatypeProperty ;
    rdfs:label "has Publication Date"@en ;
    rdfs:comment "Publication date of the Standard"@en ;
    rdfs:domain sto:Standard ;
    rdfs:range xsd:date .

sto:hasPublisher a owl:ObjectProperty ;
    rdfs:label "has Publisher"@en ;
    rdfs:comment "The organization that published this Standard"@en ;
    rdfs:domain sto:Standard ;
    rdfs:range sto:StandardOrganization ;
    rdfs:subPropertyOf foaf:maker .

sto:hasStabilityDate a owl:DatatypeProperty ;
    rdfs:label "has Stability Date"@en ;
    rdfs:comment "The contents of the publications will remain unchanged up to the Stability date. At this date, the publication will be either reconfirmed, withdrawn, replaced by a revised edition or amended. If there is a revision or amendment on-going then this is mentioned under the publication in the \"Work in progress\" tab, if you don't see this tab it means that there is no project under development."@en ;
    rdfs:domain sto:Standard ;
    rdfs:range xsd:gYear ;
    rdfs:seeAlso <https://webstore.iec.ch/webstore/webstore.nsf/xpFAQ.xsp?Open&id=ADMN-7NALM5> ;
    skos:note "The data specified is not actually a Date but an Year " .

sto:hasStatus a owl:DatatypeProperty ;
    rdfs:label "has Status"@en ;
    rdfs:comment "Publication status of the Standard, e.g., Published, under preparation, Released"@en ;
    rdfs:domain sto:Standard ;
    rdfs:range xsd:string .

sto:hasTag a owl:DatatypeProperty,
        owl:ObjectProperty ;
    rdfs:label "has Tag"@en ;
    rdfs:comment "Points to the identification of the standards"@en ;
    rdfs:domain sto:Standard ;
    rdfs:range muto:Tag,
        rdfs:Literal .

sto:hasTask a owl:DatatypeProperty ;
    rdfs:label "has Task"@en ;
    rdfs:comment "Specifies the tasks for the different ISA 95 levels."@en ;
    rdfs:domain sto:ISA95Level ;
    rdfs:range xsd:string .

sto:hasTechnicalCommittee a owl:ObjectProperty ;
    rdfs:label "has Technical Committee"@en ;
    rdfs:comment "Specifies the Technical Committe or a Sub-Committee that is responsible for creation and maintenance of a standard"@en ;
    rdfs:domain sto:Standard ;
    rdfs:range sto:TechnicalCommittee .

sto:hasWikipediaArticle a owl:DatatypeProperty ;
    rdfs:label "has Wikipedia Article"@en ;
    rdfs:comment "Wikipedia Article about the Standard"@en ;
    rdfs:range rdfs:Literal .

sto:isDescribedin a owl:ObjectProperty ;
    rdfs:label "is Described in"@en ;
    rdfs:comment "Links the Standarization Frameworks with the Classification of Standards"@en ;
    rdfs:domain sto:StandardClassification ;
    rdfs:range sto:StandardizationFramework .

sto:isImplementationOf a owl:ObjectProperty ;
    rdfs:label "is Implementation Of"@en ;
    rdfs:comment "Represent the relation that connects two standards when standard A is the implementation of standard B, e.g., B2MML isImplementationOf ISA-95."@en ;
    rdfs:subPropertyOf sto:relatedTo .

sto:isPartOf a owl:ObjectProperty ;
    rdfs:label "is Part Of"@en ;
    rdfs:comment "Represents Standards that are part of other Standards"@en ;
    rdfs:domain sto:Standard ;
    rdfs:range sto:Standard ;
    rdfs:subPropertyOf sto:relatedTo .

sto:orgName a owl:DatatypeProperty ;
    rdfs:label "Org Name"@en ;
    rdfs:commment "Name of the Organization"@en ;
    rdfs:domain sto:StandardOrganization ;
    rdfs:range rdf:PlainLiteral .

sto:stoPartName a owl:DatatypeProperty ;
    rdfs:label "std Part Name"@en ;
    rdfs:comment "Name of the standard part."@en ;
    rdfs:domain sto:StandardPart ;
    rdfs:range xsd:string .

sto:useStructureOf a owl:ObjectProperty ;
    rdfs:label "useStructureOf"@en ;
    rdfs:comment "Standard A uses the structure of Standard B. For example, OPC UA uses Structure Of IEC_61804 (EDDL)"@en ;
    rdfs:subPropertyOf sto:relatedTo .

sto:uses a owl:ObjectProperty ;
    rdfs:label "uses"@en ;
    rdfs:comment "Defines that Standard A uses Standard B. For example, IEC_62714(AML) uses MathML."@en ;
    rdfs:subPropertyOf sto:relatedTo .

dbo:Country a owl:Class .

dbo:Place a owl:Class .

dbr:Beijing a owl:NamedIndividual .

dbr:Berlin a owl:NamedIndividual .

dbr:Boston a owl:NamedIndividual .

dbr:Chicago a owl:NamedIndividual .

dbr:China a owl:NamedIndividual .

dbr:Cologne a owl:NamedIndividual .

dbr:Eumseong a owl:NamedIndividual .

dbr:Frankfurt a owl:NamedIndividual .

dbr:Höhenkirchen-Siegertsbrunn a owl:NamedIndividual .

dbr:New_York_City a owl:NamedIndividual .

dbr:Paris a owl:NamedIndividual .

dbr:South_Korea a owl:NamedIndividual .

dbr:Switzerland a owl:NamedIndividual .

dbr:United_States a owl:NamedIndividual .

dbr:Valbonne a owl:NamedIndividual .

<http://dbpedia.org/resource#Washington,_D.C.> a owl:NamedIndividual .

dbr:_California a owl:NamedIndividual .

dbr:_Georgia a owl:NamedIndividual .

dbr:_Maryland a owl:NamedIndividual .

dbr:_Michigan a owl:NamedIndividual .

dbr:_New_York a owl:NamedIndividual .

dbr:_North_Carolina a owl:NamedIndividual .

dbr:_Texas a owl:NamedIndividual .

dcterms:language a owl:DatatypeProperty .

muto:Tag a owl:Class .

deo:Motivation a owl:Class .

om2:Measure a owl:Class .

xsd:gYear a rdfs:Datatype .

owl:thing a owl:Class .

foaf:Organization a owl:Class .

rami:CommunicationSubModel a owl:NamedIndividual .

rami:Communications a owl:NamedIndividual .

rami:ConditionMonitoring a owl:NamedIndividual .

rami:EnergyEfficiency a owl:NamedIndividual,
        rami:AdminShellSubmodel ;
    sto:isDescribedin sto:AdministrationShell .

rami:InformationLayer a owl:NamedIndividual,
        rami:RAMIITLayer ;
    rdfs:label "Information Layer"@en ;
    sto:isDescribedin sto:RAMI40 .

rami:LifeCycle_Status a owl:NamedIndividual .

rami:Lifecycle_Status a owl:NamedIndividual .

rami:Other a owl:NamedIndividual .

rami:Work_Centers a owl:NamedIndividual .

sto: a owl:Ontology ;
    dc11:description "An ontology to describe industry standards related to Smart Manufacturing" ;
    dc11:title "Standards Ontology"@en ;
    dcterms:created "2017-01-25"^^xsd:date ;
    dcterms:creator <http://data.semanticweb.org/person/steffen-lohmann>,
        <http://http://sda.cs.uni-bonn.de/people/irlan-grangel-gonzalez/>,
        <https://www.linkedin.com/in/paul-baptista-601177b2> ;
    dcterms:modified "2017-09-08"^^xsd:date ;
    dcterms:publisher <http://de.dbpedia.org/resource/Fraunhofer-Gesellschaft> ;
    dcterms:rights "This work is distributed under a Creative Commons Attribution License (http://creativecommons.org/licenses/by/3.0/)."@en ;
    vann:preferredNamespacePrefix "sto" ;
    vann:preferredNamespaceUri "https://w3id.org/i40/sto#" ;
    doap:repository <https://github.com/i40-Tools/StandardsOntology> ;
    owl:imports sto: ;
    owl:versionInfo "0.2" .

sto:APICS a dbpcy:Abstraction100002137,
        dbpcy:Association108049401,
        dbpcy:Business108061042,
        dbpcy:Enterprise108056231,
        dbpcy:Group100031264,
        dbpcy:Organization108008335,
        dbpcy:ProfessionalAssociation108242675,
        dbpcy:SocialGroup107950920,
        dbpcy:WikicatBusinessOrganizations,
        dbpcy:WikicatNon-profitOrganizations,
        <http://dbpedia.org/class/yago/WikicatOrganizationsBasedInChicago,Illinois>,
        dbpcy:WikicatOrganizationsBasedInTheUnitedStates,
        dbpcy:WikicatOrganizationsEstablishedIn1957,
        dbpcy:WikicatProfessionalAssociations,
        dbpcy:WikicatProfessionalAssociationsBasedInTheUnitedStates,
        dbpcy:WikicatStandardsOrganizations,
        dbpcy:YagoLegalActor,
        dbpcy:YagoLegalActorGeo,
        dbpcy:YagoPermanentlyLocatedEntity,
        dbont:Agent,
        dbont:Company,
        dbont:Organisation,
        schema:Organization,
        dul:Agent,
        dul:SocialPerson,
        owl:NamedIndividual,
        owl:Thing,
        wike:Q24229398,
        wike:Q43229,
        sto:StandardOrganization ;
    rdfs:label "APICS"@en ;
    dcterms:subject <http://dbpedia.org/resource/Category:1957_establishments_in_Ohio>,
        dbrc:Business_and_finance_professional_associations,
        dbrc:Organizations_based_in_Chicago,
        dbrc:Organizations_established_in_1957,
        dbrc:Professional_associations_based_in_the_United_States,
        dbrc:Standards_organizations ;
    lingg:hypernym dbres:Organization ;
    rdfs:comment "American Production and Inventory Control Society."@en ;
    sto:formationDate "1957-01-01"^^xsd:date ;
    sto:hasDBpediaResource <http://dbpedia.org/page/APICS> ;
    sto:hasHeadquaterIn dbr:Chicago ;
    sto:hasOfficialResource <http://www.apics.org/apics> ;
    sto:hasWikipediaArticle <https://en.wikipedia.org/wiki/APICS> ;
    sto:orgName "American Production and Inventory Control Society"@en .

sto:ASAM a dbont:Agent,
        dbont:Organisation,
        schema:Organization,
        dul:Agent,
        dul:SocialPerson,
        owl:NamedIndividual,
        owl:Thing,
        wike:Q24229398,
        wike:Q43229,
        sto:StandardOrganization ;
    rdfs:label "ASAM" ;
    dcterms:subject dbrc:Automotive_standards,
        dbrc:Professional_associations_based_in_Germany ;
    lingg:hypernym dbres:Association ;
    rdfs:comment "Association for Standardization of Automation and Measuring Systems or ASAM is an incorporated association under German law. Its members are primarily international car manufacturers, suppliers and engineering service providers from the automotive industry. The association coordinates the development of technical standards, which are developed by working groups composed of experts from its member companies. ASAM pursues the vision that the tools of a development process chain can be freely interconnected and allow a seamless exchange of data. The standards define protocols, data models, file formats and application programming interfaces (APIs) for the use in the development and testing of automotive electronic control units. A large amount of popular tools in the areas of simulation, measurement, calibration and test automation are compliant to ASAM standards. Compliance shall guarantee interoperability of tools from different vendors, allow data exchange without the need for converters, and facilitate the exchange of unambiguous specification between customers and suppliers."@en ;
    sto:abbreviation "ASAM" ;
    sto:belongsTo dbr:Germany ;
    sto:formationDate "1998-12-01"^^xsd:date ;
    sto:hasDBpediaResource dbres:Association_for_Standardisation_of_Automation_and_Measuring_Systems,
        "http://dbpedia.org/page/Association_for_Standardisation_of_Automation_and_Measuring_Systems" ;
    sto:hasHeadquaterIn dbr:Höhenkirchen-Siegertsbrunn ;
    sto:hasOfficialResource <https://www.asam.net/> ;
    sto:hasWikipediaArticle <https://en.wikipedia.org/wiki/Association_for_Standardisation_of_Automation_and_Measuring_Systems>,
        "https://en.wikipedia.org/wiki/Association_for_Standardisation_of_Automation_and_Measuring_Systems" ;
    sto:orgName "Association for Standardization of Automation and Measuring Systems"@en .

sto:ASME a dbpcy:Abstraction100002137,
        dbpcy:Association108049401,
        dbpcy:Company108058098,
        dbpcy:Group100031264,
        dbpcy:Institution108053576,
        dbpcy:Organization108008335,
        dbpcy:ProfessionalAssociation108242675,
        dbpcy:SocialGroup107950920,
        dbpcy:WikicatEngineeringOrganizations,
        dbpcy:WikicatOrganizationsBasedInNewYork,
        dbpcy:WikicatOrganizationsBasedInNewYorkCity,
        dbpcy:WikicatOrganizationsBasedInTheUnitedStates,
        dbpcy:WikicatOrganizationsEstablishedIn1880,
        dbpcy:WikicatProfessionalAssociations,
        dbpcy:WikicatStandardsOrganizations,
        dbpcy:YagoLegalActor,
        dbpcy:YagoLegalActorGeo,
        dbpcy:YagoPermanentlyLocatedEntity,
        dbont:Agent,
        dbont:Organisation,
        schema:Organization,
        dul:Agent,
        dul:SocialPerson,
        owl:NamedIndividual,
        owl:Thing,
        wike:Q24229398,
        wike:Q43229,
        sto:StandardOrganization ;
    dcterms:subject <http://dbpedia.org/resource/Category:1880_establishments_in_New_York>,
        dbrc:American_Society_of_Mechanical_Engineers,
        dbrc:American_engineering_organizations,
        dbrc:American_mechanical_engineers,
        dbrc:Engineering_societies_based_in_the_United_States,
        dbrc:Historic_Mechanical_Engineering_Landmarks,
        dbrc:Mechanical_engineering_organizations,
        dbrc:Organizations_established_in_1880 ;
    lingg:hypernym dbres:Association ;
    rdfs:comment "The American Society of Mechanical Engineers (ASME) is a professional association that, promotes the art, science, and practice of multidisciplinary engineering and allied sciences around the globe via continuing education, training and professional development, codes and standards, research, conferences and publications, government relations, and other forms of outreach."@en ;
    sto:abbreviation "ASME" ;
    sto:formationDate "1880-01-01"^^xsd:date ;
    sto:hasDBpediaResource dbres:ASME ;
    sto:hasHeadquaterIn dbr:New_York_City ;
    sto:hasOfficialResource <https://www.asme.org/> ;
    sto:hasWikipediaArticle <https://en.wikipedia.org/wiki/ASME> ;
    sto:orgName "American Society of Mechanical Engineers"@en .

sto:BPMN a owl:NamedIndividual,
        sto:Standard ;
    rdfs:label "Business Process Model Notation"@en ;
    dcterms:subject dbrc:Business_process_modelling,
        dbrc:Diagrams,
        dbrc:ISO_standards,
        dbrc:Specification_languages,
        dbrc:Workflow_technology ;
    lingg:hypernym dbres:Representation ;
    rdfs:comment "Business Process Model and Notation is a graphical representation for specifying business processes in a business process model."@en ;
    sto:hasClassification sto:SCM ;
    sto:hasDBpediaResource "http://dbpedia.org/page/Business_Process_Model_and_Notation" ;
    sto:hasDeveloper sto:OMG ;
    sto:hasOfficialResource "http://www.bpmn.org/" ;
    sto:hasTag "BPMN"@en ;
    sto:hasWikipediaArticle "http://en.wikipedia.org/wiki/Business_Process_Model_and_Notation",
        "https://en.wikipedia.org/wiki/Business_Process_Model_and_Notation" .

sto:Communication a owl:NamedIndividual,
        rami:AdminShellSubmodel ;
    sto:isDescribedin sto:AdministrationShell .

sto:DMSC a owl:NamedIndividual,
        sto:StandardOrganization ;
    rdfs:label "Dimensional Metrology Standards Consortium"@en ;
    rdfs:comment "Dimensional Metrology Standards Consortium (DMSC) is to identify urgently needed standards in the field of dimensional metrology, and to promote, foster, and encourage the development and interoperability of these standards, along with related and supporting standards that will benefit the industry as a whole."@en ;
    sto:hasHeadquaterIn dbr:_Texas ;
    sto:hasOfficialResource <http://www.dmis.org/> .

sto:DeviceLevel a owl:NamedIndividual,
        sto:ISA95Level ;
    rdfs:label "Device Level"@en ;
    rdfs:comment "Describes the device level according to the ISA95 level classification."@en .

sto:EnterpriseIntegration a owl:NamedIndividual .

sto:FunctionalSafety a owl:NamedIndividual,
        sto:Domain ;
    rdfs:label "Functional Safety"@en ;
    rdfs:comment "Functional Safety"@en .

sto:GPLv2 a dcterms:LicenseDocument,
        owl:NamedIndividual ;
    rdfs:label "GNU General Public License"@en ;
    rdfs:comment "Published under Open Content License."@en ;
    rdfs:seeAlso "<https://opcfoundation.org/license/gpl.htm>" ;
    skos:prefLabel "OCL 1.0" .

sto:IBM a dbpcy:Abstraction100002137,
        dbpcy:Company108058098,
        dbpcy:ElectronicsCompany108003035,
        dbpcy:Group100031264,
        dbpcy:Institution108053576,
        dbpcy:Organization108008335,
        dbpcy:SocialGroup107950920,
        dbpcy:WikicatCompaniesBasedInNewYork,
        <http://dbpedia.org/class/yago/WikicatCompaniesBasedInWestchesterCounty,NewYork>,
        dbpcy:WikicatCompaniesEstablishedIn1896,
        dbpcy:WikicatCompaniesEstablishedIn1911,
        dbpcy:WikicatCompaniesInTheDowJonesIndustrialAverage,
        dbpcy:WikicatCompaniesListedOnNASDAQ,
        dbpcy:WikicatCompaniesListedOnTheNewYorkStockExchange,
        dbpcy:WikicatComputerCompaniesOfTheUnitedStates,
        dbpcy:WikicatComputerHardwareCompanies,
        dbpcy:WikicatComputerStorageCompanies,
        dbpcy:WikicatDisplayTechnologyCompanies,
        dbpcy:WikicatElectronicsCompaniesOfTheUnitedStates,
        dbpcy:WikicatFoundrySemiconductorCompanies,
        dbpcy:WikicatMultinationalCompanies,
        dbpcy:WikicatMultinationalCompaniesHeadquarteredInTheUnitedStates,
        dbpcy:WikicatOutsourcingCompanies,
        dbpcy:WikicatPubliclyTradedCompaniesOfTheUnitedStates,
        dbpcy:WikicatSemiconductorCompanies,
        dbpcy:WikicatSoftwareCompanies,
        dbpcy:WikicatSoftwareCompaniesBasedInNewYork,
        dbpcy:WikicatSoftwareCompaniesOfTheUnitedStates,
        dbpcy:YagoLegalActor,
        dbpcy:YagoLegalActorGeo,
        dbpcy:YagoPermanentlyLocatedEntity,
        dbont:Agent,
        dbont:Company,
        dbont:Organisation,
        schema:Organization,
        <http://umbel.org/umbel/rc/Business>,
        <http://umbel.org/umbel/rc/Organization>,
        dul:Agent,
        dul:SocialPerson,
        owl:NamedIndividual,
        owl:Thing,
        wike:Q24229398,
        wike:Q43229,
        sto:StandardOrganization ;
    dcterms:subject <http://dbpedia.org/resource/Category:1896_establishments_in_the_United_States>,
        <http://dbpedia.org/resource/Category:1911_establishments_in_New_York>,
        dbrc:American_brands,
        dbrc:Cloud_computing_providers,
        dbrc:Collier_Trophy_recipients,
        <http://dbpedia.org/resource/Category:Companies_based_in_Westchester_County,_New_York>,
        dbrc:Companies_established_in_1896,
        dbrc:Companies_in_the_Dow_Jones_Industrial_Average,
        dbrc:Companies_listed_on_the_New_York_Stock_Exchange,
        dbrc:Computer_companies_of_the_United_States,
        dbrc:Computer_hardware_companies,
        dbrc:Computer_storage_companies,
        dbrc:Display_technology_companies,
        dbrc:Electronics_companies_of_the_United_States,
        dbrc:Foundry_semiconductor_companies,
        dbrc:IBM,
        dbrc:Multinational_companies_headquartered_in_the_United_States,
        dbrc:National_Medal_of_Technology_recipients,
        dbrc:Outsourcing_companies,
        dbrc:Point_of_sale_companies,
        dbrc:Semiconductor_companies,
        dbrc:Software_companies_based_in_New_York,
        dbrc:Storage_Area_Network_companies,
        dbrc:Technology_companies_established_in_1911 ;
    lingg:hypernym dbres:Technology ;
    rdfs:comment "International Business Machines Corporation (commonly referred to as IBM) is an American multinational technology and consulting corporation, with corporate headquarters in Armonk, New York. IBM manufactures and markets computer hardware, middleware and software, and offers infrastructure, hosting and consulting services in areas ranging from mainframe computers to nanotechnology.On August 6, 2015, IBM announced that it will buy Merge Healthcare Inc for $1 billion." ;
    sto:abbreviation "IBM" ;
    sto:formationDate "1911-06-16"^^xsd:date ;
    sto:hasDBpediaResource dbres:IBM ;
    sto:hasHeadquaterIn dbr:_New_York ;
    sto:hasOfficialResource <http://www.ibm.com> ;
    sto:hasWikipediaArticle <https://en.wikipedia.org/wiki/IBM> ;
    sto:orgName "International Business Machines Corporation"@en .

sto:IEC_61131 a dbpcy:Abstraction100002137,
        dbpcy:Measure100033615,
        dbpcy:Standard107260623,
        dbpcy:SystemOfMeasurement113577171,
        dbpcy:WikicatENStandards,
        dbpcy:WikicatIECStandards,
        owl:NamedIndividual,
        sto:Standard ;
    rdfs:label "IEC 61131"@en ;
    dcterms:subject dbrc:Electronic_engineering,
        dbrc:IEC_standards,
        dbrc:Programmable_logic_controllers ;
    lingg:hypernym dbres:IEC ;
    rdfs:comment "IEC 61131 is an IEC standard for programmable controllers. It was known as IEC 1131 before the change in numbering system by IEC. The parts of the IEC 61131 standard are prepared and maintained working group 7, programmable control systems, of subcommittee SC 65B of Technical Committee TC65 of the IEC."@en ;
    sto:hasClassification rami:ControlDevice,
        rami:Station,
        rami:WorkCenter ;
    sto:hasDBpediaResource "http://dbpedia.org/page/IEC_61131" ;
    sto:hasOfficialResource "https://webstore.iec.ch/publication/4550" ;
    sto:hasPublisher sto:IEC ;
    sto:hasTag "PLC Open"@en ;
    sto:hasWikipediaArticle "http://en.wikipedia.org/wiki/IEC_61131",
        "https://en.wikipedia.org/wiki/IEC_61131" ;
    sto:isPartOf sto:IEC_62714 ;
    sto:relatedTo sto:IEC_61499 .

sto:IEC_61511 a dbpcy:Abstraction100002137,
        dbpcy:Measure100033615,
        dbpcy:Standard107260623,
        dbpcy:SystemOfMeasurement113577171,
        dbpcy:WikicatElectricalStandards,
        owl:NamedIndividual,
        sto:Standard ;
    rdfs:label "IEC 61511" ;
    dcterms:hasLicense "Private"@en ;
    dcterms:subject dbrc:Electrical_standards,
        dbrc:Industrial_processes,
        dbrc:Manufacturing,
        dbrc:Safety ;
    rdfs:comment "IEC 61511 is a technical standard which sets out practices in the engineering of systems that ensure the safety of an industrial process through the use of instrumentation."@en ;
    sto:hasDBpediaResource "http://dbpedia.org/resource/IEC_61511" ;
    sto:hasDomain sto:FunctionalSafety ;
    sto:hasMotivation "Defines the functional safety requirements established by IEC 61508 in process industry sector terminology"@en ;
    sto:hasOfficialResource "https://webstore.iec.ch/publication/24241" ;
    sto:hasPublisher sto:IEC ;
    sto:hasTag "Functional safety - Safety instrumented systems for the process industry sector"@en ;
    sto:hasWikipediaArticle "http://en.wikipedia.org/wiki/IEC_61511",
        "https://en.wikipedia.org/wiki/IEC_61511" ;
    sto:relatedTo sto:IEC_62061,
        sto:ISO_13849 .

sto:IEC_61784 a dbpcy:Abstraction100002137,
        dbpcy:Arrangement105726596,
        dbpcy:BusTopology105730591,
        dbpcy:Cognition100023271,
        dbpcy:Communication100033020,
        dbpcy:Configuration105731779,
        dbpcy:Design105728678,
        dbpcy:Direction106786629,
        dbpcy:Message106598915,
        dbpcy:Protocol106665108,
        dbpcy:PsychologicalFeature100023100,
        dbpcy:Rule106652242,
        dbpcy:Structure105726345,
        dbpcy:Topology105730365,
        dbpcy:WikicatComputerBuses,
        dbont:Work,
        owl:NamedIndividual,
        sto:Standard ;
    rdfs:label "IEC 61784"@en ;
    dcterms:hasLicense "Private"@en ;
    dcterms:subject dbrc:Automation,
        dbrc:Industrial_automation,
        dbrc:Industrial_computing,
        dbrc:Production_and_manufacturing,
        dbrc:Serial_buses ;
    lingg:hypernym dbres:Standard ;
    rdfs:comment "Industrial communication networks - Profiles - Ethernet-real-time-enabled"@en ;
    sto:hasClassification rami:Communication,
        rami:CommunicationSubModel,
        rami:ControlDevice,
        rami:FieldDevice ;
    sto:hasDBpediaResource "http://dbpedia.org/page/Profibus" ;
    sto:hasMotivation "Information description and communication mapping for fieldbus profiles"@en ;
    sto:hasOfficialResource "https://webstore.iec.ch/publication/5878" ;
    sto:hasPublicationDate "2014-08-19"^^xsd:date ;
    sto:hasPublisher sto:IEC ;
    sto:hasTag "IEC Fieldbus (Profibus)"@en ;
    sto:hasWikipediaArticle "http://en.wikipedia.org/wiki/Profibus" ;
    sto:relatedTo sto:IEC_61158 .

sto:IEC_61850 a dbpcy:Abstraction100002137,
        dbpcy:Communication100033020,
        dbpcy:Direction106786629,
        dbpcy:Measure100033615,
        dbpcy:Message106598915,
        dbpcy:Protocol106665108,
        dbpcy:Rule106652242,
        dbpcy:Standard107260623,
        dbpcy:SystemOfMeasurement113577171,
        dbpcy:WikicatIECStandards,
        dbpcy:WikicatNetworkProtocols,
        dbont:Agent,
        owl:NamedIndividual,
        sto:Standard ;
    rdfs:label "IEC 61850"@en ;
    dcterms:subject dbrc:Electric_power,
        dbrc:IEC_standards,
        dbrc:Smart_grid ;
    lingg:hypernym dbres:Communication ;
    rdfs:comment "IEC 61850 is a standard for vendor-agnostic engineering of the configuration of Intelligent Electronic Devices for electrical substation automation systems to be able to communicate with each other.."@en ;
    sto:hasDBpediaResource "http://dbpedia.org/page/IEC_61850" ;
    sto:hasOfficialResource "https://webstore.iec.ch/publication/4550" ;
    sto:hasPublisher sto:IEC ;
    sto:hasWikipediaArticle "http://en.wikipedia.org/wiki/IEC_61850",
        "https://en.wikipedia.org/wiki/IEC_61850" .

sto:IEC_61987_X a owl:NamedIndividual,
        sto:Standard ;
    rdfs:label "IEC 61987_X"@en ;
    dcterms:hasLicense "Private"@en ;
    rdfs:comment "Industrial-process measurement and control - Data structures and elements in process equipment catalogs - Measuring equipment with analogue and digital output"@en ;
    sto:hasClassification rami:ControlDevice,
        rami:Engineering,
        rami:Enterprise,
        rami:FieldDevice,
        rami:Product,
        rami:Station,
        rami:WorkCenter ;
    sto:hasMotivation "Properties and LOPs as an informational representation of the features of measuring equipment. The referenced standards define general principles (e.g. part 11) as well as specific LOPs for specific device types. These international standards also may serve as examples for description of products."@en ;
    sto:hasOfficialResource "https://webstore.iec.ch/publication/6225" ;
    sto:hasPublisher sto:IEC ;
    sto:hasTag "LOPs in PA"@en .

sto:IEC_62061 a dbpcy:Abstraction100002137,
        dbpcy:Measure100033615,
        dbpcy:Standard107260623,
        dbpcy:SystemOfMeasurement113577171,
        dbpcy:WikicatElectricalStandards,
        dbpcy:WikicatIECStandards,
        dbont:Software,
        owl:NamedIndividual,
        sto:Standard ;
    rdfs:label "IEC 60061"@en ;
    dcterms:subject dbrc:Electrical_standards,
        dbrc:IEC_standards,
        dbrc:Safety ;
    lingg:hypernym dbres:Implementation ;
    rdfs:comment "provides requirements that are applicable to the system level design of all types of machinery safety-related electrical control systems and also for the design of non-complex subsystems or devices."@en ;
    sto:hasClassification rami:Safety ;
    sto:hasDBpediaResource "http://dbpedia.org/resource/IEC_62061" ;
    sto:hasOfficialResource "https://webstore.iec.ch/publication/22797" ;
    sto:hasPublisher sto:IEC ;
    sto:hasTag "Safety of machinery"@en ;
    sto:hasWikipediaArticle "http://en.wikipedia.org/wiki/IEC_62061",
        "https://en.wikipedia.org/wiki/IEC_62061" .

sto:IEC_62337 a owl:NamedIndividual,
        sto:Standard ;
    rdfs:label "IEC 62337"@en ;
    rdfs:comment "Commissioning of electrical, instrumentation and control systems in the process industry - Specific phases and milestones."@en ;
    sto:hasClassification rami:Conditional_Monitoring,
        rami:Enterprise,
        rami:Functional,
        rami:Lifecycle_Status,
        rami:Work_Centers,
        sto:ProductionSystemModelData ;
    sto:hasDomain sto:IndustrialAutomation ;
    sto:hasOfficialResource "https://webstore.iec.ch/publication/6871" ;
    sto:hasPublicationDate "2012-02-22"^^xsd:date ;
    sto:hasPublisher sto:IEC .

sto:IEC_62443 a owl:NamedIndividual,
        sto:Standard ;
    rdfs:label "IEC 62443"@en ;
    dcterms:hasLicense "Private"@en ;
    rdfs:comment "Defines procedures for implementing electronically secure Industrial Automation and Control Systems."@en,
        "ISA/IEC-62443 is a series of standards, technical reports, and related information that define procedures for implementing electronically secure Industrial Automation and Control Systems (IACS). This guidance applies to end-users (i.e. asset owner), system integrators, security practitioners, and control systems manufacturers responsible for manufacturing, designing, implementing, or managing industrial automation and control systems."@en ;
    skos:altLabel "ISA 99" ;
    skos:note "TODO" ;
    sto:hasClassification rami:Security,
        sto:CrossLevel ;
    sto:hasDBpediaResource "http://dbpedia.org/page/Cyber_security_standards#ISA/IEC-62443_(formerly_ISA-99)" ;
    sto:hasDeveloper sto:ANSI,
        sto:ISA ;
    sto:hasMotivation "Cyber attacks threat the industry and can cause damage to property and personal injury and affect the image of companies. The Standard allows to define procedures for implementing electronically secure Industrial Automation and Control Systems (IACS). This guidance applies to end-users, system integrators, security practitioners, and control systems manufacturers responsible for manufacturing, designing, implementing, or managing industrial automation and control systems"@en ;
    sto:hasOfficialResource "https://webstore.iec.ch/publication/7029",
        "https://webstore.iec.ch/publication/7033" ;
    sto:hasPublisher sto:ANSI,
        sto:IEC,
        sto:ISA ;
    sto:hasTag "Electronically secure Industrial Automation and Control Systems"@en,
        "Network and system security for industrial-process measurement and control"@en ;
    sto:hasWikipediaArticle <https://en.wikipedia.org/wiki/Cyber_security_standards#ISA.2FIEC-62443_.28formerly_ISA-99.29> .

sto:IEC_62453 a owl:NamedIndividual,
        sto:Standard ;
    rdfs:label "IEC 62453"@en ;
    rdfs:comment "Field device tool (FDT) interface specification - Overview and guidance"@en ;
    sto:hasClassification rami:Configuration,
        rami:ControlDevice,
        rami:FieldDevice,
        rami:Station ;
    sto:hasMotivation "FDT is an interface for integration of devices into a system (e.g. control system or engineering system). The standard supports factory automation as well as process automation with a wide range of fieldbus protocols. The interface defines fieldbus-independent mechanisms for accessing data and functions of the devices."@en ;
    sto:hasOfficialResource "https://webstore.iec.ch/publication/7040" ;
    sto:hasPublisher sto:IEC ;
    sto:hasTag "FDT"@en .

sto:IEC_62890 a owl:NamedIndividual,
        sto:Standard ;
    rdfs:label "IEC 62890"@en ;
    dcterms:hasLicense "Private"@en ;
    rdfs:comment "Defines standards for lifecycle management for systems and products used in industrial process measurement, control and automation"@en,
        "MES KPIs"@en ;
    sto:hasClassification rami:LifecycleStatus,
        rami:Station,
        rami:WorkCenter,
        sto:ProductionLifeCycleDataManagement ;
    sto:hasMotivation "Stations need to describe their operational state and performance parameters towards superior I4.0-Components"@en ;
    sto:hasOfficialResource "http://www.iec.ch/dyn/www/f?p=103:38:16824039984463::::FSP_ORG_ID,FSP_APEX_PAGE,FSP_PROJECT_ID:1250,23,20929" ;
    sto:hasPublisher sto:IEC ;
    sto:hasTag "IEC 62890"@en .

sto:IEC_TS_62832 a owl:NamedIndividual,
        sto:Standard ;
    rdfs:label "IEC TS 62832"@en ;
    dcterms:hasLicense "Private"@en ;
    rdfs:comment "Digital Factory Reference model TS"@en ;
    sto:hasClassification rami:AdminShellGeneral,
        rami:ControlDevice,
        rami:FieldDevice,
        rami:GeneralAdminShell,
        rami:Station,
        rami:WorkCenter ;
    sto:hasMotivation "The standards for Digital Factory define methods and information models, which are required for self description of I40-components. IEC TS 62832 defines methods, which allow to validate or plan connections between assets."@en ;
    sto:hasOfficialResource "https://webstore.iec.ch/publication/33023" ;
    sto:hasPublisher sto:IEC ;
    sto:hasTag "DF/TS"@en .

sto:ISO_10303 a dbpcy:Abstraction100002137,
        dbpcy:Communication100033020,
        dbpcy:Format106636806,
        dbpcy:Information106634376,
        dbpcy:Measure100033615,
        dbpcy:Message106598915,
        dbpcy:Standard107260623,
        dbpcy:SystemOfMeasurement113577171,
        dbpcy:WikicatCADFileFormats,
        dbpcy:WikicatGraphicsFileFormats,
        dbpcy:WikicatISOStandards,
        dbont:Organisation,
        owl:NamedIndividual,
        sto:Standard ;
    rdfs:label "ISO 10303"@en ;
    dcterms:subject dbrc:CAD_file_formats,
        dbrc:ISO_standards ;
    lingg:hypernym dbres:ISO ;
    rdfs:comment "Standard for the Exchange of Product model data. ISO 10303 can represent 3D objects in Computer-aided design (CAD) and related information."@en ;
    skos:note "TODO - Split properly and classify it - check the NIST paper" ;
    sto:hasClassification sto:ProductLifeCycleManagement ;
    sto:hasDBpediaResource "http://dbpedia.org/page/ISO_10303" ;
    sto:hasOfficialResource "https://www.steptools.com/stds/step/" ;
    sto:hasPublisher sto:ISO ;
    sto:hasTag "STEP"@en ;
    sto:hasWikipediaArticle "http://en.wikipedia.org/wiki/ISO_10303",
        "https://en.wikipedia.org/wiki/ISO_10303" .

sto:ISO_11783 a dbpcy:Abstraction100002137,
        dbpcy:Communication100033020,
        dbpcy:Direction106786629,
        dbpcy:Measure100033615,
        dbpcy:Message106598915,
        dbpcy:Protocol106665108,
        dbpcy:Rule106652242,
        dbpcy:Standard107260623,
        dbpcy:SystemOfMeasurement113577171,
        dbpcy:WikicatISOStandards,
        dbpcy:WikicatNetworkProtocols,
        dbont:Software,
        owl:NamedIndividual,
        sto:Standard ;
    rdfs:label "ISO 11783"@en ;
    dcterms:subject dbrc:ISO_standards,
        dbrc:Network_protocols ;
    lingg:hypernym dbres:Protocol ;
    rdfs:comment "ISO 11783, known as Tractors and machinery for agriculture and forestry—Serial control and communications data network is a communication protocol for the agriculture industry based on the SAE J1939 protocol (which includes CANbus)."@en ;
    sto:hasDBpediaResource "http://dbpedia.org/resource/ISO_11783" ;
    sto:hasOfficialResource "https://www.iso.org/standard/61646.html" ;
    sto:hasPublisher sto:ISO ;
    sto:hasTag "ISOBUS"@en ;
    sto:hasWikipediaArticle "http://en.wikipedia.org/wiki/ISO_11783",
        "https://en.wikipedia.org/wiki/ISO_11783" .

sto:ISO_13374 a owl:NamedIndividual,
        sto:Standard ;
    rdfs:label "ISO 13374"@en ;
    rdfs:comment "Condition monitoring and diagnostics of machines -- Data processing, communication and presentation"@en ;
    sto:hasClassification rami:Business,
        rami:Conditional_Monitoring,
        rami:Enterprise,
        sto:ProductionSystemEngineering ;
    sto:hasDomain sto:IndustrialAutomation ;
    sto:hasOfficialResource "https://www.iso.org/standard/61131.html" ;
    sto:hasPublicationDate "2012-02-01"^^xsd:date ;
    sto:hasPublisher sto:ISO .

sto:ISO_13849 a dbpcy:Abstraction100002137,
        dbpcy:Code106667317,
        dbpcy:Communication100033020,
        dbpcy:Measure100033615,
        dbpcy:Standard107260623,
        dbpcy:SystemOfMeasurement113577171,
        dbpcy:WikicatISOStandards,
        dbpcy:WikicatSafetyCodes,
        dbpcy:WrittenCommunication106349220,
        owl:NamedIndividual,
        sto:Standard ;
    rdfs:label "ISO 13849"@en ;
    dcterms:subject dbrc:ISO_standards,
        dbrc:Safety_codes ;
    rdfs:comment "Provides safety requirements and guidance on the principles for the design and integration of safety-related parts of control systems (SRP/CS), including the design of software."@en ;
    sto:hasClassification rami:Safety ;
    sto:hasDBpediaResource "http://dbpedia.org/resource/ISO_13849" ;
    sto:hasDomain "Safety of machinery"@en ;
    sto:hasOfficialResource "http://www.iso.org/iso/home/store/catalogue_tc/catalogue_detail.htm?csnumber=69883" ;
    sto:hasPublisher sto:ISO ;
    sto:hasWikipediaArticle "http://en.wikipedia.org/wiki/ISO_13849",
        "https://en.wikipedia.org/wiki/ISO_13849" .

sto:ISO_14306 a owl:NamedIndividual,
        sto:Standard ;
    rdfs:label "ISO 14306"@en ;
    rdfs:comment "It provides the description of the structure and content for a binary file having the extension of .jt. A binary file with the .jt extension is generally referred to as a JT file. The JT format described in ISO 14306:2012 is used primarily in industrial use cases as the means for capturing and repurposing lightweight 3D product definition data"@en ;
    sto:hasClassification rami:Asset,
        rami:Engineering,
        rami:Identification,
        rami:Product,
        sto:ProcessPlanning,
        sto:ProductionSystemModelData ;
    sto:hasDomain sto:CAD ;
    sto:hasOfficialResource "https://www.iso.org/standard/60572.html" ;
    sto:hasPublicationDate "2017-07-01"^^xsd:date ;
    sto:hasPublisher sto:ISO ;
    sto:relatedTo sto:IEC_62541 .

sto:ISO_14443 a owl:NamedIndividual .

sto:ISO_15459 a owl:NamedIndividual .

sto:ISO_19439 a dbpcy:Abstraction100002137,
        dbpcy:Measure100033615,
        dbpcy:Standard107260623,
        dbpcy:SystemOfMeasurement113577171,
        dbpcy:WikicatISOStandards,
        dbont:Work,
        owl:NamedIndividual,
        sto:Standard ;
    rdfs:label "ISO 19439"@en ;
    dcterms:subject dbrc:Enterprise_modelling,
        dbrc:ISO_standards ;
    lingg:hypernym dbres:Standard ;
    rdfs:comment "Provides a unified conceptual basis for model-based enterprise engineering that enables consistency, convergence and interoperability of the various modelling methodologies and supporting tools."@en ;
    sto:hasClassification rami:Business ;
    sto:hasDBpediaResource "http://dbpedia.org/page/ISO_19439" ;
    sto:hasOfficialResource "https://www.iso.org/standard/33833.html" ;
    sto:hasPublisher sto:ISO ;
    sto:hasTag "19439"@en ;
    sto:hasWikipediaArticle "http://en.wikipedia.org/wiki/ISO_19439",
        "https://en.wikipedia.org/wiki/ISO_19439" .

sto:ISO_29161 a owl:NamedIndividual,
        sto:Standard ;
    rdfs:label "ISO 29161" ;
    rdfs:comment "ISO/IEC 29161:2016 establishes a unique identification scheme for the Internet of Things (IoT), based on existing and evolving data structures."@en ;
    sto:hasOfficialResource "https://www.iso.org/standard/45240.html" .

sto:ITSecurity a owl:NamedIndividual,
        sto:Domain ;
    rdfs:label "IT Security"@en .

sto:ManufacturingModelData a owl:NamedIndividual,
        sto:ProductDevelopmentLifeCycle ;
    rdfs:label "Manufacturing Model Data"@en ;
    rdfs:comment "Manufacturing Model Data Standards define the data needed to manufacture a product from a design."@en ;
    sto:isDescribedin sto:NISTInitiative .

sto:MathML a dbpcy:Abstraction100002137,
        dbpcy:Application106570110,
        dbpcy:Browser106571301,
        dbpcy:Code106355894,
        dbpcy:CodingSystem106353757,
        dbpcy:Communication100033020,
        dbpcy:Format106636806,
        dbpcy:Information106634376,
        dbpcy:LanguageUnit106284225,
        dbpcy:MarkupLanguage106787835,
        dbpcy:Measure100033615,
        dbpcy:Message106598915,
        dbpcy:Part113809207,
        dbpcy:Program106568978,
        dbpcy:Relation100031921,
        dbpcy:Software106566077,
        dbpcy:Standard107260623,
        dbpcy:SystemOfMeasurement113577171,
        dbpcy:Terminology106304059,
        dbpcy:WikicatMarkupLanguages,
        dbpcy:WikicatMathematicalMarkupLanguages,
        dbpcy:WikicatWebBrowsers,
        dbpcy:WikicatWebStandards,
        dbpcy:WikicatWorldWideWebConsortiumStandards,
        dbpcy:WikicatXML-basedStandards,
        dbpcy:Word106286395,
        dbpcy:Writing106359877,
        dbpcy:WrittenCommunication106349220,
        dbont:Language,
        owl:NamedIndividual,
        owl:Thing,
        sto:Standard ;
    rdfs:label "MathML"@en ;
    dcterms:subject dbrc:Articles_with_example_Scheme_code,
        dbrc:MathML,
        dbrc:Mathematical_markup_languages,
        dbrc:World_Wide_Web_Consortium_standards,
        dbrc:XML-based_standards,
        dbrc:XML_markup_languages ;
    lingg:hypernym dbres:Language ;
    rdfs:comment "MathML is a low-level specification for mathematical and scientific content on the Web and beyond"@en ;
    sto:hasDBpediaResource "http://dbpedia.org/page/MathML" ;
    sto:hasOfficialResource "https://www.w3.org/Math/" ;
    sto:hasPublisher sto:W3C ;
    sto:hasWikipediaArticle "http://en.wikipedia.org/wiki/MathML",
        "https://en.wikipedia.org/wiki/MathML" .

sto:OAGi a owl:NamedIndividual,
        sto:StandardOrganization ;
    rdfs:label "OAGi"@en ;
    rdfs:comment "The Open Applications Group is a not-for-profit standards development organization. Founded in 1994, is focused on building enterprise ready process-based data exchange standards for both B2B and A2A integration."@en ;
    sto:abbreviation "OAGi" ;
    sto:formationDate "1994-01-01"^^xsd:date ;
    sto:hasHeadquaterIn dbr:_Georgia ;
    sto:hasOfficialResource "http://www.oagi.org/dnn2/Home.aspx" ;
    sto:orgName "Open Applications Group"@en .

sto:OPC_Foundation a dbpcy:Abstraction100002137,
        dbpcy:Group100031264,
        dbpcy:Organization108008335,
        dbpcy:SocialGroup107950920,
        dbpcy:WikicatStandardsOrganizations,
        dbpcy:YagoLegalActor,
        dbpcy:YagoLegalActorGeo,
        dbpcy:YagoPermanentlyLocatedEntity,
        dbont:Organisation,
        owl:NamedIndividual,
        sto:StandardOrganization ;
    rdfs:label "OPC Foundation"@en ;
    dcterms:subject dbrc:Automation ;
    lingg:hypernym dbres:Consortium ;
    rdfs:comment "Is an industry consortium that creates and maintains standards for open connectivity of industrial automation devices and systems, such as industrial control systems and process control generally"@en ;
    sto:abbreviation "OPC" ;
    sto:formationDate "1994-01-01"^^xsd:date ;
    sto:hasDBpediaResource "http://dbpedia.org/page/OPC_Foundation" ;
    sto:hasHeadquaterIn dbr:_Arizona ;
    sto:hasOfficialResource "https://opcfoundation.org/" ;
    sto:hasWikipediaArticle "http://en.wikipedia.org/wiki/OPC_Foundation",
        "https://en.wikipedia.org/wiki/OPC_Foundation" ;
    sto:orgName "OPC Foundation"@en .

sto:ProcessPlanning a owl:NamedIndividual .

sto:Prodcut a owl:NamedIndividual .

sto:Product a owl:NamedIndividual .

sto:ProductionLifeCycleDataManagement a owl:NamedIndividual,
        sto:ProductionSystemLifeCycle ;
    rdfs:label "Production Life Cycle Data Management"@en ;
    rdfs:comment "Production lifecycle data management standards define general models of data integration, sharing, exchange, and hand-over for lifecycle support of production facilities."@en ;
    sto:isDescribedin sto:NISTInitiative .

sto:SCADALevel a owl:NamedIndividual,
        sto:ISA95Level ;
    rdfs:label "SCADA Level"@en ;
    rdfs:comment "Describes the SCADA level according to the ISA95 level classification."@en ;
    skos:definition "Supervisory control and data acquisition according to ISA 95"@en ;
    sto:isDescribedin sto:ISA95 .

sto:SE a dbpcy:Abstraction100002137,
        dbpcy:Business108061042,
        dbpcy:Company108058098,
        dbpcy:ElectronicsCompany108003035,
        dbpcy:Enterprise108056231,
        dbpcy:Group100031264,
        dbpcy:Institution108053576,
        dbpcy:Manufacturer108060446,
        dbpcy:Organization108008335,
        dbpcy:SocialGroup107950920,
        dbpcy:WikicatCompaniesBasedInParis,
        dbpcy:WikicatCompaniesEstablishedIn1836,
        dbpcy:WikicatCompaniesListedOnTheEuronextExchanges,
        dbpcy:WikicatCompaniesListedOnTheEuronextParis,
        dbpcy:WikicatCompaniesListedOnTheFrankfurtStockExchange,
        dbpcy:WikicatCompaniesOfFrance,
        dbpcy:WikicatDefenceCompaniesOfFrance,
        dbpcy:WikicatElectricalEquipmentManufacturers,
        dbpcy:WikicatElectronicsCompaniesOfFrance,
        dbpcy:WikicatLocomotiveManufacturersOfFrance,
        dbpcy:WikicatManufacturersOfIndustrialAutomation,
        dbpcy:WikicatManufacturingCompaniesOfFrance,
        dbpcy:WikicatMultinationalCompaniesHeadquarteredInFrance,
        dbpcy:YagoLegalActor,
        dbpcy:YagoLegalActorGeo,
        dbpcy:YagoPermanentlyLocatedEntity,
        dbont:Agent,
        dbont:Company,
        dbont:Organisation,
        schema:Organization,
        dul:Agent,
        dul:SocialPerson,
        owl:NamedIndividual,
        owl:Thing,
        wike:Q24229398,
        wike:Q43229,
        sto:StandardOrganization ;
    dcterms:subject <http://dbpedia.org/resource/Category:1836_establishments_in_France>,
        dbrc:CAC_40,
        dbrc:Companies_established_in_1836,
        dbrc:Companies_in_the_Euro_Stoxx_50,
        dbrc:Conglomerate_companies_of_France,
        dbrc:Electrical_engineering_companies_of_France,
        dbrc:Electrical_wiring_and_construction_supplies_manufacturers,
        dbrc:French_brands,
        dbrc:Locomotive_manufacturers_of_France,
        dbrc:MES_software,
        dbrc:Manufacturers_of_industrial_automation,
        dbrc:Manufacturing_companies_of_France,
        dbrc:Multinational_companies_headquartered_in_France,
        dbrc:Power_engineering,
        dbrc:Schneider_Electric,
        dbrc:Societates_Europaeae ;
    lingg:hypernym dbres:Corporation ;
    rdfs:comment "The Broadband Forum is a non-profit industry consortium dedicated to developing broadband network specifications. Members include telecommunications networking and service provider companies, broadband device and equipment vendors, consultants and independent testing labs (ITLs). Service provider members are primarily wire-line service providers (non-mobile) telephone companies."@en ;
    sto:abbreviation "SE" ;
    sto:formationDate "1936-01-01"^^xsd:date ;
    sto:hasDBpediaResource "http://dbpedia.org/page/Schneider_Electric" ;
    sto:hasHeadquaterIn dbr:Paris ;
    sto:hasOfficialResource "http://www.schneider-electric.com/ww/en/" ;
    sto:hasWikipediaArticle "http://en.wikipedia.org/wiki/Schneider_Electric",
        "https://en.wikipedia.org/wiki/Schneider_Electric" ;
    sto:orgName "Schneider Electric"@en .

sto:TechnicalCommittee a owl:Class,
        owl:NamedIndividual ;
    rdfs:label "Technical Committe"@en ;
    rdfs:comment "Specifies the representitive code name of the Technical or Sub-Committee that covers a Standard for e.g, TC 1, SC 3C."@en ;
    rdfs:isDefinedBy sto:IEC ;
    rdfs:seeAlso <http://www.iec.ch/dyn/www/f?p=103:62:9979528650478:::62:FSP_ORG_ID,FSP_LANG_ID:,25> ;
    skos:note """1.sto:hastitle property needs to be added. Description of the Committee Code
                                  2. sto:       a property explaining that TC and SC are managed by SMB (Standardization Management Board) needs to be added""" ;
    sto:abbreviation "TC" .

sto:UN-CEFACT a dbpcy:Abstraction100002137,
        dbpcy:Group100031264,
        dbpcy:Organization108008335,
        dbpcy:SocialGroup107950920,
        dbpcy:WikicatInternationalEconomicOrganizations,
        dbpcy:WikicatOrganizationsEstablishedByTheUnitedNations,
        dbpcy:YagoLegalActor,
        dbpcy:YagoLegalActorGeo,
        dbpcy:YagoPermanentlyLocatedEntity,
        dbont:Organisation,
        owl:NamedIndividual,
        owl:Thing,
        sto:StandardOrganization ;
    dcterms:subject dbrc:Accounting,
        dbrc:Computer_file_formats,
        dbrc:E-commerce,
        dbrc:International_trade,
        dbrc:United_Nations_Economic_Commission_for_Europe ;
    lingg:hypernym dbres:Organisation ;
    rdfs:comment "UN/CEFACT is the United Nations Centre for Trade Facilitation and Electronic Business. It was established as an intergovernmental body of the United Nations Economic Commission for Europe (UNECE) in 1996 and evolved from UNECE’s long tradition of work in trade facilitation."@en ;
    sto:abbreviation "UN/CEFACT" ;
    sto:hasDBpediaResource "http://dbpedia.org/page/UN/CEFACT" ;
    sto:hasHeadquaterIn dbr:Geneva ;
    sto:hasOfficialResource "https://www.unece.org/cefact/" ;
    sto:hasWikipediaArticle "http://en.wikipedia.org/wiki/UN/CEFACT",
        "https://en.wikipedia.org/wiki/UN/CEFACT" ;
    sto:orgName "United Nations Centre for Trade Facilitation and Electronic Business"@en .

sto:VDMA a dbpcy:Abstraction100002137,
        dbpcy:Association108049401,
        dbpcy:Group100031264,
        dbpcy:Organization108008335,
        dbpcy:ProfessionalAssociation108242675,
        dbpcy:SocialGroup107950920,
        dbpcy:WikicatProfessionalAssociations,
        dbpcy:WikicatProfessionalAssociationsBasedInGermany,
        dbpcy:YagoLegalActor,
        dbpcy:YagoLegalActorGeo,
        dbpcy:YagoPermanentlyLocatedEntity,
        dbont:Organisation,
        owl:NamedIndividual,
        sto:StandardOrganization ;
    lingg:hypernym dbres:Association ;
    rdfs:comment "The Mechanical Engineering Industry Association (Verband Deutscher Maschinen- und Anlagenbau – VDMA) has its headquarters in Frankfurt am Main, Germany, and represents around 3,200 members, making it the largest industry association in Europe. The Association represents the interests of the predominantly medium-sized companies in the mechanical engineering industry towards policymakers and society, as well as towards business, the scientific community, public authorities and the media. With more than one million employees and a turnover of around EUR 218 billion (2015), mechanical and plant engineering is Germany’s largest employer in the industrial sector.In addition, VDMA sees itself as a platform that provides its member companies with various networks where they can discuss technological challenges, interdisciplinary issues and many other topics." ;
    sto:abbreviation "VDMA" ;
    sto:formationDate "1892-11-15"^^xsd:date ;
    sto:hasDBpediaResource "http://dbpedia.org/resource/VDMA" ;
    sto:hasHeadquaterIn dbr:Frankfurt ;
    sto:hasOfficialResource "http://www.vdma.org" ;
    sto:hasWikipediaArticle "http://en.wikipedia.org/wiki/VDMA",
        "https://en.wikipedia.org/wiki/Mechanical_Engineering_Industry_Association" ;
    sto:orgName "Verband Deutscher Maschinen- und Anlagenbau"@de,
        "Mechanical Engineering Industry Association"@en .

sto:W3C_OWL a dbpcy:Abstraction100002137,
        dbpcy:Communication100033020,
        dbpcy:Format106636806,
        dbpcy:Information106634376,
        dbpcy:Language106282651,
        dbpcy:Measure100033615,
        dbpcy:Message106598915,
        dbpcy:Standard107260623,
        dbpcy:SystemOfMeasurement113577171,
        dbpcy:WikicatOntologyLanguages,
        dbpcy:WikicatWebStandards,
        dbpcy:WikicatWorldWideWebConsortiumStandards,
        dbpcy:WikicatXML-basedStandards,
        owl:NamedIndividual,
        owl:Thing,
        sto:Standard ;
    rdfs:label "Web Ontology Language"@en ;
    dcterms:hasLicense "Public"@en ;
    dcterms:subject dbrc:Declarative_programming_languages,
        dbrc:Ontology_languages,
        dbrc:Resource_Description_Framework,
        <http://dbpedia.org/resource/Category:School_of_Computer_Science,_University_of_Manchester>,
        dbrc:Semantic_Web,
        dbrc:Web_Ontology_Language,
        dbrc:World_Wide_Web_Consortium_standards,
        dbrc:XML-based_standards ;
    lingg:hypernym dbres:Family ;
    rdfs:comment "The W3C Web Ontology Language (OWL) is a Semantic Web language designed to represent rich and complex knowledge about things, groups of things, and relations between things. OWL is a computational logic-based language such that knowledge expressed in OWL can be exploited by computer programs, e.g., to verify the consistency of that knowledge or to make implicit knowledge explicit. OWL documents, known as ontologies, can be published in the World Wide Web and may refer to or be referred from other OWL ontologies. OWL is part of the W3C’s Semantic Web technology stack, which includes RDF, RDFS, SPARQL, etc."@en ;
    sto:hasDBpediaResource "http://dbpedia.org/resource/Web_Ontology_Language" ;
    sto:hasOfficialResource "https://www.w3.org/OWL/" ;
    sto:hasPublisher sto:W3C ;
    sto:hasTag "OWL"@en ;
    sto:hasWikipediaArticle "http://en.wikipedia.org/wiki/Web_Ontology_Language",
        "https://en.wikipedia.org/wiki/Web_Ontology_Language?oldformat=true" ;
    sto:relatedTo sto:W3C_RDF .

dbr:Germany a owl:NamedIndividual .

dbr:_Arizona a owl:NamedIndividual .

dbr:_Massachusetts a owl:NamedIndividual .

dcterms:LicenseDocument a owl:Class ;
    rdfs:label "License Document"@en ;
    rdfs:comment "A legal document giving official permission to do something with a Resource."@en ;
    rdfs:isDefinedBy dcterms: .

xsd:date a rdfs:Datatype .

foaf:maker a owl:ObjectProperty .

rami:AdminShellGeneral a owl:NamedIndividual,
        rami:AdminShellSubmodel ;
    sto:isDescribedin sto:AdministrationShell .

rami:Assest a owl:NamedIndividual .

rami:LifecycleStatus a owl:NamedIndividual,
        rami:AdminShellSubmodel ;
    sto:isDescribedin sto:AdministrationShell .

sto:BBF a dbpcy:Abstraction100002137,
        dbpcy:Association108049401,
        dbpcy:Consortium108236438,
        dbpcy:Group100031264,
        dbpcy:Organization108008335,
        dbpcy:SocialGroup107950920,
        dbpcy:WikicatConsortia,
        dbpcy:YagoLegalActor,
        dbpcy:YagoLegalActorGeo,
        dbpcy:YagoPermanentlyLocatedEntity,
        dbont:Agent,
        dbont:Organisation,
        schema:Organization,
        dul:Agent,
        dul:SocialPerson,
        owl:NamedIndividual,
        owl:Thing,
        wike:Q24229398,
        wike:Q43229,
        sto:StandardOrganization ;
    rdfs:label "Broadband Forum"@en ;
    dcterms:subject dbrc:Broadband,
        dbrc:Digital_subscriber_line,
        dbrc:Digital_television,
        dbrc:Technology_consortia ;
    lingg:hypernym dbres:Consortium ;
    rdfs:comment "The Broadband Forum is a non-profit industry consortium dedicated to developing broadband network specifications. Members include telecommunications networking and service provider companies, broadband device and equipment vendors, consultants and independent testing labs (ITLs). Service provider members are primarily wire-line service providers (non-mobile) telephone companies."@en ;
    sto:abbreviation "BBF" ;
    sto:formationDate "2008-01-01"^^xsd:date ;
    sto:hasDBpediaResource "http://dbpedia.org/resource/Broadband_Forum" ;
    sto:hasHeadquaterIn dbr:_California ;
    sto:hasOfficialResource "https://www.broadband-forum.org/" ;
    sto:hasWikipediaArticle "http://en.wikipedia.org/wiki/Broadband_Forum",
        "https://en.wikipedia.org/wiki/Broadband_Forum" ;
    sto:orgName "Broadband Forum"@en .

sto:BusinessCycleSCM a owl:Class ;
    rdfs:label "Business Cycle SCM"@en ;
    rdfs:comment "Suply Chain Management Business Cycle."@en ;
    rdfs:isDefinedBy "http://nvlpubs.nist.gov/nistpubs/ir/2016/NIST.IR.8107.pdf" ;
    rdfs:seeAlso "https://en.wikipedia.org/wiki/Supply_chain_management" ;
    rdfs:subClassOf sto:StandardClassification .

sto:DIN a owl:NamedIndividual,
        sto:StandardOrganization ;
    rdfs:label "Deutsches Institut für Normung"@de,
        "German Institute for Standardization"@en ;
    rdfs:comment "Deutsches Institut für Normung e.V. (DIN; in English, the German Institute for Standardization) is the German national organization for standardization and is the German ISO member body. DIN is a German Registered Association (e.V.) headquartered in Berlin. There are currently around thirty thousand DIN Standards, covering nearly every field of technology"@en ;
    sto:abbreviation "DIN"@de ;
    sto:belongsTo dbr:Germany ;
    sto:formationDate "1918-01-01"^^xsd:date ;
    sto:hasDBpediaResource <http://dbpedia.org/page/Deutsches_Institut_f%C3%BCr_Normung> ;
    sto:hasHeadquaterIn dbr:Berlin ;
    sto:hasOfficialResource <http://www.din.de/en/about-standards/din-standards> ;
    sto:hasWikipediaArticle <https://en.wikipedia.org/wiki/Deutsches_Institut_f%C3%BCr_Normung> ;
    sto:orgName "Deutsches Institut für Normung"@en .

sto:ETSI_DECT a dbpcy:Abstraction100002137,
        dbpcy:Measure100033615,
        dbpcy:Standard107260623,
        dbpcy:SystemOfMeasurement113577171,
        dbpcy:WikicatMobileTelecommunicationsStandards,
        dbont:Work,
        owl:NamedIndividual,
        owl:Thing,
        sto:Standard ;
    rdfs:label "ETSI DECT" ;
    dcterms:subject dbrc:Broadband,
        dbrc:Local_loop,
        dbrc:Mobile_telecommunications_standards,
        dbrc:Software-defined_radio ;
    lingg:hypernym dbres:Standard ;
    rdfs:comment "Digital Enhanced Cordless Telecommunications (DECT) is the ETSI standard for short-range cordless communications, which can be adapted for many applications and can be used over unlicensed frequency allocations world-wide."@en ;
    sto:hasDBpediaResource "http://dbpedia.org/resource/Digital_Enhanced_Cordless_Telecommunications" ;
    sto:hasDeveloper sto:ETSI ;
    sto:hasOfficialResource "http://www.etsi.org/technologies-clusters/technologies/dect" ;
    sto:hasPublisher sto:ETSI ;
    sto:hasTag "Digital Enhanced Cordless Telecommunications"@en ;
    sto:hasWikipediaArticle "http://en.wikipedia.org/wiki/Digital_Enhanced_Cordless_Telecommunications",
        "https://en.wikipedia.org/wiki/Digital_Enhanced_Cordless_Telecommunications" .

sto:EnterpriseLevel a owl:NamedIndividual,
        sto:ISA95Level ;
    rdfs:label "Enterprise Level"@en ;
    rdfs:comment "Describes the Enterprise level according to the ISA95 level classification."@en .

sto:IEC_61499 a dbpcy:Abstraction100002137,
        dbpcy:Measure100033615,
        dbpcy:Standard107260623,
        dbpcy:SystemOfMeasurement113577171,
        dbpcy:WikicatENStandards,
        dbpcy:WikicatIECStandards,
        owl:NamedIndividual,
        sto:Standard ;
    rdfs:label "IEC 61499"@en ;
    dcterms:subject dbrc:IEC_standards ;
    rdfs:comment "Function Blocks - Architecture Related Applications http://www.eclipse.org/4diac/ (sourceforge.net/projects/oooneida-fbench/) http://timeme.io/  not accepted by the Industry yet. http://www.holobloc.com/Proposed for IEC to overcome the restricctions of IEC 61131"@en ;
    sto:hasClassification rami:ControlDevice,
        rami:FieldDevice ;
    sto:hasDBpediaResource "http://dbpedia.org/resource/IEC_61499" ;
    sto:hasMotivation "Functional description, informational representation and communication mapping of application functionality. This standard describes how a distributed control application is composed of functional units (FB), which are executed in different context. It may help to describe how functions are distributed between different I40-Components and how the execution of the functions between the different I40-Components is controled."@en ;
    sto:hasOfficialResource "https://webstore.iec.ch/publication/5506" ;
    sto:hasPublisher sto:IEC ;
    sto:hasTag "FBs distributed systems"@en ;
    sto:hasWikipediaArticle "http://en.wikipedia.org/wiki/IEC_61499",
        "https://en.wikipedia.org/wiki/IEC_61499" ;
    sto:relatedTo sto:IEC_61131,
        sto:IEC_62541 .

sto:IEC_61804 a dbont:Language,
        owl:NamedIndividual,
        sto:Standard ;
    rdfs:label "IEC 61804"@en ;
    dcterms:subject dbrc:Automation ;
    lingg:hypernym dbres:Language ;
    rdfs:comment "Function blocks (FB) for process control - Overview of system aspects "@en ;
    sto:hasClassification rami:Configuration,
        rami:ControlDevice,
        rami:FieldDevice ;
    sto:hasDBpediaResource "http://dbpedia.org/resource/Device_Description_Language" ;
    sto:hasOfficialResource "https://webstore.iec.ch/publication/5953" ;
    sto:hasPublisher sto:IEC ;
    sto:hasTag "EDDL"@en ;
    sto:hasWikipediaArticle "http://en.wikipedia.org/wiki/Device_Description_Language",
        "https://en.wikipedia.org/wiki/Device_Description_Language" ;
    sto:relatedTo sto:IEC_62453 .

sto:ISA-95 a dbpcy:Abstraction100002137,
        dbpcy:Measure100033615,
        dbpcy:Standard107260623,
        dbpcy:SystemOfMeasurement113577171,
        dbpcy:WikicatANSIStandards,
        dbpcy:WikicatStandards,
        dbont:Work,
        owl:NamedIndividual,
        sto:Standard ;
    rdfs:label "ISA 95"@en ;
    dcterms:subject dbrc:ANSI_standards,
        dbrc:Manufacturing ;
    lingg:hypernym dbres:Standard ;
    rdfs:comment "ANSI/ISA-95, or ISA-95 as it is more commonly referred, is an international standard from the International Society of Automation for developing an automated interface between enterprise and control systems. This standard has been developed for global manufacturers. It was developed to be applied in all industries, and in all sorts of processes, like batch processes, continuous and repetitive processes.There are 5 parts of the ISA-95 standard.ISA-95 Models"@en ;
    sto:hasDBpediaResource "http://dbpedia.org/resource/ANSI/ISA-95" ;
    sto:hasDeveloper sto:ANSI,
        sto:ISA ;
    sto:hasOfficialResource "https://www.isa.org/isa95/" ;
    sto:hasPublisher sto:ANSI,
        sto:ISA ;
    sto:hasTag "Enterprise-Control System Integration"@en ;
    sto:hasWikipediaArticle "http://en.wikipedia.org/wiki/ANSI/ISA-95",
        "https://en.wikipedia.org/wiki/ANSI/ISA-95" .

sto:ISA95 a owl:NamedIndividual,
        sto:StandardizationFramework ;
    rdfs:label "ISA 95"@en ;
    rdfs:comment "Describes the ISA95 as a Standarization Initiative that classifies Standards"@en .

sto:ISO_13584 a dbpcy:Abstraction100002137,
        dbpcy:Measure100033615,
        dbpcy:Standard107260623,
        dbpcy:SystemOfMeasurement113577171,
        dbpcy:WikicatISOStandards,
        dbont:Place,
        owl:NamedIndividual,
        sto:Standard ;
    rdfs:label "ISO 13584"@en ;
    dcterms:hasLicense "Private"@en ;
    dcterms:subject dbrc:ISO_standards ;
    lingg:hypernym dbres:Systems ;
    rdfs:comment "ISO 13584 is a series of International Standards for the computer-sensible representation and exchange of parts library data. The objective is to provide a mechanism capable of transferring parts library data, independent from any particular system. The nature of this description makes it suitable not only for the exchange of files containing parts libraries, but also as a basis for implementing and sharing databases of parts library data, and archiving"@en ;
    sto:hasClassification sto:ProductCatalogData ;
    sto:hasDBpediaResource "http://dbpedia.org/resource/ISO_13584" ;
    sto:hasMotivation "Standard data elements (properties) are used as elements in administration shell"@en ;
    sto:hasOfficialResource "https://webstore.iec.ch/publication/5380%0Ahttp://www.iso.org/iso/catalogue_detail.htm?csnumber=43423" ;
    sto:hasPublisher sto:ISO ;
    sto:hasTag "Industrial automation systems and integration"@en ;
    sto:hasWikipediaArticle "http://en.wikipedia.org/wiki/ISO_13584",
        "https://en.wikipedia.org/wiki/ISO_13584" ;
    sto:relatedTo sto:IEC_61360,
        sto:eClass .

sto:ISO_15926 a owl:NamedIndividual,
        sto:Standard ;
    rdfs:label "ISO 15926"@en ;
    rdfs:comment "Industrial automation systems and integration -- Integration of life-cycle data for process plants including oil and gas production facilities."@en ;
    sto:hasClassification rami:Configuration,
        rami:Engineering,
        rami:Integration,
        rami:Product,
        sto:ProductLifeCycleManagement ;
    sto:hasDomain sto:IndustrialAutomation ;
    sto:hasOfficialResource "https://www.iso.org/standard/29557.html" ;
    sto:hasPublicationDate "2003-12-01"^^xsd:date ;
    sto:hasPublisher sto:ISO ;
    sto:relatedTo sto:ISO_ASTM_52915 .

sto:ISO_ASTM_52915 a owl:NamedIndividual,
        sto:Standard ;
    rdfs:label "ISO ASTM 52915"@en ;
    rdfs:comment "ISO ASTM 52915:2016 provides the specification for the Additive Manufacturing File Format (AMF), an interchange format to address the current and future needs of additive manufacturing technology."@en ;
    sto:hasClassification rami:Asset,
        rami:Engineering,
        rami:Identification,
        rami:Product,
        sto:ProductionSystemEngineering ;
    sto:hasDomain sto:IndustrialAutomation ;
    sto:hasOfficialResource "https://www.iso.org/standard/60572.html" ;
    sto:hasPublicationDate "2016-02-01"^^xsd:date ;
    sto:hasPublisher sto:ISO ;
    sto:relatedTo sto:IEC_62541,
        sto:ISO_14306 .

sto:IndustrialProcessMeasurementControl a owl:NamedIndividual,
        sto:Domain ;
    rdfs:comment "Industrial process measurement and control"@en ;
    sto:domainName "Industrial process measurement and control"@en .

sto:MTConnect_Institute a owl:NamedIndividual,
        sto:StandardOrganization ;
    rdfs:comment "MTConnect Institute is a collaborative effort to develop technical standards and specifications intended to foster greater interoperability between automation/control applications, field systems/devices, and business/office applications in the manufacturing industry (\"MTConnect Specifications\"), as well as schema, prototype software examples, and related documentation in order to facilitate the implementation of the MTConnect Specifications in compliant applications, drivers, and other services"@en ;
    sto:abbreviation "MTC" ;
    sto:formationDate "2006-01-01"^^xsd:date ;
    sto:hasOfficialResource "https://w3id.org/i40/www.mtconnect.org" ;
    sto:orgName "MTConnect Institute"@en .

sto:ProductCatalogData a owl:NamedIndividual,
        sto:ProductDevelopmentLifeCycle ;
    rdfs:label "Product Catalog Data"@en ;
    rdfs:comment "Product catalog data standards support the description of particular instances of products or parts in a uniform, vendor-neutral way."@en ;
    sto:isDescribedin sto:NISTInitiative .

sto:W3C_RDF a dbpcy:Abstraction100002137,
        dbpcy:Arrangement107938773,
        dbpcy:Communication100033020,
        dbpcy:Extension106335162,
        dbpcy:Format106636806,
        dbpcy:Group100031264,
        dbpcy:Information106634376,
        dbpcy:LanguageUnit106284225,
        dbpcy:MarkupLanguage106787835,
        dbpcy:Measure100033615,
        dbpcy:Message106598915,
        dbpcy:Ordering108456993,
        dbpcy:Part113809207,
        dbpcy:Relation100031921,
        dbpcy:Sequence108459252,
        dbpcy:Series108457976,
        dbpcy:Standard107260623,
        dbpcy:String107013549,
        dbpcy:SystemOfMeasurement113577171,
        dbpcy:Terminology106304059,
        dbpcy:WikicatBibliographyFileFormats,
        dbpcy:WikicatComputerFileFormats,
        dbpcy:WikicatFilenameExtensions,
        dbpcy:WikicatMarkupLanguages,
        dbpcy:WikicatOpenFormats,
        dbpcy:WikicatWebStandards,
        dbpcy:WikicatWorldWideWebConsortiumStandards,
        dbpcy:WikicatXML-basedStandards,
        dbpcy:Word106286395,
        owl:NamedIndividual,
        owl:Thing,
        sto:Standard ;
    rdfs:label "Resource Description Framework"@en ;
    dcterms:hasLicense "Public"@en ;
    dcterms:subject dbrc:Bibliography_file_formats,
        dbrc:Knowledge_representation,
        dbrc:Metadata,
        dbrc:Resource_Description_Framework,
        dbrc:Semantic_Web,
        dbrc:World_Wide_Web_Consortium_standards,
        dbrc:XML,
        dbrc:XML-based_standards ;
    lingg:hypernym dbres:Family ;
    rdfs:comment "RDF is a standard model for data interchange on the Web. RDF has features that facilitate data merging even if the underlying schemas differ, and it specifically supports the evolution of schemas over time without requiring all the data consumers to be changed. "@en ;
    sto:hasDBpediaResource "http://dbpedia.org/resource/Resource_Description_Framework" ;
    sto:hasOfficialResource "https://www.w3.org/RDF/" ;
    sto:hasPublisher sto:W3C ;
    sto:hasTag "RDF"@en ;
    sto:hasWikipediaArticle "http://en.wikipedia.org/wiki/Resource_Description_Framework",
        "https://en.wikipedia.org/wiki/Resource_Description_Framework" .

sto:eClassAssoc a owl:NamedIndividual,
        sto:StandardOrganization ;
    rdfs:comment "Der eCl@ss e. V. ist eine Non-Profit-Organisation, die den gleichnamigen Klassifikationsstandard branchenübergreifend international definiert, weiterentwickelt und verbreitet. Der Verein wird getragen von ordentlichen und fördernden Mitgliedern aus Unternehmen, Verbänden und Institutionen."@de ;
    sto:abbreviation "eCl@ss",
        "eClass" ;
    sto:formationDate "2000-11-14"^^xsd:date ;
    sto:hasHeadquaterIn dbr:Cologne ;
    sto:hasOfficialResource "https://www.eclass.eu" ;
    sto:hasWikipediaArticle "https://www.wikiwand.com/de/ECl@ss" ;
    sto:orgName "eCl@ss e. V."@de .

dbr:Geneva a owl:NamedIndividual .

foaf:Document a owl:Class .

rami:Conditional_Monitoring a owl:NamedIndividual .

rami:GeneralAdminShell a owl:NamedIndividual .

rami:Identification a owl:NamedIndividual,
        rami:AdminShellSubmodel ;
    sto:isDescribedin sto:AdministrationShell .

rami:Security a owl:NamedIndividual,
        rami:AdminShellSubmodel ;
    sto:isDescribedin sto:AdministrationShell .

sto:CrossLevel a owl:NamedIndividual,
        sto:ISA95Level ;
    rdfs:label "Cross Level"@en ;
    rdfs:comment "Describes the cross-level according to the ISA95 level classification. It means standards that are used at more than one level, e.g., manufacturing system security, etc"@en ;
    sto:isDescribedin sto:ISA95 .

sto:IEC_61158 a dbpcy:Abstraction100002137,
        dbpcy:Artifact100021939,
        dbpcy:Bus102924116,
        dbpcy:Conveyance103100490,
        dbpcy:Instrumentality103575240,
        dbpcy:Measure100033615,
        dbpcy:Object100002684,
        dbpcy:PhysicalEntity100001930,
        dbpcy:PublicTransport104019101,
        dbpcy:Standard107260623,
        dbpcy:SystemOfMeasurement113577171,
        dbpcy:Whole100003553,
        dbpcy:WikicatIECStandards,
        dbpcy:WikicatSerialBuses,
        owl:NamedIndividual,
        sto:Standard ;
    rdfs:label "IEC 61158"@en ;
    dcterms:subject dbrc:Industrial_computing,
        dbrc:Production_and_manufacturing,
        dbrc:Serial_buses ;
    lingg:hypernym dbres:Family ;
    rdfs:comment "Fieldbus is the name of a family of industrial computer network protocols used for real-time distributed control, standardized as IEC 61158. A complex automated industrial system such as manufacturing assembly line usually needs a distributed control system an organized hierarchy of controller systems to function. In this hierarchy, there is usually a Human Machine Interface (HMI) at the top, where an operator can monitor or operate the system. This is typically linked to a middle layer of programmable logic controllers (PLC) via a non-time-critical communications system (e.g. Ethernet). At the bottom of the control chain is the fieldbus that links the PLCs to the components that actually do the work, such as sensors, actuators, electric motors, console lights, switches, valves and contactors"@en ;
    sto:hasDBpediaResource "http://dbpedia.org/page/Fieldbus" ;
    sto:hasOfficialResource "http://www.fieldbus.org/" ;
    sto:hasPublisher sto:IEC ;
    sto:hasTag "Fieldbus"@en ;
    sto:hasWikipediaArticle "http://en.wikipedia.org/wiki/Fieldbus",
        "https://en.wikipedia.org/wiki/Fieldbus" ;
    sto:relatedTo sto:IEC_61784 .

sto:IEC_61360 a owl:NamedIndividual,
        sto:Standard ;
    rdfs:label "IEC 61360"@en ;
    rdfs:comment "IEC Common Data Dictionary (IEC CDD) is a common repository of concepts for all electrotechnical domains based on the methodology and the information model of IEC 61360 series. Standard data elements types with associated classification scheme for electric items."@en ;
    sto:hasClassification rami:Asset,
        rami:Engineering,
        sto:ManufacturingModelData ;
    sto:hasDomain "Electrotechnical"@en ;
    sto:hasMotivation "Standard data elements (properties) are used as elements in administration shell"@en ;
    sto:hasOfficialResource "http://cdd.iec.ch/cdd/iec61360/iec61360.nsf",
        "https://webstore.iec.ch/publication/5380" ;
    sto:hasPublisher sto:IEC ;
    sto:hasTag "IEC Common Data Dictionary"@en ;
    sto:relatedTo sto:ISO_13584,
        sto:eClass .

sto:ISO_15531 a owl:NamedIndividual,
        sto:Standard ;
    rdfs:label "ISO 15531"@en ;
    rdfs:comment "This Standard models manufacturing management data such as, Resources management data (Resource model); Time related features (Time model); Flow management data in manufacturing (Flow management model)."@en ;
    rdfs:isDefinedBy "https://www.researchgate.net/publication/220171079_ISO_15531_MANDATE_a_standardised_data_model_for_manufacturing_management" ;
    sto:hasDomain sto:IndustrialProcessMeasurementControl ;
    sto:hasOfficialResource "https://www.iso.org/standard/28144.html" ;
    sto:hasPublisher sto:ISO ;
    sto:hasTag "MANDATE" .

sto:MESA a dbont:Settlement,
        owl:NamedIndividual,
        sto:StandardOrganization ;
    dcterms:subject dbrc:MES_software ;
    lingg:hypernym dbres:Community ;
    rdfs:comment "The Manufacturing Enterprise Solutions Association International is a global community of manufacturers, producers, industry leaders, and solution providers who are focused on driving business results from manufacturing information."@en ;
    sto:abbreviation "MESA" ;
    sto:formationDate "1992-01-01"^^xsd:date ;
    sto:hasDBpediaResource "http://dbpedia.org/page/Manufacturing_Enterprise_Solutions_Association" ;
    sto:hasHeadquaterIn dbr:_Arizona ;
    sto:hasOfficialResource "http://www.mesa.org/en/index.asp" ;
    sto:hasWikipediaArticle "http://en.wikipedia.org/wiki/Manufacturing_Enterprise_Solutions_Association",
        "https://en.wikipedia.org/wiki/Manufacturing_Enterprise_Solutions_Association" ;
    sto:orgName "Manufacturing Enterprise Solutions Association"@en .

sto:OASIS a dbpcy:Abstraction100002137,
        dbpcy:Group100031264,
        dbpcy:NongovernmentalOrganization108009834,
        dbpcy:Organization108008335,
        dbpcy:SocialGroup107950920,
        dbpcy:WikicatComputerScienceOrganizations,
        dbpcy:WikicatInformationTechnologyOrganisations,
        dbpcy:WikicatInternationalNongovernmentalOrganizations,
        dbpcy:WikicatStandardsOrganizations,
        dbpcy:WikicatXMLOrganizations,
        dbpcy:YagoLegalActor,
        dbpcy:YagoLegalActorGeo,
        dbpcy:YagoPermanentlyLocatedEntity,
        dbont:Agent,
        dbont:Non-ProfitOrganisation,
        dbont:Organisation,
        schema:Organization,
        dul:Agent,
        dul:SocialPerson,
        owl:NamedIndividual,
        owl:Thing,
        wike:Q163740,
        wike:Q24229398,
        wike:Q43229,
        sto:StandardOrganization ;
    dcterms:subject dbrc:Standards_organizations,
        dbrc:Web_services,
        dbrc:XML_organizations ;
    lingg:hypernym dbres:Consortium ;
    rdfs:comment "The Organization for the Advancement of Structured Information Standards (OASIS) is a global nonprofit consortium that works on the development, convergence, and adoption of standards for security, Internet of Things, energy, content technologies, emergency management, and other areas."@en ;
    sto:abbreviation "OASIS" ;
    sto:formationDate "1993-01-01"^^xsd:date ;
    sto:hasDBpediaResource "http://dbpedia.org/page/OASIS_(organization)" ;
    sto:hasHeadquaterIn dbr:Boston ;
    sto:hasOfficialResource "https://www.oasis-open.org/" ;
    sto:hasWikipediaArticle "http://en.wikipedia.org/wiki/OASIS_(organization)",
        "https://en.wikipedia.org/wiki/OASIS_(organization)" ;
    sto:orgName "Organization for the Advancement of Structured Information Standards"@en .

sto:ProductModelDataExchange a owl:NamedIndividual,
        sto:ProductDevelopmentLifeCycle ;
    rdfs:label "Product Model Data Exchange"@en ;
    rdfs:comment "These standards capture the representation of product and engineering information to enable data exchange between CAD software from different vendors."@en ;
    sto:isDescribedin sto:NISTInitiative .

sto:ProductionSystemEngineering a owl:NamedIndividual,
        sto:ProductionSystemLifeCycle ;
    rdfs:label "Production System Engineering"@en ;
    rdfs:comment "Standards can interconnect engineering tools from different disciplines, e.g., system engineering, mechanical plant engineering, electrical design, process engineering, process control engineering, Human Machine Interface (HMI) development, PLC programming, and robotic programming."@en ;
    sto:isDescribedin sto:NISTInitiative .

sto:SCM a owl:NamedIndividual,
        sto:BusinessCycleSCM ;
    rdfs:label "Supply Chain Management"@en ;
    rdfs:comment "Describes Plan-Source-Make-Deliver-Return cycle for managing the manufacturing supply chain."@en ;
    sto:isDescribedin sto:NISTInitiative .

rami:ConnectedWorld a owl:NamedIndividual,
        rami:RAMIHierarchyLevel ;
    sto:isDescribedin sto:RAMI40 .

rami:RAMILifeCycleLayer a owl:Class ;
    rdfs:label "RAMI Life Cycle Layer"@en ;
    rdfs:seeAlso "http://www.zvei.org/en/subjects/Industry-40/Pages/The-Reference-Architectural-Model-RAMI-40-and-the-Industrie-40-Component.aspx" ;
    rdfs:subClassOf sto:StandardClassification ;
    skos:definition "It describes the different Life Cycle and Value Stream layers for the RAMI model according to the IEC 62890 Standard."@en ;
    skos:prefLabel "RAMI Life Cycle Layer"@en .

sto:ANSI a dbpcy:Abstraction100002137,
        dbpcy:Association108049401,
        dbpcy:Group100031264,
        dbpcy:Institute108407330,
        dbpcy:Organization108008335,
        dbpcy:SocialGroup107950920,
        dbpcy:WikicatInstitutes,
        dbpcy:WikicatOrganizations,
        dbpcy:WikicatOrganizationsBasedInTheUnitedStates,
        dbpcy:WikicatOrganizationsBasedInTheUnitedStatesByActivity,
        dbpcy:WikicatOrganizationsEstablishedIn1918,
        dbpcy:WikicatResearchInstitutesInTheUnitedStates,
        dbpcy:WikicatStandardsOrganizations,
        dbpcy:YagoLegalActor,
        dbpcy:YagoLegalActorGeo,
        dbpcy:YagoPermanentlyLocatedEntity,
        dbont:Agent,
        dbont:Organisation,
        schema:Organization,
        dul:Agent,
        dul:SocialPerson,
        owl:NamedIndividual,
        owl:Thing,
        wike:Q24229398,
        wike:Q43229,
        sto:StandardOrganization ;
    rdfs:label "ANSI"@en ;
    dcterms:subject <http://dbpedia.org/resource/Category:1918_establishments_in_the_United_States>,
        dbrc:ANSI_standards,
        <http://dbpedia.org/resource/Category:Charities_based_in_Washington,_D.C.>,
        dbrc:ISO_member_bodies,
        dbrc:Organizations_established_in_1918,
        dbrc:Standards_organizations,
        dbrc:Technical_specifications ;
    lingg:hypernym dbres:Organization ;
    rdfs:comment "The American National Standards Institute is a private non-profit organization that oversees the development of voluntary consensus standards for products, services, processes, systems, and personnel in the United States. The organization also coordinates U.S. standards with international standards so that American products can be used worldwide. ANSI accredits standards that are developed by representatives of other standards organizations, government agencies, consumer groups, companies, and others. These standards ensure that the characteristics and performance of products are consistent, that people use the same definitions and terms, and that products are tested the same way. ANSI also accredits organizations that carry out product or personnel certification in accordance with requirements defined in international standards."@en ;
    sto:abbreviation "ANSI" ;
    sto:formationDate "1918-05-14"^^xsd:date ;
    sto:hasDBpediaResource dbres:American_National_Standards_Institute ;
    sto:hasHeadquaterIn <http://dbpedia.org/resource#Washington,_D.C.> ;
    sto:hasOfficialResource <https://www.ansi.org/> ;
    sto:hasWikipediaArticle <https://en.wikipedia.org/wiki/American_National_Standards_Institute?oldformat=true>,
        "http://en.wikipedia.org/wiki/American_National_Standards_Institute" ;
    sto:orgName "American National Standards Institute"@en .

sto:BusinessProcessExecution a owl:NamedIndividual,
        sto:BusinessCycleSCM ;
    rdfs:label "Business Process Execution"@en ;
    rdfs:comment "Describes Business Process Execution concept."@en ;
    sto:isDescribedin sto:NISTInitiative .

sto:CAD a owl:NamedIndividual,
        owl:Thing,
        sto:Domain ;
    rdfs:label "CAD" ;
    dcterms:subject dbrc:Computer-aided_design,
        dbrc:Design_engineering,
        dbrc:Free_computer-aided_design_software ;
    lingg:hypernym dbres:Use ;
    rdfs:comment "Computer-Aided Design"@en ;
    rdfs:isDefinedBy <https://en.wikipedia.org/wiki/Computer-aided_design> ;
    sto:domainName "Computer-Aided Design"@en ;
    sto:hasDBpediaResource dbres:Computer-aided_design ;
    sto:hasWikipediaArticle "http://en.wikipedia.org/wiki/Computer-aided_design" .

sto:ISA a dbpcy:Abstraction100002137,
        dbpcy:Association108049401,
        dbpcy:Group100031264,
        dbpcy:NongovernmentalOrganization108009834,
        dbpcy:Organization108008335,
        dbpcy:ProfessionalAssociation108242675,
        dbpcy:SocialGroup107950920,
        dbpcy:WikicatInternationalNon-profitOrganizations,
        dbpcy:WikicatInternationalNongovernmentalOrganizations,
        dbpcy:WikicatProfessionalAssociations,
        dbpcy:WikicatStandardsOrganizations,
        dbpcy:YagoLegalActor,
        dbpcy:YagoLegalActorGeo,
        dbpcy:YagoPermanentlyLocatedEntity,
        dbont:Organisation,
        owl:NamedIndividual,
        sto:StandardOrganization ;
    dcterms:subject dbrc:Engineering_organizations,
        dbrc:International_organizations_based_in_the_United_States,
        dbrc:Organizations_based_in_North_Carolina,
        dbrc:Standards_organizations ;
    lingg:hypernym dbres:Society ;
    rdfs:comment "The International Society of Automation (www.isa.org) is a nonprofit professional association that sets the standard for those who apply engineering and technology to improve the management, safety, and cybersecurity of modern automation and control systems used across industry and critical infrastructure. Founded in 1945, ISA develops widely used global standards; certifies industry professionals; provides education and training; publishes books and technical articles; hosts conferences and exhibits; and provides networking and career development programs for its 40,000 members and 400,000 customers around the world."@en ;
    sto:abbreviation "ISA" ;
    sto:formationDate "1945-04-28"^^xsd:date ;
    sto:hasDBpediaResource dbres:International_Society_of_Automation ;
    sto:hasHeadquaterIn dbr:_North_Carolina ;
    sto:hasOfficialResource <https://www.isa.org/> ;
    sto:hasWikipediaArticle <https://en.wikipedia.org/wiki/International_Society_of_Automation> ;
    sto:orgName "International Society of Automation"@en .

sto:M2M a dbpcy:Abstraction100002137,
        dbpcy:Buzzword106608277,
        dbpcy:Communication100033020,
        dbpcy:Group100031264,
        dbpcy:Message106598915,
        dbpcy:Network108434259,
        dbpcy:Nonsense106607339,
        dbpcy:System108435388,
        dbpcy:WikicatBuzzwords,
        dbpcy:WikicatNetworks,
        owl:NamedIndividual,
        sto:Domain ;
    dcterms:subject dbrc:Buzzwords,
        dbrc:Machine_to_machine,
        <http://dbpedia.org/resource/Category:Service-oriented_(business_computing)> ;
    rdfs:comment "Machine to machine refers to direct communication between devices using any communications channel, including wired and wireless"@en ;
    sto:domainName "Machine to machine Communication"@en ;
    sto:hasDBpediaResource "http://dbpedia.org/resource/Machine_to_machine" ;
    sto:hasWikipediaArticle "http://en.wikipedia.org/wiki/Machine_to_machine",
        "https://en.wikipedia.org/wiki/Machine_to_machine" .

sto:OMG a dbpcy:Abstraction100002137,
        dbpcy:Company108058098,
        dbpcy:Group100031264,
        dbpcy:Institution108053576,
        dbpcy:Organization108008335,
        dbpcy:SocialGroup107950920,
        dbpcy:WikicatComputerScienceOrganizations,
        dbpcy:WikicatInformationTechnologyOrganisations,
        dbpcy:WikicatSoftwareCompanies,
        dbpcy:WikicatStandardsOrganizations,
        dbpcy:YagoLegalActor,
        dbpcy:YagoLegalActorGeo,
        dbpcy:YagoPermanentlyLocatedEntity,
        dbont:Agent,
        dbont:Organisation,
        schema:Organization,
        dul:Agent,
        dul:SocialPerson,
        owl:NamedIndividual,
        owl:Thing,
        wike:Q24229398,
        wike:Q43229,
        sto:StandardOrganization ;
    dcterms:subject dbrc:Standards_organizations,
        dbrc:Unified_Modeling_Language ;
    lingg:hypernym dbres:Membership ;
    rdfs:comment "The Object Management Group (OMG) is an international, open membership, not-for-profit technology standards consortium. OMG Task Forces develop enterprise integration standards for a wide range of technologies and industries. OMG modeling standards enable visual design, execution and maintenance of software and other processes. Originally aimed at standardizing distributed object-oriented systems, the company now focuses on modeling (programs, systems and business processes) and model-based standards." ;
    sto:abbreviation "OMG" ;
    sto:formationDate "1989-01-01"^^xsd:date ;
    sto:hasDBpediaResource "http://dbpedia.org/resource/Object_Management_Group" ;
    sto:hasHeadquaterIn dbr:_Massachusetts ;
    sto:hasOfficialResource "http://www.omg.org/" ;
    sto:hasWikipediaArticle "http://en.wikipedia.org/wiki/Object_Management_Group",
        "https://en.wikipedia.org/wiki/Object_Management_Group" ;
    sto:orgName "Object Management Group"@en .

sto:ProductLifeCycleManagement a owl:NamedIndividual,
        sto:ProductDevelopmentLifeCycle ;
    rdfs:label "Production Life Cycle Management"@en ;
    rdfs:comment "Product lifecycle data management focuses on the needs of long-term retention and access to data consistently throughout the product lifecycle."@en ;
    sto:isDescribedin sto:NISTInitiative .

sto:ProductionSystemLifeCycle a owl:Class ;
    rdfs:label "Production System Life Cycle"@en ;
    rdfs:comment "Collections of machines, equipment, and auxiliary systems organized to create goods and services from various resources."@en ;
    rdfs:isDefinedBy "http://nvlpubs.nist.gov/nistpubs/ir/2016/NIST.IR.8107.pdf" ;
    rdfs:subClassOf sto:StandardClassification .

sto:StandardPart a owl:Class ;
    rdfs:label "StandardPart" ;
    rdfs:comment "Typically Standards are divided into parts. E.g., ISA 95 has part Part 1: Models and Terminology, Part 2: Object Model Attributes, etc."@en ;
    rdfs:subClassOf foaf:Document .

sto:eClass a owl:NamedIndividual,
        sto:Standard ;
    rdfs:label "eClass"@en ;
    rdfs:comment "eCl@ss is the cross-industry product data standard for classification and clear description of products and services."@en ;
    sto:hasClassification rami:ConnectedWorld,
        rami:ControlDevice,
        rami:Engineering,
        rami:Enterprise,
        rami:Product,
        rami:Station,
        rami:WorkCenter ;
    sto:hasDBpediaResource "http://de.dbpedia.org/page/ECl@ss" ;
    sto:hasDeveloper sto:eClassAssoc ;
    sto:hasMotivation "Global identification, semantic description and automatic product classification"@en ;
    sto:hasOfficialResource "https://www.eclass.eu/eclasscontent/standard/overview.html.en" ;
    sto:hasPublisher sto:eClassAssoc ;
    sto:hasTag "eClass"@en ;
    sto:hasWikipediaArticle "https://de.wikipedia.org/wiki/ECl@ss" ;
    sto:relatedTo sto:IEC_61360,
        sto:ISO_13584 .

rami:Business a owl:NamedIndividual,
        rami:RAMIITLayer ;
    sto:isDescribedin sto:RAMI40 .

rami:Configuration a owl:NamedIndividual .

rami:Functional a owl:NamedIndividual,
        rami:RAMIITLayer ;
    sto:isDescribedin sto:RAMI40 .

rami:Information a owl:NamedIndividual,
        rami:RAMIITLayer ;
    sto:isDescribedin sto:RAMI40 .

sto:ProductDevelopmentLifeCycle a owl:Class ;
    rdfs:label "Product Development Life Cycle"@en ;
    rdfs:comment "PLM is the process of managing the entire lifecycle of a product from inception, through engineering design and manufacture, to service and disposal of manufactured products. Related areas are PLMManagement, Modeling Practice, Product Model Data exchange, Manufacturing Model Data, Product Catalog Data."@en,
        "Product Development Life-Cycle Phase"@en ;
    rdfs:isDefinedBy "https://en.wikipedia.org/wiki/Product_lifecycle" ;
    rdfs:subClassOf sto:StandardClassification .

sto:W3C a dbpcy:Abstraction100002137,
        dbpcy:Association108049401,
        dbpcy:Consortium108236438,
        dbpcy:Group100031264,
        dbpcy:NongovernmentalOrganization108009834,
        dbpcy:Organization108008335,
        dbpcy:SocialGroup107950920,
        dbpcy:WikicatConsortia,
        dbpcy:WikicatInternationalNongovernmentalOrganizations,
        dbpcy:WikicatOrganizations,
        dbpcy:WikicatOrganizationsEstablishedIn1994,
        dbpcy:WikicatStandardsOrganizations,
        dbpcy:YagoLegalActor,
        dbpcy:YagoLegalActorGeo,
        dbpcy:YagoPermanentlyLocatedEntity,
        dbont:Agent,
        dbont:Organisation,
        schema:Organization,
        <http://umbel.org/umbel/rc/Organization>,
        dul:Agent,
        dul:SocialPerson,
        owl:NamedIndividual,
        owl:Thing,
        wike:Q24229398,
        wike:Q43229,
        sto:StandardOrganization ;
    rdfs:label "W3C"@en ;
    dcterms:subject dbrc:Organizations_established_in_1994,
        dbrc:Standards_organizations,
        dbrc:Technology_consortia,
        dbrc:Web_development,
        dbrc:Web_services,
        dbrc:World_Wide_Web_Consortium ;
    lingg:hypernym dbres:Organization ;
    rdfs:comment "The World Wide Web Consortium (W3C) is the main international standards organization for the World Wide Web (abbreviated WWW or W3). Founded and currently led by Tim Berners-Lee, the consortium is made up of member organizations which maintain full-time staff for the purpose of working together in the development of standards for the World Wide Web. As of 4 November 2015, the World Wide Web Consortium (W3C) has 408 members. The W3C also engages in education and outreach, develops software and serves as an open forum for discussion about the Web."@en ;
    sto:abbreviation "W3C" ;
    sto:formationDate "1994-10-01"^^xsd:date ;
    sto:hasDBpediaResource "http://dbpedia.org/resource/World_Wide_Web_Consortium" ;
    sto:hasHeadquaterIn dbr:_Massachusetts ;
    sto:hasOfficialResource "https://www.w3.org/" ;
    sto:hasWikipediaArticle "http://en.wikipedia.org/wiki/World_Wide_Web_Consortium",
        "https://en.wikipedia.org/wiki/World_Wide_Web_Consortium" ;
    sto:orgName "World Wide Web Consortium"@en .

sto:relatedTo a owl:ObjectProperty,
        owl:SymmetricProperty,
        owl:TransitiveProperty ;
    rdfs:label "related To"@en ;
    rdfs:comment "Represent any type of relation that connects two standards."@en ;
    rdfs:domain sto:Standard ;
    rdfs:range sto:Standard ;
    skos:altLabel "has Associated Standard"@en .

sto:ETSI a dbpcy:Abstraction100002137,
        dbpcy:Group100031264,
        dbpcy:Organization108008335,
        dbpcy:SocialGroup107950920,
        dbpcy:WikicatOrganizationsEstablishedIn1988,
        dbpcy:WikicatStandardsOrganizations,
        dbpcy:WikicatTelecommunicationsOrganizations,
        dbpcy:YagoLegalActor,
        dbpcy:YagoLegalActorGeo,
        dbpcy:YagoPermanentlyLocatedEntity,
        dbont:Organisation,
        owl:NamedIndividual,
        owl:Thing,
        sto:StandardOrganization ;
    rdfs:label "ETSI"@en ;
    dcterms:subject dbrc:Organizations_established_in_1988,
        dbrc:Standards_organizations,
        dbrc:Telecommunications_in_Europe,
        dbrc:Telecommunications_organizations ;
    lingg:hypernym dbres:Organization ;
    rdfs:comment "The European Telecommunications Standards Institute (ETSI) is an independent, not-for-profit, standardization organization in the telecommunications industry (equipment makers and network operators) in Europe, headquartered in Sophia-Antipolis, France, with worldwide projection. ETSI produces globally-applicable standards for Information and Communications Technologies (ICT), including fixed, mobile, radio, converged, broadcast and internet technologies."@en ;
    sto:abbreviation "ETSI"@en ;
    sto:formationDate "1988-01-01"^^xsd:date ;
    sto:hasDBpediaResource "http://dbpedia.org/resource/ETSI" ;
    sto:hasHeadquaterIn dbr:Valbonne ;
    sto:hasOfficialResource "http://www.etsi.org/" ;
    sto:hasWikipediaArticle "http://en.wikipedia.org/wiki/ETSI",
        "https://en.wikipedia.org/wiki/ETSI" ;
    sto:orgName "European Telecommunications Standards Institute"@en .

sto:IEC_62714 a dbpcy:Abstraction100002137,
        dbpcy:Communication100033020,
        dbpcy:Format106636806,
        dbpcy:Information106634376,
        dbpcy:LanguageUnit106284225,
        dbpcy:MarkupLanguage106787835,
        dbpcy:Measure100033615,
        dbpcy:Message106598915,
        dbpcy:Part113809207,
        dbpcy:Relation100031921,
        dbpcy:Standard107260623,
        dbpcy:SystemOfMeasurement113577171,
        dbpcy:Terminology106304059,
        dbpcy:WikicatComputerFileFormats,
        dbpcy:WikicatIndustry-specificXML-basedStandards,
        dbpcy:WikicatMarkupLanguages,
        dbpcy:WikicatXML-basedStandards,
        dbpcy:Word106286395,
        dbont:Software,
        owl:NamedIndividual,
        sto:Standard ;
    rdfs:label "IEC 62714"@en ;
    dcterms:hasLicense "Open"@en ;
    dcterms:subject dbrc:Computer_file_formats,
        dbrc:Industry-specific_XML-based_standards,
        dbrc:XML_markup_languages ;
    lingg:hypernym dbres:Format ;
    rdfs:comment "Engineering data exchange format for use in industrial automation systems engineering - Automation markup language - Architecture and general requirements"@en ;
    sto:hasClassification rami:ControlDevice,
        rami:Engineering,
        rami:FieldDevice,
        rami:Information,
        rami:Product,
        sto:ProductionSystemEngineering ;
    sto:hasDBpediaResource "http://dbpedia.org/resource/AutomationML" ;
    sto:hasOfficialResource "https://www.automationml.org/" ;
    sto:hasPublisher sto:IEC ;
    sto:hasTag "AML"@en,
        "AutomationML"@en ;
    sto:hasWikipediaArticle "http://en.wikipedia.org/wiki/AutomationML",
        "https://en.wikipedia.org/wiki/AutomationML" ;
    sto:relatedTo sto:IEC_61360,
        sto:IEC_61987_X,
        sto:IEC_62541,
        sto:eClass ;
    sto:uses sto:MathML .

sto:ModelingPractice a owl:NamedIndividual,
        sto:ProductDevelopmentLifeCycle ;
    rdfs:label "Modeling Practice"@en ;
    rdfs:comment "Modeling practice standards define digital product-definition data practices for both two-dimensional (2D) drawings and three-dimensional (3D) models."@en ;
    sto:isDescribedin sto:NISTInitiative .

sto:ProductionSystemModelData a owl:NamedIndividual,
        sto:ProductionSystemLifeCycle ;
    rdfs:label "Production System Model Data"@en ;
    rdfs:comment "Provide information models for factory and production system design. They enhance information exchange among stakeholders, and enable virtual commissioning, which can improve manufacturing agility and reduce manufacturing cost."@en ;
    sto:isDescribedin sto:NISTInitiative .

sto:StandardizationFramework a owl:Class ;
    rdfs:label "Standarization Framework"@en ;
    rdfs:comment "Describes existings Standardizations Initiatives, e.g, RAMI, NIST."@en ;
    skos:altLabel "Reference Architecture"@en .

rami:Communication a owl:NamedIndividual,
        rami:RAMIITLayer ;
    sto:isDescribedin sto:RAMI40 .

rami:Integration a owl:NamedIndividual,
        rami:RAMIITLayer ;
    sto:isDescribedin sto:RAMI40 .

rami:RAMIHierarchyLevel a owl:Class ;
    rdfs:label "RAMI Hierarchy Level"@en ;
    rdfs:subClassOf sto:StandardClassification ;
    owl:equivalentClass [ a owl:Class ;
            owl:oneOf ( rami:ConnectedWorld rami:ControlDevice rami:Enterprise rami:FieldDevice rami:Product rami:Station rami:WorkCenter ) ] .

rami:RAMIITLayer a owl:Class ;
    rdfs:label "RAMI IT Layer"@en ;
    rdfs:subClassOf sto:StandardClassification ;
    owl:equivalentClass [ a owl:Class ;
            owl:oneOf ( rami:Asset rami:Business rami:Communication rami:Functional rami:Information rami:Integration ) ] .

rami:Safety a owl:NamedIndividual,
        rami:AdminShellSubmodel ;
    sto:isDescribedin sto:AdministrationShell .

sto:IEC_62541 a dbpcy:Abstraction100002137,
        dbpcy:Communication100033020,
        dbpcy:Direction106786629,
        dbpcy:Measure100033615,
        dbpcy:Message106598915,
        dbpcy:Protocol106665108,
        dbpcy:Rule106652242,
        dbpcy:Standard107260623,
        dbpcy:SystemOfMeasurement113577171,
        dbpcy:WikicatComputerStandards,
        dbpcy:WikicatNetworkProtocols,
        dbont:Software,
        owl:NamedIndividual,
        sto:Standard ;
    rdfs:label "IEC 62541"@en ;
    dcterms:hasLicense sto:GPLv2,
        "Open"@en ;
    dcterms:subject dbrc:Application_programming_interfaces,
        dbrc:Automation,
        dbrc:Computer_standards ;
    lingg:hypernym dbres:Protocol ;
    rdfs:comment "OPC Unified Architecture (OPC UA) is an industrial M2M communication protocol for interoperability developed by the OPC Foundation. It is the successor to Open Platform Communications (OPC). Although developed by the same organization, OPC UA differs significantly from its predecessor. The Foundation's goal for this project was to provide a path forward from the original OPC communications model (namely the Microsoft Windows only process exchange COM/DCOM) to a cross-platform service-oriented architecture (SOA) for process control, while enhancing security and providing an information model."@en ;
    sto:hasClassification rami:Communication,
        rami:ConnectedWorld,
        rami:ControlDevice,
        rami:Enterprise,
        rami:FieldDevice,
        rami:Station,
        rami:WorkCenter,
        sto:Communication,
        sto:SCADALevel ;
    sto:hasDBpediaResource "http://dbpedia.org/resource/OPC_Unified_Architecture" ;
    sto:hasDeveloper sto:OPC_Foundation ;
    sto:hasDomain sto:IndustrialAutomation ;
    sto:hasOfficialResource "https://opcfoundation.org/about/opc-technologies/opc-ua/" ;
    sto:hasPublisher sto:IEC ;
    sto:hasTag "OPC UA"@en ;
    sto:hasWikipediaArticle "http://en.wikipedia.org/wiki/OPC_Unified_Architecture",
        "https://en.wikipedia.org/wiki/OPC_Unified_Architecture" ;
    sto:relatedTo sto:IEC_61499,
        sto:IEC_61850,
        sto:IEC_62714 ;
    sto:useStructureOf sto:IEC_61804 .

sto:ISA95Level a owl:Class ;
    rdfs:label "ISA95 Level"@en ;
    rdfs:comment "Describes the ISA95 levels to classify the industry Standards according to those levels. Eg., Device, SCADA, etc. It has strong relation to the RAMI Hierarchy levels"@en ;
    rdfs:subClassOf sto:StandardClassification .

sto:Domain a owl:Class ;
    rdfs:label "Domain"@en ;
    rdfs:comment "Represents the Domains in which the Standards can be used"@en .

rami:Asset a owl:NamedIndividual,
        rami:RAMIITLayer ;
    sto:isDescribedin sto:RAMI40 .

rami:AdminShellSubmodel a owl:Class ;
    rdfs:label "Admin Shell Sub Model"@en ;
    rdfs:comment "Describes the Administration Shell concept to organize/classify standards into submodels"@en ;
    rdfs:isDefinedBy <https://www.plattform-i40.de/I40/Redaktion/EN/Downloads/Publikation/structure-of-the-administration-shell.pdf?__blob=publicationFile&v=7> ;
    rdfs:subClassOf sto:StandardClassification .

rami:Enterprise a owl:NamedIndividual,
        rami:RAMIHierarchyLevel ;
    sto:isDescribedin sto:RAMI40 .

sto:AdministrationShell a owl:NamedIndividual,
        sto:StandardizationFramework ;
    rdfs:label "Administration Shell"@en ;
    rdfs:comment "Represents the classifications of the standards according to the submodels of the administration shell."@en .

sto:StandardClassification a owl:Class ;
    rdfs:label "Standard Classification"@en ;
    rdfs:comment "Describes categorization areas that the different Standardizations Initiatives use to category Standards."@en .

sto:NISTInitiative a owl:NamedIndividual,
        sto:StandardizationFramework ;
    rdfs:label "NIST Initiative"@en ;
    rdfs:comment "Describes the National Institute of Standards and Technology Initiative, i.e., NIST which provides a standard landascape"@en ;
    rdfs:isDefinedBy "http://nvlpubs.nist.gov/nistpubs/ir/2016/NIST.IR.8107.pdf" .

rami:WorkCenter a owl:NamedIndividual,
        rami:RAMIHierarchyLevel ;
    sto:isDescribedin sto:RAMI40 .

rami:Engineering a owl:NamedIndividual,
        rami:AdminShellSubmodel ;
    sto:isDescribedin sto:AdministrationShell .

sto:RAMI40 a owl:NamedIndividual,
        sto:StandardizationFramework ;
    rdfs:label "RAMI 4.0"@en ;
    rdfs:comment "Describes the Reference Architecture Model for Industry 4.0, i.e., the RAMI Initiative."@en .

rami:Station a owl:NamedIndividual,
        rami:RAMIHierarchyLevel ;
    sto:isDescribedin sto:RAMI40 .

sto:IndustrialAutomation a owl:NamedIndividual,
        sto:Domain ;
    rdfs:comment "Industrial automation deals primarily with the automation of manufacturing, quality control and material handling processes. General purpose controllers for industrial processes include Programmable logic controllers, stand-alone I/O modules, and computers. Industrial automation is to replace the decision making of humans and manual command-response activities with the use of mechanized equipment and logical programming commands. One trend is increased use of Machine vision to provide automatic inspection and robot guidance functions, another is a continuing increase in the use of robots. Industrial automation is simply done at the industrial level."@en ;
    sto:domainName "Industrial Automation"@en ;
    sto:hasDBpediaResource "http://dbpedia.org/resource/Category:IndustrialAutomation" ;
    sto:hasWikipediaArticle "https://en.wikipedia.org/wiki/Automation" .

rami:FieldDevice a owl:NamedIndividual,
        rami:RAMIHierarchyLevel ;
    sto:isDescribedin sto:RAMI40 .

rami:Product a owl:NamedIndividual,
        rami:RAMIHierarchyLevel ;
    sto:isDescribedin sto:RAMI40 .

rami:ControlDevice a owl:NamedIndividual,
        rami:RAMIHierarchyLevel ;
    sto:isDescribedin sto:RAMI40 .

sto:StandardOrganization a owl:Class ;
    rdfs:label "StandardOrganization"@en ;
    rdfs:comment "Define the standards organizations that develop and publish industry standards"@en ;
    rdfs:subClassOf foaf:Organization .

sto:ISO a dbpcy:Abstraction100002137,
        dbpcy:Alliance108293982,
        dbpcy:Group100031264,
        dbpcy:Measure100033615,
        dbpcy:NongovernmentalOrganization108009834,
        dbpcy:Organization108008335,
        dbpcy:SocialGroup107950920,
        dbpcy:Standard107260623,
        dbpcy:SystemOfMeasurement113577171,
        dbpcy:WikicatInternationalNongovernmentalOrganizations,
        dbpcy:WikicatInternationalOrganizations,
        dbpcy:WikicatNon-governmentalOrganizations,
        dbpcy:WikicatOrganisationsBasedInGeneva,
        dbpcy:WikicatOrganizationsEstablishedIn1947,
        dbpcy:WikicatOrganizationsWithGeneralConsultativeStatusToTheUnitedNationsEconomicAndSocialCouncil,
        dbpcy:WikicatSocialResponsibilityOrganizations,
        dbpcy:WikicatStandardsOrganizations,
        dbpcy:WikicatWithdrawnISOStandards,
        dbpcy:WorldOrganization108294696,
        dbpcy:YagoLegalActor,
        dbpcy:YagoLegalActorGeo,
        dbpcy:YagoPermanentlyLocatedEntity,
        dbont:Agent,
        dbont:Organisation,
        schema:Organization,
        <http://umbel.org/umbel/rc/Organization>,
        dul:Agent,
        dul:SocialPerson,
        owl:NamedIndividual,
        owl:Thing,
        wike:Q24229398,
        wike:Q43229,
        sto:StandardOrganization ;
    dcterms:subject dbrc:International_Organization_for_Standardization,
        dbrc:Organisations_based_in_Geneva,
        dbrc:Organizations_established_in_1947,
        dbrc:Organizations_with_general_consultative_status_to_the_United_Nations_Economic_and_Social_Council,
        dbrc:Social_responsibility_organizations,
        dbrc:Standards_organizations,
        dbrc:Technical_specifications ;
    lingg:hypernym dbres:Body ;
    rdfs:comment "Is an independent, non-governmental organization, the members of which are the standards organizations of the 162 member countries. It is the world's largest developer of voluntary international standards and facilitates world trade by providing common standards between nations. Nearly twenty thousand standards have been set covering everything from manufactured products and technology to food safety, agriculture and healthcare."@en,
        "The International Organization for Standardization (ISO) is an international standard-setting body composed of representatives from various national standards organizations."@en ;
    sto:abbreviation "ISO" ;
    sto:belongsTo dbr:Switzerland ;
    sto:formationDate "1947-02-23"^^xsd:date ;
    sto:hasDBpediaResource <http://dbpedia.org/page/International_Organization_for_Standardization> ;
    sto:hasHeadquaterIn dbr:Geneva ;
    sto:hasOfficialResource <https://www.iso.org>,
        <https://www.iso.org/about-us.html> ;
    sto:hasWikipediaArticle <https://en.wikipedia.org/wiki/International_Organization_for_Standardization> ;
    sto:orgName "Internationale Organisation für Normung"@de,
        "International Organization for Standardization"@en,
        "The International Organization for Standardization"@en,
        "Organisation internationale de normalisation"@fr,
        "Международная организация по стандартизации"@ru .

sto:IEC a dbpcy:Abstraction100002137,
        dbpcy:Alliance108293982,
        dbpcy:Association108049401,
        dbpcy:Company108058098,
        dbpcy:Group100031264,
        dbpcy:Institute108407330,
        dbpcy:Institution108053576,
        dbpcy:Organization108008335,
        dbpcy:SocialGroup107950920,
        dbpcy:WikicatComputerScienceOrganizations,
        dbpcy:WikicatInstitutes,
        dbpcy:WikicatInternationalOrganizations,
        dbpcy:WikicatOrganisationsBasedInGeneva,
        dbpcy:WikicatOrganizationsEstablishedIn1906,
        dbpcy:WikicatStandardsOrganizations,
        dbpcy:WorldOrganization108294696,
        dbpcy:YagoLegalActor,
        dbpcy:YagoLegalActorGeo,
        dbpcy:YagoPermanentlyLocatedEntity,
        dbont:Agent,
        dbont:Organisation,
        schema:Organization,
        dul:Agent,
        dul:SocialPerson,
        owl:NamedIndividual,
        owl:Thing,
        wike:Q24229398,
        wike:Q43229,
        sto:StandardOrganization ;
    dcterms:subject dbrc:Electrical_engineering_organizations,
        dbrc:International_Electrotechnical_Commission,
        dbrc:Standards_organizations ;
    lingg:hypernym dbres:Organization ;
    rdfs:comment "Is a non-profit, non-governmental international standards organization that prepares and publishes International Standards for all electrical, electronic and related technologies – collectively known as \"electrotechnology\". IEC standards cover a vast range of technologies from power generation, transmission and distribution to home appliances and office equipment, semiconductors, fiber optics, batteries, solar energy, nanotechnology and marine energy as well as many others. The IEC also manages three global conformity assessment systems that certify whether equipment, system or components conform to its International Standards."@en ;
    sto:abbreviation "IEC" ;
    sto:formationDate "1906-06-26"^^xsd:date ;
    sto:hasDBpediaResource dbres:International_Electrotechnical_Commission ;
    sto:hasHeadquaterIn dbr:Geneva ;
    sto:hasOfficialResource <http://www.iec.ch/> ;
    sto:hasWikipediaArticle <https://en.wikipedia.org/wiki/International_Electrotechnical_Commission> ;
    sto:orgName "International Electrotechnical Commission"@en,
        "Commission électrotechnique internationale"@fr .

sto:Standard a owl:Class ;
    rdfs:label "Standard" ;
    cc:attributionName "Copyright © 2016 IEC Geneva, Switzerland." ;
    cc:attributionURL "http://www.iec.ch" ;
    rdfs:comment "A document, established by consensus and approved by a recognized body, that provides, for common and repeated use, rules, guidelines or characteristics for activities or their results, aimed at the achievement of the optimum degree of order in a given context."@en ;
    rdfs:isDefinedBy sto:IEC ;
    rdfs:seeAlso <http://www.iec.ch/standardsdev/publications/is.htm> ;
    rdfs:subClassOf foaf:Document ;
    owl:disjointWith sto:StandardOrganization .

